<?xml version="1.0"?>
<rdf:RDF xmlns="https://photogrammetry.altervista.org/collections/show/3#"
     xml:base="https://photogrammetry.altervista.org/collections/show/3"
     xmlns:dc="http://purl.org/dc/elements/1.1/"
     xmlns:owl="http://www.w3.org/2002/07/owl#"
     xmlns:rdf="http://www.w3.org/1999/02/22-rdf-syntax-ns#"
     xmlns:xml="http://www.w3.org/XML/1998/namespace"
     xmlns:xsd="http://www.w3.org/2001/XMLSchema#"
     xmlns:rdfs="http://www.w3.org/2000/01/rdf-schema#"
     xmlns:skos="http://www.w3.org/2004/02/skos/core#"
     xmlns:vann="http://purl.org/vocab/vann/"
     xmlns:terms="http://purl.org/dc/terms/"
     xmlns:schema="https://schema.org/">
    <owl:Ontology rdf:about="https://photogrammetry.altervista.org/collections/show/3">
        <owl:imports rdf:resource="http://objects.mainzed.org/metadata/ont#"/>
        <owl:imports rdf:resource="http://www.opengis.net/ont/geosparql"/>
        <owl:imports rdf:resource="http://www.w3.org/2004/02/skos/core"/>
        <dc:creator xml:lang="en">Timo Homburg, Anja Cramer, Laura Raddatz</dc:creator>
        <dc:creator xml:lang="en">Vittorio Lauro</dc:creator>
        <rdfs:comment xml:lang="en">Introduction to the PODS and Mainzed 3D Metadata Ontologies

The Protocol of Ontological Digital Survey (PODS) ontology was developed to standardize and formalize the digital survey process for cultural heritage, with a focus on accurate metadata representation at each stage of 3D data acquisition, processing, and management. Building on previous protocols like BeAPG and FOPPA, PODS integrates standards such as SKOS, QUDT, and CIDOC-CRMdig, promoting interoperability with international data-sharing platforms like Wikimedia. PODS organizes classes and properties to document each step, enabling structured and consistent cataloging of digital heritage assets.

Recently, the PODS ontology has been merged with the Mainzed 3D Metadata Ontology, an ontology curated by Timo Homburg, Anja Cramer, and Laura Raddatz, designed to classify 3D survey operations. This integration aimed to align nearly all classes between the two ontologies, creating a comprehensive framework that enhances the precision and accessibility of cultural heritage data across diverse contexts.

Despite the extensive alignment, certain classes from the Mainzed 3D Metadata Ontology were excluded for specific reasons:

indoor/outdoor: Excluded for vagueness; however, the superclass Environment was retained to account for the role of lighting in data acquisition.

algorithm: Its role as an agent is debated, and cataloging every possible algorithm was deemed impractical without an exhaustive thesaurus.

feature detection algorithm subclasses: Excluded due to their potential obsolescence as algorithms evolve over time.

measurement algorithm subclasses: Similarly excluded because they may become outdated with advancements in measurement methods.

acquisition technology subclasses: Excluded for their specificity, as evolving technologies could render these definitions obsolete.

export function subclasses: Excluded as they specify highly software-specific actions that may change over time.

remove function subclasses: Excluded for their software-specific nature, with actions that may vary across applications.

Split Function and Transformation Function: Omitted due to specificity to particular software, leading to potential incompatibility over time.

Measurement: This class and its subclasses (e.g., Agisoft and chunk measures) were excluded as they are either overly generic or specific to certain software, complicating interoperability.

measurement check, measurement project, measurement series, and measurement setup: Excluded due to ambiguities around the data type (e.g., point cloud or mesh), often linked to specific software commands.

Technology: Excluded for being overly generic, although all its subclasses were incorporated.

Raster Data: Excluded as a class, but its subclasses were integrated for granularity.

Geometry subclasses: While exhaustive, they were excluded to avoid redundancy, with a reference to ISO 19107 in the Geometry class to maintain specificity.

spatial object: Excluded for its generality, though its subclasses were retained.

tool: Excluded for being too broad, yet all subclasses were integrated.

Calibration object to calibrate a capturing device subclasses: Excluded due to their specificity to certain devices.

Through the alignment and exclusion of specific classes, this merged ontology establishes a robust, adaptable structure for digital cultural heritage documentation, enabling compatibility and integration across platforms while ensuring data precision and longevity.</rdfs:comment>
        <owl:versionInfo rdf:datatype="http://www.w3.org/2001/XMLSchema#integer">1</owl:versionInfo>
    </owl:Ontology>
    


    <!-- 
    ///////////////////////////////////////////////////////////////////////////////////////
    //
    // Annotation properties
    //
    ///////////////////////////////////////////////////////////////////////////////////////
     -->


    


    <!-- http://purl.org/dc/elements/1.1/creator -->


    <owl:AnnotationProperty rdf:about="http://purl.org/dc/elements/1.1/creator"/>
    


    <!-- 
    ///////////////////////////////////////////////////////////////////////////////////////
    //
    // Object Properties
    //
    ///////////////////////////////////////////////////////////////////////////////////////
     -->


    


    <!-- http://www.semanticweb.org/vitto/ontologies/2024/9/PODS_1#P132_spatiotemporally_overlaps_with -->


    <owl:ObjectProperty rdf:about="http://www.semanticweb.org/vitto/ontologies/2024/9/PODS_1#P132_spatiotemporally_overlaps_with">
        <rdfs:comment>URI (forward direction):	http://www.cidoc-crm.org/cidoc-crm/P132_spatiotemporally_overlaps_with
URI (inverse direction):	-
Domain:
E92 Spacetime Volume
Range:
E92 Spacetime Volume
SubProperty Of:
-
SuperProperty Of:
E92 Spacetime Volume. P10 falls within (contains): E92 Spacetime Volume
Quantification:
many to many (0,n:0,n)

Scope Note:
This symmetric property associates two instances of E92 Spacetime Volume that have some of their extents in common. If only the fuzzy boundaries of the instances of E92 Spacetime Volume overlap, this property cannot be determined from observation alone and therefore should not be applied. However, there may be other forms of justification that the two instances of E92 Spacetime Volume must have some of their extents in common regardless of where and when precisely.

If this property holds for two instances of E92 Spacetime Volume then it cannot be the case that P133 is spatiotemporally separated from also holds for the same two instances. Furthermore, there are cases where neither P132 spatiotemporally overlaps with nor P133 is spatiotemporally separated from holds between two instances of E92 Spacetime Volume. This would occur where only an overlap of the fuzzy boundaries of the two instances of E92 Spacetime Volume occurs and no other evidence is available.

This property is not transitive. This property is symmetric. This property is reflexive.

Properties:
-
Examples:
The &apos;Urnfield&apos; period (E4) spatiotemporally overlaps with the &apos;Hallstatt&apos; period (E4). (Gimbutas, 1965)</rdfs:comment>
    </owl:ObjectProperty>
    


    <!-- http://www.semanticweb.org/vitto/ontologies/2024/9/PODS_1#Y12_was_continued_by_Processing_Phase -->


    <owl:ObjectProperty rdf:about="http://www.semanticweb.org/vitto/ontologies/2024/9/PODS_1#Y12_was_continued_by_Processing_Phase">
        <rdfs:subPropertyOf rdf:resource="http://www.semanticweb.org/vitto/ontologies/2024/9/PODS_1#P134_continued_(was_continued_by)"/>
        <rdfs:subPropertyOf rdf:resource="https://photogrammetry.altervista.org/items/show/266#Y93:_was_continued_by_subsequent_phase"/>
        <rdfs:domain rdf:resource="https://photogrammetry.altervista.org/admin/items/show/88#F2_Acquisition"/>
        <rdfs:range rdf:resource="https://photogrammetry.altervista.org/items/show/89#F3_Processing"/>
        <rdfs:comment xml:lang="en">This property is redundant and can be replaced by the superproperty 
-Y93 was continued by subsequent phase-</rdfs:comment>
        <rdfs:label xml:lang="en">was_continued_by_processing_phase</rdfs:label>
        <skos:definition xml:lang="en">Y12: was continued by Processing Phase

SubProperties of: P134i was continued by

Domain: F2 Acquisition
Range: F3 Processing</skos:definition>
        <skos:example xml:lang="en">-</skos:example>
        <skos:scopeNote xml:lang="en">This property describes how the acquisition event (F2) was followed by a processing phase (F3). It links the data acquisition process to the subsequent phase where raw data is processed and refined.</skos:scopeNote>
    </owl:ObjectProperty>
    


    <!-- http://www.semanticweb.org/vitto/ontologies/2024/9/PODS_1#L10_had_input_(was_input_of) -->


    <owl:ObjectProperty rdf:about="http://www.semanticweb.org/vitto/ontologies/2024/9/PODS_1#L10_had_input_(was_input_of)">
        <rdfs:subPropertyOf rdf:resource="http://www.semanticweb.org/vitto/ontologies/2024/9/PODS_1#P16_used_specific_object_(was_used_for)"/>
        <rdfs:domain rdf:resource="http://www.cidoc-crm.org/extensions/crmdig/versions/4.0/D7_Digital_Machine_Event#D7_Digital_Machine_Event"/>
        <rdfs:range rdf:resource="http://www.cidoc-crm.org/extensions/crmdig/versions/4.0/D1_Digital_Object#D1_Digital_Object"/>
        <rdfs:comment>Domain:
D7 Digital Machine Event
Range:
D1 Digital Object
SubProperty Of:
E7 Activity. P16 used specific object (was used for): E70 Thing
SuperProperty Of:
-
Quantification:
-
Scope Note:
This property associates an instance of D7 Digital Machine Event with an instance of D1 Digital Object which is the input used to specify the machine action.

Properties:
-
Examples:
-</rdfs:comment>
    </owl:ObjectProperty>
    


    <!-- http://www.semanticweb.org/vitto/ontologies/2024/9/PODS_1#L11_had_output_(was_output_of) -->


    <owl:ObjectProperty rdf:about="http://www.semanticweb.org/vitto/ontologies/2024/9/PODS_1#L11_had_output_(was_output_of)">
        <rdfs:subPropertyOf rdf:resource="http://www.semanticweb.org/vitto/ontologies/2024/9/PODS_1#P94_has_created_(was_created_by)"/>
        <rdfs:domain rdf:resource="http://www.cidoc-crm.org/extensions/crmdig/versions/4.0/D7_Digital_Machine_Event#D7_Digital_Machine_Event"/>
        <rdfs:range rdf:resource="http://www.cidoc-crm.org/extensions/crmdig/versions/4.0/D1_Digital_Object#D1_Digital_Object"/>
        <rdfs:comment>URI; http://www.cidoc-crm.org/extensions/crmdig/versions/4.0/L11_had_output

Domain:
D7 Digital Machine Event
Range:
D1 Digital Object
SubProperty Of:
E65 Creation. P94 has created (was created by): E28 Conceptual Object
SuperProperty Of:
-
Quantification:
-
Scope Note:
This property associates an instance of D7 Digital Machine Event with an instance of D1 Digital Object which is the output of the activity.

Properties:
-
Examples:
-</rdfs:comment>
    </owl:ObjectProperty>
    


    <!-- http://www.semanticweb.org/vitto/ontologies/2024/9/PODS_1#L12_happened_on_device_(was_device_for) -->


    <owl:ObjectProperty rdf:about="http://www.semanticweb.org/vitto/ontologies/2024/9/PODS_1#L12_happened_on_device_(was_device_for)">
        <rdfs:subPropertyOf rdf:resource="http://www.semanticweb.org/vitto/ontologies/2024/9/PODS_1#P12_occurred_in_the_presence_of_(was_present_at)"/>
        <rdfs:domain rdf:resource="http://www.cidoc-crm.org/extensions/crmdig/versions/4.0/D7_Digital_Machine_Event#D7_Digital_Machine_Event"/>
        <rdfs:range rdf:resource="http://www.cidoc-crm.org/extensions/crmdig/versions/4.0/D8_Digital_Device#D8_Digital_Device"/>
        <rdfs:comment>URI: http://www.cidoc-crm.org/extensions/crmdig/versions/4.0/L12_happened_on_device

Domain:
D7 Digital Machine Event
Range:
D8 Digital Device
SubProperty Of:
E5 Event. P12 occurred in the presence of (was present at): E77 Persistent Item
SuperProperty Of:
-
Quantification:
-
Scope Note:
This property associates an instance of D7 Digital Machine Event with an object, the D8 Digital Device, which happened with, e.g a capturing event that happened on/with a digital camera, etc.

Properties:
-
Examples:
-</rdfs:comment>
    </owl:ObjectProperty>
    


    <!-- http://www.semanticweb.org/vitto/ontologies/2024/9/PODS_1#L17_measured_thing_of_type_(was_type_of_thing_measured_by) -->


    <owl:ObjectProperty rdf:about="http://www.semanticweb.org/vitto/ontologies/2024/9/PODS_1#L17_measured_thing_of_type_(was_type_of_thing_measured_by)">
        <rdfs:subPropertyOf rdf:resource="http://www.semanticweb.org/vitto/ontologies/2024/9/PODS_1#P125_used_object_of_type_(was_type_of_object_used_in)"/>
        <rdfs:domain rdf:resource="http://www.cidoc-crm.org/extensions/crmdig/versions/4.0/D11_Digital_Measurement_Event#D11_Digital_Measurement_Event"/>
        <rdfs:range rdf:resource="http://cidoc-crm.org/cidoc-crm/7.1.3/E55_Type#E55_Type"/>
        <rdfs:comment>URI: http://www.cidoc-crm.org/extensions/crmdig/versions/4.0/L17_measured_thing_of_type

Domain:
D11 Digital Measurement Event
Range:
E55 Type
SubProperty Of:
E7 Activity. P125 used object of type (was type of object used in): E55 Type
SuperProperty Of:
-
Quantification:
-
Scope Note:
This property associates an instance of D11 Digital Measurement Event with the instance of E55Type of object to which it applied.

Properties:
-
Examples:
-</rdfs:comment>
    </owl:ObjectProperty>
    


    <!-- http://www.semanticweb.org/vitto/ontologies/2024/9/PODS_1#L19_stores_(is_stored_on) -->


    <owl:ObjectProperty rdf:about="http://www.semanticweb.org/vitto/ontologies/2024/9/PODS_1#L19_stores_(is_stored_on)">
        <rdfs:subPropertyOf rdf:resource="http://www.semanticweb.org/vitto/ontologies/2024/9/PODS_1#P128_carries_(is_carried_by)"/>
        <rdfs:domain rdf:resource="http://www.cidoc-crm.org/extensions/crmdig/versions/4.0/D13_Digital_Information_Carrier#D13_Digital_Information_Carrier"/>
        <rdfs:range rdf:resource="http://www.cidoc-crm.org/extensions/crmdig/versions/4.0/D1_Digital_Object#D1_Digital_Object"/>
        <rdfs:comment>URI: http://www.cidoc-crm.org/extensions/crmdig/versions/4.0/L19_stores

Domain:
D13 Digital Information Carrier
Range:
D1 Digital Object
SubProperty Of:
E18 Physical Thing. P128 carries (is carried by): E90 Symbolic Object
SuperProperty Of:
-
Quantification:
-
Scope Note:
This property associates an instance of a D13 Digital Information Carrier with the instance of Digital Object that is stored on it.

Properties:
-
Examples:
-</rdfs:comment>
    </owl:ObjectProperty>
    


    <!-- http://www.semanticweb.org/vitto/ontologies/2024/9/PODS_1#L1_digitized_(was_digitized_by) -->


    <owl:ObjectProperty rdf:about="http://www.semanticweb.org/vitto/ontologies/2024/9/PODS_1#L1_digitized_(was_digitized_by)">
        <rdfs:subPropertyOf rdf:resource="http://www.semanticweb.org/vitto/ontologies/2024/9/PODS_1#P39_measured_(was_measured_by)"/>
        <rdfs:domain rdf:resource="http://www.cidoc-crm.org/extensions/crmdig/versions/4.0/D2_Digitization_Process#D2_Digitization_Process"/>
        <rdfs:range rdf:resource="http://cidoc-crm.org/cidoc-crm/7.1.3/E18_Physical_Thing#E18_Physical_Thing"/>
        <rdfs:comment>URI: http://www.cidoc-crm.org/extensions/crmdig/versions/4.0/L1_digitized

Domain:
D2 Digitization Process
Range:
E18 Physical Thing
SubProperty Of:
E16 Measurement. P39 measured (was measured by): E18 Physical Thing
SuperProperty Of:
-
Quantification:
-
Scope Note:
This property associates an instance of D2 Digitization Process with an instance of E18 Physical Thing which is a material thing.

Properties:
-
Examples:
-</rdfs:comment>
    </owl:ObjectProperty>
    


    <!-- http://www.semanticweb.org/vitto/ontologies/2024/9/PODS_1#L23_used_software_or_firmware_(was_software_or_firmware_used_by) -->


    <owl:ObjectProperty rdf:about="http://www.semanticweb.org/vitto/ontologies/2024/9/PODS_1#L23_used_software_or_firmware_(was_software_or_firmware_used_by)">
        <rdfs:subPropertyOf rdf:resource="http://www.semanticweb.org/vitto/ontologies/2024/9/PODS_1#P16_used_specific_object_(was_used_for)"/>
        <rdfs:domain rdf:resource="http://www.cidoc-crm.org/extensions/crmdig/versions/4.0/D7_Digital_Machine_Event#D7_Digital_Machine_Event"/>
        <rdfs:range rdf:resource="http://www.cidoc-crm.org/extensions/crmdig/versions/4.0/D14_Software#D14_Software"/>
        <rdfs:comment>URI: http://www.cidoc-crm.org/extensions/crmdig/versions/4.0/L23_used_software_or_firmware

Domain:
D7 Digital Machine Event
Range:
D14 Software
SubProperty Of:
E7 Activity. P16 used specific object (was used for): E70 Thing
SuperProperty Of:
-
Quantification:
-
Scope Note:
This property associates an instance of D7 Digital Machine Event with the instance of D14 Software that had used.

Properties:
-
Examples:
-</rdfs:comment>
    </owl:ObjectProperty>
    


    <!-- http://www.semanticweb.org/vitto/ontologies/2024/9/PODS_1#O24_measured_(was_measured_by) -->


    <owl:ObjectProperty rdf:about="http://www.semanticweb.org/vitto/ontologies/2024/9/PODS_1#O24_measured_(was_measured_by)">
        <rdfs:subPropertyOf rdf:resource="http://www.semanticweb.org/vitto/ontologies/2024/9/PODS_1#O8_observed_(was_observed_by)"/>
        <rdfs:domain rdf:resource="http://www.cidoc-crm.org/extensions/crmsci/versions/2.0/S21_Measurement#S21_Measurement"/>
        <rdfs:range rdf:resource="http://www.cidoc-crm.org/extensions/crmsci/versions/2.0/S15_Observable_Entity#S15_Observable_Entity"/>
        <rdfs:comment>RI (forward direction):	http://www.cidoc-crm.org/extensions/crmsci/O24_measured
URI (inverse direction):	http://www.cidoc-crm.org/extensions/crmsci/O24i_was_measured_by
Domain:
S21 Measurement
Range:
S15 Observable Entity
SubProperty Of:
S4 Observation. O8 observed (was observed by): S15 Observable Entity
SuperProperty Of:
E16 Measurement. P39 measured (was measured by): E18 Physical Thing
Quantification:
many to one, necessary (1,1:0,n)
Scope Note:
This property associates an instance of S21 Measurement with the instance of S15 Observable Entity to which it applied. An instance of S15 Observable Entity may be measured more than once. Material and immaterial things and processes may be measured, e.g. the number of words in a text, or the duration of an event.

Properties:
-
Examples:
The sensor measurement by IGME in 1999 (S21) measured the landslide displacement (S15) in the area of Parnitha (Lucchese et al., 2013; Kritikos et al., 2013; InGeoCloudS, 2012; InGeoCloudS, 2013)</rdfs:comment>
    </owl:ObjectProperty>
    


    <!-- http://www.semanticweb.org/vitto/ontologies/2024/9/PODS_1#O8_observed_(was_observed_by) -->


    <owl:ObjectProperty rdf:about="http://www.semanticweb.org/vitto/ontologies/2024/9/PODS_1#O8_observed_(was_observed_by)">
        <rdfs:subPropertyOf rdf:resource="http://www.semanticweb.org/vitto/ontologies/2024/9/PODS_1#P140_assigned_attribute_to_(was_attributed_by)"/>
        <rdfs:comment>URI (forward direction):	http://www.cidoc-crm.org/extensions/crmsci/O8_observed
URI (inverse direction):	http://www.cidoc-crm.org/extensions/crmsci/O8i_was_observed_by
Domain:
S4 Observation
Range:
S15 Observable Entity
SubProperty Of:
E13 Attribute Assignment. P140 assigned attribute to (was attributed by): E1 CRM Entity
SuperProperty Of:
S21 Measurement. O24 measured (was measured by): S15 Observable Entity
S23 Position Determination. O32 determined position of (was located by): S15 Observable Entity
Quantification:
many to one, necessary (1,1:0,n)
Scope Note:
This property associates an instance of S4 Observation with an instance of S15 Observable Entity that was observed. Specifically it describes that a thing, a feature, a phenomenon or its reaction is observed by an activity of Observation.

Properties:
-
Examples:
The engineers’ observation on the slope of Panagopoula coastal site, near Patras, on the 25th–26th April 1971 and the 3rd May 1971(S4) observed the rotational landslide at the same site (S15) (Tavoularis et al., 2017).
The survey (S4) of Sinai MS GREEK 418 observed a detached triple-braided clasp strap (S15) (Honey and Pickwoad, 2010).</rdfs:comment>
    </owl:ObjectProperty>
    


    <!-- http://www.semanticweb.org/vitto/ontologies/2024/9/PODS_1#P106_is_composed_of_(forms_part_of) -->


    <owl:ObjectProperty rdf:about="http://www.semanticweb.org/vitto/ontologies/2024/9/PODS_1#P106_is_composed_of_(forms_part_of)">
        <rdfs:domain rdf:resource="http://cidoc-crm.org/cidoc-crm/7.1.3/E90_Symbolic_Object#E90_Symbolic_Object"/>
        <rdfs:range rdf:resource="http://cidoc-crm.org/cidoc-crm/7.1.3/E90_Symbolic_Object#E90_Symbolic_Object"/>
        <rdfs:comment>URI (forward direction):	http://www.cidoc-crm.org/cidoc-crm/P106_is_composed_of
URI (inverse direction):	http://www.cidoc-crm.org/cidoc-crm/P106i_forms_part_of
Domain:
E90 Symbolic Object
Range:
E90 Symbolic Object
SubProperty Of:
-
SuperProperty Of:
E73 Information Object. P165 incorporates (is incorporated in): E90 Symbolic Object
Quantification:
many to many (0,n:0,n)

Scope Note:
This property associates an instance of E90 Symbolic Object with a part of it that is by itself an instance of E90 Symbolic Object, such as fragments of texts or clippings from an image.

This property is transitive asymmetric.

Properties:
-
Examples:
This Scope note of property P106 (E33) is composed of ‘fragments of texts’ (E33).
‘recognizable’ (E90) is composed of ‘ecognizabl’ (E90).</rdfs:comment>
    </owl:ObjectProperty>
    


    <!-- http://www.semanticweb.org/vitto/ontologies/2024/9/PODS_1#P108_has_produced_(was_produced_by) -->


    <owl:ObjectProperty rdf:about="http://www.semanticweb.org/vitto/ontologies/2024/9/PODS_1#P108_has_produced_(was_produced_by)">
        <rdfs:subPropertyOf rdf:resource="http://www.semanticweb.org/vitto/ontologies/2024/9/PODS_1#P31_has_modified_(was_modified_by)"/>
        <rdfs:domain rdf:resource="http://www.semanticweb.org/vitto/ontologies/2024/9/PODS_1#E12_Production"/>
        <rdfs:range rdf:resource="http://cidoc-crm.org/cidoc-crm/7.1.3/E24_Physical_Human-Made_Thing#E24_Physical_Human-Made_Thing"/>
        <rdfs:comment>URI (forward direction):	http://www.cidoc-crm.org/cidoc-crm/P108_has_produced
URI (inverse direction):	http://www.cidoc-crm.org/cidoc-crm/P108i_was_produced_by
Domain:
E12 Production
Range:
E24 Physical Human-Made Thing
SubProperty Of:
E11 Modification. P31 has modified (was modified by): E18 Physical Thing
E63 Beginning of Existence. P92 brought into existence (was brought into existence by): E77 Persistent Item
SuperProperty Of:
-
Quantification:
one to many, necessary, dependent (1,n:1,1)

Scope Note:
This property identifies the instance of E24 Physical Human-Made Thing that came into existence as a result of the instance of E12 Production.

The identity of an instance of E24 Physical Human-Made Thing is not defined by its matter, but by its existence as a subject of documentation. An E12 Production can result in the creation of multiple instances of E24 Physical Human-Made Thing.

Properties:
-
Examples:
The building of Rome (E12) has produced the Colosseum (E24). (Hopkins &amp; Beard, 2011)</rdfs:comment>
    </owl:ObjectProperty>
    


    <!-- http://www.semanticweb.org/vitto/ontologies/2024/9/PODS_1#P10_falls_within_(contains) -->


    <owl:ObjectProperty rdf:about="http://www.semanticweb.org/vitto/ontologies/2024/9/PODS_1#P10_falls_within_(contains)">
        <rdfs:subPropertyOf rdf:resource="http://www.semanticweb.org/vitto/ontologies/2024/9/PODS_1#P132_spatiotemporally_overlaps_with"/>
        <rdfs:comment>URI (forward direction):	http://www.cidoc-crm.org/cidoc-crm/P10_falls_within
URI (inverse direction):	http://www.cidoc-crm.org/cidoc-crm/P10i_contains
Domain:
E92 Spacetime Volume
Range:
E92 Spacetime Volume
SubProperty Of:
E92 Spacetime Volume. P132 spatiotemporally overlaps with: E92 Spacetime Volume
SuperProperty Of:
E93 Presence. P166 was a presence of (had presence): E92 Spacetime Volume
E4 Period. P9i forms part of (consists of): E4 Period
Quantification:
many to many, necessary, dependent (1,n:1,n)

Scope Note:
This property associates an instance of E92 Spacetime Volume with another instance of E92 Spacetime Volume that falls within the latter. In other words, all points in the former are also points in the latter.

This property is transitive and reflexive.

Properties:
-
Examples:
The Great Plague (E4) falls within The Gothic period (E4). (Porter, 2009)</rdfs:comment>
    </owl:ObjectProperty>
    


    <!-- http://www.semanticweb.org/vitto/ontologies/2024/9/PODS_1#P11_had_participant_(participated_in) -->


    <owl:ObjectProperty rdf:about="http://www.semanticweb.org/vitto/ontologies/2024/9/PODS_1#P11_had_participant_(participated_in)">
        <rdfs:subPropertyOf rdf:resource="http://www.semanticweb.org/vitto/ontologies/2024/9/PODS_1#P12_occurred_in_the_presence_of_(was_present_at)"/>
        <rdfs:comment>URI (forward direction):	http://www.cidoc-crm.org/cidoc-crm/P11_had_participant
URI (inverse direction):	http://www.cidoc-crm.org/cidoc-crm/P11i_participated_in
Domain:
E5 Event
Range:
E39 Actor
SubProperty Of:
E5 Event. P12 occurred in the presence of (was present at): E77 Persistent Item
SuperProperty Of:
E7 Activity. P14 carried out by (performed): E39 Actor
E67 Birth. P96 by mother (gave birth): E21 Person
E68 Dissolution. P99 dissolved (was dissolved by): E74 Group
E85 Joining. P143 joined (was joined by): E39 Actor
E85 Joining. P144 joined with (gained member by): E74 Group
E86 Leaving. P145 separated (left by): E39 Actor
E86 Leaving. P146 separated from (lost member by): E74 Group
E66 Formation. P151 was formed from (participated in): E74 Group
Quantification:
many to many (0,n:0,n)

Scope Note:
This property describes the active or passive participation of instances of E39 Actors in an instance of E5 Event.

It documents known events in which an instance of E39 Actor has participated during the course of that actor’s life or history. The instances of E53 Place and E52 Time-Span where and when these events happened provide constraints about the presence of the related instances of E39 Actor in the past. Collective actors, i.e. instances of E74 Group, may physically participate in events via their representing instances of E21 Persons only. The participation of multiple actors in an event is most likely an indication of their acquaintance and interaction.

The property implies that the actor was involved in the event but does not imply any causal relationship. For instance, someone having been portrayed can be said to have participated in the creation of the portrait.

Properties:
-
Examples:
Napoleon (E21) participated in The Battle of Waterloo (E7). (Dawson, 2018)
Maria (E21) participated in Photographing of Maria (E7). (fictitious)</rdfs:comment>
    </owl:ObjectProperty>
    


    <!-- http://www.semanticweb.org/vitto/ontologies/2024/9/PODS_1#P125_used_object_of_type_(was_type_of_object_used_in) -->


    <owl:ObjectProperty rdf:about="http://www.semanticweb.org/vitto/ontologies/2024/9/PODS_1#P125_used_object_of_type_(was_type_of_object_used_in)">
        <rdfs:comment>URI (forward direction):	http://www.cidoc-crm.org/cidoc-crm/P125_used_object_of_type
URI (inverse direction):	http://www.cidoc-crm.org/cidoc-crm/P125i_was_type_of_object_used_in
Domain:
E7 Activity
Range:
E55 Type
SubProperty Of:
-
SuperProperty Of:
E7 Activity. P32 used general technique (was technique of): E55 Type
Quantification:
many to many (0,n:0,n)

Scope Note:
This property associates an instance of E7 Activity to an instance of E55 Type, which classifies an instance of E70 Thing used in an instance of E7 Activity, when the specific instance is either unknown or not of interest, such as use of &apos;a hammer&apos;.

This property is a shortcut of the more fully developed path from E7 Activity through P16 used specific object, E70 Thing, P2 has type, to E55 Type.

Properties:
-
Examples:
The English archers’ activity in the Battle of Agincourt (E7) used object of type long bow (E55). (Curry, 2015)</rdfs:comment>
    </owl:ObjectProperty>
    


    <!-- http://www.semanticweb.org/vitto/ontologies/2024/9/PODS_1#P128_carries_(is_carried_by) -->


    <owl:ObjectProperty rdf:about="http://www.semanticweb.org/vitto/ontologies/2024/9/PODS_1#P128_carries_(is_carried_by)">
        <rdfs:subPropertyOf rdf:resource="http://www.semanticweb.org/vitto/ontologies/2024/9/PODS_1#P130_shows_features_of_(features_are_also_found_on)"/>
        <rdfs:comment>URI (forward direction):	http://www.cidoc-crm.org/cidoc-crm/P128_carries
URI (inverse direction):	http://www.cidoc-crm.org/cidoc-crm/P128i_is_carried_by
Domain:
E18 Physical Thing
Range:
E90 Symbolic Object
SubProperty Of:
E70 Thing. P130 shows features of (features are also found on): E70 Thing
SuperProperty Of:
E24 Physical Human-Made Thing. P65 shows visual item (is shown by): E36 Visual Item
Quantification:
many to many (0,n:0,n)

Scope Note:
This property identifies an instance E90 Symbolic Object carried by an instance of E18 Physical Thing. Since an instance of E90 Symbolic Object is defined as an immaterial idealization over potentially multiple carriers, any individual realization on a particular physical carrier may be defective, due to deterioration or shortcomings in the process of creating the realization compared to the intended ideal. As long as such defects do not substantially affect the complete recognition of the respective symbolic object, it is still regarded as carrying an instance of this E90 Symbolic Object. If these defects are of scholarly interest, the particular realization can be modelled as an instance of E25 Human-Made Feature. Note, that any instance of E90 Symbolic Object incorporated (P165) in the carried symbolic object is also carried by the same instance of E18 Physical Thing.

Properties:
-
Examples:
Matthew’s paperback copy of Reach for the Sky (E18) carries the text of Reach for the Sky (E73). [see also: (Brickhill, 2001)] (fictitious)</rdfs:comment>
    </owl:ObjectProperty>
    


    <!-- http://www.semanticweb.org/vitto/ontologies/2024/9/PODS_1#P12_occurred_in_the_presence_of_(was_present_at) -->


    <owl:ObjectProperty rdf:about="http://www.semanticweb.org/vitto/ontologies/2024/9/PODS_1#P12_occurred_in_the_presence_of_(was_present_at)">
        <rdfs:comment>URI (forward direction):	http://www.cidoc-crm.org/cidoc-crm/P12_occurred_in_the_presence_of
URI (inverse direction):	http://www.cidoc-crm.org/cidoc-crm/P12i_was_present_at
Domain:
E5 Event
Range:
E77 Persistent Item
SubProperty Of:
-
SuperProperty Of:
E5 Event. P11 had participant (participated in): E39 Actor
E7 Activity. P16 used specific object (was used for): E70 Thing
E9 Move. P25 moved (moved by): E19 Physical Object
E11 Modification. P31 has modified (was modified by): E18 Physical Thing
E63 Beginning of Existence. P92 brought into existence (was brought into existence by): E77 Persistent Item
E64 End of Existence. P93 took out of existence (was taken out of existence by): E77 Persistent Item
E80 Part Removal. P113 removed (was removed by): E18 Physical Thing
Quantification:
many to many, necessary (1,n:0,n)

Scope Note:
This property describes the active or passive presence of an E77 Persistent Item in an instance of E5 Event without implying any specific role.

It documents known events in which an instance of E77 Persistent Item was present during the course of its life or history. For example, an object may be the desk, now in a museum, on which a treaty was signed. The instance of E53 Place and the instance of E52 Time-Span where and when these events happened provide constraints about the presence of the related instance E77 Persistent Item in the past. Instances of E90 Symbolic Object, in particular information objects, are physically present in events via at least one of the instances of E18 Physical Thing carrying them. Note, that the human mind can be such a carrier. A precondition for a transfer of information to a person or another new physical carrier is the presence of the respective information object and this person or physical thing in one event.

Properties:
-
Examples:
Deckchair 42 (E19) was present at the sinking of the Titanic (E5). (Aldridge, 2008)</rdfs:comment>
    </owl:ObjectProperty>
    


    <!-- http://www.semanticweb.org/vitto/ontologies/2024/9/PODS_1#P130_shows_features_of_(features_are_also_found_on) -->


    <owl:ObjectProperty rdf:about="http://www.semanticweb.org/vitto/ontologies/2024/9/PODS_1#P130_shows_features_of_(features_are_also_found_on)">
        <rdfs:comment>URI (forward direction):	http://www.cidoc-crm.org/cidoc-crm/P130_shows_features_of
URI (inverse direction):	http://www.cidoc-crm.org/cidoc-crm/P130i_features_are_also_found_on
Domain:
E70 Thing
Range:
E70 Thing
SubProperty Of:
-
SuperProperty Of:
E18 Physical Thing. P128 carries (is carried by): E90 Symbolic Object
E33 Linguistic Object. P73i is translation of (has translation): E33 Linguistic Object
Quantification:
many to many (0,n:0,n)

Scope Note:
This property generalises the notions of &apos;copy of&apos; and &apos;similar to&apos; into a directed relationship, where the domain expresses the derivative or influenced item and the range the source or influencing item, if such a direction can be established. The property can also be used to express similarity in cases that can be stated between two objects only, without historical knowledge about its reasons. The property expresses a symmetric relationship in case no direction of influence can be established either from evidence on the item itself or from historical knowledge. This holds in particular for siblings of a derivation process from a common source or non-causal cultural parallels, such as some weaving patterns.

The P130.1 kind of similarity property of the P130 shows features of (features are also found on) property enables the relationship between the domain and the range to be further clarified, in the sense from domain to range, if applicable. For example, it may be expressed if both items are product &apos;of the same mould&apos;, or if two texts &apos;contain identical paragraphs&apos;.

If the reason for similarity is a sort of derivation process, i.e. that the creator has used or had in mind the form of a particular thing during the creation or production, this process should be explicitly modelled. In these cases, P130 shows features of can be regarded as a shortcut of such a process. However, the current model does not contain any path specific enough to infer this property. Specializations of the CIDOC CRM may however be more explicit, for instance describing the use of moulds etc.

This property is not transitive. This property is irreflexive.

Properties:
P130.1 kind of similarity: E55 Type

Examples:
Mary Lamb’s Cymbeline from Charles and Mary Lamb’s Tales from Shakespeare (E89) shows features of William Shakespeare’s Cymbeline (E89). (Carrington, 1954)
The audio recording of Dante Alighieri’s La divina commedia read by Enrico de Negri (E73) shows features of the text of Dante Alighieri’s La divina commedia (E89). (Alighieri, 1956)</rdfs:comment>
    </owl:ObjectProperty>
    


    <!-- http://www.semanticweb.org/vitto/ontologies/2024/9/PODS_1#P134_continued_(was_continued_by) -->


    <owl:ObjectProperty rdf:about="http://www.semanticweb.org/vitto/ontologies/2024/9/PODS_1#P134_continued_(was_continued_by)">
        <rdfs:subPropertyOf rdf:resource="http://www.semanticweb.org/vitto/ontologies/2024/9/PODS_1#P15_was_influenced_by_(influenced)"/>
        <rdfs:domain rdf:resource="http://cidoc-crm.org/cidoc-crm/7.1.3/E7_Activity#E7_Activity"/>
        <rdfs:range rdf:resource="http://cidoc-crm.org/cidoc-crm/7.1.3/E7_Activity#E7_Activity"/>
        <rdfs:comment>URI (forward direction):	http://www.cidoc-crm.org/cidoc-crm/P134_continued
URI (inverse direction):	http://www.cidoc-crm.org/cidoc-crm/P134i_was_continued_by
Domain:
E7 Activity
Range:
E7 Activity
SubProperty Of:
E7 Activity. P15 was influenced by (influenced): E1 CRM Entity
E2 Temporal Entity. P176i starts after the start of (starts before the start of): E2 Temporal Entity
SuperProperty Of:
-
Quantification:
many to many (0,n:0,n)

Scope Note:
This property associates two instances of E7 Activity, where the domain is considered as an intentional continuation of the range. A continuation of an activity may happen when the continued activity is still ongoing or after the continued activity has completely ended. The continuing activity may have started already before it decided to continue the other one. Continuation implies a coherence of intentions and outcomes of the involved activities.

This property is not transitive. This property is asymmetric.

Properties:
-
Examples:
The construction of the Kölner Dom (Cologne Cathedral), abandoned in the 15th century (E7), was continued by construction in the 19th century (E7). [The construction in the 19th century adapted the initial plans so as to preserve the intended appearance.] (Wolff, 1999)</rdfs:comment>
    </owl:ObjectProperty>
    


    <!-- http://www.semanticweb.org/vitto/ontologies/2024/9/PODS_1#P140_assigned_attribute_to_(was_attributed_by) -->


    <owl:ObjectProperty rdf:about="http://www.semanticweb.org/vitto/ontologies/2024/9/PODS_1#P140_assigned_attribute_to_(was_attributed_by)">
        <rdfs:comment>URI (forward direction):	http://www.cidoc-crm.org/cidoc-crm/P140_assigned_attribute_to
URI (inverse direction):	http://www.cidoc-crm.org/cidoc-crm/P140i_was_attributed_by
Domain:
E13 Attribute Assignment
Range:
E1 CRM Entity
SubProperty Of:
-
SuperProperty Of:
E14 Condition Assessment. P34 concerned (was assessed by): E18 Physical Thing
E16 Measurement. P39 measured (was measured by): E18 Physical Thing
E17 Type Assignment. P41 classified (was classified by): E1 CRM Entity
Quantification:
many to many (0,n:0,n)

Scope Note:
This property associates an instance of E13 Attribute Assignment with the instance of E1 CRM Entity about which it made an attribution. The instance of E1 CRM Entity plays the role of the domain of the attribution.

The kind of attribution made should be documented using P177 assigned property of type (is type of property assigned).

Properties:
-
Examples:
The Current Ownership Assessment of Martin Doerr’s silver cup February 1997 (E13) assigned attribute to Martin Doerr’s silver cup (E22). (fictitious)
The Identifier Assignment on 1st June 1997 of the silver cup donated by Martin Doerr (E15) assigned attribute to silver cup 232 (E22). (fictitious)
The examination of MS Sinai Greek 418 (E13) assigned attribute to MS Sinai Greek 418 (E22). (Honey and Pickwoad, 2010)</rdfs:comment>
    </owl:ObjectProperty>
    


    <!-- http://www.semanticweb.org/vitto/ontologies/2024/9/PODS_1#P141_assigned_(was_assigned_by) -->


    <owl:ObjectProperty rdf:about="http://www.semanticweb.org/vitto/ontologies/2024/9/PODS_1#P141_assigned_(was_assigned_by)">
        <rdfs:comment>URI (forward direction):	http://www.cidoc-crm.org/cidoc-crm/P141_assigned
URI (inverse direction):	http://www.cidoc-crm.org/cidoc-crm/P141i_was_assigned_by
Domain:
E13 Attribute Assignment
Range:
E1 CRM Entity
SubProperty Of:
-
SuperProperty Of:
E14 Condition Assessment. P35 has identified (was identified by): E3 Condition State
E15 Identifier Assignment. P37 assigned (was assigned by): E42 Identifier
E15 Identifier Assignment. P38 deassigned (was deassigned by): E42 Identifier
E16 Measurement. P40 observed dimension (was observed in): E54 Dimension
E17 Type Assignment. P42 assigned (was assigned by): E55 Type
Quantification:
many to many (0,n:0,n)

Scope Note:
This property associates an instance of E13 Attribute Assignment with the instance of E1 CRM Entity used in the attribution. The instance of E1 CRM Entity here plays the role of the range of the attribution.

The kind of attribution made should be documented using P177 assigned property of type (is type of property assigned).

Properties:
-
Examples:
The Current Ownership Assessment of Martin Doerr’s silver cup February 1997 (E13) assigned Martin Doerr (E21). (fictitious)
The Identifier Assignment on 1st June 1997 of the silver cup donated by Martin Doerr (E15) assigned 232 (E42). (fictitious)
The examination of MS Sinai Greek 418 (E13) assigned unsupported (E55.) (Honey &amp; Pickwoad, 2010)</rdfs:comment>
    </owl:ObjectProperty>
    


    <!-- http://www.semanticweb.org/vitto/ontologies/2024/9/PODS_1#P14_carried_out_by_(performed) -->


    <owl:ObjectProperty rdf:about="http://www.semanticweb.org/vitto/ontologies/2024/9/PODS_1#P14_carried_out_by_(performed)">
        <rdfs:subPropertyOf rdf:resource="http://www.semanticweb.org/vitto/ontologies/2024/9/PODS_1#P11_had_participant_(participated_in)"/>
        <rdfs:domain rdf:resource="http://cidoc-crm.org/cidoc-crm/7.1.3/E7_Activity#E7_Activity"/>
        <rdfs:range rdf:resource="http://cidoc-crm.org/cidoc-crm/7.1.3/E39_Actor#E39_Actor"/>
        <rdfs:comment>URI (forward direction):	http://www.cidoc-crm.org/cidoc-crm/P14_carried_out_by
URI (inverse direction):	http://www.cidoc-crm.org/cidoc-crm/P14i_performed
Domain:
E7 Activity
Range:
E39 Actor
SubProperty Of:
E5 Event. P11 had participant (participated in): E39 Actor
SuperProperty Of:
E8 Acquisition. P22 transferred title to (acquired title through): E39 Actor
E8 Acquisition. P23 transferred title from (surrendered title through): E39 Actor
E10 Transfer of Custody. P28 custody surrendered by (surrendered custody through): E39 Actor
E10 Transfer of Custody. P29 custody received by (received custody through): E39 Actor
Quantification:
many to many, necessary (1,n:0,n)

Scope Note:
This property describes the active participation of an instance of E39 Actor in an instance of E7 Activity.

It implies causal or legal responsibility. The P14.1 in the role of property of the property specifies the nature of an Actor’s participation.

Properties:
P14.1 in the role of: E55 Type

Examples:
The painting of the Sistine Chapel (E7) carried out by Michelangelo Buonaroti (E21) in the role of master craftsman (E55). (Goldscheider, 1953)</rdfs:comment>
    </owl:ObjectProperty>
    


    <!-- http://www.semanticweb.org/vitto/ontologies/2024/9/PODS_1#P15_was_influenced_by_(influenced) -->


    <owl:ObjectProperty rdf:about="http://www.semanticweb.org/vitto/ontologies/2024/9/PODS_1#P15_was_influenced_by_(influenced)">
        <rdfs:comment>URI (forward direction):	http://www.cidoc-crm.org/cidoc-crm/P15_was_influenced_by
URI (inverse direction):	http://www.cidoc-crm.org/cidoc-crm/P15i_influenced
Domain:
E7 Activity
Range:
E1 CRM Entity
SubProperty Of:
-
SuperProperty Of:
E7 Activity. P16 used specific object (was used for): E70 Thing
E7 Activity. P17 was motivated by (motivated): E1 CRM Entity
E7 Activity. P134 continued (was continued by): E7 Activity
E83 Type Creation. P136 was based on (supported type creation): E1 CRM Entity
Quantification:
many to many (0,n:0,n)

Scope Note:
This is a high-level property, which captures the relationship between an instance of E7 Activity and anything, that is, an instance of E1 CRM Entity, that may have had some bearing upon it.

The property has more specific subproperties.

Properties:
-
Examples:
The designing of the Sydney Harbour Bridge (E7) was influenced by the Tyne Bridge (E22). (Dorman Long, 1932)</rdfs:comment>
    </owl:ObjectProperty>
    


    <!-- http://www.semanticweb.org/vitto/ontologies/2024/9/PODS_1#P161_has_spatial_projection_(is_spatial_projection_of) -->


    <owl:ObjectProperty rdf:about="http://www.semanticweb.org/vitto/ontologies/2024/9/PODS_1#P161_has_spatial_projection_(is_spatial_projection_of)">
        <rdfs:domain rdf:resource="http://cidoc-crm.org/cidoc-crm/7.1.3/E4_Period#E4_Period"/>
        <rdfs:range rdf:resource="http://cidoc-crm.org/cidoc-crm/7.1.3/E53_Place#E53_Place"/>
        <rdfs:comment>URI (forward direction):	http://www.cidoc-crm.org/cidoc-crm/P161_has_spatial_projection
URI (inverse direction):	http://www.cidoc-crm.org/cidoc-crm/P161i_is_spatial_projection_of
Domain:
E92 Spacetime Volume
Range:
E53 Place
SubProperty Of:
-
SuperProperty Of:
-
Quantification:
many to many, necessary (1,n:0,n)

Scope Note:
This property associates an instance of E92 Spacetime Volume with an instance of E53 Place that is the result of the spatial projection of the instance of the E92 Spacetime Volume on a reference space.

In general, there can be more than one useful reference space (for reference space see P156 occupies and P157 is at rest relative to) to describe the spatial projection of a spacetime volume, for example, in describing a sea battle, the difference between the battle ship and the seafloor as reference spaces. Thus, it can be seen that the projection is not unique.

The spatial projection is the actual spatial coverage of a spacetime volume, which normally has fuzzy boundaries except for instances of E92 Spacetime Volume which are geometrically defined in the same reference system as the range of this property and are an exception to this and do not have fuzzy boundaries. Modelling explicitly fuzzy spatial projections serves therefore as a common topological reference of different spatial approximations rather than absolute geometric determination, for instance for relating outer or inner spatial boundaries for the respective spacetime volumes.

The spatial projection is unique with respect to the reference system. For instance, there is exactly one spatial projection of Lord Nelson’s dying relative to the ship HMS Victory, i.e. the location of his body relative to the ship HMS Victory at the time of his death.

In case the domain of an instance of P161 has spatial projection is an instance of E4 Period, the spatial projection describes all areas that period was ever present at, for instance, the Roman Empire.

This property is part of the fully developed path from E18 Physical Thing through P196 defines, E92 Spacetime Volume, P161 has spatial projection to E53 Place, which in turn is implied by P156 occupies (is occupied by).

Properties:
-
Examples:
The Roman Empire (E4) has spatial projection all areas ever claimed by Rome (E53). (Clare &amp; Edwards, 1992)</rdfs:comment>
    </owl:ObjectProperty>
    


    <!-- http://www.semanticweb.org/vitto/ontologies/2024/9/PODS_1#P169_defines_spacetime_volume_(spacetime_volume_is_defined_by) -->


    <owl:ObjectProperty rdf:about="http://www.semanticweb.org/vitto/ontologies/2024/9/PODS_1#P169_defines_spacetime_volume_(spacetime_volume_is_defined_by)">
        <rdfs:subPropertyOf rdf:resource="http://www.semanticweb.org/vitto/ontologies/2024/9/PODS_1#P1_is_identified_by_(identifies)"/>
        <rdfs:domain rdf:resource="http://cidoc-crm.org/cidoc-crm/7.1.3/E94_Space_Primitive#E94_Space_Primitive"/>
        <rdfs:range rdf:resource="http://www.cidoc-crm.org/cidoc-crm/E1_CRM_Entity#E1_CRM_Entity"/>
        <rdfs:comment>URI (forward direction):	-
URI (inverse direction):	http://www.cidoc-crm.org/cidoc-crm/P169i_spacetime_volume_is_defined_by
Domain:
E95 Spacetime Primitive
Range:
E92 Spacetime Volume
SubProperty Of:
E41 Appellation. P1i identifies (is identified by): E1 CRM Entity
SuperProperty Of:
-
Quantification:
many to one, necessary (1,1:0,n)

Scope Note:
This property associates an instance of E95 Spacetime Primitive with the instance of E92 Spacetime Volume it defines.

Properties:
-
Examples:
{40°30&apos;23&quot;N 21°14&apos;53&quot;E, 40°31&apos;40&quot;N 21°16&apos;43&quot;E, 200BC-2020AD} (E95) defines spacetime volume Martin’s spatiotemporal enclosure 2020 for the evolution of the settlement of today’s city of Kastoria, Greece, since its conquest by the Romans (E92). [A square covering the current built settlement structure of Kastoria, Greece, through the years 200BC to 2020AD, which includes the extents of earlier phases of the city]</rdfs:comment>
    </owl:ObjectProperty>
    


    <!-- http://www.semanticweb.org/vitto/ontologies/2024/9/PODS_1#P16_used_specific_object_(was_used_for) -->


    <owl:ObjectProperty rdf:about="http://www.semanticweb.org/vitto/ontologies/2024/9/PODS_1#P16_used_specific_object_(was_used_for)">
        <rdfs:subPropertyOf rdf:resource="http://www.semanticweb.org/vitto/ontologies/2024/9/PODS_1#P12_occurred_in_the_presence_of_(was_present_at)"/>
        <rdfs:subPropertyOf rdf:resource="http://www.semanticweb.org/vitto/ontologies/2024/9/PODS_1#P15_was_influenced_by_(influenced)"/>
        <rdfs:comment>URI (forward direction):	http://www.cidoc-crm.org/cidoc-crm/P16_used_specific_object
URI (inverse direction):	http://www.cidoc-crm.org/cidoc-crm/P16i_was_used_for
Domain:
E7 Activity
Range:
E70 Thing
SubProperty Of:
E5 Event. P12 occurred in the presence of (was present at): E77 Persistent Item
E7 Activity. P15 was influenced by (influenced): E1 CRM Entity
SuperProperty Of:
E7 Activity. P33 used specific technique (was used by): E29 Design or Procedure
E79 Part Addition. P111 added (was added by): E18 Physical Thing
E15 Identifier Assignment. P142 used constituent (was used in): E90 Symbolic Object
Quantification:
many to many (0,n:0,n)

Scope Note:
This property describes the use of material or immaterial things in a way essential to the performance or the outcome of an instance of E7 Activity.

This property typically applies to tools, instruments, moulds, raw materials and items embedded in a product. It implies that the presence of the object in question was a necessary condition for the action. For example, the activity of writing this text required the use of a computer. An immaterial thing can be used if at least one of its carriers is present. For example, the software tools on a computer.

Another example is the use of a particular name by a particular group of people over some span to identify a thing, such as a settlement. In this case, the physical carriers of this name are at least the people understanding its use.

Properties:
P16.1 mode of use: E55 Type

Examples:
The writing of the scope note of the CIDOC CRM property &apos;P16 used specific object&apos; contained in the CIDOC CRM version 4.1 (E7) used specific object Nicholas Crofts’ computer (E22) mode of use Typing Tool; Storage Medium (E55). [the original scope note was later extended in the CIDOC CRM version 4.3]
The people of Iraq calling the place identified by TGN ‘7017998’ (E7) used specific object &apos;Quyunjig&apos; (E41) mode of use current; vernacular (E55).</rdfs:comment>
    </owl:ObjectProperty>
    


    <!-- http://www.semanticweb.org/vitto/ontologies/2024/9/PODS_1#P17_was_motivated_by_(motivated) -->


    <owl:ObjectProperty rdf:about="http://www.semanticweb.org/vitto/ontologies/2024/9/PODS_1#P17_was_motivated_by_(motivated)">
        <rdfs:subPropertyOf rdf:resource="http://www.semanticweb.org/vitto/ontologies/2024/9/PODS_1#P15_was_influenced_by_(influenced)"/>
        <rdfs:domain rdf:resource="http://cidoc-crm.org/cidoc-crm/7.1.3/E7_Activity#E7_Activity"/>
        <rdfs:range rdf:resource="http://www.cidoc-crm.org/cidoc-crm/E1_CRM_Entity#E1_CRM_Entity"/>
        <rdfs:comment>URI (forward direction):	http://www.cidoc-crm.org/cidoc-crm/P17_was_motivated_by
URI (inverse direction):	http://www.cidoc-crm.org/cidoc-crm/P17i_motivated
Domain:
E7 Activity
Range:
E1 CRM Entity
SubProperty Of:
E7 Activity. P15 was influenced by (influenced): E1 CRM Entity
SuperProperty Of:
-
Quantification:
many to many (0,n:0,n)

Scope Note:
This property describes an item or items that are regarded as a reason for carrying out the instance of E7 Activity.

For example, the discovery of a large hoard of treasure may call for a celebration, an order from headquarters can start a military manoeuvre.

Properties:
-
Examples:
The resignation of the chief executive (E7) was motivated by the collapse of SwissAir (E68).
The coronation of Elizabeth II (E7) was motivated by the death of George VI (E69). (Strong, 2005)</rdfs:comment>
    </owl:ObjectProperty>
    


    <!-- http://www.semanticweb.org/vitto/ontologies/2024/9/PODS_1#P1_is_identified_by_(identifies) -->


    <owl:ObjectProperty rdf:about="http://www.semanticweb.org/vitto/ontologies/2024/9/PODS_1#P1_is_identified_by_(identifies)">
        <rdfs:comment>P1 is identified by (identifies)
URI (forward direction):	http://www.cidoc-crm.org/cidoc-crm/P1_is_identified_by
URI (inverse direction):	http://www.cidoc-crm.org/cidoc-crm/P1i_identifies
Domain:
E1 CRM Entity
Range:
E41 Appellation
SubProperty Of:
-
SuperProperty Of:
E1 CRM Entity. P48 has preferred identifier (is preferred identifier of): E42 Identifier
E71 Human-Made Thing. P102 has title (is title of): E35 Title
E53 Place. P168 place is defined by (defines place): E94 Space Primitive
E92 Spacetime Volume. P169i spacetime volume is defined by (defines spacetime volume): E95 Spacetime Primitive
E52 Time-Span. P170i time is defined by (defines time): E61 Time Primitive
Quantification:
many to many (0,n:0,n)

Scope Note:
This property describes the naming or identification of any real-world item by a name or any other identifier.

This property is intended for identifiers in general use, which form part of the world the model intends to describe, and not merely for internal database identifiers which are specific to a technical system, unless these latter also have a more general use outside the technical context. This property includes in particular identification by mathematical expressions such as coordinate systems used for the identification of instances of E53 Place. The property does not reveal anything about when, where and by whom this identifier was used. A more detailed representation can be made using the fully developed (i.e. indirect) path through E15 Identifier Assignment.

This property is a shortcut for the path from E1 CRM Entity through P140i was attributed by, E15 Identifier Assignment, P37 assigned to E42 Identifier.

It is also a shortcut for the path from E1 CRM Entity through P1 is identified by, E41 Appellation, P139 has alternative form to E41 Appellation.

Properties:
-
Examples:
The capital of Italy (E53) is identified by &apos;Rome&apos; (E41). (Leach, 2017)
Text 25014–32 (E33) is identified by &apos;The Decline and Fall of the Roman Empire&apos; (E35). (Gibbon, 2013)</rdfs:comment>
    </owl:ObjectProperty>
    


    <!-- http://www.semanticweb.org/vitto/ontologies/2024/9/PODS_1#P2__has_type_(is_type_of) -->


    <owl:ObjectProperty rdf:about="http://www.semanticweb.org/vitto/ontologies/2024/9/PODS_1#P2__has_type_(is_type_of)">
        <rdfs:domain rdf:resource="http://www.cidoc-crm.org/cidoc-crm/E1_CRM_Entity#E1_CRM_Entity"/>
        <rdfs:range rdf:resource="http://cidoc-crm.org/cidoc-crm/7.1.3/E55_Type#E55_Type"/>
        <rdfs:comment>URI (forward direction):	http://www.cidoc-crm.org/cidoc-crm/P2_has_type
URI (inverse direction):	http://www.cidoc-crm.org/cidoc-crm/P2i_is_type_of
Domain:
E1 CRM Entity
Range:
E55 Type
SubProperty Of:
-
SuperProperty Of:
E1 CRM Entity. P137 exemplifies (is exemplified by): E55 Type
E13 Attribute Assignment. P177 assigned property of type (is type of property assigned): E55 Type
Quantification:
many to many (0,n:0,n)

Scope Note:
This property allows sub-typing of CIDOC CRM entities –a form of specialisation – through the use of a terminological hierarchy, or thesaurus.

The CIDOC CRM is intended to focus on the high-level entities and relationships needed to describe data structures. Consequently, it does not specialise entities any further than is required for this immediate purpose. However, entities in the isA hierarchy of the CIDOC CRM may by specialised into any number of sub-entities, which can be defined in the E55 Type hierarchy. E41 Appellation, for example, may be specialised into &apos;e-mail address&apos;, &apos;telephone number&apos;, &apos;post office box&apos;, &apos;URL&apos;, etc., none of which figures explicitly in the CIDOC CRM class hierarchy. A comprehensive explanation about refining CIDOC CRM concepts by E55 Type is given in the section &apos;About Types&apos; in the section on &apos;Specific Modelling Constructs&apos; of this document.

This property is a shortcut for the path from E1 CRM Entity through P41i was classified by, E17 Type Assignment, P42 assigned to E55 Type.

Properties:
-
Examples:
&apos;enquiries@cidoc-crm.org&apos; (e41) has type e-mail address (e55). (fictitious)</rdfs:comment>
    </owl:ObjectProperty>
    


    <!-- http://www.semanticweb.org/vitto/ontologies/2024/9/PODS_1#P31_has_modified_(was_modified_by) -->


    <owl:ObjectProperty rdf:about="http://www.semanticweb.org/vitto/ontologies/2024/9/PODS_1#P31_has_modified_(was_modified_by)">
        <rdfs:subPropertyOf rdf:resource="http://www.semanticweb.org/vitto/ontologies/2024/9/PODS_1#P12_occurred_in_the_presence_of_(was_present_at)"/>
        <rdfs:comment>URI (forward direction):	http://www.cidoc-crm.org/cidoc-crm/P31_has_modified
URI (inverse direction):	http://www.cidoc-crm.org/cidoc-crm/P31i_was_modified_by
Domain:
E11 Modification
Range:
E18 Physical Thing
SubProperty Of:
E5 Event. P12 occurred in the presence of (was present at): E77 Persistent Item
SuperProperty Of:
E12 Production. P108 has produced (was produced by): E24 Physical Human-Made Thing
E79 Part Addition. P110 augmented (was augmented by): E18 Physical Thing
E80 Part Removal. P112 diminished (was diminished by): E18 Physical Thing
Quantification:
many to many, necessary (1,n:0,n)

Scope Note:
This property identifies the instance of E18 Physical Thing modified in an instance of E11 Modification.

Properties:
-
Examples:
The rebuilding of the German Reichstag in Berlin (E11) has modified the Reichstag in Berlin (E24). (Foster, 2000)</rdfs:comment>
    </owl:ObjectProperty>
    


    <!-- http://www.semanticweb.org/vitto/ontologies/2024/9/PODS_1#P33_used_specific_technique_(was_used_by) -->


    <owl:ObjectProperty rdf:about="http://www.semanticweb.org/vitto/ontologies/2024/9/PODS_1#P33_used_specific_technique_(was_used_by)">
        <rdfs:subPropertyOf rdf:resource="http://www.semanticweb.org/vitto/ontologies/2024/9/PODS_1#P16_used_specific_object_(was_used_for)"/>
        <rdfs:domain rdf:resource="http://cidoc-crm.org/cidoc-crm/7.1.3/E7_Activity#E7_Activity"/>
        <rdfs:range rdf:resource="http://cidoc-crm.org/cidoc-crm/7.1.3/E29_Design_or_Procedure#E29_Design_or_Procedure"/>
        <rdfs:comment>URI (forward direction):	http://www.cidoc-crm.org/cidoc-crm/P33_used_specific_technique
URI (inverse direction):	http://www.cidoc-crm.org/cidoc-crm/P33i_was_used_by
Domain:
E7 Activity
Range:
E29 Design or Procedure
SubProperty Of:
E7 Activity. P16 used specific object (was used for): E70 Thing
SuperProperty Of:
-
Quantification:
many to many (0,n:0,n)

Scope Note:
This property identifies a specific instance of E29 Design or Procedure in order to carry out an instance of E7 Activity or parts of it.

The property differs from P32 used general technique (was technique of) in that P33 refers to an instance of E29 Design or Procedure, which is a concrete information object in its own right rather than simply being a term or a method known by tradition.

Typical examples would include intervention plans for conservation or the construction plans of a building.

Properties:
-
Examples:
The ornamentation of silver cup 232 (E11) used specific technique ‘Instructions for golden chase work by A N Other’ (E29). (fictitious)
The rebuilding of the German Reichstag in Berlin (E11) used specific technique Architectural plans by Foster and Partners (E29). (Foster, 2000)</rdfs:comment>
    </owl:ObjectProperty>
    


    <!-- http://www.semanticweb.org/vitto/ontologies/2024/9/PODS_1#P39_measured_(was_measured_by) -->


    <owl:ObjectProperty rdf:about="http://www.semanticweb.org/vitto/ontologies/2024/9/PODS_1#P39_measured_(was_measured_by)">
        <rdfs:subPropertyOf rdf:resource="http://www.semanticweb.org/vitto/ontologies/2024/9/PODS_1#P140_assigned_attribute_to_(was_attributed_by)"/>
        <rdfs:comment>URI (forward direction):	http://www.cidoc-crm.org/cidoc-crm/P39_measured
URI (inverse direction):	http://www.cidoc-crm.org/cidoc-crm/P39i_was_measured_by
Domain:
E16 Measurement
Range:
E18 Physical Thing
SubProperty Of:
E13 Attribute Assignment. P140 assigned attribute to (was attributed by): E1 CRM Entity
SuperProperty Of:
-
Quantification:
many to one, necessary (1,1:0,n)

Scope Note:
This property associates an instance of E16 Measurement with the instance of E18 Physical Thing upon which it acted. The instance of E16 Measurement is specific to the measured object. An instance of E18 Physical Thing may be measured more than once with different results, constituting different instances of E16 Measurement.

Properties:
-
Examples:
The measurement of the height of silver cup 232 on 31st August 1997 (E16) measured silver cup 232 (E22). (fictitious)
The carbon 14 dating of the &apos;Schoeninger Speer II&apos; in 1996 (E16) measured the &apos;Schoeninger Speer II&apos; (E22). [The carbon 14 dating of an approximately 400.000 year old complete Old Palaeolithic wooden spear found in Schoeningen, Niedersachsen, Germany, in 1995. See also, E16 Measurement.] (Kouwenhoven, 1997)</rdfs:comment>
    </owl:ObjectProperty>
    


    <!-- http://www.semanticweb.org/vitto/ontologies/2024/9/PODS_1#P43_has_dimension_(is_dimension_of) -->


    <owl:ObjectProperty rdf:about="http://www.semanticweb.org/vitto/ontologies/2024/9/PODS_1#P43_has_dimension_(is_dimension_of)">
        <rdfs:domain rdf:resource="http://cidoc-crm.org/cidoc-crm/7.1.3/E70_Thing#E70_Thing"/>
        <rdfs:range rdf:resource="http://cidoc-crm.org/cidoc-crm/7.1.3/E54_Dimension#E54_Dimension"/>
        <rdfs:comment>URI (forward direction):	http://www.cidoc-crm.org/cidoc-crm/P43_has_dimension
URI (inverse direction):	http://www.cidoc-crm.org/cidoc-crm/P43i_is_dimension_of
Domain:
E70 Thing
Range:
E54 Dimension
SubProperty Of:
-
SuperProperty Of:
-
Quantification:
one to many, dependent (0,n:1,1)

Scope Note:
This property records an instance of E54 Dimension of some instance of E70 Thing.

In the case that the recorded property is a result of a measurement of an instance of E18 Physical Thing, this property is a shortcut of the more fully developed path from E18 Physical Thing through P39i was measured by, E16 Measurement, P40 observed dimension to E54 Dimension.

It offers no information about how and when an E54 Dimension was established, nor by whom. Knowledge about an instance of E54 Dimension need not be the result of a measurement; it may be the result of evaluating data or other information, which should be documented as an instance of E13 Attribute Assignment.

An instance of E54 Dimension is specific to an instance of E70 Thing.

Properties:
-
Examples:
Silver cup 232 (E22) has dimension height of silver cup 232 (E54). [which has unit (P91) mm (E58), has value (P90) 224 (E60)] (fictitious)</rdfs:comment>
    </owl:ObjectProperty>
    


    <!-- http://www.semanticweb.org/vitto/ontologies/2024/9/PODS_1#P45_consists_of_(is_incorporated_in) -->


    <owl:ObjectProperty rdf:about="http://www.semanticweb.org/vitto/ontologies/2024/9/PODS_1#P45_consists_of_(is_incorporated_in)"/>
    


    <!-- http://www.semanticweb.org/vitto/ontologies/2024/9/PODS_1#P4_has_time-span_(is_time-span_of) -->


    <owl:ObjectProperty rdf:about="http://www.semanticweb.org/vitto/ontologies/2024/9/PODS_1#P4_has_time-span_(is_time-span_of)">
        <rdfs:domain rdf:resource="http://cidoc-crm.org/cidoc-crm/7.1.3/E2_Temporal_Entity#E2_Temporal_Entity"/>
        <rdfs:range rdf:resource="http://cidoc-crm.org/cidoc-crm/7.1.3/E52_Time-Span#E52_Time-Span"/>
        <rdfs:comment>URI (forward direction):	http://www.cidoc-crm.org/cidoc-crm/P4_has_time-span
URI (inverse direction):	http://www.cidoc-crm.org/cidoc-crm/P4i_is_time-span_of
Domain:
E2 Temporal Entity
Range:
E52 Time-Span
SubProperty Of:
-
SuperProperty Of:
-
Quantification:
many to one, necessary (1,1:0,n)

Scope Note:
This property associates an instance of E2 Temporal Entity with the instance of E52 Time-Span during which it was on-going. The associated instance of E52 Time-Span is understood as the real time-span during which the phenomena making up the temporal entity instance were active. More than one instance of E2 Temporal Entity may share a common instance of E52 Time-Span only if they come into being and end being due to identical declarations or events.

Properties:
-
Examples:
The Yalta Conference (E7) has time-span Yalta Conference time-span (E52). (Harbutt, 2010)</rdfs:comment>
    </owl:ObjectProperty>
    


    <!-- http://www.semanticweb.org/vitto/ontologies/2024/9/PODS_1#P92_brought_into_existence_(was_brought_into_existence_by) -->


    <owl:ObjectProperty rdf:about="http://www.semanticweb.org/vitto/ontologies/2024/9/PODS_1#P92_brought_into_existence_(was_brought_into_existence_by)">
        <rdfs:subPropertyOf rdf:resource="http://www.semanticweb.org/vitto/ontologies/2024/9/PODS_1#P12_occurred_in_the_presence_of_(was_present_at)"/>
        <rdfs:comment>URI (forward direction):	http://www.cidoc-crm.org/cidoc-crm/P92_brought_into_existence
URI (inverse direction):	http://www.cidoc-crm.org/cidoc-crm/P92i_was_brought_into_existence_by
Domain:
E63 Beginning of Existence
Range:
E77 Persistent Item
SubProperty Of:
E5 Event. P12 occurred in the presence of (was present at): E77 Persistent Item
SuperProperty Of:
E65 Creation. P94 has created (was created by): E28 Conceptual Object
E66 Formation. P95 has formed (was formed by): E74 Group
E67 Birth. P98 brought into life (was born): E21 Person
E12 Production. P108 has produced (was produced by): E24 Physical Human-Made Thing
E81 Transformation. P123 resulted in (resulted from): E18 Physical Thing
Quantification:
one to many, necessary, dependent (1,n:1,1)

Scope Note:
This property links an instance of E63 Beginning of Existence to the instance of E77 Persistent Item brought into existence by it.

It allows a &apos;start&apos; to be attached to any instance of E77 Persistent Item being documented, i.e., as instances of E70 Thing, E72 Legal Object, E39 Actor, E41 Appellation and E55 Type.

Properties:
-
Examples:
The birth of Mozart (E67) brought into existence Mozart (E21). (Deutsch, 1965)</rdfs:comment>
    </owl:ObjectProperty>
    


    <!-- http://www.semanticweb.org/vitto/ontologies/2024/9/PODS_1#P94_has_created_(was_created_by) -->


    <owl:ObjectProperty rdf:about="http://www.semanticweb.org/vitto/ontologies/2024/9/PODS_1#P94_has_created_(was_created_by)">
        <rdfs:subPropertyOf rdf:resource="http://www.semanticweb.org/vitto/ontologies/2024/9/PODS_1#P92_brought_into_existence_(was_brought_into_existence_by)"/>
        <rdfs:comment>URI (forward direction):	http://www.cidoc-crm.org/cidoc-crm/P94_has_created
URI (inverse direction):	http://www.cidoc-crm.org/cidoc-crm/P94i_was_created_by
Domain:
E65 Creation
Range:
E28 Conceptual Object
SubProperty Of:
E63 Beginning of Existence. P92 brought into existence (was brought into existence by): E77 Persistent Item
SuperProperty Of:
E83 Type Creation. P135 created type (was created by): E55 Type
Quantification:
one to many, necessary, dependent (1,n:1,1)

Scope Note:
This property links an instance of E65 Creation to the instance of E28 Conceptual Object created by it.

It represents the act of conceiving the intellectual content of the instance of E28 Conceptual Object. It does not represent the act of creating the first physical carrier of the instance of E28 Conceptual Object. As an example, this is the composition of a poem, not its commitment to paper.

Properties:
-
Examples:
The composition of &apos;The Four Friends&apos; by A. A. Milne (E65) has created &apos;The Four Friends&apos; by A. A. Milne (E33). (Milne, 2012)</rdfs:comment>
    </owl:ObjectProperty>
    


    <!-- http://www.semanticweb.org/vitto/ontologies/2024/9/PODS_1#P9_consists_of_(forms_part_of) -->


    <owl:ObjectProperty rdf:about="http://www.semanticweb.org/vitto/ontologies/2024/9/PODS_1#P9_consists_of_(forms_part_of)">
        <rdfs:subPropertyOf rdf:resource="http://www.semanticweb.org/vitto/ontologies/2024/9/PODS_1#P10_falls_within_(contains)"/>
        <rdfs:domain rdf:resource="http://cidoc-crm.org/cidoc-crm/7.1.3/E4_Period#E4_Period"/>
        <rdfs:range rdf:resource="http://cidoc-crm.org/cidoc-crm/7.1.3/E4_Period#E4_Period"/>
        <rdfs:comment>URI (forward direction):	http://www.cidoc-crm.org/cidoc-crm/P9_consists_of
URI (inverse direction):	http://www.cidoc-crm.org/cidoc-crm/P9i_forms_part_of
Domain:
E4 Period
Range:
E4 Period
SubProperty Of:
E92 Spacetime Volume. P10i contains (falls within): E92 Spacetime Volume
SuperProperty Of:
-
Quantification:
many to many (0,n:0,n)

Scope Note:
This property associates an instance of E4 Period with another instance of E4 Period that is defined by a subset of the phenomena that define the former. Therefore, the spacetime volume of the latter must fall within the spacetime volume of the former.

This property is transitive and asymmetric.

Properties:
-
Examples:
Cretan Bronze Age (E4) consists of Middle Minoan (E4). (Hood, 1971)</rdfs:comment>
    </owl:ObjectProperty>
    


    <!-- https://photogrammetry.altervista.org/admin/items/show/253#Y62_has_modelling_operator -->


    <owl:ObjectProperty rdf:about="https://photogrammetry.altervista.org/admin/items/show/253#Y62_has_modelling_operator">
        <rdfs:subPropertyOf rdf:resource="http://www.semanticweb.org/vitto/ontologies/2024/9/PODS_1#P14_carried_out_by_(performed)"/>
        <rdfs:domain rdf:resource="https://photogrammetry.altervista.org/items/show/90#F4_Modelling"/>
        <rdfs:range rdf:resource="https://photogrammetry.altervista.org/items/show/125#F39_Modelling_Operator"/>
        <rdfs:label xml:lang="en">has_modifying_operator</rdfs:label>
        <skos:definition xml:lang="en">Y62: has modelling operator

Subproperty of: P14 carried out by
Domain: F4 Modelling
Range: F39 Modelling Operator</skos:definition>
        <skos:example xml:lang="en">A F4 Modelling process was carried out by a F39 Modelling Operator, such as a skilled 3D artist or modeller.</skos:example>
        <skos:scopeNote xml:lang="en">This property relates a modelling process (F4) to the operator (F39) responsible for carrying out the modelling work.</skos:scopeNote>
    </owl:ObjectProperty>
    


    <!-- https://photogrammetry.altervista.org/admin/items/show/256#Y66_is_Digital_Twin_physical_carrier -->


    <owl:ObjectProperty rdf:about="https://photogrammetry.altervista.org/admin/items/show/256#Y66_is_Digital_Twin_physical_carrier">
        <rdfs:subPropertyOf rdf:resource="http://www.semanticweb.org/vitto/ontologies/2024/9/PODS_1#L19_stores_(is_stored_on)"/>
        <rdfs:domain rdf:resource="https://photogrammetry.altervista.org/items/show/155#F68_Digital_Twin_Physical_Carrier"/>
        <rdfs:range rdf:resource="https://photogrammetry.altervista.org/items/show/145#F100_3D_Digital_Twin"/>
        <rdfs:label xml:lang="en">is_tridimensional_digital_twin_physical_carrier</rdfs:label>
        <skos:definition xml:lang="en">Y66: is Digital Twin physical carrier

Subproperty of: L19 stores
Domain: F68 Model Physical Carrier
Range: F100 Digital Twin</skos:definition>
        <skos:example xml:lang="en">A F68 Model Physical Carrier (a hard drive) stores a F100 Digital Twin of a heritage monument.</skos:example>
        <skos:scopeNote xml:lang="en">This property links the physical carrier of a model (F68), such as a hard drive or other storage medium, to the digital twin (F100) it contains.</skos:scopeNote>
    </owl:ObjectProperty>
    


    <!-- https://photogrammetry.altervista.org/items/show/192#Y1:_is_acquired_object_of -->


    <owl:ObjectProperty rdf:about="https://photogrammetry.altervista.org/items/show/192#Y1:_is_acquired_object_of">
        <rdfs:subPropertyOf rdf:resource="http://www.semanticweb.org/vitto/ontologies/2024/9/PODS_1#L1_digitized_(was_digitized_by)"/>
        <rdfs:domain rdf:resource="https://photogrammetry.altervista.org/admin/items/show/88#F2_Acquisition"/>
        <rdfs:range rdf:resource="https://photogrammetry.altervista.org/admin/items/show/87#F1_Survey_Object"/>
        <rdfs:label xml:lang="en">is_acquired_of</rdfs:label>
        <skos:definition xml:lang="en">Y1: is acquired object of

SubProperties of: L1 digitized

Domain
F2 Acquisition

Range
F1 Survey Object</skos:definition>
        <skos:example xml:lang="en">-</skos:example>
        <skos:scopeNote xml:lang="en">This property refers to the specific survey object (F1) that was the subject of the acquisition process (F2). It indicates the object being digitized or acquired during a particular survey or documentation effort.</skos:scopeNote>
    </owl:ObjectProperty>
    


    <!-- https://photogrammetry.altervista.org/items/show/193#Y2:__had_pictures_input -->


    <owl:ObjectProperty rdf:about="https://photogrammetry.altervista.org/items/show/193#Y2:__had_pictures_input">
        <rdfs:subPropertyOf rdf:resource="http://www.semanticweb.org/vitto/ontologies/2024/9/PODS_1#L10_had_input_(was_input_of)"/>
        <rdfs:domain rdf:resource="https://photogrammetry.altervista.org/admin/items/show/88#F2_Acquisition"/>
        <rdfs:range rdf:resource="https://photogrammetry.altervista.org/items/show/93#F7_Picture_Set"/>
        <rdfs:label xml:lang="en">had_pictures_input</rdfs:label>
        <skos:definition xml:lang="en">Y2: had pictures input

SubProperties of: L10 had input

Domain: F2 Acquisition
Range: F7 Picture Set</skos:definition>
        <skos:example xml:lang="en">-</skos:example>
        <skos:scopeNote xml:lang="en">This property refers to the set of pictures (F7) that were used as input during an acquisition event (F2). It connects the acquisition process to the photographic data that was collected or processed.</skos:scopeNote>
    </owl:ObjectProperty>
    


    <!-- https://photogrammetry.altervista.org/items/show/194#Y3:_has_Type_Of_Acquisition -->


    <owl:ObjectProperty rdf:about="https://photogrammetry.altervista.org/items/show/194#Y3:_has_Type_Of_Acquisition">
        <rdfs:subPropertyOf rdf:resource="http://www.semanticweb.org/vitto/ontologies/2024/9/PODS_1#P2__has_type_(is_type_of)"/>
        <rdfs:domain rdf:resource="http://www.semanticweb.org/vitto/ontologies/2024/9/PODS_1Protocol_of_Ontological_Digital_Survey/extensions/versions/1_1/F12_Acquisition_Trajectory#F12_Acquisition_Trajectory"/>
        <rdfs:range rdf:resource="https://photogrammetry.altervista.org/items/show/103#F17_Acquisition_Trajectory_Type"/>
        <rdfs:label xml:lang="en">has_type_of_acquisition</rdfs:label>
        <skos:definition xml:lang="en">Y3: has Type Of Acquisition

SubProperties of: P2 has type

Domain: F12 Acquisition Trajectory
Range: F17 Acquisition Trajectory Type</skos:definition>
        <skos:example xml:lang="en">-</skos:example>
        <skos:scopeNote xml:lang="en">This property identifies the type of trajectory used during an acquisition event (F12). It specifies the method or approach taken to move through space and acquire data, such as linear, circular, or other types of trajectories.</skos:scopeNote>
    </owl:ObjectProperty>
    


    <!-- https://photogrammetry.altervista.org/items/show/195#Y4_has_dominant_geometry_type -->


    <owl:ObjectProperty rdf:about="https://photogrammetry.altervista.org/items/show/195#Y4_has_dominant_geometry_type">
        <rdfs:subPropertyOf rdf:resource="http://www.semanticweb.org/vitto/ontologies/2024/9/PODS_1#P2__has_type_(is_type_of)"/>
        <rdfs:domain rdf:resource="https://photogrammetry.altervista.org/items/show/99#F13_Acquisition_Method"/>
        <rdfs:range rdf:resource="https://photogrammetry.altervista.org/items/show/104#F18_Dominant_Geometry_Type"/>
        <rdfs:label xml:lang="en">has_dominant_geometry_type</rdfs:label>
        <skos:definition xml:lang="en">Y4: has dominant geometry type

SubProperties of: P2 has type

Domain: F13 Acquisition Method
Range: F18 Geometry Type</skos:definition>
        <skos:example xml:lang="en">-</skos:example>
        <skos:scopeNote xml:lang="en">This property describes the dominant geometry type (F18) captured during an acquisition method (F13). It indicates whether the acquisition primarily involved points, lines, surfaces, or volumes.</skos:scopeNote>
    </owl:ObjectProperty>
    


    <!-- https://photogrammetry.altervista.org/items/show/196#Y5_has_scale_type -->


    <owl:ObjectProperty rdf:about="https://photogrammetry.altervista.org/items/show/196#Y5_has_scale_type">
        <rdfs:subPropertyOf rdf:resource="http://www.semanticweb.org/vitto/ontologies/2024/9/PODS_1#P2__has_type_(is_type_of)"/>
        <rdfs:domain rdf:resource="https://photogrammetry.altervista.org/items/show/99#F13_Acquisition_Method"/>
        <rdfs:range rdf:resource="https://photogrammetry.altervista.org/items/show/105#F19_Scale_Type"/>
        <rdfs:label xml:lang="en">has_scale_type</rdfs:label>
        <skos:definition xml:lang="en">Y5: has scale type

SubProperties of: P2 has type

Domain: F13 Acquisition Method
Range: F19 Scale Type</skos:definition>
        <skos:example xml:lang="en">-</skos:example>
        <skos:scopeNote xml:lang="en">This property refers to the scale type (F19) associated with the acquisition method (F13). It defines whether the acquisition was performed on a small, medium, or large scale, according to the object and purpose of the survey.</skos:scopeNote>
    </owl:ObjectProperty>
    


    <!-- https://photogrammetry.altervista.org/items/show/197#Y6_used_trajectory -->


    <owl:ObjectProperty rdf:about="https://photogrammetry.altervista.org/items/show/197#Y6_used_trajectory">
        <rdfs:subPropertyOf rdf:resource="http://www.semanticweb.org/vitto/ontologies/2024/9/PODS_1#P33_used_specific_technique_(was_used_by)"/>
        <rdfs:domain rdf:resource="https://photogrammetry.altervista.org/admin/items/show/88#F2_Acquisition"/>
        <rdfs:range rdf:resource="http://www.semanticweb.org/vitto/ontologies/2024/9/PODS_1Protocol_of_Ontological_Digital_Survey/extensions/versions/1_1/F12_Acquisition_Trajectory#F12_Acquisition_Trajectory"/>
        <rdfs:label xml:lang="en">used_trajectory</rdfs:label>
        <skos:definition xml:lang="en">Y6: used trajectory

SubProperties of: P33 used specific technique

Domain: F2 Acquisition
Range: F12 Acquisition Trajectory</skos:definition>
        <skos:example xml:lang="en">-</skos:example>
        <skos:scopeNote xml:lang="en">This property describes the specific trajectory (F12) used during the acquisition event (F2). It denotes the path or movement employed to capture data.</skos:scopeNote>
    </owl:ObjectProperty>
    


    <!-- https://photogrammetry.altervista.org/items/show/198#Y7_has_method_of_acquisition -->


    <owl:ObjectProperty rdf:about="https://photogrammetry.altervista.org/items/show/198#Y7_has_method_of_acquisition">
        <rdfs:subPropertyOf rdf:resource="http://www.semanticweb.org/vitto/ontologies/2024/9/PODS_1#P33_used_specific_technique_(was_used_by)"/>
        <rdfs:domain rdf:resource="https://photogrammetry.altervista.org/admin/items/show/88#F2_Acquisition"/>
        <rdfs:range rdf:resource="https://photogrammetry.altervista.org/items/show/99#F13_Acquisition_Method"/>
        <rdfs:label xml:lang="en">has_method_of_acquisition</rdfs:label>
        <skos:definition xml:lang="en">Y7: has method of acquisition

SubProperties of: P33 used specific technique

Domain: F2 Acquisition
Range: F13 Acquisition Method</skos:definition>
        <skos:example xml:lang="en">-</skos:example>
        <skos:scopeNote xml:lang="en">This property refers to the method (F13) utilized in an acquisition process (F2). It identifies the particular technique or procedure, such as photogrammetry or LiDAR scanning, used to acquire data.</skos:scopeNote>
    </owl:ObjectProperty>
    


    <!-- https://photogrammetry.altervista.org/items/show/199#Y8_happened_on_acquisition_device -->


    <owl:ObjectProperty rdf:about="https://photogrammetry.altervista.org/items/show/199#Y8_happened_on_acquisition_device">
        <rdfs:subPropertyOf rdf:resource="http://www.semanticweb.org/vitto/ontologies/2024/9/PODS_1#L12_happened_on_device_(was_device_for)"/>
        <rdfs:domain rdf:resource="https://photogrammetry.altervista.org/admin/items/show/88#F2_Acquisition"/>
        <rdfs:range rdf:resource="https://photogrammetry.altervista.org/items/show/95#F9_Acquisition_Device"/>
        <rdfs:label xml:lang="en">happened_on_acquisition_device</rdfs:label>
        <skos:definition xml:lang="en">Y8: happened on acquisition device

SubProperties of: L12 happened on device

Domain: F2 Acquisition
Range: F9 Acquisition Device</skos:definition>
        <skos:example xml:lang="en">-</skos:example>
        <skos:scopeNote xml:lang="en">This property refers to the acquisition device (F9) on which the acquisition process (F2) occurred. It links the acquisition event to the specific piece of hardware or equipment used.</skos:scopeNote>
    </owl:ObjectProperty>
    


    <!-- https://photogrammetry.altervista.org/items/show/200#Y9_has_acquisition_device_type -->


    <owl:ObjectProperty rdf:about="https://photogrammetry.altervista.org/items/show/200#Y9_has_acquisition_device_type">
        <rdfs:subPropertyOf rdf:resource="http://www.semanticweb.org/vitto/ontologies/2024/9/PODS_1#L17_measured_thing_of_type_(was_type_of_thing_measured_by)"/>
        <rdfs:domain rdf:resource="https://photogrammetry.altervista.org/admin/items/show/88#F2_Acquisition"/>
        <rdfs:range rdf:resource="https://photogrammetry.altervista.org/items/show/106#F20_Acquisition_Device_Type"/>
        <rdfs:label xml:lang="en">has_acquisition_device_type</rdfs:label>
        <skos:definition xml:lang="en">This property specifies the type of acquisition device (F20) used during the acquisition process (F2). It identifies the general category or kind of device employed, such as a camera, scanner, or drone.</skos:definition>
        <skos:definition xml:lang="en">Y9: has acquisition device type

SubProperties of: L17 measured thing of type

Domain: F2 Acquisition
Range: F20 Acquisition Device Type</skos:definition>
        <skos:example xml:lang="en">-</skos:example>
    </owl:ObjectProperty>
    


    <!-- https://photogrammetry.altervista.org/items/show/201#Y10_has_created_raw_data -->


    <owl:ObjectProperty rdf:about="https://photogrammetry.altervista.org/items/show/201#Y10_has_created_raw_data">
        <rdfs:subPropertyOf rdf:resource="http://www.semanticweb.org/vitto/ontologies/2024/9/PODS_1#L11_had_output_(was_output_of)"/>
        <rdfs:domain rdf:resource="https://photogrammetry.altervista.org/admin/items/show/88#F2_Acquisition"/>
        <rdfs:range rdf:resource="https://photogrammetry.altervista.org/items/show/92#F6_Acquisition_Raw_Data"/>
        <rdfs:label xml:lang="en">has_created_raw_data</rdfs:label>
        <skos:definition xml:lang="en">Y10: has created raw data

SubProperties of: L11 has output

Domain: F2 Acquisition
Range: F6 Acquisition Raw Data</skos:definition>
        <skos:example xml:lang="en">The relation between the point cloud data generated and the  laser scanning session.</skos:example>
        <skos:example xml:lang="en">The relation between the raw images captured and the photogrammetric survey of a building façade.</skos:example>
        <skos:scopeNote xml:lang="en">This property refers to the raw data (F6) generated as a result of the acquisition event (F2). It connects the acquisition process to the unprocessed, primary data produced during the survey.</skos:scopeNote>
    </owl:ObjectProperty>
    


    <!-- https://photogrammetry.altervista.org/items/show/202#Y11_used_acquisition_software -->


    <owl:ObjectProperty rdf:about="https://photogrammetry.altervista.org/items/show/202#Y11_used_acquisition_software">
        <rdfs:subPropertyOf rdf:resource="http://www.semanticweb.org/vitto/ontologies/2024/9/PODS_1#L23_used_software_or_firmware_(was_software_or_firmware_used_by)"/>
        <rdfs:domain rdf:resource="https://photogrammetry.altervista.org/admin/items/show/88#F2_Acquisition"/>
        <rdfs:range rdf:resource="https://photogrammetry.altervista.org/items/show/116#F30_Acquisition_Software"/>
        <rdfs:label xml:lang="en">used_acquisition_software</rdfs:label>
        <skos:definition xml:lang="en">Y11: used acquisition software

SubProperties of: L23 used software or firmware

Domain: F2 Acquisition
Range: F30 Acquisition Software</skos:definition>
        <skos:example xml:lang="en">-</skos:example>
        <skos:scopeNote xml:lang="en">This property refers to the specific software (F30) used during the acquisition event (F2). It identifies the software that controlled the data capture or processed the initial acquisition.</skos:scopeNote>
    </owl:ObjectProperty>
    


    <!-- https://photogrammetry.altervista.org/items/show/204#Y13:_used_Acquisition_Instruction -->


    <owl:ObjectProperty rdf:about="https://photogrammetry.altervista.org/items/show/204#Y13:_used_Acquisition_Instruction">
        <rdfs:subPropertyOf rdf:resource="http://www.semanticweb.org/vitto/ontologies/2024/9/PODS_1#P33_used_specific_technique_(was_used_by)"/>
        <rdfs:domain rdf:resource="https://photogrammetry.altervista.org/admin/items/show/88#F2_Acquisition"/>
        <rdfs:range rdf:resource="https://photogrammetry.altervista.org/items/show/119#F33_Acquisition_Phase"/>
        <rdfs:label xml:lang="en">used_acquisition_instruction</rdfs:label>
        <skos:definition xml:lang="en">Y13: used Acquisition Instruction

Subproperty of: P33 used specific technique

Domain: F2 Acquisition
Range: F33 Acquisition Phase</skos:definition>
        <skos:example xml:lang="en">-</skos:example>
        <skos:scopeNote xml:lang="en">This property links the acquisition event (F2) to the specific acquisition instructions or procedures (F33) that were used to guide the process. These instructions may define steps, settings, or approaches used during the acquisition phase.</skos:scopeNote>
    </owl:ObjectProperty>
    


    <!-- https://photogrammetry.altervista.org/items/show/205#Y14:_stores_acquisition_Picture -->


    <owl:ObjectProperty rdf:about="https://photogrammetry.altervista.org/items/show/205#Y14:_stores_acquisition_Picture">
        <rdfs:subPropertyOf rdf:resource="http://www.semanticweb.org/vitto/ontologies/2024/9/PODS_1#L19_stores_(is_stored_on)"/>
        <rdfs:domain rdf:resource="https://photogrammetry.altervista.org/items/show/121#F35_Raw_Data_Carrier"/>
        <rdfs:range rdf:resource="https://photogrammetry.altervista.org/items/show/94#F8_Picture"/>
        <rdfs:label xml:lang="en">stores_acquisition_picture</rdfs:label>
        <skos:definition xml:lang="en">Y14: stores acquisition Picture

Subproperty of: L19 stores

Domain: F35 Raw Data Carrier
Range: F8 Picture</skos:definition>
        <skos:example xml:lang="en">-</skos:example>
        <skos:scopeNote xml:lang="en">This property connects a raw data carrier (F35) to the pictures (F8) it stores. It identifies the images that were collected during the acquisition process and are saved on a specific storage device or medium.</skos:scopeNote>
    </owl:ObjectProperty>
    


    <!-- https://photogrammetry.altervista.org/items/show/206#Y15:_is_composed_of_picture -->


    <owl:ObjectProperty rdf:about="https://photogrammetry.altervista.org/items/show/206#Y15:_is_composed_of_picture">
        <rdfs:subPropertyOf rdf:resource="http://www.semanticweb.org/vitto/ontologies/2024/9/PODS_1#P106_is_composed_of_(forms_part_of)"/>
        <rdfs:domain rdf:resource="https://photogrammetry.altervista.org/items/show/93#F7_Picture_Set"/>
        <rdfs:range rdf:resource="https://photogrammetry.altervista.org/items/show/94#F8_Picture"/>
        <rdfs:label xml:lang="en">is_composed_of_picture</rdfs:label>
        <skos:definition xml:lang="en">Y15: is composed of picture

Subproperty of: P106 is composed of
Domain: F7 Picture Set
Range: F8 Picture</skos:definition>
        <skos:example xml:lang="en">-</skos:example>
        <skos:scopeNote xml:lang="en">This property indicates that a picture set (F7) is composed of individual pictures (F8). It defines the relationship between the collection of images used for acquisition and the individual pictures that constitute the set.</skos:scopeNote>
    </owl:ObjectProperty>
    


    <!-- https://photogrammetry.altervista.org/items/show/208#Y17:_has_acquisition_operator -->


    <owl:ObjectProperty rdf:about="https://photogrammetry.altervista.org/items/show/208#Y17:_has_acquisition_operator">
        <rdfs:subPropertyOf rdf:resource="http://www.semanticweb.org/vitto/ontologies/2024/9/PODS_1#P14_carried_out_by_(performed)"/>
        <rdfs:domain rdf:resource="https://photogrammetry.altervista.org/admin/items/show/88#F2_Acquisition"/>
        <rdfs:range rdf:resource="https://photogrammetry.altervista.org/items/show/123#F37_Survey_Operator"/>
        <rdfs:label xml:lang="en">has_acquisition_operator</rdfs:label>
        <skos:definition xml:lang="en">Y17: has acquisition operator

Subproperty of: P14 carried out by

Domain: F2 Acquisition
Range: F37 Survey Operator</skos:definition>
        <skos:example xml:lang="en">-</skos:example>
        <skos:scopeNote xml:lang="en">This property links the acquisition process (F2) to the survey operator (F37) responsible for carrying out the data collection. It defines the role of the person or team who performed the acquisition.</skos:scopeNote>
    </owl:ObjectProperty>
    


    <!-- https://photogrammetry.altervista.org/items/show/209#Y18:_has_place_of_acquisition -->


    <owl:ObjectProperty rdf:about="https://photogrammetry.altervista.org/items/show/209#Y18:_has_place_of_acquisition">
        <rdfs:subPropertyOf rdf:resource="http://www.semanticweb.org/vitto/ontologies/2024/9/PODS_1#P161_has_spatial_projection_(is_spatial_projection_of)"/>
        <rdfs:domain rdf:resource="https://photogrammetry.altervista.org/admin/items/show/88#F2_Acquisition"/>
        <rdfs:range rdf:resource="https://photogrammetry.altervista.org/items/show/128#F42_Place_Of_Acquisition"/>
        <rdfs:label xml:lang="en">has_place_of_acquisition</rdfs:label>
        <skos:definition xml:lang="en">Y18: has place of acquisition

Subproperty of: P161 has spatial projection
Domain
F2 Acquisition
Range
F42 Place of Acquisition</skos:definition>
        <skos:example xml:lang="en">-</skos:example>
        <skos:scopeNote xml:lang="en">This property refers to the specific location (F42) where the acquisition event (F2) took place. It identifies the spatial setting or area in which the survey or documentation occurred.</skos:scopeNote>
    </owl:ObjectProperty>
    


    <!-- https://photogrammetry.altervista.org/items/show/210#Y19:_has_date_of_acquisition -->


    <owl:ObjectProperty rdf:about="https://photogrammetry.altervista.org/items/show/210#Y19:_has_date_of_acquisition">
        <rdfs:subPropertyOf rdf:resource="http://www.semanticweb.org/vitto/ontologies/2024/9/PODS_1#P4_has_time-span_(is_time-span_of)"/>
        <rdfs:domain rdf:resource="https://photogrammetry.altervista.org/admin/items/show/88#F2_Acquisition"/>
        <rdfs:range rdf:resource="https://photogrammetry.altervista.org/items/show/129#F43_Survey_Date"/>
        <rdfs:label xml:lang="en">has_date_of_acquisition</rdfs:label>
        <skos:definition xml:lang="en">Y19: has date of acquisition

Subproperty of: P4 has time span
Domain
F2 Acquisition
Range
F43 Survey Date</skos:definition>
        <skos:example xml:lang="en">-</skos:example>
        <skos:scopeNote xml:lang="en">This property identifies the date (F43) on which the acquisition process (F2) took place. It specifies when the data collection or survey was performed.</skos:scopeNote>
    </owl:ObjectProperty>
    


    <!-- https://photogrammetry.altervista.org/items/show/212#Y21:_has_coordinates_of_acquisition -->


    <owl:ObjectProperty rdf:about="https://photogrammetry.altervista.org/items/show/212#Y21:_has_coordinates_of_acquisition">
        <rdfs:subPropertyOf rdf:resource="http://www.semanticweb.org/vitto/ontologies/2024/9/PODS_1#P169_defines_spacetime_volume_(spacetime_volume_is_defined_by)"/>
        <rdfs:domain rdf:resource="https://photogrammetry.altervista.org/items/show/131#F45__Acquisition_Coordinates"/>
        <rdfs:range rdf:resource="https://photogrammetry.altervista.org/admin/items/show/88#F2_Acquisition"/>
        <rdfs:label xml:lang="en">has_coordinates_of_acquisition</rdfs:label>
        <skos:definition xml:lang="en">Y21: has coordinates of acquisition

Subproperty of: P169 defines spacetime volume
Domain
F45 Acquisition Coordinates
Range
F2 Acquisition</skos:definition>
        <skos:example xml:lang="en">-</skos:example>
        <skos:scopeNote xml:lang="en">This property specifies the geographic coordinates (F45) at which the acquisition event (F2) occurred. It links the acquisition process to the precise spatial coordinates where the data collection took place.</skos:scopeNote>
    </owl:ObjectProperty>
    


    <!-- https://photogrammetry.altervista.org/items/show/213#Y22_had_acquisition_input -->


    <owl:ObjectProperty rdf:about="https://photogrammetry.altervista.org/items/show/213#Y22_had_acquisition_input">
        <rdfs:subPropertyOf rdf:resource="http://www.semanticweb.org/vitto/ontologies/2024/9/PODS_1#L10_had_input_(was_input_of)"/>
        <rdfs:domain rdf:resource="https://photogrammetry.altervista.org/items/show/89#F3_Processing"/>
        <rdfs:range rdf:resource="https://photogrammetry.altervista.org/items/show/111#F25_Acquisition_Raw_Data"/>
        <rdfs:label xml:lang="en">had_acquisition_input</rdfs:label>
        <skos:definition xml:lang="en">Y22: had acquisition input

Subproperty of: L10 had input
Domain
F3 Processing
Range
F25 Acquisition Raw Data</skos:definition>
        <skos:example xml:lang="en">A processing phase F3 Processing has as input F25 Acquisition Raw Data, which was generated by a laser scan.</skos:example>
        <skos:scopeNote xml:lang="en">This property links the processing phase (F3) to the acquisition raw data (F25) used as input for the processing.</skos:scopeNote>
    </owl:ObjectProperty>
    


    <!-- https://photogrammetry.altervista.org/items/show/214#Y23_has_type_of_matching -->


    <owl:ObjectProperty rdf:about="https://photogrammetry.altervista.org/items/show/214#Y23_has_type_of_matching">
        <rdfs:subPropertyOf rdf:resource="http://www.semanticweb.org/vitto/ontologies/2024/9/PODS_1#P2__has_type_(is_type_of)"/>
        <rdfs:domain rdf:resource="https://photogrammetry.altervista.org/items/show/100#F14_Matching_Method"/>
        <rdfs:range rdf:resource="https://photogrammetry.altervista.org/items/show/107#F21_Matching_Algorithm_Type"/>
        <rdfs:label xml:lang="en">has_type_of_matching</rdfs:label>
        <skos:definition xml:lang="en">Y23: has type of matching

Subproperty of: P2 has type
Domain
F14 Matching Method
Range
21 Matching Algorithm Type</skos:definition>
        <skos:example xml:lang="en">The F14 Matching Method uses a F21 Matching Algorithm Type, such as a keypoint-based algorithm.</skos:example>
        <skos:scopeNote xml:lang="en">This property specifies the type of algorithm (F21) used during the matching method (F14) to align or correlate data.</skos:scopeNote>
    </owl:ObjectProperty>
    


    <!-- https://photogrammetry.altervista.org/items/show/215#Y24_happened_on_processing_device -->


    <owl:ObjectProperty rdf:about="https://photogrammetry.altervista.org/items/show/215#Y24_happened_on_processing_device">
        <rdfs:subPropertyOf rdf:resource="http://www.semanticweb.org/vitto/ontologies/2024/9/PODS_1#L12_happened_on_device_(was_device_for)"/>
        <rdfs:domain rdf:resource="https://photogrammetry.altervista.org/items/show/142#F56_Mesh_Reconstruction"/>
        <rdfs:domain rdf:resource="https://photogrammetry.altervista.org/items/show/143#F57_Texturing_Mesh"/>
        <rdfs:domain rdf:resource="https://photogrammetry.altervista.org/items/show/89#F3_Processing"/>
        <rdfs:range rdf:resource="https://photogrammetry.altervista.org/items/show/96#F10_Processing_Device"/>
        <rdfs:label xml:lang="en">happened_on_processing_device</rdfs:label>
        <skos:definition xml:lang="en">Y24: happened on processing device

Subproperty of: L12 happened on device
Domain
F3 Processing
Range
F10 Processing Device, F56 Mesh Reconstruction, F57 Texturing Mesh</skos:definition>
        <skos:example xml:lang="en">A  processing phase F3 Processing happens on a F10 Processing Device, such as a high-performance server.</skos:example>
        <skos:scopeNote xml:lang="en">This property associates the processing phase (F3) with the processing device (F10) on which the processing occurred.</skos:scopeNote>
    </owl:ObjectProperty>
    


    <!-- https://photogrammetry.altervista.org/items/show/216#Y25_Processing_is_composed_of -->


    <owl:ObjectProperty rdf:about="https://photogrammetry.altervista.org/items/show/216#Y25_Processing_is_composed_of">
        <rdfs:subPropertyOf rdf:resource="http://www.semanticweb.org/vitto/ontologies/2024/9/PODS_1#P9_consists_of_(forms_part_of)"/>
        <rdfs:domain rdf:resource="https://photogrammetry.altervista.org/items/show/89#F3_Processing"/>
        <rdfs:range rdf:resource="http://www.semanticweb.org/vitto/ontologies/2024/9/PODS_1Protocol_of_Ontological_Digital_Survey/extensions/versions/1_1/F47_Densification#F47__Densification"/>
        <rdfs:label xml:lang="en">processing_is_composed_of</rdfs:label>
        <skos:definition xml:lang="en">Y25: Processing is composed of

Subproperty of: P9 consists of (forms part of)
Domain
F3 Processing
Range
F46 Matching / F47 Densification</skos:definition>
        <skos:example xml:lang="en">A F3 Processing phase is composed of a F46 Matching phase followed by a F47 Densification phase, the property connect this relation.</skos:example>
        <skos:scopeNote xml:lang="en">This property indicates that a processing phase (F3) is composed of subprocesses like matching (F46) or densification (F47).</skos:scopeNote>
    </owl:ObjectProperty>
    


    <!-- https://photogrammetry.altervista.org/items/show/217#Y26__used_processing_software -->


    <owl:ObjectProperty rdf:about="https://photogrammetry.altervista.org/items/show/217#Y26__used_processing_software">
        <rdfs:subPropertyOf rdf:resource="http://www.semanticweb.org/vitto/ontologies/2024/9/PODS_1#L23_used_software_or_firmware_(was_software_or_firmware_used_by)"/>
        <rdfs:domain rdf:resource="https://photogrammetry.altervista.org/items/show/142#F56_Mesh_Reconstruction"/>
        <rdfs:domain rdf:resource="https://photogrammetry.altervista.org/items/show/143#F57_Texturing_Mesh"/>
        <rdfs:domain rdf:resource="https://photogrammetry.altervista.org/items/show/89#F3_Processing"/>
        <rdfs:range rdf:resource="https://photogrammetry.altervista.org/items/show/117#F31_Processing_Software"/>
        <rdfs:label xml:lang="en">used_processing_software</rdfs:label>
        <skos:definition xml:lang="en">Y26: used processing software

Subproperty of: L23 used software or firmware
Domain
F3 Processing, 56 Mesh Reconstruction, F57 Texturing Mesh
Range
F31 Processing Software</skos:definition>
        <skos:example xml:lang="en">A F3 Processing phase uses F31 Processing Software, such as CloudCompare for handling point cloud data.</skos:example>
        <skos:scopeNote xml:lang="en">This property identifies the software (F31) used during the processing phase (F3).</skos:scopeNote>
    </owl:ObjectProperty>
    


    <!-- https://photogrammetry.altervista.org/items/show/218#Y27_has_method_of_densification -->


    <owl:ObjectProperty rdf:about="https://photogrammetry.altervista.org/items/show/218#Y27_has_method_of_densification">
        <rdfs:subPropertyOf rdf:resource="http://www.semanticweb.org/vitto/ontologies/2024/9/PODS_1#P33_used_specific_technique_(was_used_by)"/>
        <rdfs:domain rdf:resource="http://www.semanticweb.org/vitto/ontologies/2024/9/PODS_1Protocol_of_Ontological_Digital_Survey/extensions/versions/1_1/F47_Densification#F47__Densification"/>
        <rdfs:range rdf:resource="https://photogrammetry.altervista.org/items/show/134#F48_Densification_Method"/>
        <rdfs:label xml:lang="en">has_method_of_densification</rdfs:label>
        <skos:definition xml:lang="en">Y27: has method of densification

Subproperty of: P33 used specific technique

Domain: F47 Densification
Range: F48 Densification Method</skos:definition>
        <skos:example xml:lang="en">A F47 Densification phase uses a F48 Densification Method, such as Multi-View Stereo (MVS) to increase point density.</skos:example>
        <skos:scopeNote xml:lang="en">This property links the densification process (F47) to the specific method (F48) used to increase the density of a point cloud or model.</skos:scopeNote>
    </owl:ObjectProperty>
    


    <!-- https://photogrammetry.altervista.org/items/show/219#Y28__has_type_of_densification -->


    <owl:ObjectProperty rdf:about="https://photogrammetry.altervista.org/items/show/219#Y28__has_type_of_densification">
        <rdfs:subPropertyOf rdf:resource="http://www.semanticweb.org/vitto/ontologies/2024/9/PODS_1#P2__has_type_(is_type_of)"/>
        <rdfs:domain rdf:resource="https://photogrammetry.altervista.org/items/show/134#F48_Densification_Method"/>
        <rdfs:range rdf:resource="https://photogrammetry.altervista.org/items/show/108#F22_Densification_Algorithm_Type"/>
        <rdfs:label xml:lang="en">has_type_of_densification</rdfs:label>
        <skos:definition xml:lang="en">Y28: has type of densification

Subproperty of: P2 has type

Domain: F48 Densification Method
Range: F22 Densification Algorithm Type</skos:definition>
        <skos:example xml:lang="en">A F48 Densification Method uses a F22 Densification Algorithm Type, such as a dense feature matching algorithm.</skos:example>
        <skos:scopeNote xml:lang="en">This property indicates the type of algorithm (F22) used in the densification method (F48) to enhance the density of a point cloud.</skos:scopeNote>
    </owl:ObjectProperty>
    


    <!-- https://photogrammetry.altervista.org/items/show/220#Y29_has_matching_input -->


    <owl:ObjectProperty rdf:about="https://photogrammetry.altervista.org/items/show/220#Y29_has_matching_input">
        <rdfs:subPropertyOf rdf:resource="http://www.semanticweb.org/vitto/ontologies/2024/9/PODS_1#L10_had_input_(was_input_of)"/>
        <rdfs:domain rdf:resource="http://www.semanticweb.org/vitto/ontologies/2024/9/PODS_1Protocol_of_Ontological_Digital_Survey/extensions/versions/1_1/F47_Densification#F47__Densification"/>
        <rdfs:range rdf:resource="https://photogrammetry.altervista.org/items/show/112#F26_Point_Cloud"/>
        <rdfs:label xml:lang="en">has_matching_input</rdfs:label>
        <skos:definition xml:lang="en">Y29: has matching input

Subproperty of: L10 had input
Domain
F47 Densification
Range
F26 Point Cloud</skos:definition>
        <skos:example xml:lang="en">A F47 Densification phase uses an input F26 Point Cloud, obtained from a preliminary laser scan.</skos:example>
        <skos:scopeNote xml:lang="en">This property links the densification phase (F47) to the input point cloud (F26) used in the matching process.</skos:scopeNote>
    </owl:ObjectProperty>
    


    <!-- https://photogrammetry.altervista.org/items/show/221#Y30_has_created_point_cloud -->


    <owl:ObjectProperty rdf:about="https://photogrammetry.altervista.org/items/show/221#Y30_has_created_point_cloud">
        <rdfs:subPropertyOf rdf:resource="http://www.semanticweb.org/vitto/ontologies/2024/9/PODS_1#L11_had_output_(was_output_of)"/>
        <rdfs:range rdf:resource="https://photogrammetry.altervista.org/items/show/112#F26_Point_Cloud"/>
        <rdfs:label xml:lang="en">has_created_point_cloud</rdfs:label>
        <skos:definition xml:lang="en">Y30: has created point cloud

Subproperty of: L11 has output
Domain
F46 Matching
Range
F26 Point Cloud</skos:definition>
        <skos:example xml:lang="en">The relation that from F46 Matching process creates a F26 Point Cloud as its final output.</skos:example>
        <skos:scopeNote xml:lang="en">This property links the matching phase (F46) to the creation of a point cloud (F26) as a result of the matching.</skos:scopeNote>
    </owl:ObjectProperty>
    


    <!-- https://photogrammetry.altervista.org/items/show/222#Y32_has_method_of_matching -->


    <owl:ObjectProperty rdf:about="https://photogrammetry.altervista.org/items/show/222#Y32_has_method_of_matching">
        <rdfs:subPropertyOf rdf:resource="http://www.semanticweb.org/vitto/ontologies/2024/9/PODS_1#P33_used_specific_technique_(was_used_by)"/>
        <rdfs:range rdf:resource="https://photogrammetry.altervista.org/items/show/100#F14_Matching_Method"/>
        <rdfs:label xml:lang="en">has_method_of_matching</rdfs:label>
        <skos:definition xml:lang="en">Y32: has method of matching

Subproperty of: P33 used specific technique
Domain
F46 Matching
Range
F14 Matching Method</skos:definition>
        <skos:example xml:lang="en">The relation between a F46 Matching process and the F14 Matching Method, such as feature-based matching from images.</skos:example>
        <skos:scopeNote xml:lang="en">This property links the matching process (F46) to the specific matching method (F14) used.</skos:scopeNote>
    </owl:ObjectProperty>
    


    <!-- https://photogrammetry.altervista.org/items/show/223#Y31_has_created_densified_point_cloud -->


    <owl:ObjectProperty rdf:about="https://photogrammetry.altervista.org/items/show/223#Y31_has_created_densified_point_cloud">
        <rdfs:subPropertyOf rdf:resource="http://www.semanticweb.org/vitto/ontologies/2024/9/PODS_1#L11_had_output_(was_output_of)"/>
        <rdfs:domain rdf:resource="http://www.semanticweb.org/vitto/ontologies/2024/9/PODS_1Protocol_of_Ontological_Digital_Survey/extensions/versions/1_1/F47_Densification#F47__Densification"/>
        <rdfs:range rdf:resource="https://photogrammetry.altervista.org/items/show/113#F27_Densified_Point_Cloud"/>
        <rdfs:label xml:lang="en">has_created_densified_point_cloud</rdfs:label>
        <skos:definition xml:lang="en">Y31: has created densified point cloud

Subproperty of: L11 has output
Domain
F47 Densification
Range
F27 Densified Point Cloud</skos:definition>
        <skos:example xml:lang="en">The relation why a F47 Densification phase creates a F27 Densified Point Cloud with a higher density than the original input.</skos:example>
        <skos:scopeNote xml:lang="en">This property indicates that the result of the densification phase (F47) is a densified point cloud (F27).</skos:scopeNote>
    </owl:ObjectProperty>
    


    <!-- https://photogrammetry.altervista.org/items/show/225#Y34_was_measured_in__number_of_points -->


    <owl:ObjectProperty rdf:about="https://photogrammetry.altervista.org/items/show/225#Y34_was_measured_in__number_of_points">
        <rdfs:subPropertyOf rdf:resource="http://www.semanticweb.org/vitto/ontologies/2024/9/PODS_1#O24_measured_(was_measured_by)"/>
        <rdfs:subPropertyOf rdf:resource="https://photogrammetry.altervista.org/items/show/264#Y95:_was_measured_in_number_of_points"/>
        <rdfs:domain rdf:resource="https://photogrammetry.altervista.org/items/show/112#F26_Point_Cloud"/>
        <rdfs:range rdf:resource="https://photogrammetry.altervista.org/items/show/136#F50_Point_Cloud_Measurement"/>
        <rdfs:comment xml:lang="en">This property is redundant and can be replaced by the superproperty
- Y95: was measured in number of points -</rdfs:comment>
        <rdfs:label xml:lang="en">pc_was_measured_in_number_of_points</rdfs:label>
        <skos:definition xml:lang="en">Y34: was measured in number of points



Subproperty of: O24i was measured by
Domain
F26 Point Cloud
Range
F50 Point Cloud Measurement</skos:definition>
        <skos:example xml:lang="en">A F26 Point Cloud was measured in an F50 Point Cloud Measurement, which recorded the total number of points.</skos:example>
        <skos:scopeNote xml:lang="en">This property indicates that the number of points in a point cloud (F26) was measured in a point cloud measurement (F50).</skos:scopeNote>
    </owl:ObjectProperty>
    


    <!-- https://photogrammetry.altervista.org/items/show/226#Y35_has_vertex_quality_assignment -->


    <owl:ObjectProperty rdf:about="https://photogrammetry.altervista.org/items/show/226#Y35_has_vertex_quality_assignment">
        <rdfs:subPropertyOf rdf:resource="http://www.semanticweb.org/vitto/ontologies/2024/9/PODS_1#P141_assigned_(was_assigned_by)"/>
        <rdfs:domain rdf:resource="https://photogrammetry.altervista.org/items/show/112#F26_Point_Cloud"/>
        <rdfs:range rdf:resource="http://www.semanticweb.org/vitto/ontologies/2024/9/PODS_1Protocol_of_Ontological_Digital_Survey/extensions/versions/1_1/F54_Point_Cloud_Vertex_Quality#F54_Point_Cloud_Vertex_Quality"/>
        <rdfs:label xml:lang="en">has_vertex_quality_assignment</rdfs:label>
        <skos:definition xml:lang="en">Subproperty of: P141i was assigned by

Domain: F26 Point Cloud
Range: F54 Point Cloud Quality Assignment</skos:definition>
        <skos:example xml:lang="en">A F26 Point Cloud has an assigned F54 Point Cloud Quality Assignment, indicating the quality of the vertices based on precision.</skos:example>
        <skos:scopeNote xml:lang="en">This property links a point cloud (F26) to the assignment of its quality (F54), such as assessing the accuracy of each vertex.</skos:scopeNote>
    </owl:ObjectProperty>
    


    <!-- https://photogrammetry.altervista.org/items/show/227#Y36_has_Depth_Noise_Filtering -->


    <owl:ObjectProperty rdf:about="https://photogrammetry.altervista.org/items/show/227#Y36_has_Depth_Noise_Filtering">
        <rdfs:subPropertyOf rdf:resource="http://www.semanticweb.org/vitto/ontologies/2024/9/PODS_1#P141_assigned_(was_assigned_by)"/>
        <rdfs:domain rdf:resource="https://photogrammetry.altervista.org/items/show/113#F27_Densified_Point_Cloud"/>
        <rdfs:range rdf:resource="https://photogrammetry.altervista.org/items/show/141#F55_Depth_Noise_Filtering"/>
        <rdfs:label xml:lang="en">has_depth_noise_filtering</rdfs:label>
        <skos:definition xml:lang="en">Definition
Y36: has Depth Noise Filtering

Subproperty of: P141i was assigned by
Domain
F27 Dense Point Cloud
Range
F55 Depth Noise Filtering</skos:definition>
        <skos:example xml:lang="en">A F27 Dense Point Cloud undergoes F55 Depth Noise Filtering to remove noise from the depth data.</skos:example>
        <skos:scopeNote xml:lang="en">This property associates a dense point cloud (F27) with the application of a depth noise filtering technique (F55).</skos:scopeNote>
    </owl:ObjectProperty>
    


    <!-- https://photogrammetry.altervista.org/items/show/229#Y38_was_measured_in__number_of_points -->


    <owl:ObjectProperty rdf:about="https://photogrammetry.altervista.org/items/show/229#Y38_was_measured_in__number_of_points">
        <rdfs:subPropertyOf rdf:resource="http://www.semanticweb.org/vitto/ontologies/2024/9/PODS_1#O24_measured_(was_measured_by)"/>
        <rdfs:subPropertyOf rdf:resource="https://photogrammetry.altervista.org/items/show/264#Y95:_was_measured_in_number_of_points"/>
        <rdfs:domain rdf:resource="https://photogrammetry.altervista.org/items/show/113#F27_Densified_Point_Cloud"/>
        <rdfs:range rdf:resource="https://photogrammetry.altervista.org/items/show/138#F52_Dense_Point_Cloud_Measurement"/>
        <rdfs:comment xml:lang="en">This property is redundant and can be replaced by the superproperty 
- Y95: was measured in number of points -</rdfs:comment>
        <rdfs:label xml:lang="en">dpc_was_measured_in_number_of_points</rdfs:label>
        <skos:definition xml:lang="en">Y38: was measured in number of points (for dense point clouds)


Subproperty of: O24i was measured by
Domain: F27 Dense Point Cloud
Range: F52 Dense Point Cloud Measurement</skos:definition>
        <skos:example xml:lang="en">A F27 Dense Point Cloud was measured in an F52 Dense Point Cloud Measurement, which recorded the number of points after densification.</skos:example>
        <skos:scopeNote xml:lang="en">This property relates a dense point cloud (F27) to the measurement of its number of points (F52).</skos:scopeNote>
    </owl:ObjectProperty>
    


    <!-- https://photogrammetry.altervista.org/items/show/230#Y39_has_Sampling_Points_Range -->


    <owl:ObjectProperty rdf:about="https://photogrammetry.altervista.org/items/show/230#Y39_has_Sampling_Points_Range">
        <rdfs:subPropertyOf rdf:resource="http://www.semanticweb.org/vitto/ontologies/2024/9/PODS_1#P141_assigned_(was_assigned_by)"/>
        <rdfs:domain rdf:resource="https://photogrammetry.altervista.org/items/show/113#F27_Densified_Point_Cloud"/>
        <rdfs:range rdf:resource="https://photogrammetry.altervista.org/items/show/135#F49__Near_Sampling_Points_Range_SFM_Point_Seeds"/>
        <rdfs:label xml:lang="en">has_sampling_points_range</rdfs:label>
        <skos:definition xml:lang="en">Y39: has Sampling Points Range

Subproperty of: P141i was assigned by
Domain: F27 Dense Point Cloud
Range: F49 Near Sample Point Range</skos:definition>
        <skos:example xml:lang="en">The relation that connect a F27 Dense Point Cloud that has a F49 Near Sample Point Range, describing the spread of sampling points in the dataset.</skos:example>
        <skos:scopeNote xml:lang="en">This property indicates the range of points in the dense point cloud (F27) near a sample point range (F49).</skos:scopeNote>
    </owl:ObjectProperty>
    


    <!-- https://photogrammetry.altervista.org/items/show/231#Y40:_has_processing_operator -->


    <owl:ObjectProperty rdf:about="https://photogrammetry.altervista.org/items/show/231#Y40:_has_processing_operator">
        <rdfs:subPropertyOf rdf:resource="http://www.semanticweb.org/vitto/ontologies/2024/9/PODS_1#P14_carried_out_by_(performed)"/>
        <rdfs:domain rdf:resource="https://photogrammetry.altervista.org/items/show/89#F3_Processing"/>
        <rdfs:range rdf:resource="https://photogrammetry.altervista.org/items/show/124#F38_Processing_Operator"/>
        <rdfs:label xml:lang="en">has_processing_operator</rdfs:label>
        <skos:definition xml:lang="en">Y40: has processing operator

Subproperty of: P14 carried out by
Domain: F3 Processing
Range: F38 Processing Operator</skos:definition>
        <skos:example xml:lang="en">A F3 Processing phase is carried out by a F38 Processing Operator, such as an engineer overseeing the data processing.</skos:example>
        <skos:scopeNote xml:lang="en">This property connects a processing phase (F3) to the operator (F38) who performed the processing.</skos:scopeNote>
    </owl:ObjectProperty>
    


    <!-- https://photogrammetry.altervista.org/items/show/232#Y41_used_Processing_Instruction -->


    <owl:ObjectProperty rdf:about="https://photogrammetry.altervista.org/items/show/232#Y41_used_Processing_Instruction">
        <rdfs:subPropertyOf rdf:resource="http://www.semanticweb.org/vitto/ontologies/2024/9/PODS_1#P33_used_specific_technique_(was_used_by)"/>
        <rdfs:domain rdf:resource="https://photogrammetry.altervista.org/items/show/89#F3_Processing"/>
        <rdfs:range rdf:resource="https://photogrammetry.altervista.org/items/show/120#F34_Processing_Phase"/>
        <rdfs:label xml:lang="en">used_processing_phase_instruction</rdfs:label>
        <skos:definition xml:lang="en">Y41: used Phase Instruction

Subproperty of: P33 used specific technique
Domain: F3 Processing
Range: F34 Processing Phase</skos:definition>
        <skos:example xml:lang="en">A F3 Processing phase uses specific F34 Processing Phase Instructions, detailing how to process a point cloud such as the BeAPG Protocol in the processing of AFMNM005 (Lauro 2019).</skos:example>
        <skos:scopeNote xml:lang="en">This property links the processing phase (F3) to the instructions (F34) used during that phase.</skos:scopeNote>
    </owl:ObjectProperty>
    


    <!-- https://photogrammetry.altervista.org/items/show/233#Y42_was_continued_by_Modelling_phase -->


    <owl:ObjectProperty rdf:about="https://photogrammetry.altervista.org/items/show/233#Y42_was_continued_by_Modelling_phase">
        <rdfs:subPropertyOf rdf:resource="http://www.semanticweb.org/vitto/ontologies/2024/9/PODS_1#P134_continued_(was_continued_by)"/>
        <rdfs:subPropertyOf rdf:resource="https://photogrammetry.altervista.org/items/show/266#Y93:_was_continued_by_subsequent_phase"/>
        <rdfs:domain rdf:resource="https://photogrammetry.altervista.org/items/show/89#F3_Processing"/>
        <rdfs:range rdf:resource="https://photogrammetry.altervista.org/items/show/90#F4_Modelling"/>
        <rdfs:comment xml:lang="en">This property is redundant and can be replaced by the superproperty 
-Y93 was continued by subsequent phase-</rdfs:comment>
        <rdfs:label xml:lang="en">was_continued_by_modelling_phase</rdfs:label>
        <skos:definition xml:lang="en">Y42: was continued by Modelling phase

Subproperty of: P134i was continued by
Domain: F3 Processing
Range: F4 Modelling</skos:definition>
        <skos:example xml:lang="en">A F3 Processing phase was continued by an F4 Modelling phase, where a 3D model was generated from the processed data.</skos:example>
    </owl:ObjectProperty>
    


    <!-- https://photogrammetry.altervista.org/items/show/234#Y43_has_type_of_texturing -->


    <owl:ObjectProperty rdf:about="https://photogrammetry.altervista.org/items/show/234#Y43_has_type_of_texturing">
        <rdfs:subPropertyOf rdf:resource="http://www.semanticweb.org/vitto/ontologies/2024/9/PODS_1#P2__has_type_(is_type_of)"/>
        <rdfs:domain rdf:resource="https://photogrammetry.altervista.org/items/show/102#F16_Texturing_Method"/>
        <rdfs:range rdf:resource="https://photogrammetry.altervista.org/items/show/110#F24__Texturing_Type"/>
        <rdfs:label xml:lang="en">has_type_of_texturing</rdfs:label>
        <skos:definition xml:lang="en">Y43: has type of texturing

Subproperty of: P2 has type
Domain: F16 Texturing Method
Range: F24 Texturing Type</skos:definition>
        <skos:example xml:lang="en">A F16 Texturing Method has a F24 Texturing Type, such as UV Mapping applied to a 3D model.</skos:example>
        <skos:scopeNote xml:lang="en">This property relates a texturing method (F16) to the type of texturing (F24) applied, such as UV mapping or procedural texturing.</skos:scopeNote>
    </owl:ObjectProperty>
    


    <!-- https://photogrammetry.altervista.org/items/show/235#Y44_has_type_of_reconstruction -->


    <owl:ObjectProperty rdf:about="https://photogrammetry.altervista.org/items/show/235#Y44_has_type_of_reconstruction">
        <rdfs:subPropertyOf rdf:resource="http://www.semanticweb.org/vitto/ontologies/2024/9/PODS_1#P2__has_type_(is_type_of)"/>
        <rdfs:domain rdf:resource="https://photogrammetry.altervista.org/items/show/101#F15_Recontruction_Method"/>
        <rdfs:range rdf:resource="https://photogrammetry.altervista.org/items/show/109#F23_Reconstruction_Algorithm_Type"/>
        <rdfs:label xml:lang="en">has_type_of_reconstruction</rdfs:label>
        <skos:definition xml:lang="en">Y44: has type of reconstruction

Subproperty of: P2 has type
Domain: F15 Reconstruction Method
Range: F23 Reconstruction Algorithm Type</skos:definition>
        <skos:example xml:lang="en">A F15 Reconstruction Method uses a F23 Reconstruction Algorithm Type, such as a volumetric method for mesh creation.</skos:example>
        <skos:scopeNote xml:lang="en">This property links a reconstruction method (F15) to the type of algorithm used for the reconstruction (F23), such as volumetric or point-based reconstruction.</skos:scopeNote>
    </owl:ObjectProperty>
    


    <!-- https://photogrammetry.altervista.org/items/show/236#Y45_point_cloud_input -->


    <owl:ObjectProperty rdf:about="https://photogrammetry.altervista.org/items/show/236#Y45_point_cloud_input">
        <rdfs:subPropertyOf rdf:resource="http://www.semanticweb.org/vitto/ontologies/2024/9/PODS_1#L10_had_input_(was_input_of)"/>
        <rdfs:domain rdf:resource="https://photogrammetry.altervista.org/items/show/142#F56_Mesh_Reconstruction"/>
        <rdfs:range rdf:resource="https://photogrammetry.altervista.org/items/show/113#F27_Densified_Point_Cloud"/>
        <rdfs:label xml:lang="en">point_cloud_input</rdfs:label>
        <skos:definition xml:lang="en">Y45: point cloud input

Subproperty of: L10 had input
Domain: F56 Mesh Reconstruction
Range: F27 Densified Point Cloud</skos:definition>
        <skos:example xml:lang="en">A F56 Mesh Reconstruction process takes in a F27 Densified Point Cloud as input for generating a 3D mesh.</skos:example>
        <skos:scopeNote xml:lang="en">This property connects a mesh reconstruction process (F56) with the input densified point cloud (F27) used to create the mesh.</skos:scopeNote>
    </owl:ObjectProperty>
    


    <!-- https://photogrammetry.altervista.org/items/show/237#Y46_has_created_3D_Mesh -->


    <owl:ObjectProperty rdf:about="https://photogrammetry.altervista.org/items/show/237#Y46_has_created_3D_Mesh">
        <rdfs:subPropertyOf rdf:resource="http://www.semanticweb.org/vitto/ontologies/2024/9/PODS_1#L11_had_output_(was_output_of)"/>
        <rdfs:domain rdf:resource="https://photogrammetry.altervista.org/items/show/142#F56_Mesh_Reconstruction"/>
        <rdfs:range rdf:resource="https://photogrammetry.altervista.org/items/show/114#F28_3D_Mesh"/>
        <rdfs:label xml:lang="en">has_created_tridimensional_mesh</rdfs:label>
        <skos:definition xml:lang="en">Y46: has created 3D Mesh

Subproperty of: L11 has output
Domain: F56 Mesh Reconstruction
Range: F28 3D Mesh</skos:definition>
        <skos:example xml:lang="en">A F56 Mesh Reconstruction process has created a F28 3D Mesh representing the geometry of the scanned object.</skos:example>
        <skos:scopeNote xml:lang="en">This property indicates that the output of a mesh reconstruction process (F56) is a 3D mesh (F28).</skos:scopeNote>
    </owl:ObjectProperty>
    


    <!-- https://photogrammetry.altervista.org/items/show/238#Y47_has_method_of_reconstruction -->


    <owl:ObjectProperty rdf:about="https://photogrammetry.altervista.org/items/show/238#Y47_has_method_of_reconstruction">
        <rdfs:subPropertyOf rdf:resource="http://www.semanticweb.org/vitto/ontologies/2024/9/PODS_1#P33_used_specific_technique_(was_used_by)"/>
        <rdfs:domain rdf:resource="https://photogrammetry.altervista.org/items/show/142#F56_Mesh_Reconstruction"/>
        <rdfs:range rdf:resource="https://photogrammetry.altervista.org/items/show/101#F15_Recontruction_Method"/>
        <rdfs:label xml:lang="en">has_method_of_reconstruction</rdfs:label>
        <skos:definition xml:lang="en">Y47: has method of reconstruction

Subproperty of: P33 used specific technique
Domain: F56 Mesh Reconstruction
Range: F15 Reconstruction Method</skos:definition>
        <skos:example xml:lang="en">A F56 Mesh Reconstruction process uses a F15 Reconstruction Method, such as a surface reconstruction technique.</skos:example>
        <skos:scopeNote xml:lang="en">This property associates a mesh reconstruction process (F56) with the specific reconstruction method (F15) it used, such as surface reconstruction or volumetric reconstruction.</skos:scopeNote>
    </owl:ObjectProperty>
    


    <!-- https://photogrammetry.altervista.org/items/show/239#Y48_has_method_of_texturing -->


    <owl:ObjectProperty rdf:about="https://photogrammetry.altervista.org/items/show/239#Y48_has_method_of_texturing">
        <rdfs:subPropertyOf rdf:resource="http://www.semanticweb.org/vitto/ontologies/2024/9/PODS_1#P33_used_specific_technique_(was_used_by)"/>
        <rdfs:domain rdf:resource="https://photogrammetry.altervista.org/items/show/143#F57_Texturing_Mesh"/>
        <rdfs:range rdf:resource="https://photogrammetry.altervista.org/items/show/102#F16_Texturing_Method"/>
        <rdfs:label xml:lang="en">has_method_of_texturing</rdfs:label>
        <skos:definition xml:lang="en">Y48: has method of texturing

Subproperty of: P33 used specific technique
Domain: F57 Texturing Mesh
Range: F16 Texturing Method</skos:definition>
        <skos:example xml:lang="en">A F57 Texturing Mesh process uses a F16 Texturing Method, such as UV Mapping for applying textures to a 3D mesh.</skos:example>
        <skos:scopeNote xml:lang="en">This property connects a texturing process (F57) with the specific texturing method (F16) it employs, such as UV mapping or projective texturing.</skos:scopeNote>
    </owl:ObjectProperty>
    


    <!-- https://photogrammetry.altervista.org/items/show/240#Y49_has_created_Digital_Twin -->


    <owl:ObjectProperty rdf:about="https://photogrammetry.altervista.org/items/show/240#Y49_has_created_Digital_Twin">
        <rdfs:subPropertyOf rdf:resource="http://www.semanticweb.org/vitto/ontologies/2024/9/PODS_1#L11_had_output_(was_output_of)"/>
        <rdfs:domain rdf:resource="https://photogrammetry.altervista.org/items/show/144#F58_Modifying_Mesh"/>
        <rdfs:range rdf:resource="https://photogrammetry.altervista.org/items/show/145#F100_3D_Digital_Twin"/>
        <rdfs:label xml:lang="en">has_created_digital_twin</rdfs:label>
        <skos:definition xml:lang="en">Y49: has created Digital Twin

Subproperty of: L11 has output
Domain: F58 Modifying Mesh
Range: F100 Digital Twin</skos:definition>
        <skos:example xml:lang="en">A F58 Modifying Mesh process has created a F100 Digital Twin, accurately representing the physical object.</skos:example>
        <skos:scopeNote xml:lang="en">This property indicates that the output of a mesh modification process (F58) is a digital twin (F100), which is a precise digital replica of a real-world object.</skos:scopeNote>
    </owl:ObjectProperty>
    


    <!-- https://photogrammetry.altervista.org/items/show/241#Y50_happened_on_modelling_device -->


    <owl:ObjectProperty rdf:about="https://photogrammetry.altervista.org/items/show/241#Y50_happened_on_modelling_device">
        <rdfs:subPropertyOf rdf:resource="http://www.semanticweb.org/vitto/ontologies/2024/9/PODS_1#L12_happened_on_device_(was_device_for)"/>
        <rdfs:domain rdf:resource="https://photogrammetry.altervista.org/items/show/144#F58_Modifying_Mesh"/>
        <rdfs:range rdf:resource="https://photogrammetry.altervista.org/items/show/97#F11_Modelling_Device"/>
        <rdfs:label xml:lang="en">happened_on_modelling_device</rdfs:label>
        <skos:definition xml:lang="en">Y50: happened on modelling device

Subproperty of: L12 happened on device
Domain: F58 Modifying Mesh
Range: F11 Modelling Device</skos:definition>
        <skos:example xml:lang="en">A F58 Modifying Mesh process happened on an F11 Modelling Device, such as a high-end 3D modelling workstation.</skos:example>
        <skos:scopeNote xml:lang="en">This property connects a mesh modification process (F58) with the device (F11) on which it was carried out, such as a computer or a specific 3D modelling workstation.</skos:scopeNote>
    </owl:ObjectProperty>
    


    <!-- https://photogrammetry.altervista.org/items/show/242#Y51_Modelling_is_composed_of -->


    <owl:ObjectProperty rdf:about="https://photogrammetry.altervista.org/items/show/242#Y51_Modelling_is_composed_of">
        <rdfs:subPropertyOf rdf:resource="http://www.semanticweb.org/vitto/ontologies/2024/9/PODS_1#P9_consists_of_(forms_part_of)"/>
        <rdfs:domain rdf:resource="https://photogrammetry.altervista.org/items/show/90#F4_Modelling"/>
        <rdfs:range rdf:resource="https://photogrammetry.altervista.org/items/show/142#F56_Mesh_Reconstruction"/>
        <rdfs:range rdf:resource="https://photogrammetry.altervista.org/items/show/143#F57_Texturing_Mesh"/>
        <rdfs:range rdf:resource="https://photogrammetry.altervista.org/items/show/144#F58_Modifying_Mesh"/>
        <rdfs:label xml:lang="en">modelling_is_composed_of</rdfs:label>
        <skos:definition xml:lang="en">Y51: Modelling is composed of

Subproperty of: P9 consists of
Domain: F4 Modelling
Range: F56 Mesh Reconstruction / F57 Texturing Mesh / F58 Modifying Mesh</skos:definition>
        <skos:example xml:lang="en">A F4 Modelling process consists of F56 Mesh Reconstruction, F57 Texturing Mesh, and F58 Modifying Mesh, to complete the full 3D model.</skos:example>
        <skos:scopeNote xml:lang="en">This property indicates that a modelling process (F4) is composed of various sub-processes such as mesh reconstruction (F56), texturing (F57), and modifying mesh (F58).</skos:scopeNote>
    </owl:ObjectProperty>
    


    <!-- https://photogrammetry.altervista.org/items/show/243#Y52_had_3d_mesh_input -->


    <owl:ObjectProperty rdf:about="https://photogrammetry.altervista.org/items/show/243#Y52_had_3d_mesh_input">
        <rdfs:subPropertyOf rdf:resource="http://www.semanticweb.org/vitto/ontologies/2024/9/PODS_1#L10_had_input_(was_input_of)"/>
        <rdfs:domain rdf:resource="https://photogrammetry.altervista.org/items/show/114#F28_3D_Mesh"/>
        <rdfs:range rdf:resource="https://photogrammetry.altervista.org/items/show/143#F57_Texturing_Mesh"/>
        <rdfs:label xml:lang="en">tridimensional_mesh_input</rdfs:label>
        <skos:definition xml:lang="en">Y52: 3D mesh input
Subproperty of: L10 had input
Domain: F28 3D Mesh
Range: F57 Texturing Mesh</skos:definition>
        <skos:example xml:lang="en">A F28 3D Mesh is the input for a F57 Texturing Mesh process, where textures will be applied to the mesh.</skos:example>
        <skos:scopeNote xml:lang="en">This property links a 3D mesh (F28) as input for a texturing mesh process (F57).</skos:scopeNote>
    </owl:ObjectProperty>
    


    <!-- https://photogrammetry.altervista.org/items/show/244#Y53_had_Textured__3d_mesh_input -->


    <owl:ObjectProperty rdf:about="https://photogrammetry.altervista.org/items/show/244#Y53_had_Textured__3d_mesh_input">
        <rdfs:subPropertyOf rdf:resource="http://www.semanticweb.org/vitto/ontologies/2024/9/PODS_1#L10_had_input_(was_input_of)"/>
        <rdfs:domain rdf:resource="https://photogrammetry.altervista.org/items/show/115#F29_Textured_3D_Mesh"/>
        <rdfs:range rdf:resource="https://photogrammetry.altervista.org/items/show/144#F58_Modifying_Mesh"/>
        <rdfs:label xml:lang="en">textured_tridimensional_mesh_input</rdfs:label>
        <skos:definition xml:lang="en">Y53: Textured 3D mesh input

Subproperty of: L10 had input
Domain: F29 Textured Mesh
Range: F58 Modifying Mesh</skos:definition>
        <skos:example xml:lang="en">A F29 Textured Mesh serves as the input for an F58 Modifying Mesh process, where the textured mesh will undergo further refinement.</skos:example>
        <skos:scopeNote xml:lang="en">This property connects a textured 3D mesh (F29) as input for a mesh modification process (F58).</skos:scopeNote>
    </owl:ObjectProperty>
    


    <!-- https://photogrammetry.altervista.org/items/show/245#Y54_has_created_textured_3d_mesh -->


    <owl:ObjectProperty rdf:about="https://photogrammetry.altervista.org/items/show/245#Y54_has_created_textured_3d_mesh">
        <rdfs:subPropertyOf rdf:resource="http://www.semanticweb.org/vitto/ontologies/2024/9/PODS_1#L11_had_output_(was_output_of)"/>
        <rdfs:domain rdf:resource="https://photogrammetry.altervista.org/items/show/143#F57_Texturing_Mesh"/>
        <rdfs:range rdf:resource="https://photogrammetry.altervista.org/items/show/115#F29_Textured_3D_Mesh"/>
        <rdfs:label xml:lang="en">has_created_textured_tridimensional_mesh</rdfs:label>
        <skos:definition xml:lang="en">Y54: has created textured 3D mesh

Subproperty of: L11 has output
Domain: F57 Texturing Mesh
Range: F29 Textured Mesh</skos:definition>
        <skos:example xml:lang="en">A F57 Texturing Mesh process has created a F29 Textured Mesh, which includes both geometry and applied textures.</skos:example>
        <skos:scopeNote xml:lang="en">This property indicates that the output of a texturing mesh process (F57) is a textured 3D mesh (F29).</skos:scopeNote>
    </owl:ObjectProperty>
    


    <!-- https://photogrammetry.altervista.org/items/show/246#Y55_has_digital_scale -->


    <owl:ObjectProperty rdf:about="https://photogrammetry.altervista.org/items/show/246#Y55_has_digital_scale">
        <rdfs:subPropertyOf rdf:resource="http://www.semanticweb.org/vitto/ontologies/2024/9/PODS_1#P43_has_dimension_(is_dimension_of)"/>
        <rdfs:domain rdf:resource="https://photogrammetry.altervista.org/items/show/145#F100_3D_Digital_Twin"/>
        <rdfs:range rdf:resource="https://photogrammetry.altervista.org/items/show/146#F59_Digital_Scale"/>
        <rdfs:label xml:lang="en">has_digital_scale</rdfs:label>
        <skos:definition xml:lang="en">Y55: has digital scale

Subproperty of: P43 has dimension
Domain: F100 Digital Twin
Range: F59 Digital Scale</skos:definition>
        <skos:example xml:lang="en">A F100 Digital Twin has a F59 Digital Scale of 1:50, representing the scale used to model the digital twin.</skos:example>
        <skos:scopeNote xml:lang="en">This property links a digital twin (F100) to its digital scale (F59), which represents the measurement scale in the digital environment.</skos:scopeNote>
    </owl:ObjectProperty>
    


    <!-- https://photogrammetry.altervista.org/items/show/247#Y56_has_smoothing_filter -->


    <owl:ObjectProperty rdf:about="https://photogrammetry.altervista.org/items/show/247#Y56_has_smoothing_filter">
        <rdfs:subPropertyOf rdf:resource="http://www.semanticweb.org/vitto/ontologies/2024/9/PODS_1#P141_assigned_(was_assigned_by)"/>
        <rdfs:domain rdf:resource="https://photogrammetry.altervista.org/items/show/114#F28_3D_Mesh"/>
        <rdfs:range rdf:resource="https://photogrammetry.altervista.org/items/show/147#F60_Smoothing_Filter"/>
        <rdfs:label xml:lang="en">has_smoothing_filter</rdfs:label>
        <skos:definition xml:lang="en">Y56: has smoothing filter

Subproperty of: P141i was assigned by
Domain: F28 3D Mesh
Range: F60 Smoothing Filter</skos:definition>
        <skos:example xml:lang="en">A F28 3D Mesh has been assigned a F60 Smoothing Filter to soften rough areas in the model.</skos:example>
        <skos:scopeNote xml:lang="en">This property connects a 3D mesh (F28) with the smoothing filter (F60) applied to reduce noise or irregularities in the mesh.</skos:scopeNote>
    </owl:ObjectProperty>
    


    <!-- https://photogrammetry.altervista.org/items/show/248#Y57_has_color_balance/multiband -->


    <owl:ObjectProperty rdf:about="https://photogrammetry.altervista.org/items/show/248#Y57_has_color_balance/multiband">
        <rdfs:subPropertyOf rdf:resource="http://www.semanticweb.org/vitto/ontologies/2024/9/PODS_1#P141_assigned_(was_assigned_by)"/>
        <rdfs:domain rdf:resource="https://photogrammetry.altervista.org/items/show/149#F62_Texture_Set_of_3D_Mesh"/>
        <rdfs:range rdf:resource="https://photogrammetry.altervista.org/items/show/148#F61_Color_Balance/Multiband_Texture"/>
        <rdfs:label xml:lang="en">has_color_balance_or_multiband</rdfs:label>
        <skos:definition xml:lang="en">Y57: has color balance/multiband

Subproperty of: P141i was assigned by
Domain: F62 Texture Set of 3D Mesh
Range: F61 Color Balance/Multiband Texture</skos:definition>
        <skos:example xml:lang="en">A F62 Texture Set of 3D Mesh has a F61 Color Balance/Multiband Texture applied to achieve a natural and balanced appearance.</skos:example>
        <skos:scopeNote xml:lang="en">This property relates a set of textures on a 3D mesh (F62) to the color balance or multiband processing (F61) used in its creation.</skos:scopeNote>
    </owl:ObjectProperty>
    


    <!-- https://photogrammetry.altervista.org/items/show/250#Y59__is_texture_set_of -->


    <owl:ObjectProperty rdf:about="https://photogrammetry.altervista.org/items/show/250#Y59__is_texture_set_of">
        <rdfs:subPropertyOf rdf:resource="http://www.semanticweb.org/vitto/ontologies/2024/9/PODS_1#P106_is_composed_of_(forms_part_of)"/>
        <rdfs:domain rdf:resource="https://photogrammetry.altervista.org/items/show/149#F62_Texture_Set_of_3D_Mesh"/>
        <rdfs:range rdf:resource="https://photogrammetry.altervista.org/items/show/115#F29_Textured_3D_Mesh"/>
        <rdfs:label xml:lang="en">is_texture_set_of</rdfs:label>
        <skos:definition xml:lang="en">Y59: is texture set of

Subproperty of: P106i forms part of
Domain: F62 Texture Set of 3D Mesh
Range: F29 Textured Mesh</skos:definition>
        <skos:example xml:lang="en">A F62 Texture Set of 3D Mesh is part of a F29 Textured Mesh, providing the texture details for the mesh.</skos:example>
        <skos:scopeNote xml:lang="en">This property indicates that a texture set (F62) forms part of a textured 3D mesh (F29), contributing to its visual representation.</skos:scopeNote>
    </owl:ObjectProperty>
    


    <!-- https://photogrammetry.altervista.org/items/show/252#Y61_used_modelling_software -->


    <owl:ObjectProperty rdf:about="https://photogrammetry.altervista.org/items/show/252#Y61_used_modelling_software">
        <rdfs:subPropertyOf rdf:resource="http://www.semanticweb.org/vitto/ontologies/2024/9/PODS_1#L23_used_software_or_firmware_(was_software_or_firmware_used_by)"/>
        <rdfs:domain rdf:resource="https://photogrammetry.altervista.org/items/show/144#F58_Modifying_Mesh"/>
        <rdfs:range rdf:resource="https://photogrammetry.altervista.org/items/show/118#F32_Modelling_Software"/>
        <rdfs:label xml:lang="en">used_modifying_software</rdfs:label>
        <skos:definition xml:lang="en">Y61: used modelling software

Subproperty of: L23 used software or firmware
Domain: F58 Modifying 3D Mesh
Range: F32 Modelling Software</skos:definition>
        <skos:example xml:lang="en">A F58 Modifying 3D Mesh process used F32 Modelling Software, such as Blender or Autodesk Maya, to alter the 3D model.</skos:example>
        <skos:scopeNote xml:lang="en">This property connects a 3D mesh modification process (F58) with the software (F32) used during the modification.</skos:scopeNote>
    </owl:ObjectProperty>
    


    <!-- https://photogrammetry.altervista.org/items/show/254#Y63_has_date_of_modelling -->


    <owl:ObjectProperty rdf:about="https://photogrammetry.altervista.org/items/show/254#Y63_has_date_of_modelling">
        <rdfs:subPropertyOf rdf:resource="http://www.semanticweb.org/vitto/ontologies/2024/9/PODS_1#P4_has_time-span_(is_time-span_of)"/>
        <rdfs:domain rdf:resource="https://photogrammetry.altervista.org/items/show/144#F58_Modifying_Mesh"/>
        <rdfs:range rdf:resource="https://photogrammetry.altervista.org/items/show/152#F65_Modelling_Date"/>
        <rdfs:label xml:lang="en">has_date_of_acquisition</rdfs:label>
        <skos:definition xml:lang="en">Y63: has date of acquisition

Subproperty of: P4 has time span
Domain: F58 Modifying Mesh
Range: F65 Modelling Date</skos:definition>
        <skos:example xml:lang="en">A F58 Modifying Mesh process has a F65 Modelling Date, such as &quot;August 12, 2023,&quot; marking when the model was altered.</skos:example>
        <skos:scopeNote xml:lang="en">This property connects a 3D mesh modification process (F58) with the date (F65) on which the modification was carried out.</skos:scopeNote>
    </owl:ObjectProperty>
    


    <!-- https://photogrammetry.altervista.org/items/show/255#Y65_Modelling_is_influenced_by -->


    <owl:ObjectProperty rdf:about="https://photogrammetry.altervista.org/items/show/255#Y65_Modelling_is_influenced_by">
        <rdfs:subPropertyOf rdf:resource="http://www.semanticweb.org/vitto/ontologies/2024/9/PODS_1#P15_was_influenced_by_(influenced)"/>
        <rdfs:domain rdf:resource="https://photogrammetry.altervista.org/items/show/144#F58_Modifying_Mesh"/>
        <rdfs:range rdf:resource="https://photogrammetry.altervista.org/items/show/153#F66_Modelling_Determination"/>
        <rdfs:range rdf:resource="https://photogrammetry.altervista.org/items/show/154#F67_Modelling_Elimination"/>
        <rdfs:label xml:lang="en">modifying_is_influenced_by</rdfs:label>
        <skos:definition xml:lang="en">Y65: Modelling is influenced by

Subproperty of: P15i influenced
Domain: F58 Modifying Mesh
Range: F66 Modelling Determination / F67 Modelling Elimination</skos:definition>
        <skos:example xml:lang="en">A F58 Modifying Mesh process is influenced by a F66 Modelling Determination, such as a specific requirement to improve edge flow or reduce polygon count in the model.</skos:example>
        <skos:scopeNote xml:lang="en">This property links a 3D mesh modification process (F58) to the factors (F66/F67) that influenced or eliminated aspects of the model.</skos:scopeNote>
    </owl:ObjectProperty>
    


    <!-- https://photogrammetry.altervista.org/items/show/257#Y67_was_continued_by_Exporting_phase -->


    <owl:ObjectProperty rdf:about="https://photogrammetry.altervista.org/items/show/257#Y67_was_continued_by_Exporting_phase">
        <rdfs:subPropertyOf rdf:resource="http://www.semanticweb.org/vitto/ontologies/2024/9/PODS_1#P134_continued_(was_continued_by)"/>
        <rdfs:subPropertyOf rdf:resource="https://photogrammetry.altervista.org/items/show/266#Y93:_was_continued_by_subsequent_phase"/>
        <rdfs:domain rdf:resource="https://photogrammetry.altervista.org/items/show/90#F4_Modelling"/>
        <rdfs:range rdf:resource="https://photogrammetry.altervista.org/items/show/91#F5_Exporting"/>
        <rdfs:comment xml:lang="en">This property is redundant and can be replaced by the superproperty
-Y93 was continued by subsequent phase-</rdfs:comment>
        <rdfs:label xml:lang="en">was_continued_by_exporting_phase</rdfs:label>
        <skos:definition xml:lang="en">Y67: was continued by Exporting phase

Subproperty of: P134i was continued by

Domain
F4 Modelling

Range
F5 Exporting</skos:definition>
        <skos:example xml:lang="en">A F4 Modelling process was continued by a F5 Exporting phase, where the model was exported in a standard format, like OBJ or STL.</skos:example>
        <skos:scopeNote xml:lang="en">This property indicates that a modelling process (F4) was continued by an exporting phase (F5), marking the transition from modelling to exporting the model into a usable format.</skos:scopeNote>
    </owl:ObjectProperty>
    


    <!-- https://photogrammetry.altervista.org/items/show/258#Y68_has_Textured_3D_Model_as_input -->


    <owl:ObjectProperty rdf:about="https://photogrammetry.altervista.org/items/show/258#Y68_has_Textured_3D_Model_as_input">
        <rdfs:subPropertyOf rdf:resource="http://www.semanticweb.org/vitto/ontologies/2024/9/PODS_1#L10_had_input_(was_input_of)"/>
        <rdfs:domain rdf:resource="https://photogrammetry.altervista.org/items/show/91#F5_Exporting"/>
        <rdfs:range rdf:resource="https://photogrammetry.altervista.org/items/show/115#F29_Textured_3D_Mesh"/>
        <rdfs:label xml:lang="en">has_textured_tridimensional_model_as_input</rdfs:label>
        <skos:definition xml:lang="en">Y68: has Textured 3D Model as input
Subproperty of: L10 had input

Domain
F5 Exporting

Range
F29 Textured 3D Model</skos:definition>
        <skos:example xml:lang="en">During the F5 Exporting process, a F29 Textured 3D Model was used as input for generating a final 3D product.</skos:example>
        <skos:scopeNote xml:lang="en">This property relates the exporting phase (F5) to a textured 3D model (F29) that serves as input during the exporting process.</skos:scopeNote>
    </owl:ObjectProperty>
    


    <!-- https://photogrammetry.altervista.org/items/show/259#Y69_has_Digital_Twin_as_output -->


    <owl:ObjectProperty rdf:about="https://photogrammetry.altervista.org/items/show/259#Y69_has_Digital_Twin_as_output">
        <rdfs:subPropertyOf rdf:resource="http://www.semanticweb.org/vitto/ontologies/2024/9/PODS_1#L11_had_output_(was_output_of)"/>
        <rdfs:domain rdf:resource="https://photogrammetry.altervista.org/items/show/91#F5_Exporting"/>
        <rdfs:range rdf:resource="https://photogrammetry.altervista.org/items/show/145#F100_3D_Digital_Twin"/>
        <rdfs:label xml:lang="en">has_tridimensional_digital_twin_as_output</rdfs:label>
        <skos:definition xml:lang="en">Y69: has Digital Twin as output
Subproperty of: L11 had output

Domain
F5 Exporting

Range
F100 Digital Twin</skos:definition>
        <skos:example xml:lang="en">A F5 Exporting phase has produced a F100 Digital Twin, representing the final exported digital copy of the model.</skos:example>
        <skos:scopeNote xml:lang="en">This property indicates that the result of the exporting phase (F5) is a digital twin (F100), which is the digital output of the process.</skos:scopeNote>
    </owl:ObjectProperty>
    


    <!-- https://photogrammetry.altervista.org/items/show/260#Y70_Final_Use_of_3D_Model_consist_of -->


    <owl:ObjectProperty rdf:about="https://photogrammetry.altervista.org/items/show/260#Y70_Final_Use_of_3D_Model_consist_of">
        <rdfs:subPropertyOf rdf:resource="http://www.semanticweb.org/vitto/ontologies/2024/9/PODS_1#P9_consists_of_(forms_part_of)"/>
        <rdfs:domain rdf:resource="https://photogrammetry.altervista.org/items/show/91#F5_Exporting"/>
        <rdfs:range rdf:resource="https://photogrammetry.altervista.org/items/show/158#F71_Final_Use_of_Digital_Twin"/>
        <rdfs:label xml:lang="en">exporting_tridimensional_digital_twin_consists_of</rdfs:label>
        <skos:definition xml:lang="en">Y70: Final Use of 3D Model consists of
Subproperty of: P9 consists of

Domain
F5 Exporting

Range
F71 Final Use of 3D Model</skos:definition>
        <skos:example xml:lang="en">The F5 Exporting phase defines that the F71 Final Use of the 3D Model will be for 3D printing.</skos:example>
        <skos:scopeNote xml:lang="en">This property indicates that the final use of the 3D model (F71) is defined or composed during the exporting phase (F5).</skos:scopeNote>
    </owl:ObjectProperty>
    


    <!-- https://photogrammetry.altervista.org/items/show/262#Y72_had_final_use_output -->


    <owl:ObjectProperty rdf:about="https://photogrammetry.altervista.org/items/show/262#Y72_had_final_use_output">
        <rdfs:subPropertyOf rdf:resource="http://www.semanticweb.org/vitto/ontologies/2024/9/PODS_1#L11_had_output_(was_output_of)"/>
        <rdfs:domain rdf:resource="https://photogrammetry.altervista.org/items/show/158#F71_Final_Use_of_Digital_Twin"/>
        <rdfs:range rdf:resource="https://photogrammetry.altervista.org/items/show/159#F72_3D_Model_Video_Rendering"/>
        <rdfs:range rdf:resource="https://photogrammetry.altervista.org/items/show/163#F76_3D_Model_for_3D_Print"/>
        <rdfs:range rdf:resource="https://photogrammetry.altervista.org/items/show/168#F81_3D_Model_for_G.I.S."/>
        <rdfs:range rdf:resource="https://photogrammetry.altervista.org/items/show/171#F84_3D_Model_for_Prospectus"/>
        <rdfs:range rdf:resource="https://photogrammetry.altervista.org/items/show/174#F87_3D_Model_Prospectus"/>
        <rdfs:range rdf:resource="https://photogrammetry.altervista.org/items/show/175#F88_Archaeometric_3D_Model"/>
        <rdfs:range rdf:resource="https://photogrammetry.altervista.org/items/show/178#F91_Model_for_Interactive"/>
        <rdfs:range rdf:resource="https://photogrammetry.altervista.org/items/show/181#F94_3D_Model_for_Database"/>
        <rdfs:range rdf:resource="https://photogrammetry.altervista.org/items/show/184#F97_AR_3D_Model"/>
        <rdfs:label xml:lang="en">exporting_has_output</rdfs:label>
        <skos:definition xml:lang="en">Y72: had final use output
Subproperty of: L11 had output

Domain
F71 Final Use of 3D Model

Range
F72 3D Model Video Rendering, F76 3D Model for 3D Print, F81 3D Model for G.I.S., F84 3D Model for Prospectuses, F88 3D Model for Research, F91 3D Model for Interactive, F94 3D Model for Database</skos:definition>
        <skos:example xml:lang="en">The F71 Final Use of the 3D Model has produced F72 3D Model Video Rendering and F76 3D Model for 3D Print as output formats for different applications.</skos:example>
        <skos:scopeNote xml:lang="en">This property connects the final use of a 3D model (F71) to its specific output form (F72, F76, F81, etc.), depending on the intended application of the model.</skos:scopeNote>
    </owl:ObjectProperty>
    


    <!-- https://photogrammetry.altervista.org/items/show/263#Y73:_had_rendering_as_input -->


    <owl:ObjectProperty rdf:about="https://photogrammetry.altervista.org/items/show/263#Y73:_had_rendering_as_input">
        <rdfs:subPropertyOf rdf:resource="http://www.semanticweb.org/vitto/ontologies/2024/9/PODS_1#L10_had_input_(was_input_of)"/>
        <rdfs:domain rdf:resource="https://photogrammetry.altervista.org/items/show/160#F73_Editing_Video"/>
        <rdfs:range rdf:resource="https://photogrammetry.altervista.org/items/show/159#F72_3D_Model_Video_Rendering"/>
        <rdfs:label xml:lang="en">had_rendering_as_input</rdfs:label>
        <skos:definition xml:lang="en">Y73: had rendering as input
Subproperty of: L10 had input

Domain
Editing Video

Range
3D Model Video Rendering</skos:definition>
        <skos:example xml:lang="en">The Editing Video process had a Rendering as input, handled by Video Editing Software such as Adobe Premiere.</skos:example>
        <skos:scopeNote xml:lang="en">This property links the rendering process (as part of video creation) to the video editing software that serves as the input for further editing.</skos:scopeNote>
    </owl:ObjectProperty>
    


    <!-- https://photogrammetry.altervista.org/items/show/264#Y95:_was_measured_in_number_of_points -->


    <owl:ObjectProperty rdf:about="https://photogrammetry.altervista.org/items/show/264#Y95:_was_measured_in_number_of_points">
        <rdfs:subPropertyOf rdf:resource="http://www.semanticweb.org/vitto/ontologies/2024/9/PODS_1#O24_measured_(was_measured_by)"/>
        <rdfs:domain rdf:resource="https://photogrammetry.altervista.org/items/show/112#F26_Point_Cloud"/>
        <rdfs:domain rdf:resource="https://photogrammetry.altervista.org/items/show/113#F27_Densified_Point_Cloud"/>
        <rdfs:range rdf:resource="https://photogrammetry.altervista.org/items/show/136#F50_Point_Cloud_Measurement"/>
        <rdfs:range rdf:resource="https://photogrammetry.altervista.org/items/show/138#F52_Dense_Point_Cloud_Measurement"/>
        <rdfs:label xml:lang="en">was_measured_in_number_of_points</rdfs:label>
        <skos:definition xml:lang="en">Y95: was measured in number of points
Subproperty of: O24 measured

Domain
F26 Point Cloud, F27 Dense Point Cloud

Range
F50 Point Cloud Measurement, F52 Dense Point Cloud Measurement</skos:definition>
        <skos:example xml:lang="en">A F26 Point Cloud was measured in F50 Point Cloud Measurement, which recorded 600,000 points in a typical scan.</skos:example>
        <skos:example xml:lang="en">A F27 Dense Point Cloud was measured in F52 Dense Point Cloud Measurement, which recorded 15,000,000 points in a high-resolution scan.</skos:example>
        <skos:scopeNote xml:lang="en">This property connects a Point Cloud (F26) or a Dense Point Cloud (F27) with the corresponding Point Cloud Measurement (F50) or Dense Point Cloud Measurement (F52), indicating that the cloud was measured in terms of the number of points it contains. It defines the relationship between the point cloud as a data set and the measurement process that captures its resolution by counting the number of individual points within the cloud.</skos:scopeNote>
    </owl:ObjectProperty>
    


    <!-- https://photogrammetry.altervista.org/items/show/266#Y93:_was_continued_by_subsequent_phase -->


    <owl:ObjectProperty rdf:about="https://photogrammetry.altervista.org/items/show/266#Y93:_was_continued_by_subsequent_phase">
        <rdfs:subPropertyOf rdf:resource="http://www.semanticweb.org/vitto/ontologies/2024/9/PODS_1#P134_continued_(was_continued_by)"/>
        <rdfs:domain rdf:resource="https://photogrammetry.altervista.org/items/show/187#F101_Survey_Phase"/>
        <rdfs:range rdf:resource="https://photogrammetry.altervista.org/items/show/187#F101_Survey_Phase"/>
        <rdfs:label xml:lang="en">was_continued_by_subsequent_phase</rdfs:label>
        <skos:definition xml:lang="en">Y93: was continued by subsequent phase
Subproperty of: 
P134i was continued by
Domain: F101 Survey Phase
Range: F101 Survey Phase</skos:definition>
        <skos:example xml:lang="en">A Survey Phase focused on preliminary data gathering was continued by a subsequent Survey Phase dedicated to higher-resolution data acquisition.</skos:example>
        <skos:scopeNote xml:lang="en">This property connects one Survey Phase (F101) to a subsequent Survey Phase (F101), marking the progression of the survey process from one phase to another. The aim of this property is to articulate the sequence of phases involved in a survey, often defined by different design choices or procedural steps. It highlights how a given survey phase transitions into a new one, either in terms of methodology or operational focus.</skos:scopeNote>
    </owl:ObjectProperty>
    


    <!-- https://photogrammetry.altervista.org/items/show/267#Y92:_used_AR/MR_software -->


    <owl:ObjectProperty rdf:about="https://photogrammetry.altervista.org/items/show/267#Y92:_used_AR/MR_software">
        <rdfs:subPropertyOf rdf:resource="http://www.semanticweb.org/vitto/ontologies/2024/9/PODS_1#L23_used_software_or_firmware_(was_software_or_firmware_used_by)"/>
        <rdfs:domain rdf:resource="https://photogrammetry.altervista.org/items/show/185#F98_AR/MR_Project_Implementation"/>
        <rdfs:range rdf:resource="https://photogrammetry.altervista.org/items/show/186#F99_AR_Software_Modelling"/>
        <rdfs:label xml:lang="en">used_augmented_or_mixed_reality_software</rdfs:label>
        <skos:definition xml:lang="en">Y92: used AR/MR software
Subproperty of: L23 used software

Domain
AR/MR Project

Range
AR Software Modelling</skos:definition>
        <skos:example xml:lang="en">-</skos:example>
        <skos:scopeNote xml:lang="en">This property indicates that the AR/MR project (AR/MR Project) used augmented reality software (AR Software Modelling) for developing and presenting AR content.</skos:scopeNote>
    </owl:ObjectProperty>
    


    <!-- https://photogrammetry.altervista.org/items/show/268#Y91:_had_3D_model_for_AR_as_input -->


    <owl:ObjectProperty rdf:about="https://photogrammetry.altervista.org/items/show/268#Y91:_had_3D_model_for_AR_as_input">
        <rdfs:subPropertyOf rdf:resource="http://www.semanticweb.org/vitto/ontologies/2024/9/PODS_1#L10_had_input_(was_input_of)"/>
        <rdfs:domain rdf:resource="https://photogrammetry.altervista.org/items/show/185#F98_AR/MR_Project_Implementation"/>
        <rdfs:range rdf:resource="https://photogrammetry.altervista.org/items/show/184#F97_AR_3D_Model"/>
        <rdfs:label xml:lang="en">had_tridimensional_model_for_augmented_reality_as_input</rdfs:label>
        <skos:definition xml:lang="en">Y91: had 3D model for AR as input
Subproperty of: L10 had input

Domain
AR/MR Project

Range
3D Model for Augmented Reality</skos:definition>
        <skos:example xml:lang="en">-</skos:example>
        <skos:scopeNote xml:lang="en">This property specifies that the AR/MR project (AR/MR Project) used a 3D model for augmented reality (3D Model for Augmented Reality) as its input.</skos:scopeNote>
    </owl:ObjectProperty>
    


    <!-- https://photogrammetry.altervista.org/items/show/269#Y90:_used_database_software/architecture -->


    <owl:ObjectProperty rdf:about="https://photogrammetry.altervista.org/items/show/269#Y90:_used_database_software/architecture">
        <rdfs:subPropertyOf rdf:resource="http://www.semanticweb.org/vitto/ontologies/2024/9/PODS_1#L23_used_software_or_firmware_(was_software_or_firmware_used_by)"/>
        <rdfs:domain rdf:resource="https://photogrammetry.altervista.org/items/show/182#F95_Database_Project_Implementation"/>
        <rdfs:range rdf:resource="https://photogrammetry.altervista.org/items/show/183#F96_Database_Architecture"/>
        <rdfs:label xml:lang="en">used_database_architecture</rdfs:label>
        <skos:definition xml:lang="en">Y90: used database software/architecture
Subproperty of: L23 used software

Domain
Database Project

Range
Database Architecture</skos:definition>
        <skos:example xml:lang="en">-</skos:example>
        <skos:scopeNote xml:lang="en">This property indicates that the database project (Database Project) used specific database software or architecture (Database Architecture) for managing and storing data.</skos:scopeNote>
    </owl:ObjectProperty>
    


    <!-- https://photogrammetry.altervista.org/items/show/270#Y89:_had_3D_model_for_database_as_input -->


    <owl:ObjectProperty rdf:about="https://photogrammetry.altervista.org/items/show/270#Y89:_had_3D_model_for_database_as_input">
        <rdfs:subPropertyOf rdf:resource="http://www.semanticweb.org/vitto/ontologies/2024/9/PODS_1#L10_had_input_(was_input_of)"/>
        <rdfs:domain rdf:resource="https://photogrammetry.altervista.org/items/show/182#F95_Database_Project_Implementation"/>
        <rdfs:range rdf:resource="https://photogrammetry.altervista.org/items/show/181#F94_3D_Model_for_Database"/>
        <rdfs:label xml:lang="en">had_model_for_database_as_input</rdfs:label>
        <skos:definition xml:lang="en">Y89: had 3D model for database as input
Subproperty of: L10 had input

Domain
Database Project

Range
3D Model for Database</skos:definition>
        <skos:example xml:lang="en">-</skos:example>
        <skos:scopeNote xml:lang="en">This property shows that the database project (Database Project) used a 3D model meant for database storage (3D Model for Database) as its input.</skos:scopeNote>
    </owl:ObjectProperty>
    


    <!-- https://photogrammetry.altervista.org/items/show/271#Y88:_used_interactive_software -->


    <owl:ObjectProperty rdf:about="https://photogrammetry.altervista.org/items/show/271#Y88:_used_interactive_software">
        <rdfs:subPropertyOf rdf:resource="http://www.semanticweb.org/vitto/ontologies/2024/9/PODS_1#L23_used_software_or_firmware_(was_software_or_firmware_used_by)"/>
        <rdfs:domain rdf:resource="https://photogrammetry.altervista.org/items/show/179#F92_Interactive_Project_Implementation"/>
        <rdfs:range rdf:resource="https://photogrammetry.altervista.org/items/show/180#F93_Interactive_Software"/>
        <rdfs:label xml:lang="en">used_interactive_software</rdfs:label>
        <skos:definition xml:lang="en">Y88: used interactive software
Subproperty of: L23 used software

Domain
Interactive Project

Range
Interactive Software</skos:definition>
        <skos:example xml:lang="en">-</skos:example>
        <skos:scopeNote xml:lang="en">This property indicates that the interactive project (Interactive Project) used interactive software (Interactive Software) to facilitate the project&apos;s immersive features.</skos:scopeNote>
    </owl:ObjectProperty>
    


    <!-- https://photogrammetry.altervista.org/items/show/272#Y87:_had_3D_model_interactive_as_input -->


    <owl:ObjectProperty rdf:about="https://photogrammetry.altervista.org/items/show/272#Y87:_had_3D_model_interactive_as_input">
        <rdfs:subPropertyOf rdf:resource="http://www.semanticweb.org/vitto/ontologies/2024/9/PODS_1#L10_had_input_(was_input_of)"/>
        <rdfs:domain rdf:resource="https://photogrammetry.altervista.org/items/show/179#F92_Interactive_Project_Implementation"/>
        <rdfs:range rdf:resource="https://photogrammetry.altervista.org/items/show/178#F91_Model_for_Interactive"/>
        <rdfs:label xml:lang="en">had_interactive_tridimensional_model_as_input</rdfs:label>
        <skos:definition xml:lang="en">Y87: had 3D model interactive as input
Subproperty of: L10 had input

Domain
Interactive Project

Range
3D Model for Interactive</skos:definition>
        <skos:example xml:lang="en">-</skos:example>
        <skos:scopeNote xml:lang="en">This property shows that the interactive project (Interactive Project) used a 3D model designed for interactive use (3D Model for Interactive) as its input.</skos:scopeNote>
    </owl:ObjectProperty>
    


    <!-- https://photogrammetry.altervista.org/items/show/273#Y86:_had_data_log_analysis_output -->


    <owl:ObjectProperty rdf:about="https://photogrammetry.altervista.org/items/show/273#Y86:_had_data_log_analysis_output">
        <rdfs:subPropertyOf rdf:resource="http://www.semanticweb.org/vitto/ontologies/2024/9/PODS_1#L11_had_output_(was_output_of)"/>
        <rdfs:domain rdf:resource="https://photogrammetry.altervista.org/items/show/176#F89_Project_Analysis"/>
        <rdfs:range rdf:resource="https://photogrammetry.altervista.org/items/show/177#F90_Data_Log_Analysis"/>
        <rdfs:label xml:lang="en">had_data_log_analysis_output</rdfs:label>
        <skos:definition xml:lang="en">Y86: had data log analysis output
Subproperty of: L11 had output

Domain
Project Analysis

Range
Data Log Analysis</skos:definition>
        <skos:example xml:lang="en">-</skos:example>
        <skos:scopeNote xml:lang="en">This property indicates that the project analysis phase (Project Analysis) resulted in a data log analysis (Data Log Analysis) as its output.</skos:scopeNote>
    </owl:ObjectProperty>
    


    <!-- https://photogrammetry.altervista.org/items/show/274#Y85:_had_archaeometric_input -->


    <owl:ObjectProperty rdf:about="https://photogrammetry.altervista.org/items/show/274#Y85:_had_archaeometric_input">
        <rdfs:subPropertyOf rdf:resource="http://www.semanticweb.org/vitto/ontologies/2024/9/PODS_1#L10_had_input_(was_input_of)"/>
        <rdfs:domain rdf:resource="https://photogrammetry.altervista.org/items/show/176#F89_Project_Analysis"/>
        <rdfs:range rdf:resource="https://photogrammetry.altervista.org/items/show/175#F88_Archaeometric_3D_Model"/>
        <rdfs:label xml:lang="en">had_archaeometric_input</rdfs:label>
        <skos:definition xml:lang="en">Y85: had archaeometric input
Subproperty of: L10 had input

Domain
Project Analysis

Range
Archaeometric 3D Model</skos:definition>
        <skos:example xml:lang="en">-</skos:example>
        <skos:scopeNote xml:lang="en">This property specifies that the project analysis (Project Analysis) used an archaeometric 3D model (Archaeometric 3D Model) as an input for detailed material or structural analysis.</skos:scopeNote>
    </owl:ObjectProperty>
    


    <!-- https://photogrammetry.altervista.org/items/show/275#Y74:_use_video_editing_software -->


    <owl:ObjectProperty rdf:about="https://photogrammetry.altervista.org/items/show/275#Y74:_use_video_editing_software">
        <rdfs:subPropertyOf rdf:resource="http://www.semanticweb.org/vitto/ontologies/2024/9/PODS_1#L23_used_software_or_firmware_(was_software_or_firmware_used_by)"/>
        <rdfs:domain rdf:resource="https://photogrammetry.altervista.org/items/show/160#F73_Editing_Video"/>
        <rdfs:range rdf:resource="https://photogrammetry.altervista.org/items/show/161#F74_Video_Editing_Software"/>
        <rdfs:label xml:lang="en">used_video_editing_software</rdfs:label>
        <skos:definition xml:lang="en">Y74: use video editing software
Subproperty of: L23 used software or firmware
Domain
F73 Editing Video
Range
F74 Video Editing Software</skos:definition>
        <skos:example xml:lang="en">The Editing Video phase used Video Editing Software like Final Cut Pro to edit a 3D rendering video</skos:example>
        <skos:scopeNote xml:lang="en">This property specifies that the video editing process (Editing Video) used specific video editing software</skos:scopeNote>
    </owl:ObjectProperty>
    


    <!-- https://photogrammetry.altervista.org/items/show/276#Y75:_had_Video_output -->


    <owl:ObjectProperty rdf:about="https://photogrammetry.altervista.org/items/show/276#Y75:_had_Video_output">
        <rdfs:subPropertyOf rdf:resource="http://www.semanticweb.org/vitto/ontologies/2024/9/PODS_1#L11_had_output_(was_output_of)"/>
        <rdfs:domain rdf:resource="https://photogrammetry.altervista.org/items/show/160#F73_Editing_Video"/>
        <rdfs:range rdf:resource="https://photogrammetry.altervista.org/items/show/162#F75_Project_Video"/>
        <rdfs:label xml:lang="en">had_video_output</rdfs:label>
        <skos:definition xml:lang="en">Y75: had Video output
Subproperty of: L11 had output

Domain
F73 Editing Video

Range
F75 Project Video</skos:definition>
        <skos:example xml:lang="en">The Editing Video process produced a Project Video as output, which can be used for presentation or further rendering.</skos:example>
        <skos:scopeNote xml:lang="en">This property indicates that the video editing process (Editing Video) results in a project video (Project Video) as its output.</skos:scopeNote>
    </owl:ObjectProperty>
    


    <!-- https://photogrammetry.altervista.org/items/show/277#Y76:_printing_based_on -->


    <owl:ObjectProperty rdf:about="https://photogrammetry.altervista.org/items/show/277#Y76:_printing_based_on">
        <rdfs:subPropertyOf rdf:resource="http://www.semanticweb.org/vitto/ontologies/2024/9/PODS_1#P17_was_motivated_by_(motivated)"/>
        <rdfs:domain rdf:resource="https://photogrammetry.altervista.org/items/show/164#F77_Printing_Digital_Twin"/>
        <rdfs:range rdf:resource="https://photogrammetry.altervista.org/items/show/163#F76_3D_Model_for_3D_Print"/>
        <rdfs:label xml:lang="en">printing_based_on</rdfs:label>
        <skos:editorialNote xml:lang="en">Y76: printing based on
Subproperty of: P17 was motivated by

Domain
F77 Printing Digital Twin

Range
F76 3D Model for 3D Print</skos:editorialNote>
        <skos:example xml:lang="en">The Printing Digital Twin process is based on the 3D Model for 3D Print that was developed during the modelling phase.</skos:example>
        <skos:scopeNote xml:lang="en">This property shows that the printing process of a digital twin (Printing Digital Twin) is motivated by or based on a specific 3D model intended for 3D printing.</skos:scopeNote>
    </owl:ObjectProperty>
    


    <!-- https://photogrammetry.altervista.org/items/show/278#Y77:_has_printed_physical_digital_twin -->


    <owl:ObjectProperty rdf:about="https://photogrammetry.altervista.org/items/show/278#Y77:_has_printed_physical_digital_twin">
        <rdfs:subPropertyOf rdf:resource="http://www.semanticweb.org/vitto/ontologies/2024/9/PODS_1#P108_has_produced_(was_produced_by)"/>
        <rdfs:domain rdf:resource="https://photogrammetry.altervista.org/items/show/164#F77_Printing_Digital_Twin"/>
        <rdfs:range rdf:resource="https://photogrammetry.altervista.org/items/show/167#F80_Printed_Digital_Twin"/>
        <rdfs:label xml:lang="en">has_printed_physical_digital_twin</rdfs:label>
        <skos:definition xml:lang="en">Y77: has printed physical digital twin
Subproperty of: P108 has produced
Domain
F77 Printing Digital Twin
Range
F80 Printed Digital Twin</skos:definition>
        <skos:example xml:lang="en">The Printing Digital Twin process produced a Printed Digital Twin, representing the physical counterpart of the digital model.</skos:example>
        <skos:scopeNote xml:lang="en">This property links the printing process of a digital twin (Printing Digital Twin) to the final physical output, a Printed Digital Twin.</skos:scopeNote>
    </owl:ObjectProperty>
    


    <!-- https://photogrammetry.altervista.org/items/show/279#Y78:_used_specific_printing_machine -->


    <owl:ObjectProperty rdf:about="https://photogrammetry.altervista.org/items/show/279#Y78:_used_specific_printing_machine">
        <rdfs:subPropertyOf rdf:resource="http://www.semanticweb.org/vitto/ontologies/2024/9/PODS_1#P16_used_specific_object_(was_used_for)"/>
        <rdfs:domain rdf:resource="https://photogrammetry.altervista.org/items/show/164#F77_Printing_Digital_Twin"/>
        <rdfs:range rdf:resource="https://photogrammetry.altervista.org/items/show/166#F79_Printing_Device"/>
        <rdfs:label xml:lang="en">used_specific_printing_machine</rdfs:label>
        <skos:definition xml:lang="en">Y78: used specific printing machine
Subproperty of: P16 used specific object

Domain
F77 Printing Digital Twin

Range
F79 Printing Device</skos:definition>
        <skos:example xml:lang="en">The Printing Digital Twin process used a Printing Device like an SLS 3D printer</skos:example>
        <skos:scopeNote xml:lang="en">This property defines the specific printing machine (Printing Device) used in the process of printing a digital twin (Printing Digital Twin).</skos:scopeNote>
    </owl:ObjectProperty>
    


    <!-- https://photogrammetry.altervista.org/items/show/280#Y79:_consists_of_printing_material -->


    <owl:ObjectProperty rdf:about="https://photogrammetry.altervista.org/items/show/280#Y79:_consists_of_printing_material">
        <rdfs:subPropertyOf rdf:resource="http://www.semanticweb.org/vitto/ontologies/2024/9/PODS_1#P45_consists_of_(is_incorporated_in)"/>
        <rdfs:domain rdf:resource="https://photogrammetry.altervista.org/items/show/167#F80_Printed_Digital_Twin"/>
        <rdfs:range rdf:resource="https://photogrammetry.altervista.org/items/show/165#F78_Material_for_3D_Printing"/>
        <rdfs:label xml:lang="en">consists_of_printing_material</rdfs:label>
        <skos:definition xml:lang="en">Y79: consists of printing material

Subproperty of: P45 consists of

Domain
F80 Printed Digital Twin

Range
F78 Material for 3D Printed</skos:definition>
        <skos:example xml:lang="en">The Printed Digital Twin consists of Material for 3D Raw, such as PLA or resin.</skos:example>
        <skos:scopeNote xml:lang="en">This property indicates the materials (Material for 3D Raw) used in the creation of a Printed Digital Twin.</skos:scopeNote>
    </owl:ObjectProperty>
    


    <!-- https://photogrammetry.altervista.org/items/show/281#Y80:_is_in_GIS -->


    <owl:ObjectProperty rdf:about="https://photogrammetry.altervista.org/items/show/281#Y80:_is_in_GIS">
        <rdfs:subPropertyOf rdf:resource="http://www.semanticweb.org/vitto/ontologies/2024/9/PODS_1#P106_is_composed_of_(forms_part_of)"/>
        <rdfs:domain rdf:resource="https://photogrammetry.altervista.org/items/show/168#F81_3D_Model_for_G.I.S."/>
        <rdfs:range rdf:resource="https://photogrammetry.altervista.org/items/show/169#F82_Reference_GIS_System"/>
        <rdfs:label xml:lang="en">is_in_GIS</rdfs:label>
        <skos:definition xml:lang="en">Y80: is in GIS
Subproperty of: P106i forms part of

Domain
F81 3D Model for GIS

Range
F82 Reference GIS System</skos:definition>
        <skos:example xml:lang="en">The 3D Model for GIS is included in a Reference GIS System like ArcGIS for geospatial analysis.</skos:example>
        <skos:scopeNote xml:lang="en">This property indicates that a 3D model for GIS (3D Model for GIS) is integrated within a specific GIS system (Reference GIS System).</skos:scopeNote>
    </owl:ObjectProperty>
    


    <!-- https://photogrammetry.altervista.org/items/show/282#Y81:_used_GIS_software -->


    <owl:ObjectProperty rdf:about="https://photogrammetry.altervista.org/items/show/282#Y81:_used_GIS_software">
        <rdfs:subPropertyOf rdf:resource="http://www.semanticweb.org/vitto/ontologies/2024/9/PODS_1#L23_used_software_or_firmware_(was_software_or_firmware_used_by)"/>
        <rdfs:domain rdf:resource="https://photogrammetry.altervista.org/items/show/169#F82_Reference_GIS_System"/>
        <rdfs:range rdf:resource="https://photogrammetry.altervista.org/items/show/170#F83_GIS_Software"/>
        <rdfs:label xml:lang="en">used_GIS_software</rdfs:label>
        <skos:definition xml:lang="en">Y81: used GIS software
Subproperty of: L23 used software or firmware

Domain
F82 Reference GIS System

Range
F83 GIS Software</skos:definition>
        <skos:example xml:lang="en">The Reference GIS System used GIS Software such as QGIS to integrate the 3D model with geographic data.</skos:example>
        <skos:scopeNote xml:lang="en">This property specifies the GIS software (GIS Software) that was used to manage or process the 3D model within the GIS system.</skos:scopeNote>
    </owl:ObjectProperty>
    


    <!-- https://photogrammetry.altervista.org/items/show/283#Y82:_had_model_prospectuses_for_CAD_as_input -->


    <owl:ObjectProperty rdf:about="https://photogrammetry.altervista.org/items/show/283#Y82:_had_model_prospectuses_for_CAD_as_input">
        <rdfs:subPropertyOf rdf:resource="http://www.semanticweb.org/vitto/ontologies/2024/9/PODS_1#L10_had_input_(was_input_of)"/>
        <rdfs:domain rdf:resource="https://photogrammetry.altervista.org/items/show/172#F85_CAD_Analysis"/>
        <rdfs:range rdf:resource="https://photogrammetry.altervista.org/items/show/174#F87_3D_Model_Prospectus"/>
        <rdfs:label xml:lang="en">had_model_prospectus_as_input</rdfs:label>
        <skos:definition xml:lang="en">Y82: had model prospectuses for CAD as input
Subproperty of: L10 had input
Domain
F85 CAD Analysis
Range
F87 3D Model for Prospectuses</skos:definition>
        <skos:example xml:lang="en">-</skos:example>
        <skos:scopeNote xml:lang="en">This property indicates that the CAD analysis phase (CAD Analysis) used a 3D model designed for prospectuses (3D Model for Prospectuses) as an input.</skos:scopeNote>
    </owl:ObjectProperty>
    


    <!-- https://photogrammetry.altervista.org/items/show/284#Y83:_used_CAD_software -->


    <owl:ObjectProperty rdf:about="https://photogrammetry.altervista.org/items/show/284#Y83:_used_CAD_software">
        <rdfs:subPropertyOf rdf:resource="http://www.semanticweb.org/vitto/ontologies/2024/9/PODS_1#L23_used_software_or_firmware_(was_software_or_firmware_used_by)"/>
        <rdfs:domain rdf:resource="https://photogrammetry.altervista.org/items/show/172#F85_CAD_Analysis"/>
        <rdfs:range rdf:resource="https://photogrammetry.altervista.org/items/show/173#F86_Software_CAD"/>
        <rdfs:label xml:lang="en">used_CAD_software</rdfs:label>
        <skos:definition xml:lang="en">Y83: used CAD software
Subproperty of: L23 used software
Domain
F85 CAD Analysis
Range
F86 Software CAD</skos:definition>
        <skos:example xml:lang="en">-</skos:example>
        <skos:scopeNote xml:lang="en">This property specifies that the CAD analysis phase (CAD Analysis) used a specific CAD software (Software CAD) for its operations.</skos:scopeNote>
    </owl:ObjectProperty>
    


    <!-- https://photogrammetry.altervista.org/items/show/285#Y84:_had_prospectus_output -->


    <owl:ObjectProperty rdf:about="https://photogrammetry.altervista.org/items/show/285#Y84:_had_prospectus_output">
        <rdfs:subPropertyOf rdf:resource="http://www.semanticweb.org/vitto/ontologies/2024/9/PODS_1#L11_had_output_(was_output_of)"/>
        <rdfs:domain rdf:resource="https://photogrammetry.altervista.org/items/show/172#F85_CAD_Analysis"/>
        <rdfs:range rdf:resource="https://photogrammetry.altervista.org/items/show/171#F84_3D_Model_for_Prospectus"/>
        <rdfs:label xml:lang="en">had_prospectus_output</rdfs:label>
        <skos:definition xml:lang="en">Y84: had prospectus output
Subproperty of: L11 had output
Domain
F85 CAD Analysis
Range
F84 3D Model Prospectus</skos:definition>
        <skos:example xml:lang="en">-</skos:example>
        <skos:scopeNote xml:lang="en">This property indicates that the CAD analysis (CAD Analysis) produced a 3D model prospectus (3D Model Prospectus) as its output.</skos:scopeNote>
    </owl:ObjectProperty>
    


    <!-- 
    ///////////////////////////////////////////////////////////////////////////////////////
    //
    // Data properties
    //
    ///////////////////////////////////////////////////////////////////////////////////////
     -->


    


    <!-- http://www.opengis.net/ont/geosparql#dimension -->


    <owl:DatatypeProperty rdf:about="http://www.opengis.net/ont/geosparql#dimension"/>
    


    <!-- http://www.semanticweb.org/vitto/ontologies/2024/9/PODS_1#P3_has_note -->


    <owl:DatatypeProperty rdf:about="http://www.semanticweb.org/vitto/ontologies/2024/9/PODS_1#P3_has_note">
        <rdfs:domain rdf:resource="http://www.cidoc-crm.org/cidoc-crm/E1_CRM_Entity#E1_CRM_Entity"/>
        <rdfs:range rdf:resource="http://www.w3.org/2001/XMLSchema#string"/>
        <skos:definition xml:lang="en">URI (forward direction):	http://www.cidoc-crm.org/cidoc-crm/P3_has_note
URI (inverse direction):	-
Domain:
E1 CRM Entity
Range:
E62 String
SubProperty Of:
-
SuperProperty Of:
E52 Time-Span. P79 beginning is qualified by: E62 String
E52 Time-Span. P80 end is qualified by: E62 String
E90 Symbolic Object. P190 has symbolic content: E62 String
Quantification:
one to many (0,n:0,1)

Scope Note:
This property is a container for all informal descriptions about an object that have not been expressed in terms of CIDOC CRM constructs.

In particular, it captures the characterisation of the item itself, its internal structures, appearance, etc.

Like property P2 has type (is type of), this property is a consequence of the restricted focus of the CIDOC CRM. The aim is not to capture, in a structured form, everything that can be said about an item; indeed, the CIDOC CRM formalism is not regarded as sufficient to express everything that can be said. Good practice requires use of distinct note fields for different aspects of a characterisation. The P3.1 has type property of P3 has note allows differentiation of specific notes, e.g. &apos;construction&apos;, &apos;decoration&apos;, etc.

An item may have many notes, but a note is attached to a specific item.

Properties:
P3.1 has type: E55 Type

Examples:
Coffee mug – OXCMS:1983.1.1 (E19) has note &apos;chipped at edge of handle&apos; (E62) has type Condition (E55). (fictitious)</skos:definition>
    </owl:DatatypeProperty>
    


    <!-- http://www.semanticweb.org/vitto/ontologies/2024/9/PODS_1#Y63_has_date_of_modelling -->


    <owl:DatatypeProperty rdf:about="http://www.semanticweb.org/vitto/ontologies/2024/9/PODS_1#Y63_has_date_of_modelling">
        <rdfs:domain rdf:resource="https://photogrammetry.altervista.org/items/show/144#F58_Modifying_Mesh"/>
        <rdfs:range rdf:resource="http://www.w3.org/2001/XMLSchema#dateTime"/>
    </owl:DatatypeProperty>
    


    <!-- http://www.semanticweb.org/vitto/ontologies/2024/9/PODS_1#P40_observed_dimension_(was_observed_in) -->


    <owl:DatatypeProperty rdf:about="http://www.semanticweb.org/vitto/ontologies/2024/9/PODS_1#P40_observed_dimension_(was_observed_in)">
        <rdfs:domain rdf:resource="http://cidoc-crm.org/cidoc-crm/7.1.3/E16_Measurement#E16_Measurement"/>
        <rdfs:range rdf:resource="http://www.w3.org/2002/07/owl#rational"/>
        <skos:definition xml:lang="en">URI (forward direction):	http://www.cidoc-crm.org/cidoc-crm/P40_observed_dimension
URI (inverse direction):	http://www.cidoc-crm.org/cidoc-crm/P40i_was_observed_in
Domain:
E16 Measurement
Range:
E54 Dimension
SubProperty Of:
E13 Attribute Assignment. P141 assigned (was assigned by): E1 CRM Entity
SuperProperty Of:
-
Quantification:
many to many, necessary (1,n:0,n)

Scope Note:
This property records the dimension that was observed in an E16 Measurement Event.

E54 Dimension can be any quantifiable aspect of E70 Thing. Weight, image colour depth and monetary value are dimensions in this sense. One measurement activity may determine more than one dimension of one object.

Dimensions may be determined either by direct observation or using recorded evidence. In the latter case the measured Thing does not need to be present or extant.

Even though knowledge of the value of a dimension requires measurement, the dimension may be an object of discourse prior to, or even without, any measurement being made.

Properties:
-
Examples:
The measurement of the height of silver cup 232 on 31st August 1997 (E16) observed dimension silver cup 232 height (E54). [which has unit mm (E58), has value 224 (E60)] (fictitious)
The carbon 14 dating of the &apos;Schoeninger Speer II&apos; in 1996 (E16) observed dimension the carbon 14 based temporal distance from 1996 to the growth of the wood of the &apos;Schoeninger Speer II&apos; (E60). [The carbon 14 dating of an approximately 400.000 year old complete Old Palaeolithic wooden spear found in Schoeningen, Niederachsen, Germany, in 1995. See also: E16 Measurement.] (Kouwenhoven, 1997)</skos:definition>
    </owl:DatatypeProperty>
    


    <!-- http://www.semanticweb.org/vitto/ontologies/2024/9/PODS_1#Y19:_has_date_of_acquisition -->


    <owl:DatatypeProperty rdf:about="http://www.semanticweb.org/vitto/ontologies/2024/9/PODS_1#Y19:_has_date_of_acquisition">
        <rdfs:domain rdf:resource="https://photogrammetry.altervista.org/admin/items/show/88#F2_Acquisition"/>
        <rdfs:range rdf:resource="http://www.w3.org/2001/XMLSchema#dateTime"/>
    </owl:DatatypeProperty>
    


    <!-- http://www.semanticweb.org/vitto/ontologies/2024/9/PODS_1#Y21:_has_coordinates_of_acquisition -->


    <owl:DatatypeProperty rdf:about="http://www.semanticweb.org/vitto/ontologies/2024/9/PODS_1#Y21:_has_coordinates_of_acquisition">
        <rdfs:subPropertyOf rdf:resource="http://www.opengis.net/ont/geosparql#dimension"/>
        <rdfs:domain rdf:resource="https://photogrammetry.altervista.org/admin/items/show/88#F2_Acquisition"/>
        <rdfs:range rdf:resource="http://www.w3.org/2001/XMLSchema#integer"/>
    </owl:DatatypeProperty>
    


    <!-- http://www.semanticweb.org/vitto/ontologies/2024/9/PODS_1#Y95:_was_measured_in_number_of_points -->


    <owl:DatatypeProperty rdf:about="http://www.semanticweb.org/vitto/ontologies/2024/9/PODS_1#Y95:_was_measured_in_number_of_points">
        <rdfs:domain rdf:resource="https://photogrammetry.altervista.org/items/show/112#F26_Point_Cloud"/>
        <rdfs:domain rdf:resource="https://photogrammetry.altervista.org/items/show/113#F27_Densified_Point_Cloud"/>
        <rdfs:range rdf:resource="http://www.w3.org/2002/07/owl#rational"/>
    </owl:DatatypeProperty>
    


    <!-- https://photogrammetry.altervista.org/items/show/207#Y16:_has_number_of_picture -->


    <owl:DatatypeProperty rdf:about="https://photogrammetry.altervista.org/items/show/207#Y16:_has_number_of_picture">
        <rdfs:domain rdf:resource="https://photogrammetry.altervista.org/items/show/93#F7_Picture_Set"/>
        <rdfs:range rdf:resource="http://www.w3.org/2002/07/owl#rational"/>
        <rdfs:label xml:lang="en">has_number_of_picture</rdfs:label>
        <skos:definition xml:lang="en">Y16: has number of picture

Not a subproperty of any other property
Domain
F7 Picture Set
Range
F41 Number of Picture</skos:definition>
        <skos:example xml:lang="en">-</skos:example>
        <skos:scopeNote xml:lang="en">This property describes the number of individual pictures contained in a picture set (F7). It specifies the quantity of images used in an acquisition process.</skos:scopeNote>
    </owl:DatatypeProperty>
    


    <!-- https://photogrammetry.altervista.org/items/show/211#Y20:_has_acquisition_description -->


    <owl:DatatypeProperty rdf:about="https://photogrammetry.altervista.org/items/show/211#Y20:_has_acquisition_description">
        <rdfs:subPropertyOf rdf:resource="http://www.semanticweb.org/vitto/ontologies/2024/9/PODS_1#P3_has_note"/>
        <rdfs:domain rdf:resource="https://photogrammetry.altervista.org/admin/items/show/88#F2_Acquisition"/>
        <rdfs:range rdf:resource="http://www.w3.org/2001/XMLSchema#string"/>
        <rdfs:label xml:lang="en">has_acquisition_description</rdfs:label>
        <skos:definition xml:lang="en">Y20: has acquisition description

Subproperty of: P3 has note
Domain
F2 Acquisition
Range
F44 Acquisition Description</skos:definition>
        <skos:example xml:lang="en">-</skos:example>
        <skos:scopeNote xml:lang="en">This property refers to a description (F44) of the acquisition event (F2). It provides additional notes or commentary on the method, conditions, or purpose of the data collection.</skos:scopeNote>
    </owl:DatatypeProperty>
    


    <!-- https://photogrammetry.altervista.org/items/show/224#Y33:_has_observed_number_of_points -->


    <owl:DatatypeProperty rdf:about="https://photogrammetry.altervista.org/items/show/224#Y33:_has_observed_number_of_points">
        <rdfs:subPropertyOf rdf:resource="https://photogrammetry.altervista.org/items/show/265#Y94:_has_observed_number_of_points"/>
        <rdfs:domain rdf:resource="https://photogrammetry.altervista.org/items/show/136#F50_Point_Cloud_Measurement"/>
        <rdfs:range rdf:resource="http://www.w3.org/2002/07/owl#rational"/>
        <rdfs:comment xml:lang="en">This property is redundant and can be replaced by the superproperty 
- Y94: has observed number of points -</rdfs:comment>
        <rdfs:label xml:lang="en">pc_has_observed_number_of_points</rdfs:label>
        <skos:definition xml:lang="en">Y33: has observed number of points



Subproperty of: P40 observed dimension
Domain: F50 Point Cloud Measurement
Range: F51 Point Cloud Number of Points</skos:definition>
        <skos:example xml:lang="en">A F50 Point Cloud Measurement records an observed number of F51 Point Cloud Number of Points, such as 1,000,000 points in a scan.</skos:example>
        <skos:scopeNote xml:lang="en">This property associates a point cloud measurement (F50) with the observed number of points (F51).</skos:scopeNote>
    </owl:DatatypeProperty>
    


    <!-- https://photogrammetry.altervista.org/items/show/228#Y37:_has_observed_number_of_points_(for_dense_point_clouds) -->


    <owl:DatatypeProperty rdf:about="https://photogrammetry.altervista.org/items/show/228#Y37:_has_observed_number_of_points_(for_dense_point_clouds)">
        <rdfs:subPropertyOf rdf:resource="https://photogrammetry.altervista.org/items/show/265#Y94:_has_observed_number_of_points"/>
        <rdfs:domain rdf:resource="https://photogrammetry.altervista.org/items/show/138#F52_Dense_Point_Cloud_Measurement"/>
        <rdfs:range rdf:resource="http://www.w3.org/2002/07/owl#rational"/>
        <rdfs:comment xml:lang="en">This property is redundant and can be replaced by the superproperty 
- Y94: has observed number of points -</rdfs:comment>
        <rdfs:label xml:lang="en">dpc_has_observed_number_of_points</rdfs:label>
        <skos:definition xml:lang="en">Y37: has observed number of points (for dense point clouds)


Subproperty of: P40 observed dimension
Domain
F52 Dense Point Cloud Measurement
Range
F53 Dense Point Cloud Number of Points</skos:definition>
        <skos:example xml:lang="en">A F52 Dense Point Cloud Measurement records an observed number of F53 Dense Point Cloud Number of Points, such as 10,000,000 points in a densified scan.</skos:example>
        <skos:scopeNote xml:lang="en">This property specifically refers to the number of points observed in a dense point cloud (F53) during a measurement (F52).</skos:scopeNote>
    </owl:DatatypeProperty>
    


    <!-- https://photogrammetry.altervista.org/items/show/249#Y58:_has_number_of_texture -->


    <owl:DatatypeProperty rdf:about="https://photogrammetry.altervista.org/items/show/249#Y58:_has_number_of_texture">
        <rdfs:label xml:lang="en">has_number_of_texture</rdfs:label>
        <skos:definition xml:lang="en">Y58: has number of texture

(Not a subproperty)
Domain: F62 Texture Set of 3D Mesh
Range: F63 Number of Texture</skos:definition>
        <skos:example xml:lang="en">A F62 Texture Set of 3D Mesh has F63 Number of Texture, indicating the number of individual texture files used in the set.</skos:example>
        <skos:scopeNote xml:lang="en">This property defines the number of textures (F63) present in a texture set (F62) for a 3D mesh.</skos:scopeNote>
    </owl:DatatypeProperty>
    


    <!-- https://photogrammetry.altervista.org/items/show/251#Y60:_has_modelling_description -->


    <owl:DatatypeProperty rdf:about="https://photogrammetry.altervista.org/items/show/251#Y60:_has_modelling_description">
        <rdfs:subPropertyOf rdf:resource="http://www.semanticweb.org/vitto/ontologies/2024/9/PODS_1#P3_has_note"/>
        <rdfs:domain rdf:resource="https://photogrammetry.altervista.org/items/show/90#F4_Modelling"/>
        <rdfs:label xml:lang="en">has_modelling_description</rdfs:label>
        <skos:definition xml:lang="en">Y60: has modelling description

Subproperty of: P3 has note
Domain: F4 Modelling
Range: F64 Modelling Description</skos:definition>
        <skos:example xml:lang="en">A F4 Modelling process has a F64 Modelling Description, such as an explanation of the procedural steps used to create the 3D model.</skos:example>
        <skos:scopeNote xml:lang="en">This property links a modelling process (F4) with a descriptive note (F64) detailing the process, method, or specifics about the model.</skos:scopeNote>
    </owl:DatatypeProperty>
    


    <!-- https://photogrammetry.altervista.org/items/show/261#Y71:_has_number_of_final_destination -->


    <owl:DatatypeProperty rdf:about="https://photogrammetry.altervista.org/items/show/261#Y71:_has_number_of_final_destination">
        <rdfs:domain rdf:resource="https://photogrammetry.altervista.org/items/show/158#F71_Final_Use_of_Digital_Twin"/>
        <rdfs:range rdf:resource="http://www.w3.org/2002/07/owl#rational"/>
        <rdfs:label xml:lang="en">tridimensional_digital_twin_has_number_of_use</rdfs:label>
        <skos:definition xml:lang="en">Y71: has number of final destination
(Not a subproperty)

Domain
F71 Final Use of 3D Model

Range
F70 Number of Final Destination</skos:definition>
        <skos:example xml:lang="en">The F71 Final Use of the 3D Model has F70 Number of Final Destination, such as three different output formats: video rendering, printing, and research.</skos:example>
        <skos:scopeNote xml:lang="en">This property indicates the number of final destinations (F70) for the 3D model based on the final use (F71).</skos:scopeNote>
    </owl:DatatypeProperty>
    


    <!-- https://photogrammetry.altervista.org/items/show/265#Y94:_has_observed_number_of_points -->


    <owl:DatatypeProperty rdf:about="https://photogrammetry.altervista.org/items/show/265#Y94:_has_observed_number_of_points">
        <rdfs:subPropertyOf rdf:resource="http://www.semanticweb.org/vitto/ontologies/2024/9/PODS_1#P40_observed_dimension_(was_observed_in)"/>
        <rdfs:domain rdf:resource="https://photogrammetry.altervista.org/items/show/136#F50_Point_Cloud_Measurement"/>
        <rdfs:domain rdf:resource="https://photogrammetry.altervista.org/items/show/138#F52_Dense_Point_Cloud_Measurement"/>
        <rdfs:range rdf:resource="http://www.w3.org/2002/07/owl#rational"/>
        <rdfs:label xml:lang="en">has_observed_number_of_points</rdfs:label>
        <skos:definition xml:lang="en">Y94: has observed number of points
Subproperty of: P40 observed dimension

Domain
F50 Point Cloud Measurement, F52 Dense Point Cloud Measurement

Range
F51 Point Cloud Number of Points, F53 Dense Point Cloud Number of Points</skos:definition>
        <skos:example xml:lang="en">A F50 Point Cloud Measurement records an observed number of F51 Point Cloud Number of Points, such as 500,000 points in a basic scan.</skos:example>
        <skos:example xml:lang="en">A F52 Dense Point Cloud Measurement records an observed number of F53 Dense Point Cloud Number of Points, such as 12,000,000 points in a densified scan.</skos:example>
        <skos:scopeNote xml:lang="en">This property refers to the number of points observed in a Point Cloud (F51) or Dense Point Cloud (F53) during a Point Cloud Measurement (F50) or a Dense Point Cloud Measurement (F52). It captures the quantity of individual data points that have been identified and recorded in the measurement phase, allowing for the specification of the point cloud&apos;s resolution.</skos:scopeNote>
    </owl:DatatypeProperty>
    


    <!-- 
    ///////////////////////////////////////////////////////////////////////////////////////
    //
    // Classes
    //
    ///////////////////////////////////////////////////////////////////////////////////////
     -->


    


    <!-- http://cidoc-crm.org/cidoc-crm/7.1.3/E11_Modification#E11_Modification -->


    <owl:Class rdf:about="http://cidoc-crm.org/cidoc-crm/7.1.3/E11_Modification#E11_Modification">
        <rdfs:subClassOf rdf:resource="http://cidoc-crm.org/cidoc-crm/7.1.3/E7_Activity#E7_Activity"/>
        <rdfs:comment>URI:	http://www.cidoc-crm.org/cidoc-crm/E11_Modification
SubClass Of:
E7 Activity
SuperClass Of:
E12 Production
E79 Part Addition
E80 Part Removal
Scope Note:
This class comprises instances of E7 Activity that are undertaken to create, alter or change instances of E24 Physical Human-Made Thing.

This class includes the production of an item from raw materials and other so far undocumented objects. It also includes the conservation treatment of an object.

Since the distinction between modification and production is not always clear, modification is regarded as the more generally applicable concept. This implies that some items may be consumed or destroyed in an instance of E11 Modification, and that others may be produced as a result of it. An event should also be documented using an instance of E81 Transformation if it results in the destruction of one or more objects and the simultaneous production of others using parts or material from the originals. In this case, the new items have separate identities.

An activity undertaken on an object which was designed to alter it, but which, in fact, it did not in any seemingly significant way (such as the application of a solvent during conservation which failed to dissolve any part of the object), is still considered as an instance of E11 Modification. Typically, any such activity will leave at least forensic traces of evidence on the object.

If the instance of E29 Design or Procedure utilized for the modification prescribes the use of specific materials, they should be documented using property P68 foresees use of (use foreseen by): E57 Material of E29 Design or Procedure, rather than via P126 employed (was employed in): E57 Material.

Examples:
the construction of the SS Great Britain (E12) (Gregor, 1971)
the impregnation of the Vasa warship in Stockholm for preservation after 1956 (Håfors, 2010)
the transformation of the Enola Gay into a museum exhibit by the National Air and Space Museum in Washington DC between 1993 and 1995 (E12, E81) (Yakel, 2000)
the last renewal of the gold coating of the Toshogu shrine in Nikko, Japan (Cali and Dougil, 2012)</rdfs:comment>
    </owl:Class>
    


    <!-- http://cidoc-crm.org/cidoc-crm/7.1.3/E13_Attribute_Assignment#E13_Attribute_Assignment -->


    <owl:Class rdf:about="http://cidoc-crm.org/cidoc-crm/7.1.3/E13_Attribute_Assignment#E13_Attribute_Assignment">
        <rdfs:subClassOf rdf:resource="http://cidoc-crm.org/cidoc-crm/7.1.3/E7_Activity#E7_Activity"/>
        <rdfs:comment>URI:	http://www.cidoc-crm.org/cidoc-crm/E13_Attribute_Assignment
SubClass Of:
E7 Activity
SuperClass Of:
E14 Condition Assessment
E15 Identifier Assignment
E16 Measurement
E17 Type Assignment
Scope Note:
This class comprises the actions of making assertions about one property of an object or any single relation between two items or concepts. The type of the property asserted to hold between two items or concepts can be described by the property P177 assigned property of type (is type of property assigned): E55 Type.

For example, the class describes the actions of people making propositions and statements during certain scientific/scholarly procedures, e.g. the person and date when a condition statement was made, an identifier was assigned, the museum object was measured, etc. Which kinds of such assignments and statements need to be documented explicitly in structures of a schema rather than free text, depends on whether this information should be accessible by structured queries.

This class allows for the documentation of how the respective assignment came about, and whose opinion it was. Note that all instances of properties described in a knowledge base are the opinion of someone. Per default, they are the opinion of the team maintaining the knowledge base. This fact must not individually be registered for all instances of properties provided by the maintaining team, because it would result in an endless recursion of whose opinion was the description of an opinion. Therefore, the use of instances of E13 Attribute Assignment marks the fact that the maintaining team is in general neutral to the validity of the respective assertion, but registers someone else’s opinion and how it came about.

All properties assigned in such an action can also be seen as directly relating the respective pair of items or concepts. Multiple use of instances of E13 Attribute Assignment may possibly lead to a collection of contradictory values.

Examples:
the examination of MS Sinai Greek 418 by Nicholas Pickwoad in November 2003 (Honey &amp; Pickwoad, 2010)
the assessment of the current ownership of Martin Doerr’s silver cup in February 1997 (fictitious)</rdfs:comment>
    </owl:Class>
    


    <!-- http://cidoc-crm.org/cidoc-crm/7.1.3/E16_Measurement#E16_Measurement -->


    <owl:Class rdf:about="http://cidoc-crm.org/cidoc-crm/7.1.3/E16_Measurement#E16_Measurement">
        <rdfs:subClassOf rdf:resource="http://cidoc-crm.org/cidoc-crm/7.1.3/E13_Attribute_Assignment#E13_Attribute_Assignment"/>
        <rdfs:comment>URI:	http://www.cidoc-crm.org/cidoc-crm/E16_Measurement
SubClass Of:
E13 Attribute Assignment
SuperClass Of:
-
Scope Note:
This class comprises actions measuring physical properties and other values that can be determined by a systematic, objective procedure of direct observation of particular states of physical reality.

An instance of E16 Measurement may use simple counting or tools, such as yardsticks or radiation detection devices. The interest is in the method and care applied, so that the reliability of the result may be judged at a later stage, or research continued on the associated documents. The date of the event is important for dimensions, which may change value over time, such as the length of an object subject to shrinkage. Methods and devices employed should be associated with instances of E16 Measurement by properties such as P33 used specific technique: E29 Design or Procedure, P125 used object of type: E55 Type, P16 used specific object (was used for): E70 Thing, whereas basic techniques such as &quot;carbon-14 dating&quot; should be encoded using P2 has type (is type of): E55 Type. Details of methods and devices reused or reusable in other instances of E16 Measurement should be documented for these entities rather than the measurements themselves, whereas details of particular execution may be documented by free text or by instantiating adequate sub-activities, if the detail may be of interest for an overarching query.

Regardless whether a measurement is made by an instrument or by human senses, it represents the initial transition from physical reality to information without any other documented information object in between within the reasoning chain that would represent the result of the interaction of the observer or device with reality. Therefore, determining properties of an instance of E90 Symbolic Object is regarded as an instance of E13 Attribute Assignment, which may be inferred from observing and measuring representative carriers. In the case that the carrier can be named, the property P16 used specific object (was used for) should be used to indicate the instance(s) of E18 Physical Thing that was used as the empirical basis for the attribute assignment. For instance, inferring properties of depicted items using image material, such as satellite images, is not regarded as an instance of E16 Measurement, but as a subsequent instance of E13 Attribute Assignment. Rather, only the production of the images, understood as arrays of radiation intensities, is regarded as an instance of E16 Measurement. The same reasoning holds for other sensor data.

Examples:
measurement of the height of silver cup 232 on 31st August 1997 (fictitious)
the carbon 14 dating of the &apos;Schoeninger Speer II&apos; in 1996 [The carbon 14 dating of an approximately 400.000 year old complete Old Palaeolithic wooden spear found in Schoeningen, Niedersachsen, Germany, in 1995.] (Kouwenhoven, 1997)</rdfs:comment>
    </owl:Class>
    


    <!-- http://cidoc-crm.org/cidoc-crm/7.1.3/E18_Physical_Thing#E18_Physical_Thing -->


    <owl:Class rdf:about="http://cidoc-crm.org/cidoc-crm/7.1.3/E18_Physical_Thing#E18_Physical_Thing">
        <rdfs:subClassOf rdf:resource="http://cidoc-crm.org/cidoc-crm/7.1.3/E72_Legal_Object#E72_Legal_Object"/>
        <rdfs:comment>URI:	http://www.cidoc-crm.org/cidoc-crm/E18_Physical_Thing
SubClass Of:
E72 Legal Object
SuperClass Of:
E19 Physical Object
E24 Physical Human-Made Thing
E26 Physical Feature
Scope Note:
This class comprises all persistent physical items with a relatively stable form, human-made or natural.

Depending on the existence of natural boundaries of such things, the CIDOC CRM distinguishes the instances of E19 Physical Object from instances of E26 Physical Feature, such as holes, rivers, pieces of land, etc. Most instances of E19 Physical Object can be moved (if not too heavy), whereas features are integral to the surrounding matter.

An instance of E18 Physical Thing occupies not only a particular geometric space at any instant of its existence, but in the course of its existence it also forms a trajectory through spacetime, which occupies a real, that is phenomenal, volume in spacetime. We include in the occupied space the space filled by the matter of the physical thing and all its inner spaces, such as the interior of a box. For the purpose of more detailed descriptions of the presence of an instance of E18 Physical Thing in space and time it can be associated with its specific instance of E92 Spacetime Volume by the property P196 defines (is defined by).

The CIDOC CRM is generally not concerned with amounts of matter in fluid or gaseous states, as long as they are not confined in an identifiable way for an identifiable minimal time-span.</rdfs:comment>
    </owl:Class>
    


    <!-- http://cidoc-crm.org/cidoc-crm/7.1.3/E22_Human-Made_Object#E22_Human-Made_Object -->


    <owl:Class rdf:about="http://cidoc-crm.org/cidoc-crm/7.1.3/E22_Human-Made_Object#E22_Human-Made_Object">
        <rdfs:subClassOf rdf:resource="http://cidoc-crm.org/cidoc-crm/7.1.3/E24_Physical_Human-Made_Thing#E24_Physical_Human-Made_Thing"/>
        <rdfs:comment>URI:	http://www.cidoc-crm.org/cidoc-crm/E22_Human-Made_Object
SubClass Of:
E19 Physical Object
E24 Physical Human-Made Thing
SuperClass Of:
-
Scope Note:
This class comprises all persistent physical objects of any size that are purposely created by human activity and have physical boundaries that separate them completely in an objective way from other objects.

The class also includes all aggregates of objects made for functional purposes of whatever kind, independent of physical coherence, such as a set of chessmen.

Examples:
the Rosetta Stone (E22)
LNER Class A4 4468 Mallard [the World’s fastest steam locomotive, preserved at the National Railway Museum of York, UK] (Solomon, 2003)
the Portland Vase (Walker, 2004)</rdfs:comment>
    </owl:Class>
    


    <!-- http://cidoc-crm.org/cidoc-crm/7.1.3/E24_Physical_Human-Made_Thing#E24_Physical_Human-Made_Thing -->


    <owl:Class rdf:about="http://cidoc-crm.org/cidoc-crm/7.1.3/E24_Physical_Human-Made_Thing#E24_Physical_Human-Made_Thing">
        <rdfs:subClassOf rdf:resource="http://cidoc-crm.org/cidoc-crm/7.1.3/E71_Human-Made_Thing#E71_Human-Made_Thing"/>
        <rdfs:comment>URI:	http://www.cidoc-crm.org/cidoc-crm/E24_Physical_Human-Made_Thing
SubClass Of:
E18 Physical Thing
E71 Human-Made Thing
SuperClass Of:
E22 Human-Made Object
E25 Human-Made Feature
E78 Curated Holding
Scope Note:
This class comprises all persistent physical items of any size that are purposely created by human activity. This class comprises, besides others, human-made objects, such as a sword, and human-made features, such as rock art. For example, a &apos;cup and ring&apos; carving on bedrock is regarded as instance of E24 Physical Human-Made Thing.

Instances of E24 Physical Human-Made Thing may be the result of modifying pre-existing physical things, preserving larger parts or most of the original matter and structure, which poses the question if they are new or even human-made, the respective interventions of production made on such original material should be obvious and sufficient to regard that the product has a new, distinct identity and intended function and is human-made. Substantial continuity of the previous matter and structure in the new product can be documented by describing the production process also as an instance of E81 Transformation.

Whereas interventions of conservation and repair are not regarded to produce a new instance of E24 Physical Human-Made Thing, the results of preparation of natural history specimens that substantially change their natural or original state should be regarded as instances of E24 Physical Human-Made Things, including the uncovering of petrified biological features from a solid piece of stone. On the other side, scribbling a museum number on a natural object should not be regarded to make it human-made. This notwithstanding, parts, sections, segments, or features of an instance of E24 Physical Human-Made Thing may continue to be non-human-made and preserved during the production process, for example natural pearls used as a part of an eardrop.

Examples:
the Forth Railway Bridge (Shipway, Bouch, Baker and Fowler, 1990).
the Channel Tunnel (E25) (Holliday, Marcou and Vickerman, 1991)
the Palace of Knossos (Evans, 1921)
the Colosseum in Rome, Italy (Hopkins and Beard, 2011)
the Historical Collection of the Museum Benaki in Athens (E78) (Georgoula, 2005)
the Rosetta Stone (E22)
my paperback copy of Crime &amp; Punishment (E22) (fictitious)
the computer disk at ICS-FORTH that stores the canonical Definition of the CIDOC CRM v.3.2 (E22)
my empty DVD disk (E22) (fictitious)</rdfs:comment>
    </owl:Class>
    


    <!-- http://cidoc-crm.org/cidoc-crm/7.1.3/E28_Conceptual_Object#E28_Conceptual_Object -->


    <owl:Class rdf:about="http://cidoc-crm.org/cidoc-crm/7.1.3/E28_Conceptual_Object#E28_Conceptual_Object">
        <rdfs:subClassOf rdf:resource="http://cidoc-crm.org/cidoc-crm/7.1.3/E71_Human-Made_Thing#E71_Human-Made_Thing"/>
        <rdfs:comment>URI:	http://www.cidoc-crm.org/cidoc-crm/E28_Conceptual_Object
SubClass Of:
E71 Human-Made Thing
SuperClass Of:
E55 Type
E89 Propositional Object
E90 Symbolic Object
Scope Note:
This class comprises non-material products of our minds and other human produced data that have become objects of a discourse about their identity, circumstances of creation, or historical implication. The production of such information might have been supported by the use of technical devices such as cameras or computers.

Characteristically, instances of this class are created, invented or thought by someone, and then may be documented or communicated between persons. Instances of E28 Conceptual Object have the ability to exist on more than one particular carrier at the same time, such as paper, electronic signals, marks, audio media, paintings, photos, human memories, etc.

They cannot be destroyed. They exist as long as they can be found on at least one carrier or in at least one human memory. Their existence ends when the last carrier and the last memory are lost.

Examples:
Beethoven’s &apos;Ode an die Freude&apos; (Ode to Joy) (E73) (Kershaw, 1999)
the definition of &apos;ontology&apos; in the Oxford English Dictionary (E73) (Oxford University Press, 1989)
the knowledge about the victory at Marathon carried by the famous runner (E89) (Lagos &amp; Karyanos, 2020)
[Explanation note: The following examples illustrate the distinction between a propositional object, its names and its encoded forms. The Maxwell equations (Ball, 1962) are a good example, because they belong to the fundamental laws of physics and their mathematical content yields identical, unambiguous results regardless formulation and encoding.]
&apos;Maxwell equations&apos; (E41) [preferred subject access point from LCSH, http://lccn.loc.gov/sh85082387, accessed 18th April 2021. This is only the name for the Maxwell equations as standardized by the Library of Congress and not the equations themselves.]
&apos;Equations, Maxwell&apos; (E41) [variant subject access point from LCSH, http://lccn.loc.gov/sh85082387, accessed 18th April 2021. This is another name for the equation standardized by the Library of Congress and not the equations themselves.]
Maxwell&apos;s equations (E89) [This is the propositional content of the equations proper, independent of any particular notation or mathematical formalism.] (Ball, 1962)
The encoding of Maxwells equations as in https://upload.wikimedia.org/wikipedia/commons/c/c4/Maxwell%27sEquations.svg (E73) [accessed 18th April 2021. This is one possible symbolic encoding of the propositional content of the equations.]</rdfs:comment>
    </owl:Class>
    


    <!-- http://cidoc-crm.org/cidoc-crm/7.1.3/E29_Design_or_Procedure#E29_Design_or_Procedure -->


    <owl:Class rdf:about="http://cidoc-crm.org/cidoc-crm/7.1.3/E29_Design_or_Procedure#E29_Design_or_Procedure">
        <rdfs:subClassOf rdf:resource="http://cidoc-crm.org/cidoc-crm/7.1.3/E73_Information_Object#E73_Information_Object"/>
        <rdfs:comment>URI:	http://www.cidoc-crm.org/cidoc-crm/E29_Design_or_Procedure
SubClass Of:
E73 Information Object
SuperClass Of:
-
Scope Note:
This class comprises documented plans for the execution of actions in order to achieve a result of a specific quality, form, or contents. In particular, it comprises plans for deliberate human activities that may result in new instances of E71 Human-Made Thing or for shaping or guiding the execution of an instance of E7 Activity.

Instances of E29 Design or Procedure can be structured in parts and sequences or depend on others.

This is modelled using P69 has association with (is associated with): E29 Design or Procedure.

Designs or procedures can be seen as one of the following:

A schema for the activities it describes
A schema of the products that result from their application
An independent intellectual product that may have never been applied, such as Leonardo da Vinci’s famous plans for flying machines
Because designs or procedures may never be applied or only partially executed, the CIDOC CRM models a loose relationship between the plan and the respective product.

Examples:
the ISO standardisation procedure
the musical notation for Beethoven’s &apos;Ode to Joy&apos; (Kershaw, 1999)
the architectural drawings for the Kölner Dom (Cologne Cathedral) in Cologne, Germany (Wolff, 1999)
the drawing found on Folio 860 of the Codex Atlanticus from Leonardo da Vinci, 1486 to 1490, kept in the Biblioteca Ambrosiana in Milan</rdfs:comment>
    </owl:Class>
    


    <!-- http://cidoc-crm.org/cidoc-crm/7.1.3/E2_Temporal_Entity#E2_Temporal_Entity -->


    <owl:Class rdf:about="http://cidoc-crm.org/cidoc-crm/7.1.3/E2_Temporal_Entity#E2_Temporal_Entity">
        <rdfs:subClassOf rdf:resource="http://www.cidoc-crm.org/cidoc-crm/E1_CRM_Entity#E1_CRM_Entity"/>
        <rdfs:comment>URI:	http://www.cidoc-crm.org/cidoc-crm/E2_Temporal_Entity
SubClass Of:
E1 CRM Entity
SuperClass Of:
E3 Condition State
E4 Period
Scope Note:
This class comprises all phenomena, such as the instances of E4 Periods and E5 Events, which happen over a limited extent in time. This extent in time must be contiguous, i.e., without gaps. In case the defining kinds of phenomena for an instance of E2 Temporal Entity cease to happen, and occur later again at another time, we regard that the former instance of E2 Temporal Entity has ended and a new instance has come into existence. In more intuitive terms, the same event cannot happen twice.

In some contexts, such phenomena are also called perdurants. This class is disjoint from E77 Persistent Item and is an abstract class that typically has no direct instances. E2 Temporal Entity is specialized into E4 Period, which applies to a particular geographic area (defined with a greater or lesser degree of precision), and E3 Condition State, which applies to instances of E18 Physical Thing.

Examples:
Bronze Age (E4) (Childe, 1963)
the earthquake in Lisbon 1755 (E5) (Chester, 2001)
the Peterhof Palace near Saint Petersburg being in ruins from 1944 to 1946 (E3) (Maddox, 2015)</rdfs:comment>
    </owl:Class>
    


    <!-- http://cidoc-crm.org/cidoc-crm/7.1.3/E39_Actor#E39_Actor -->


    <owl:Class rdf:about="http://cidoc-crm.org/cidoc-crm/7.1.3/E39_Actor#E39_Actor">
        <owl:equivalentClass rdf:resource="http://xmlns.com/foaf/0.1/Person"/>
        <rdfs:subClassOf rdf:resource="http://cidoc-crm.org/cidoc-crm/7.1.3/E77_Persistent_Item#E77_Persistent_Item"/>
        <rdfs:comment>URI:	http://www.cidoc-crm.org/cidoc-crm/E39_Actor
SubClass Of:
E77 Persistent Item
SuperClass Of:
E21 Person
E74 Group
Scope Note:
This class comprises people, either individually or in groups, who have the potential to perform intentional actions of kinds for which they can be held responsible.

Examples:
London and Continental Railways (E74)
the Governor of the Bank of England in 1975 (E21)
Sir Ian McKellen (E21) (Gibson, 1986)</rdfs:comment>
    </owl:Class>
    


    <!-- http://cidoc-crm.org/cidoc-crm/7.1.3/E4_Period#E4_Period -->


    <owl:Class rdf:about="http://cidoc-crm.org/cidoc-crm/7.1.3/E4_Period#E4_Period">
        <rdfs:subClassOf rdf:resource="http://cidoc-crm.org/cidoc-crm/7.1.3/E2_Temporal_Entity#E2_Temporal_Entity"/>
        <rdfs:comment>URI:	http://www.cidoc-crm.org/cidoc-crm/E4_Period
SubClass Of:
E2 Temporal Entity
E92 Spacetime Volume
SuperClass Of:
E5 Event
Scope Note:
This class comprises sets of coherent phenomena or cultural manifestations occurring in time and space.

It is the social or physical coherence of these phenomena that identify an instance of E4 Period and not the associated spatiotemporal extent. This extent is only the &apos;ground&apos; or space in an abstract physical sense that the actual process of growth, spread and retreat has covered. Consequently, different periods can overlap and coexist in time and space, such as when a nomadic culture exists in the same area and time as a sedentary culture. This also means that overlapping land use rights, common among first nations, amounts to overlapping periods.

Often, this class is used to describe prehistoric or historic periods such as the &apos;Neolithic Period&apos;, the &apos;Ming Dynasty&apos; or the &apos;McCarthy Era&apos;, but also geopolitical units and activities of settlements are regarded as special cases of E4 Period. However, there are no assumptions about the scale of the associated phenomena. In particular all events are seen as synthetic processes consisting of coherent phenomena. Therefore, E4 Period is a superclass of E5 Event. For example, a modern clinical birth, an instance of E67 Birth, can be seen as both a single event, i.e. an instance of E5 Event, and as an extended period, i.e. an instance of E4 Period, that consists of multiple physical processes and complementary activities performed by multiple instances of E39 Actor.

E4 Period is a subclass of E2 Temporal Entity and of E92 Spacetime Volume. The latter is intended as a phenomenal spacetime volume as defined in CIDOC CRMgeo (Doerr &amp; Hiebel, 2013). By virtue of this multiple inheritance, it is possible to discuss the physical extent of an instance of E4 Period without representing each instance of it together with an instance of its associated spacetime volume. This model combines two quite different kinds of substance: an instance of E4 Period is a phenomenon while an instance of E92 Spacetime Volume is an aggregation of points in spacetime. However, the real spatiotemporal extent of an instance of E4 Period is regarded to be unique to it due to all its details and fuzziness; its identity and existence depends uniquely on the identity of the instance of E4 Period. Therefore, this multiple inheritance is unambiguous and effective and furthermore corresponds to the intuitions of natural language.

Typical use of this class in cultural heritage documentation is for documenting cultural and artistic periods. There are two different conceptualisations of ‘artistic style’, defined either by physical features or by historical context. For example, &apos;Impressionism&apos; can be viewed as a period in the European sphere of influence lasting from approximately 1870 to 1905 during which paintings with particular characteristics were produced by a group of artists that included (among others) Monet, Renoir, Pissarro, Sisley and Degas. Alternatively, it can be regarded as a style applicable to all paintings sharing the characteristics of the works produced by the Impressionist painters, regardless of historical context. The first interpretation is an instance of E4 Period, and the second defines morphological object types that fall under E55 Type.

A geopolitical unit as a specific case of an instance of E4 Period is the set of activities and phenomena related to the claim of power, the consequences of belonging to a jurisdictional area and an administrative system that establishes a geopolitical unit. Examples from the modern period are countries or administrative areas of countries such as districts whose actions and structures define activities and phenomena in the area that they intend to govern. The borders of geopolitical units are often defined in contracts or treaties although they may deviate from the actual practice. The spatiotemporal properties of Geopolitical units can be modelled through the properties inherited from E92 Spacetime Volume.

Another specific case of an instance of E4 Period is the actual extent of the set of activities and phenomena as evidenced by their physical traces that define a settlement, such as the populated period of Nineveh.

Examples:
Jurassic (Hallam, 1975)
Populated Period of Nineveh
Imperial Rome under Marcus Aurelius
European Bronze Age (Harrison, 2004)
Italian Renaissance (Macdonald, 1992)
Thirty Years War (Lee, 1991)
Sturm und Drang (Berkoff, 2013)
Cubism (Cox, 2000)
The Capital of Russia (E4) [the capital of Russia in the sense of an administrative unit moved in historical times from Moscow to St Petersburg and then back to Moscow. This exemplifies an administrative unit changing place over time without temporal discontinuity]
The settling activity of the community of Helsinki (a.k.a. Helsingfors) (E7) [the original settlement called Helsinki was located in the area of the modern airport. The community moved later to settle on the coast. This exemplifies a continued activity changing place over time without temporal discontinuity]
Bronze Age (E4) [Bronze Age, in the sense of technological adoption, spread over disjoint areas including islands such as the British Isles without temporal discontinuity]
Japan, the state (E4) [In 2021, the Japanese state as a political unit comprised in 6852 islands extending along the Pacific coast of Asia]</rdfs:comment>
    </owl:Class>
    


    <!-- http://cidoc-crm.org/cidoc-crm/7.1.3/E52_Time-Span#E52_Time-Span -->


    <owl:Class rdf:about="http://cidoc-crm.org/cidoc-crm/7.1.3/E52_Time-Span#E52_Time-Span">
        <rdfs:subClassOf rdf:resource="http://www.cidoc-crm.org/cidoc-crm/E1_CRM_Entity#E1_CRM_Entity"/>
        <rdfs:comment>URI:	http://www.cidoc-crm.org/cidoc-crm/E52_Time-Span
SubClass Of:
E1 CRM Entity
SuperClass Of:
-
Scope Note:
This class comprises abstract temporal extents, in the sense of Galilean physics, having a beginning, an end, and a duration.

Instances of E52 Time-Span have no semantic connotations about phenomena happening within the temporal extent they represent. They do not convey any meaning other than a positioning on the &apos;time-line&apos; of chronology. The actual extent of an instance of E52 Time-Span can be approximated by properties of E52 Time-Span giving inner and outer bounds in the form of dates (instances of E61 Time Primitive). Comparing knowledge about time-spans is fundamental for chronological reasoning.

Some instances of E52 Time-Span may be defined as the actual, in principle observable, temporal extent of instances of E2 Temporal Entity via the property P4 has time-span (is time-span of): E52 Time-Span. They constitute phenomenal time-spans as defined in CRMgeo (Doerr &amp; Hiebel 2013). Since our knowledge of history is imperfect and physical phenomena are fuzzy in nature, the extent of phenomenal time-spans can only be described in approximation. An extreme case of approximation, might, for example, define an instance of E52 Time-Span having unknown beginning, end and duration. It may, nevertheless, be associated with other descriptions by which people can infer knowledge about it, such as in relative chronologies.

Some instances of E52 may be defined precisely as representing a declaration of a temporal extent, as, for instance, done in a business contract. They constitute declarative time-spans as defined in CRMgeo (Doerr &amp; Hiebel 2013) and can be described via the property E61 Time Primitive P170 defines time (time is defined by): E52 Time-Span.

When used as a common E52 Time-Span for two events, it will nevertheless describe them as being simultaneous, even if nothing else is known.

Examples:
1961
From 12-17-1993 to 12-8-1996
14h30 to 16h22 4th July 1945
9.30 am 1.1.1999 to 2.00 pm 1.1.1999
the time-span of the Ming Dynasty (Chan, 2011)</rdfs:comment>
    </owl:Class>
    


    <!-- http://cidoc-crm.org/cidoc-crm/7.1.3/E53_Place#E53_Place -->


    <owl:Class rdf:about="http://cidoc-crm.org/cidoc-crm/7.1.3/E53_Place#E53_Place">
        <rdfs:subClassOf rdf:resource="http://www.cidoc-crm.org/cidoc-crm/E1_CRM_Entity#E1_CRM_Entity"/>
        <rdfs:comment>URI:	http://www.cidoc-crm.org/cidoc-crm/E53_Place
SubClass Of:
E1 CRM Entity
SuperClass Of:
-
Scope Note:
This class comprises extents in the natural space where people live, in particular on the surface of the Earth, in the pure sense of physics: independent from temporal phenomena and matter. They may serve describing the physical location of things or phenomena or other areas of interest. Geometrically, instances of E53 Place constitute single contiguous areas or a finite aggregation of disjoint areas in space which are each individually contiguous. They may have fuzzy boundaries.

The instances of E53 Place are usually determined by reference to the position of &apos;immobile&apos; objects such as buildings, cities, mountains, rivers, or dedicated geodetic marks, but may also be determined by reference to mobile objects. A Place can be determined by combining a frame of reference and a location with respect to this frame.

It is sometimes argued that instances of E53 Place are best identified by global coordinates or absolute reference systems. However, relative references are often more relevant in the context of cultural documentation and tend to be more precise. In particular, people are often interested in position in relation to large, mobile objects, such as ships. For example, the Place at which Nelson died is known with reference to a large mobile object, i.e. H.M.S Victory. A resolution of this Place in terms of absolute coordinates would require knowledge of the movements of the vessel and the precise time of death, either of which may be revised, and the result would lack historical and cultural relevance.

Any instance of E18 Physical Thing can serve as a frame of reference for an instance of E53 Place. This may be documented using the property P157 is at rest relative to (provides reference space for).

Examples:
the extent of the UK in the year 2003
the position of the hallmark on the inside of my wedding ring (fictitious)
the place referred to in the phrase: &apos;Fish collected at three miles north of the confluence of the Arve and the Rhone&apos;
here -&gt; &lt;- [the place between these two arrows in one of the reader&apos;s paper copy of this document. Each copy constitutes a different place of this spot.]</rdfs:comment>
    </owl:Class>
    


    <!-- http://cidoc-crm.org/cidoc-crm/7.1.3/E54_Dimension#E54_Dimension -->


    <owl:Class rdf:about="http://cidoc-crm.org/cidoc-crm/7.1.3/E54_Dimension#E54_Dimension">
        <rdfs:subClassOf rdf:resource="http://www.cidoc-crm.org/cidoc-crm/E1_CRM_Entity#E1_CRM_Entity"/>
        <rdfs:comment>URI:	http://www.cidoc-crm.org/cidoc-crm/E54_Dimension
SubClass Of:
E1 CRM Entity
SuperClass Of:
E97 Monetary Amount
Scope Note:
This class comprises quantifiable properties that can be measured by some calibrated means and can be approximated by values, i.e. points or regions in a mathematical or conceptual space, such as natural or real numbers, RGB values, etc.

An instance of E54 Dimension represents the empirical or theoretically derived quantity, including the precision tolerances resulting from the particular method or calculation. The identity of an instance of E54 Dimension depends on the method of its determination because each method may produce different values even when determining comparable qualities. For instance, the wingspan of a bird alive or dead is a different dimension. Thermoluminescence dating and Rehydroxylation [RHX] dating are different dimensions of temporal distance from now, even if they aim at dating the same object. The method of determination should be expressed using the property P2 has type (is type of). Note that simple terms such as &apos;diameter&apos; or &apos;length&apos; are normally insufficient to unambiguously describe a respective dimension. In contrast, &apos;maximum linear extent&apos; may be sufficient.

The properties of the class E54 Dimension allow for expressing the numerical approximation of the values of instances of E54 Dimension adequate to the precision of the applied method of determination. If the respective quantity belongs to a non-discrete space according to the laws of physics, such as spatial distances, it is recommended to record them as approximations by intervals or regions of indeterminacy enclosing the assumed true values. For instance, a length of 5 cm may be recorded as 4.5-5.5 cm, according to the precision of the respective observation. Note, that comparability of values described in different units depends critically on the representation as value regions.

Numerical approximations in archaic instances of E58 Measurement Unit used in historical records should be preserved. Equivalents corresponding to current knowledge should be recorded as additional instances of E54 Dimension, as appropriate.

Examples:
the weight of the Luxor Obelisk [250 metric tons]
the vertical height of the statue of David by Michelangelo [5.17 metres]
the weight of the Great Star of Africa diamond [530.2 carats]
the calibrated C14 date for the Shroud of Turin [AD1262-1312, 1303-1384]
the horizontal diameter of the Stonehenge Sarsen Circle [33 metres] (Pryor, 2016)
the length of the sides of the Great Pyramid at Giza [230.34 metres] (Lehner and Hawass, 2017)
the duration of the time-span of the Battle of Issos/Issus on 15th November 333 B.C.E. [less than 12 hours] (Howard, 2012)
Christie’s hammer price, in British Pounds, for Vincent van Gogh&apos;s &quot;Still Life: Vase with Fifteen Sunflowers&quot; in London on 30th March 1987 (E97) [24.75 million GBP (British Pounds)]</rdfs:comment>
    </owl:Class>
    


    <!-- http://cidoc-crm.org/cidoc-crm/7.1.3/E55_Type#E55_Type -->


    <owl:Class rdf:about="http://cidoc-crm.org/cidoc-crm/7.1.3/E55_Type#E55_Type">
        <rdfs:subClassOf rdf:resource="http://cidoc-crm.org/cidoc-crm/7.1.3/E28_Conceptual_Object#E28_Conceptual_Object"/>
        <rdfs:comment>URI:	http://www.cidoc-crm.org/cidoc-crm/E55_Type
SubClass Of:
E28 Conceptual Object
SuperClass Of:
E56 Language
E57 Material
E58 Measurement Unit
E99 Product Type
Scope Note:
This class comprises concepts denoted by terms from thesauri and controlled vocabularies used to characterize and classify instances of CIDOC CRM classes. Instances of E55 Type represent concepts, in contrast to instances of E41 Appellation which are used to name instances of CIDOC CRM classes.

E55 Type provides an interface to domain specific ontologies and thesauri. These can be represented in the CIDOC CRM as subclasses of E55 Type, forming hierarchies of terms, i.e. instances of E55 Type linked via P127 has broader term (has narrower term): E55 Type. Such hierarchies may be extended with additional properties.

Examples:
weight, length, depth [types for instances of E54 Dimension]
portrait, sketch, animation [types for instances of E36 Visual Item]
French, English, German [types for instances of E56 Language]
excellent, good, poor [types for instances of E3 Condition State]
Ford Model T, chop stick [types for instances of E22 Human-Made Object]
cave, doline, scratch [types for instances of E26 Physical Feature]
poem, short story [types for instances of E33 Linguistic Object]
wedding, earthquake, skirmish [types for instances of E5 Event]</rdfs:comment>
    </owl:Class>
    


    <!-- http://cidoc-crm.org/cidoc-crm/7.1.3/E57_Material#E57_Material -->


    <owl:Class rdf:about="http://cidoc-crm.org/cidoc-crm/7.1.3/E57_Material#E57_Material">
        <rdfs:subClassOf rdf:resource="http://cidoc-crm.org/cidoc-crm/7.1.3/E55_Type#E55_Type"/>
        <rdfs:comment>URI:	http://www.cidoc-crm.org/cidoc-crm/E57_Material
SubClass Of:
E55 Type
SuperClass Of:
-
Scope Note:
This class is a specialization of E55 Type and comprises the concepts of materials.

Instances of E57 Material may denote properties of matter before its use, during its use, and as incorporated in an object, such as ultramarine powder, tempera paste, reinforced concrete. Discrete pieces of raw-materials kept in museums, such as bricks, sheets of fabric, pieces of metal, should be modelled individually in the same way as other objects. Discrete used or processed pieces, such as the stones from Nefer Titi&apos;s temple, should be modelled as parts (cf. P46 is composed of (forms part of): E18 Physical Thing).

This type is used categorically in the model without reference to instances of it, i.e. the Model does not foresee the description of instances of instances of E57 Material, e.g. &apos;instances of gold&apos;.

It is recommended that internationally or nationally agreed codes and terminology should be used.

Examples:
brick (Gurcke, 1987)
gold (Watson, 1990)
aluminium (Norman, 1986)
polycarbonate (Mhaske, 2011)
resin (Barton, 1992)</rdfs:comment>
    </owl:Class>
    


    <!-- http://cidoc-crm.org/cidoc-crm/7.1.3/E59_Primitive_Value#E59_Primitive_Value -->


    <owl:Class rdf:about="http://cidoc-crm.org/cidoc-crm/7.1.3/E59_Primitive_Value#E59_Primitive_Value">
        <rdfs:subClassOf rdf:resource="http://www.cidoc-crm.org/cidoc-crm/E1_CRM_Entity#E1_CRM_Entity"/>
        <rdfs:comment>URI:	-
SubClass Of:
E1 CRM Entity
SuperClass Of:
E60 Number
E61 Time Primitive
E62 String
E94 Space Primitive
E95 Spacetime Primitive
Scope Note:
This class comprises values of primitive data types of programming languages or database management systems and data types composed of such values used as documentation elements, as well as their mathematical abstractions.

The instances of E59 Primitive Value and its subclasses are not considered elements of the universe of discourse the CIDOC CRM aims to define and analyse. Rather, they play the role of a symbolic interface between the scope of the model and the world of mathematical and computational manipulations and the symbolic objects they define and handle.

In particular, they comprise lexical forms encoded as &apos;strings&apos; or series of characters and symbols based on encoding schemes (characterised by being a limited subset of the respective mathematical abstractions) such as UNICODE and values of datatypes that can be encoded in a lexical form, including quantitative specifications of time-spans and geometry. They have in common that instances of E59 Primitive Value define themselves by virtue of their encoded value, regardless of the nature of their mathematical abstractions.

Therefore, in an implementation, instances of E59 Primitive should be represented directly in the encoded symbolic form supported by the respective platform, such as a character string or a formatted date. They must not be represented in an implementation indirectly via, another a universal resource identifier, which in turn is linked to the actual encoded symbolic form. In a concrete application, it is recommended that the primitive value system from a chosen implementation platform and/or data definition language be used to substitute for this class and its subclasses.</rdfs:comment>
    </owl:Class>
    


    <!-- http://cidoc-crm.org/cidoc-crm/7.1.3/E5_Event#E5_Event -->


    <owl:Class rdf:about="http://cidoc-crm.org/cidoc-crm/7.1.3/E5_Event#E5_Event">
        <rdfs:subClassOf rdf:resource="http://cidoc-crm.org/cidoc-crm/7.1.3/E4_Period#E4_Period"/>
        <rdfs:comment>URI:	http://www.cidoc-crm.org/cidoc-crm/E5_Event
SubClass Of:
E4 Period
SuperClass Of:
E7 Activity
E63 Beginning of Existence
E64 End of Existence
Scope Note:
This class comprises distinct, delimited and coherent processes and interactions of a material nature, in cultural, social or physical systems, involving and affecting instances of E77 Persistent Item in a way characteristic of the kind of process. Typical examples are meetings, births, deaths, actions of decision taking, making or inventing things, but also more complex and extended ones such as conferences, elections, building of a castle, or battles.

While the continuous growth of a tree lacks the limits characteristic of an event, its germination from a seed does qualify as an event. Similarly, the blowing of the wind lacks the distinctness and limits of an event, but a hurricane, flood or earthquake would qualify as an event. Mental processes are considered as events, in cases where they are connected with the material externalization of their results; for example, the creation of a poem, a performance or a change of intention that becomes obvious from subsequent actions or declarations.

The effects of an instance of E5 Event may not lead to relevant permanent changes of properties or relations of the items involved in it, for example an unrecorded performance. Of course, in order to be documented, some kind of evidence for an event must exist, be it witnesses, traces or products of the event.

While instances of E4 Period always require some form of coherence between its constituent phenomena, in addition, the essential constituents of instances of E5 Event should contribute to an overall effect; for example, the statements made during a meeting and the listening of the audience.

Viewed at a coarse level of detail, an instance of E5 Event may appear as if it had an ‘instantaneous’ overall effect, but any process or interaction of material nature in reality have an extent in time and space. At a fine level, instances of E5 Event may be analysed into component phenomena and phases within a space and timeframe, and as such can be seen as a period, regardless of the size of the phenomena. The reverse is not necessarily the case: not all instances of E4 Period give rise to a noteworthy overall effect and are thus not instances of E5 Event.

Examples:
the birth of Cleopatra (E67) (Pomeroy, 1984)
the destruction of Herculaneum by volcanic eruption in 79 AD (E6) (Camardo, 2013)
World War II (E7) (Barber, 1994)
the Battle of Stalingrad (E7) (Hoyt, 1993)
the Yalta Conference (E7) (Harbutt, 2010)
my birthday celebration 28-6-1995 (E7)
the falling of a tile from my roof last Sunday (fictitious)
the CIDOC conference 2003 (E7)</rdfs:comment>
    </owl:Class>
    


    <!-- http://cidoc-crm.org/cidoc-crm/7.1.3/E60_Number#E60_Number -->


    <owl:Class rdf:about="http://cidoc-crm.org/cidoc-crm/7.1.3/E60_Number#E60_Number">
        <rdfs:subClassOf rdf:resource="http://cidoc-crm.org/cidoc-crm/7.1.3/E59_Primitive_Value#E59_Primitive_Value"/>
        <rdfs:comment>URI:	-
SubClass Of:
E59 Primitive Value
SuperClass Of:
-
Scope Note:
This class comprises any encoding of computable (algebraic) values such as integers, real numbers, complex numbers, vectors, tensors, etc., including intervals of these values to express limited precision.

Numbers are fundamentally distinct from identifiers in continua, which are instances of E41 Appellation, such as Gregorian dates or spatial coordinates, even though their encoding may be similar. Instances of E60 Number can be combined with each other in algebraic operations to yield other instances of E60 Number, e.g. 1 + 1 = 2. Identifiers in continua may be combined with numbers expressing distances to yield new identifiers, e.g., 1924-01-31 + 2 days = 1924-02-02. Cf. E54 Dimension.</rdfs:comment>
    </owl:Class>
    


    <!-- http://cidoc-crm.org/cidoc-crm/7.1.3/E62_String#E62_String -->


    <owl:Class rdf:about="http://cidoc-crm.org/cidoc-crm/7.1.3/E62_String#E62_String">
        <rdfs:subClassOf rdf:resource="http://cidoc-crm.org/cidoc-crm/7.1.3/E59_Primitive_Value#E59_Primitive_Value"/>
        <rdfs:comment>URI:	-
SubClass Of:
E59 Primitive Value
SuperClass Of:
-
Scope Note:
This class comprises coherent sequences of binary-encoded symbols. They correspond to the content of an instance of E90 Symbolic object. Instances of E62 String represent only the symbol sequence itself. They may or may not contain a language code.

In contrast, instances of other subclasses of E59 Primitive value represent entities in mathematical spaces other than that of symbol sequences, by using binary-encoded symbols, such as date expressions or numbers in decimal encoding. For instance, different syntactic forms of a date expression may represent the same date but consist of different strings.

Examples:
&apos;the quick brown fox jumps over the lazy dog&apos;
&apos;6F 6E 54 79 70 31 0D 9E&apos;</rdfs:comment>
    </owl:Class>
    


    <!-- http://cidoc-crm.org/cidoc-crm/7.1.3/E65_Creation#E65_Creation -->


    <owl:Class rdf:about="http://cidoc-crm.org/cidoc-crm/7.1.3/E65_Creation#E65_Creation">
        <rdfs:subClassOf rdf:resource="http://cidoc-crm.org/cidoc-crm/7.1.3/E7_Activity#E7_Activity"/>
        <rdfs:comment>URI:	http://www.cidoc-crm.org/cidoc-crm/E65_Creation
SubClass Of:
E7 Activity
E63 Beginning of Existence
SuperClass Of:
E83 Type Creation
Scope Note:
This class comprises events that result in the creation of conceptual items or immaterial products, such as legends, poems, texts, music, images, movies, laws, types, etc.

Examples:
the framing of the U.S. Constitution (Farrand, 1913)
the drafting of U.N. Resolution 1441 (United Nations Security Council, 2002)</rdfs:comment>
    </owl:Class>
    


    <!-- http://cidoc-crm.org/cidoc-crm/7.1.3/E70_Thing#E70_Thing -->


    <owl:Class rdf:about="http://cidoc-crm.org/cidoc-crm/7.1.3/E70_Thing#E70_Thing">
        <rdfs:subClassOf rdf:resource="http://cidoc-crm.org/cidoc-crm/7.1.3/E77_Persistent_Item#E77_Persistent_Item"/>
        <rdfs:comment>URI:	http://www.cidoc-crm.org/cidoc-crm/E70_Thing
SubClass Of:
E77 Persistent Item
SuperClass Of:
E71 Human-Made Thing
E72 Legal Object
Scope Note:
This general class comprises discrete, identifiable, instances of E77 Persistent Item that are documented as single units, that either consist of matter or depend on being carried by matter and are characterized by relative stability.

They may be intellectual products or physical things. They may, for instance, have a solid physical form, an electronic encoding, or they may be a logical concept or structure.

Examples:
my photograph collection (E78) (fictitious)
the bottle of milk in my refrigerator (E22) (fictitious)
the Riss A1 plan of the Straßburger Münster (French: Cathédrale Notre-Dame de Strasbourg) (E29) (Liess, R., 1985)
the thing on the top of Otto Hahn’s desk (E19)
the form of the no-smoking sign (E36)
the cave of Dirou, Mani, Greece (E26) (Psimenos, 2005)</rdfs:comment>
    </owl:Class>
    


    <!-- http://cidoc-crm.org/cidoc-crm/7.1.3/E71_Human-Made_Thing#E71_Human-Made_Thing -->


    <owl:Class rdf:about="http://cidoc-crm.org/cidoc-crm/7.1.3/E71_Human-Made_Thing#E71_Human-Made_Thing">
        <rdfs:subClassOf rdf:resource="http://cidoc-crm.org/cidoc-crm/7.1.3/E70_Thing#E70_Thing"/>
        <rdfs:comment>URI:	http://www.cidoc-crm.org/cidoc-crm/E71_Human-Made_Thing
SubClass Of:
E70 Thing
SuperClass Of:
E24 Physical Human-Made Thing
E28 Conceptual Object
Scope Note:
This class comprises discrete, identifiable human-made items that are documented as single units.

These items are either intellectual products or human-made physical things, and are characterized by relative stability. They may, for instance, have a solid physical form, an electronic encoding, or they may be logical concepts or structures.

Examples:
Beethoven’s 5th Symphony (E73) (Lockwood, 2015)
Michelangelo’s David (E22) (Paoletti and Bagemihl, 2015)
Einstein’s Theory of General Relativity (E89) (Hartle, 2003)
the taxon ‘Fringilla coelebs Linnaeus,1758’ (E55) (Sinkevicius and Narusevicius, 2002)</rdfs:comment>
    </owl:Class>
    


    <!-- http://cidoc-crm.org/cidoc-crm/7.1.3/E72_Legal_Object#E72_Legal_Object -->


    <owl:Class rdf:about="http://cidoc-crm.org/cidoc-crm/7.1.3/E72_Legal_Object#E72_Legal_Object">
        <rdfs:subClassOf rdf:resource="http://cidoc-crm.org/cidoc-crm/7.1.3/E70_Thing#E70_Thing"/>
        <rdfs:comment>URI:	http://www.cidoc-crm.org/cidoc-crm/E72_Legal_Object
SubClass Of:
E70 Thing
SuperClass Of:
E18 Physical Thing
E90 Symbolic Object
Scope Note:
This class comprises those material or immaterial items to which instances of E30 Right, such as the right of ownership or use, can be applied.

This is generally true for all instances of E18 Physical Thing. In the case of instances of E28 Conceptual Object, however, the identity of an instance of E28 Conceptual Object or the method of its use may be too ambiguous to reliably establish instances of E30 Right, as in the case of taxa and inspirations. Ownership of corporations is currently regarded as out of scope of the CIDOC CRM.

Examples:
the Cullinan diamond (E19) (Scarratt and Shor, 2006)
definition of the CIDOC Conceptual Reference Model Version 5.0.4 (E73) (ISO 21127: 2014)</rdfs:comment>
    </owl:Class>
    


    <!-- http://cidoc-crm.org/cidoc-crm/7.1.3/E73_Information_Object#E73_Information_Object -->


    <owl:Class rdf:about="http://cidoc-crm.org/cidoc-crm/7.1.3/E73_Information_Object#E73_Information_Object">
        <rdfs:subClassOf rdf:resource="http://cidoc-crm.org/cidoc-crm/7.1.3/E90_Symbolic_Object#E90_Symbolic_Object"/>
        <rdfs:comment>URI:	http://www.cidoc-crm.org/cidoc-crm/E73_Information_Object
SubClass Of:
E89 Propositional Object
E90 Symbolic Object
SuperClass Of:
E29 Design or Procedure
E31 Document
E33 Linguistic Object
E36 Visual Item
Scope Note:
This class comprises identifiable immaterial items, such as poems, jokes, data sets, images, texts, multimedia objects, procedural prescriptions, computer program code, algorithm or mathematical formulae, that have an objectively recognizable structure and are documented as single units. The encoding structure known as a &apos;named graph&apos; also falls under this class, so that each &apos;named graph&apos; is an instance of E73 Information Object.

An instance of E73 Information Object does not depend on a specific physical carrier, which can include human memory, and it can exist on one or more carriers simultaneously.

Instances of E73 Information Object of a linguistic nature should be declared as instances of the E33 Linguistic Object subclass. Instances of E73 Information Object of a documentary nature should be declared as instances of the E31 Document subclass. Conceptual items such as types and classes are not instances of E73 Information Object, nor are ideas without a reproducible expression.

Examples:
image BM000038850.JPG from the Clayton Herbarium in London (E31) (Natural History Museum, 2021)
E. A. Poe&apos;s &apos;The Raven&apos; (Poe, 1869)
the movie &apos;The Seven Samurai&apos; by Akira Kurosawa (Mellen, 2002)
the text of Huray describing the Maxwell Equations (Huray, 2010)
the Getty AAT as published as Linked Open Data, accessed 1/10/2014</rdfs:comment>
    </owl:Class>
    


    <!-- http://cidoc-crm.org/cidoc-crm/7.1.3/E77_Persistent_Item#E77_Persistent_Item -->


    <owl:Class rdf:about="http://cidoc-crm.org/cidoc-crm/7.1.3/E77_Persistent_Item#E77_Persistent_Item">
        <rdfs:subClassOf rdf:resource="http://www.cidoc-crm.org/cidoc-crm/E1_CRM_Entity#E1_CRM_Entity"/>
        <rdfs:comment>URI:	http://www.cidoc-crm.org/cidoc-crm/E77_Persistent_Item
SubClass Of:
E1 CRM Entity
SuperClass Of:
E39 Actor
E70 Thing
Scope Note:
This class comprises items that have persistent characteristics of structural nature substantially related to their identity and their integrity, sometimes known as &apos;endurants&apos; in philosophy. Persistent Items may be physical entities, such as people, animals or things, conceptual entities such as ideas, concepts, products of the imagination or even names.

Instances of E77 Persistent Item may be present or be part of interactions in different periods or events. They can repeatedly be recognized at disparate occasions during their existence by characteristics of structural nature. The respective characteristics need not be exactly the same during all the existence of an instance of E77 Persistent Item. Often, they undergo gradual change, still bearing some similarities with that of previous times, or disappear completely and new emerge. For instance, a person, from the time of being born on, will gradually change all its features and acquire new ones, such as a scar. Even the DNA in different body cells will develop defects and mutations. Nevertheless, relevant characteristics used should be sufficiently similar to recognize the instance for some substantial period of time.

The more specific criteria that determine the identity of instances of subclasses of E77 Persistent Item may vary considerably and are described or referred to in the respective scope notes. The decision about which exact criteria to use depends on whether the observable behaviour of the respective part of reality such confined conforms to the reasoning the user is interested in. For example, a building can be regarded as no longer existing if it is dismantled and the materials reused in a different configuration. On the other hand, human beings go through radical and profound changes during their life-span, affecting both material composition and form, yet preserve their identity by other criteria, such as being bodily separated from other persons. Similarly, inanimate objects may be subject to exchange of parts and matter. On the opposite, the identity of a (version of a) text of a scientific publication is given by the exact arrangement of its relevant symbols.

The main classes of objects that fall outside the scope of the E77 Persistent Item class are temporal objects such as periods, events and acts, and descriptive properties.

An instance of E77 Persistent Item does not require actual knowledge of the identifying features of the instance being currently known. There may be cases, where the actual identifying features of an instance of E77 Persistent Item are not decidable at a particular state of knowledge.

Examples:
Leonardo da Vinci (E21) (Strano, 1953)
Stonehenge (E24) (Pryor, 2016)
the hole in the ozone layer (E4) (Hufford and Horwitz, 2005)
the First Law of Thermodynamics (E89) (Craig and Gislason, 2002)
the Bermuda Triangle (E53) (Dolan, 2005)</rdfs:comment>
    </owl:Class>
    


    <!-- http://cidoc-crm.org/cidoc-crm/7.1.3/E7_Activity#E7_Activity -->


    <owl:Class rdf:about="http://cidoc-crm.org/cidoc-crm/7.1.3/E7_Activity#E7_Activity">
        <owl:equivalentClass rdf:resource="http://www.w3.org/ns/prov#Activity"/>
        <rdfs:subClassOf rdf:resource="http://cidoc-crm.org/cidoc-crm/7.1.3/E5_Event#E5_Event"/>
        <rdfs:comment>URI:	http://www.cidoc-crm.org/cidoc-crm/E7_Activity
SubClass Of:
E5 Event
SuperClass Of:
E8 Acquisition
E9 Move
E10 Transfer of Custody
E11 Modification
E13 Attribute Assignment
E65 Creation
E66 Formation
E85 Joining
E86 Leaving
E87 Curation Activity
Scope Note:
This class comprises actions intentionally carried out by instances of E39 Actor that result in changes of state in the cultural, social, or physical systems documented.

This notion includes complex, composite, and long-lasting actions such as the building of a settlement or a war, as well as simple, short-lived actions such as the opening of a door.

Examples:
the Battle of Stalingrad (Hoyt, 1993)
the Yalta Conference (Harbutt, 2010)
my birthday celebration 28-6-1995
the writing of &apos;Faust&apos; by Goethe (E65) (Williams, 2020)
the formation of the Bauhaus 1919 (E66) (Droste, 2006)
the people of Iraq giving the name ‘Quyunjig’ to the place identified by the TGN as ‘7017998’
Kira Weber working in glass art from 1984 to 1993
Kira Weber working in oil and pastel painting from 1993</rdfs:comment>
    </owl:Class>
    


    <!-- http://cidoc-crm.org/cidoc-crm/7.1.3/E90_Symbolic_Object#E90_Symbolic_Object -->


    <owl:Class rdf:about="http://cidoc-crm.org/cidoc-crm/7.1.3/E90_Symbolic_Object#E90_Symbolic_Object">
        <rdfs:subClassOf rdf:resource="http://cidoc-crm.org/cidoc-crm/7.1.3/E28_Conceptual_Object#E28_Conceptual_Object"/>
        <rdfs:comment>URI:	http://www.cidoc-crm.org/cidoc-crm/E90_Symbolic_Object
SubClass Of:
E28 Conceptual Object
E72 Legal Object
SuperClass Of:
E41 Appellation
E73 Information Object
Scope Note:
This class comprises identifiable symbols and any aggregation of symbols, such as characters, identifiers, traffic signs, emblems, texts, data sets, images, musical scores, multimedia objects, computer program code, or mathematical formulae that have an objectively recognizable structure and that are documented as single units.

It includes sets of signs of any nature, which may serve to designate something, or to communicate some propositional content. An instance of E90 Symbolic Object may or may not have a specific meaning, for example an arbitrary character string.

In some cases, the content of an instance of E90 Symbolic Object may completely be represented by a serialized digital content model, such as a sequence of ASCII-encoded characters, an XML or HTML document, or a TIFF image. The property P3 has note and its subproperty P190 has symbolic content allow for the description of this content model. In order to disambiguate which symbolic level is the carrier of the meaning, the property P3.1 has type can be used to specify the encoding (e.g. &apos;bit&apos;, &apos;Latin character&apos;, RGB pixel).

Examples:
‘ecognizabl’
the &apos;no-smoking&apos; sign (E36)
&apos;BM000038850.JPG&apos; (E41) [identifies a digital image] (Natural History Museum, 2021)
image BM000038850.JPG from the Clayton Herbarium in London (E36) [depicts specimen of Verbesina virginica] (Natural History Museum, 2021)
the distribution of form, tone and colour found on Leonardo da Vinci’s painting named &apos;Mona Lisa&apos; in daylight (E36)
the Italian text of Dante’s &apos;Divina Commedia&apos; as found in the authoritative critical edition &apos;La Commedia secondo l’antica vulgata a cura di Giorgio Petrocchi&apos; (E33) (Petrocchi, 1967)</rdfs:comment>
    </owl:Class>
    


    <!-- http://cidoc-crm.org/cidoc-crm/7.1.3/E94_Space_Primitive#E94_Space_Primitive -->


    <owl:Class rdf:about="http://cidoc-crm.org/cidoc-crm/7.1.3/E94_Space_Primitive#E94_Space_Primitive">
        <rdfs:subClassOf rdf:resource="http://cidoc-crm.org/cidoc-crm/7.1.3/E59_Primitive_Value#E59_Primitive_Value"/>
        <rdfs:comment>URI:	-
SubClass Of:
E41 Appellation
E59 Primitive Value
SuperClass Of:
-
Scope Note:
This class comprises instances of E59 Primitive Value for space that should be implemented with appropriate validation, precision and references to spatial coordinate systems to express geometries on or relative to Earth, or on any other stable constellations of matter, relevant to cultural and scientific documentation.

An instance of E94 Space Primitive defines an instance of E53 Place in the sense of a declarative place as elaborated in CRMgeo (Doerr &amp; Hiebel 2013), which means that the identity of the place is derived from its geometric definition. Such a declarative place may allow for the approximation of instances of E53 Place defined by the actual extent of some phenomenon, such as a settlement or a riverbed, or other forms of identification rather than by an instance of E94 Space Primitive. Note that using an instance of E94 Space Primitive for approximating the actual extent of some place always defines a (declarative) instance of E53 Place in its own right.

Definitions of instances of E53 Place using different spatial reference systems are always definitions of different instances of E53 Place.

Instances of E94 Space Primitive provide the ability to link CIDOC CRM encoded data to the kinds of geometries used in maps or Geoinformation systems. They may be used for visualization of the instances of E53 Place they define, in their geographic context and for computing topological relations between places based on these geometries. E94 Space Primitive is not further elaborated upon within this model. It is considered good practice to maintain compatibility with OGC standards.

Examples:
&lt;gml:Point gml:id=&quot;p21&quot; srsName=&quot;http://www.opengis.net/def/crs/EPSG/0/4326&quot;&gt;
  &lt;gml:coordinates&gt;45.67, 88.56&lt;/gml:coordinates&gt;
&lt;/gml:Point&gt;
[Coordinate Information in GML]
&apos;40°31&apos;17.9&quot;N 21°15&apos;48.3&quot;E&apos; [A single point for approximating the centre of the city of Kastoria, Greece]
POLYGON ((30 10, 40 40, 20 40, 10 20, 30 10)) [Well-Known Text (WKT)]</rdfs:comment>
    </owl:Class>
    


    <!-- http://objects.mainzed.org/agent/ont#Archeologist -->


    <owl:Class rdf:about="http://objects.mainzed.org/agent/ont#Archeologist">
        <owl:equivalentClass rdf:resource="https://photogrammetry.altervista.org/items/show/123#F37_Survey_Operator"/>
        <owl:equivalentClass rdf:resource="https://photogrammetry.altervista.org/items/show/124#F38_Processing_Operator"/>
    </owl:Class>
    


    <!-- http://objects.mainzed.org/agent/ont#Engineer -->


    <owl:Class rdf:about="http://objects.mainzed.org/agent/ont#Engineer">
        <owl:equivalentClass rdf:resource="https://photogrammetry.altervista.org/items/show/123#F37_Survey_Operator"/>
        <owl:equivalentClass rdf:resource="https://photogrammetry.altervista.org/items/show/124#F38_Processing_Operator"/>
        <owl:equivalentClass rdf:resource="https://photogrammetry.altervista.org/items/show/125#F39_Modelling_Operator"/>
    </owl:Class>
    


    <!-- http://objects.mainzed.org/function/ont#ExportFunction -->


    <owl:Class rdf:about="http://objects.mainzed.org/function/ont#ExportFunction">
        <owl:equivalentClass rdf:resource="https://photogrammetry.altervista.org/items/show/91#F5_Exporting"/>
    </owl:Class>
    


    <!-- http://objects.mainzed.org/function/ont#FeatureDetectionAlgorithm -->


    <owl:Class rdf:about="http://objects.mainzed.org/function/ont#FeatureDetectionAlgorithm">
        <owl:equivalentClass rdf:resource="https://photogrammetry.altervista.org/items/show/107#F21_Matching_Algorithm_Type"/>
    </owl:Class>
    


    <!-- http://objects.mainzed.org/function/ont#MeasurementAlgorithm -->


    <owl:Class rdf:about="http://objects.mainzed.org/function/ont#MeasurementAlgorithm">
        <owl:equivalentClass rdf:resource="https://photogrammetry.altervista.org/items/show/191#F105:_Interrogation_Tools"/>
    </owl:Class>
    


    <!-- http://objects.mainzed.org/function/ont#ModificationFunction -->


    <owl:Class rdf:about="http://objects.mainzed.org/function/ont#ModificationFunction">
        <owl:equivalentClass rdf:resource="https://photogrammetry.altervista.org/items/show/90#F4_Modelling"/>
    </owl:Class>
    


    <!-- http://objects.mainzed.org/function/ont#ProcessingFunction -->


    <owl:Class rdf:about="http://objects.mainzed.org/function/ont#ProcessingFunction">
        <owl:equivalentClass rdf:resource="https://photogrammetry.altervista.org/items/show/89#F3_Processing"/>
    </owl:Class>
    


    <!-- http://objects.mainzed.org/function/ont#RemoveFunction -->


    <owl:Class rdf:about="http://objects.mainzed.org/function/ont#RemoveFunction">
        <owl:equivalentClass rdf:resource="https://photogrammetry.altervista.org/items/show/154#F67_Modelling_Elimination"/>
    </owl:Class>
    


    <!-- http://objects.mainzed.org/metadata/ont#AcquisitionTechnology -->


    <owl:Class rdf:about="http://objects.mainzed.org/metadata/ont#AcquisitionTechnology">
        <owl:equivalentClass rdf:resource="https://photogrammetry.altervista.org/items/show/106#F20_Acquisition_Device_Type"/>
    </owl:Class>
    


    <!-- http://objects.mainzed.org/metadata/ont#Calibration -->


    <owl:Class rdf:about="http://objects.mainzed.org/metadata/ont#Calibration">
        <owl:equivalentClass rdf:resource="https://photogrammetry.altervista.org/items/show/287#F108_Calibration_of_the_Instrument"/>
        <rdfs:subClassOf rdf:resource="http://www.w3.org/ns/prov#Entity"/>
    </owl:Class>
    


    <!-- http://objects.mainzed.org/metadata/ont#CalibrationAlgorithm -->


    <owl:Class rdf:about="http://objects.mainzed.org/metadata/ont#CalibrationAlgorithm">
        <owl:equivalentClass rdf:resource="https://photogrammetry.altervista.org/items/show/189#F103:_Calibration_(Camera_Calibration)"/>
    </owl:Class>
    


    <!-- http://objects.mainzed.org/metadata/ont#CapturingDevice -->


    <owl:Class rdf:about="http://objects.mainzed.org/metadata/ont#CapturingDevice">
        <owl:equivalentClass rdf:resource="https://photogrammetry.altervista.org/items/show/95#F9_Acquisition_Device"/>
    </owl:Class>
    


    <!-- http://objects.mainzed.org/metadata/ont#Enviroment -->


    <owl:Class rdf:about="http://objects.mainzed.org/metadata/ont#Enviroment">
        <owl:equivalentClass rdf:resource="https://photogrammetry.altervista.org/items/show/286#F106_Acquisition_Location_Type"/>
    </owl:Class>
    


    <!-- http://objects.mainzed.org/metadata/ont#FusionAlgorithm -->


    <owl:Class rdf:about="http://objects.mainzed.org/metadata/ont#FusionAlgorithm">
        <owl:equivalentClass rdf:resource="https://photogrammetry.altervista.org/items/show/190#F104:_Registration_(Fusion_of_Multiple_Point_Clouds_or_3D_Models)"/>
    </owl:Class>
    


    <!-- http://objects.mainzed.org/metadata/ont#MeasurementActivity -->


    <owl:Class rdf:about="http://objects.mainzed.org/metadata/ont#MeasurementActivity">
        <owl:equivalentClass rdf:resource="http://www.cidoc-crm.org/extensions/crmsci/versions/2.0/S21_Measurement#S21_Measurement"/>
    </owl:Class>
    


    <!-- http://objects.mainzed.org/metadata/ont#MeshProcessingActivity -->


    <owl:Class rdf:about="http://objects.mainzed.org/metadata/ont#MeshProcessingActivity">
        <owl:equivalentClass rdf:resource="https://photogrammetry.altervista.org/items/show/142#F56_Mesh_Reconstruction"/>
    </owl:Class>
    


    <!-- http://objects.mainzed.org/metadata/ont#PointCloud -->


    <owl:Class rdf:about="http://objects.mainzed.org/metadata/ont#PointCloud">
        <owl:equivalentClass rdf:resource="https://photogrammetry.altervista.org/items/show/112#F26_Point_Cloud"/>
    </owl:Class>
    


    <!-- http://objects.mainzed.org/metadata/ont#VertexMeasures -->


    <owl:Class rdf:about="http://objects.mainzed.org/metadata/ont#VertexMeasures">
        <owl:equivalentClass rdf:resource="http://www.semanticweb.org/vitto/ontologies/2024/9/PODS_1Protocol_of_Ontological_Digital_Survey/extensions/versions/1_1/F54_Point_Cloud_Vertex_Quality#F54_Point_Cloud_Vertex_Quality"/>
    </owl:Class>
    


    <!-- http://objects.mainzed.org/type/ont#CalibrationObject -->


    <owl:Class rdf:about="http://objects.mainzed.org/type/ont#CalibrationObject">
        <owl:equivalentClass rdf:resource="https://photogrammetry.altervista.org/items/show/288#F109_Marker_and_Calibration_Tools"/>
        <rdfs:subClassOf rdf:resource="http://objects.mainzed.org/type/ont#Tool"/>
    </owl:Class>
    


    <!-- http://objects.mainzed.org/type/ont#GeometricalRepresentation -->


    <owl:Class rdf:about="http://objects.mainzed.org/type/ont#GeometricalRepresentation">
        <owl:equivalentClass rdf:resource="https://photogrammetry.altervista.org/items/show/104#F18_Dominant_Geometry_Type"/>
    </owl:Class>
    


    <!-- http://objects.mainzed.org/type/ont#Mesh -->


    <owl:Class rdf:about="http://objects.mainzed.org/type/ont#Mesh">
        <owl:equivalentClass rdf:resource="https://photogrammetry.altervista.org/items/show/114#F28_3D_Mesh"/>
    </owl:Class>
    


    <!-- http://objects.mainzed.org/type/ont#PointSet -->


    <owl:Class rdf:about="http://objects.mainzed.org/type/ont#PointSet">
        <owl:equivalentClass rdf:resource="https://photogrammetry.altervista.org/items/show/113#F27_Densified_Point_Cloud"/>
    </owl:Class>
    


    <!-- http://objects.mainzed.org/type/ont#PrintableMesh -->


    <owl:Class rdf:about="http://objects.mainzed.org/type/ont#PrintableMesh">
        <owl:equivalentClass rdf:resource="https://photogrammetry.altervista.org/items/show/163#F76_3D_Model_for_3D_Print"/>
    </owl:Class>
    


    <!-- http://objects.mainzed.org/type/ont#ShapeRepresentation -->


    <owl:Class rdf:about="http://objects.mainzed.org/type/ont#ShapeRepresentation">
        <owl:equivalentClass rdf:resource="https://photogrammetry.altervista.org/items/show/188#F102:_3D_Digital_Asset"/>
    </owl:Class>
    


    <!-- http://objects.mainzed.org/type/ont#Tool -->


    <owl:Class rdf:about="http://objects.mainzed.org/type/ont#Tool">
        <rdfs:subClassOf rdf:resource="http://www.w3.org/ns/prov#Entity"/>
    </owl:Class>
    


    <!-- http://objects.mainzed.org/type/ont#2DRaster -->


    <owl:Class rdf:about="http://objects.mainzed.org/type/ont#2DRaster">
        <owl:equivalentClass rdf:resource="https://photogrammetry.altervista.org/items/show/174#F87_3D_Model_Prospectus"/>
    </owl:Class>
    


    <!-- http://objects.mainzed.org/type/ont#3DRaster -->


    <owl:Class rdf:about="http://objects.mainzed.org/type/ont#3DRaster">
        <owl:equivalentClass rdf:resource="https://photogrammetry.altervista.org/items/show/171#F84_3D_Model_for_Prospectus"/>
    </owl:Class>
    


    <!-- http://objects.mainzed.org/type/ont#4DRaster -->


    <owl:Class rdf:about="http://objects.mainzed.org/type/ont#4DRaster">
        <owl:equivalentClass rdf:resource="https://photogrammetry.altervista.org/items/show/159#F72_3D_Model_Video_Rendering"/>
    </owl:Class>
    


    <!-- http://www.cidoc-crm.org/cidoc-crm/E1_CRM_Entity#E1_CRM_Entity -->


    <owl:Class rdf:about="http://www.cidoc-crm.org/cidoc-crm/E1_CRM_Entity#E1_CRM_Entity">
        <rdfs:comment>URI:	http://www.cidoc-crm.org/cidoc-crm/E1_CRM_Entity
SubClass Of:
-
SuperClass Of:
E2 Temporal Entity
E52 Time-Span
E53 Place
E54 Dimension
E59 Primitive Value
E77 Persistent Item
E92 Spacetime Volume
Scope Note:
This class comprises all things in the universe of discourse of the CIDOC Conceptual Reference Model.

It is an abstract concept providing for three general properties:

Identification by name or appellation, and in particular by a preferred identifier
Classification by type, allowing further refinement of the specific subclass to which an instance belongs
Attachment of free text and other unstructured data for the expression of anything not captured by formal properties
All other classes within the CIDOC CRM are directly or indirectly specialisations of E1 CRM Entity.

Examples:
the earthquake in Lisbon 1755 (E5) (Chester, 2001)</rdfs:comment>
    </owl:Class>
    


    <!-- http://www.cidoc-crm.org/extensions/crmdig/versions/4.0/D11_Digital_Measurement_Event#D11_Digital_Measurement_Event -->


    <owl:Class rdf:about="http://www.cidoc-crm.org/extensions/crmdig/versions/4.0/D11_Digital_Measurement_Event#D11_Digital_Measurement_Event">
        <rdfs:subClassOf rdf:resource="http://cidoc-crm.org/cidoc-crm/7.1.3/E16_Measurement#E16_Measurement"/>
        <rdfs:subClassOf rdf:resource="http://www.cidoc-crm.org/extensions/crmdig/versions/4.0/D7_Digital_Machine_Event#D7_Digital_Machine_Event"/>
        <rdfs:comment>URI: http://www.cidoc-crm.org/extensions/crmdig/versions/4.0/D11_Digital_Measurement_Event

SubClass Of:
D7 Digital Machine Event
E16 Measurement
SuperClass Of:
D2 Digitization Process
Scope Note:
This class comprises actions measuring physical properties using a digital device, that are determined by a systematic procedure and creates an instance of D9 Data Object, which is stored on an instance of D13 Digital Information Carrier.

In contrast to instances of D10 Software Execution, environmental factors have an intended influence on the outcome of an instance of D11 Digital Measurement Event.

Measurement devices may include running distinct software, such as the RAW to JPEG conversion in digital cameras.

In this case, the event is regarded as instance of both classes, D10 Software Execution and D11 Digital Measurement Event.

Examples:
-</rdfs:comment>
    </owl:Class>
    


    <!-- http://www.cidoc-crm.org/extensions/crmdig/versions/4.0/D13_Digital_Information_Carrier#D13_Digital_Information_Carrier -->


    <owl:Class rdf:about="http://www.cidoc-crm.org/extensions/crmdig/versions/4.0/D13_Digital_Information_Carrier#D13_Digital_Information_Carrier">
        <rdfs:subClassOf rdf:resource="http://www.cidoc-crm.org/cidoc-crm/E1_CRM_Entity#E1_CRM_Entity"/>
        <rdfs:comment>SubClass Of:
E1 CRM Entity
SuperClass Of:
-
Scope Note:
This class comprises all instances of E84 Information Carrier that are explicitly designed to be used as persistent digital physical carriers of instances of D1 Digital Object. A D13 Digital Information Carrier may or may not contain information, e.g., an empty diskette.

Examples:
-</rdfs:comment>
    </owl:Class>
    


    <!-- http://www.cidoc-crm.org/extensions/crmdig/versions/4.0/D14_Software#D14_Software -->


    <owl:Class rdf:about="http://www.cidoc-crm.org/extensions/crmdig/versions/4.0/D14_Software#D14_Software">
        <rdfs:subClassOf rdf:resource="http://www.cidoc-crm.org/extensions/crmdig/versions/4.0/D1_Digital_Object#D1_Digital_Object"/>
        <rdfs:comment>URI: http://www.cidoc-crm.org/extensions/crmdig/versions/4.0/D14_Software

SubClass Of:
D1 Digital Object
SuperClass Of:
-
Scope Note:
This class comprises software codes, computer programs, procedures and functions that are used to operate a system of digital objects.

Examples:
-</rdfs:comment>
    </owl:Class>
    


    <!-- http://www.cidoc-crm.org/extensions/crmdig/versions/4.0/D1_Digital_Object#D1_Digital_Object -->


    <owl:Class rdf:about="http://www.cidoc-crm.org/extensions/crmdig/versions/4.0/D1_Digital_Object#D1_Digital_Object">
        <rdfs:subClassOf rdf:resource="http://cidoc-crm.org/cidoc-crm/7.1.3/E73_Information_Object#E73_Information_Object"/>
        <rdfs:comment>URI: http://www.cidoc-crm.org/extensions/crmdig/versions/4.0/D1_Digital_Object

SubClass Of:
E73 Information Object
SuperClass Of:
D9 Data Object
D14 Software
D35 Area
Scope Note:
This class comprises identifiable immaterial items that can be represented as sets of bit sequences, such as data sets, e-texts, images, audio or video items, software, etc., and are documented as single units.

Any aggregation of instances of D1 Digital Object into a whole treated as single unit is also regarded as an instance of D1 Digital Object.

This means that for instance, the content of a DVD, an XML file on it, and an element of this file, are regarded as distinct instances of D1 Digital Object, mutually related by the P106 is composed of (forms part of) property.

A D1 Digital Object does not depend on a specific physical carrier, and it can exist on one or more carriers simultaneously.</rdfs:comment>
    </owl:Class>
    


    <!-- http://www.cidoc-crm.org/extensions/crmdig/versions/4.0/D2_Digitization_Process#D2_Digitization_Process -->


    <owl:Class rdf:about="http://www.cidoc-crm.org/extensions/crmdig/versions/4.0/D2_Digitization_Process#D2_Digitization_Process">
        <rdfs:subClassOf rdf:resource="http://www.cidoc-crm.org/extensions/crmdig/versions/4.0/D11_Digital_Measurement_Event#D11_Digital_Measurement_Event"/>
        <rdfs:comment>URI: http://www.cidoc-crm.org/extensions/crmdig/versions/4.0/D2_Digitization_Process

SubClass Of:
D11 Digital Measurement Event
SuperClass Of:
-
Scope Note:
This class comprises events that result in the creation of instances of D9 Data Object that represent the appearance and/or form of an instance of E18 Physical Thing such as paper documents, statues, buildings, paintings, etc.

A particular case is the analogue-to-digital conversion of audiovisual material.

This class represents the transition from a material thing to an immaterial representation of it.

The characteristic subsequent processing steps on digital objects are regarded as instances of D3 Formal Derivation.

Examples:
-</rdfs:comment>
    </owl:Class>
    


    <!-- http://www.cidoc-crm.org/extensions/crmdig/versions/4.0/D7_Digital_Machine_Event#D7_Digital_Machine_Event -->


    <owl:Class rdf:about="http://www.cidoc-crm.org/extensions/crmdig/versions/4.0/D7_Digital_Machine_Event#D7_Digital_Machine_Event">
        <rdfs:subClassOf rdf:resource="http://cidoc-crm.org/cidoc-crm/7.1.3/E11_Modification#E11_Modification"/>
        <rdfs:subClassOf rdf:resource="http://cidoc-crm.org/cidoc-crm/7.1.3/E65_Creation#E65_Creation"/>
        <rdfs:comment>URI: http://www.cidoc-crm.org/extensions/crmdig/versions/4.0/D7_Digital_Machine_Event

SubClass Of:
E11 Modification
E65 Creation
SuperClass Of:
D10 Software Execution
D11 Digital Measurement Event
D12 Data Transfer Event
Scope Note:
This class comprises events that happen on physical digital devices following a human activity that intentionally caused its immediate or delayed initiation and results in the creation of a new instance of D1 Digital Object on behalf of the human actor.

The input of a D7 Digital Machine Event may be parameter settings and/or data to be processed. Some D7 Digital Machine Events may form part of a wider E65 Creation event. In this case, all machine output of the partial events is regarded as creation of the overall activity.

Examples:
-</rdfs:comment>
    </owl:Class>
    


    <!-- http://www.cidoc-crm.org/extensions/crmdig/versions/4.0/D8_Digital_Device#D8_Digital_Device -->


    <owl:Class rdf:about="http://www.cidoc-crm.org/extensions/crmdig/versions/4.0/D8_Digital_Device#D8_Digital_Device">
        <rdfs:subClassOf rdf:resource="http://cidoc-crm.org/cidoc-crm/7.1.3/E22_Human-Made_Object#E22_Human-Made_Object"/>
        <rdfs:comment>SubClass Of:
E22 Human-Made Object
SuperClass Of:
-
Scope Note:
This class comprises identifiable material items such as computers, scanners, cameras, etc. that have the capability to process or produce instances of D1 Digital Object.

Examples:
-</rdfs:comment>
    </owl:Class>
    


    <!-- http://www.cidoc-crm.org/extensions/crmdig/versions/4.0/D9_Data_Object#D9_Data_Object -->


    <owl:Class rdf:about="http://www.cidoc-crm.org/extensions/crmdig/versions/4.0/D9_Data_Object#D9_Data_Object">
        <rdfs:subClassOf rdf:resource="http://www.cidoc-crm.org/extensions/crmdig/versions/4.0/D1_Digital_Object#D1_Digital_Object"/>
        <rdfs:comment>URI: http://www.cidoc-crm.org/extensions/crmdig/versions/4.0/D9_Data_Object

SubClass Of:
D1 Digital Object
E54 Dimension
SuperClass Of:
-
Scope Note:
This class comprises instances of D1 Digital Object that are the direct result of a digital measurement or a formal derivative of it, containing quantitative properties of some physical things or other constellations of matter.

Examples:
-</rdfs:comment>
    </owl:Class>
    


    <!-- http://www.cidoc-crm.org/extensions/crmsci/versions/2.0/S10_Material_Substantial#S10_Material_Substantial -->


    <owl:Class rdf:about="http://www.cidoc-crm.org/extensions/crmsci/versions/2.0/S10_Material_Substantial#S10_Material_Substantial">
        <rdfs:subClassOf rdf:resource="http://cidoc-crm.org/cidoc-crm/7.1.3/E70_Thing#E70_Thing"/>
        <rdfs:subClassOf rdf:resource="http://www.cidoc-crm.org/extensions/crmsci/versions/2.0/S15_Observable_Entity#S15_Observable_Entity"/>
        <rdfs:comment>URI:	http://www.cidoc-crm.org/extensions/crmsci/S10_Material_Substantial
SubClass Of:
E70 Thing
S15 Observable Entity
SuperClass Of:
S14 Fluid Body
S11 Amount of Matter
E18 Physical Thing
Scope Note:
This class comprises constellations of matter with a relative stability of any form sufficient to associate them with a persistent identity, such as being confined to certain extent, having a relative stability of form or structure, or containing a fixed amount of matter. In particular, it comprises physical things in the narrower sense and fluid bodies. It is an abstraction of physical substance for solid and non-solid things of matter.

Examples:
the groundwater of the 5-22 basin of Central Macedonia (S10) (Lucchese et al., 2013; Kritikos et al., 2013; InGeoCloudS, 2012; InGeoCloudS, 2013)
the Mesozoic carbonate sequence with flysch extracted from the area of Nafplion that was mapped and studied by Tattaris in 1970 (S10) (Photiades, 2010)
Parnassos, the limestone mountain (Strid, 1986)</rdfs:comment>
    </owl:Class>
    


    <!-- http://www.cidoc-crm.org/extensions/crmsci/versions/2.0/S15_Observable_Entity#S15_Observable_Entity -->


    <owl:Class rdf:about="http://www.cidoc-crm.org/extensions/crmsci/versions/2.0/S15_Observable_Entity#S15_Observable_Entity">
        <rdfs:subClassOf rdf:resource="http://www.cidoc-crm.org/cidoc-crm/E1_CRM_Entity#E1_CRM_Entity"/>
        <rdfs:comment>URI:	http://www.cidoc-crm.org/extensions/crmsci/S15_Observable_Entity
SubClass Of:
E1 CRM Entity
SuperClass Of:
E5 Event
S10 Material Substantial
Scope Note:
This class comprises instances of E5 Event or S10 Material Substantial (i.e. items or phenomena, such as physical things, their behaviour, states and interactions or events), that can be observed by measurement or detection devices or by human sensory impression including when enhanced by tools.

In order to be observable, instances of E5 Event must consist of some interaction or action of material substance. In some cases, the spatiotemporal confinement of the event itself, such as a flash, a car stopping etc. marks the limits of a documented observation of an event. In other cases, such as the situation of a car passing by a certain object, the spatiotemporal limits of the event of observing itself, as well as the direction of attention or the orientation of used instruments, may constrain the observed detail of a larger process, e.g., noticing the sight of a car passing by; a light emission, etc.

Conceptual objects manifest through their carriers such as books, digital media, or even human memory. Attributes of conceptual objects, such as number of words, can be observed on their carriers. If the respective properties between carriers differ, either they carry different instances of conceptual objects or the difference can be attributed to accidental deficiencies in one of the carriers. In that sense even immaterial objects are observable. By this model we address the fact that frequently, the actually observed carriers of conceptual objects are not explicitly identified in documentation, i.e., they are assumed to have existed but they are unknown as individuals.

Examples:
the domestic goose from Guangdong/1/1996 (H5N1) that was identified in 1996 in farmed geese in southern China as circulating highly pathogenic H5N1 (E20) (Wan, 2012)
the flight of a male Bearded Vulture observed near Loukia, Heraklion, Crete in the morning of the 24th of October 2020 (E5) [The Bearded Vulture (Gypaetus Barbatus) is a threatened species in Crete] (Claes, 2020)
the eruption of Krakatoa volcano at Indonesia in 1883 (E5) (Symons et al., 1888)
the cupid head area in the X-Ray of the painting ‘Cupid complaining to Venus’ (E25) (The National Gallery, London, 1963)</rdfs:comment>
    </owl:Class>
    


    <!-- http://www.cidoc-crm.org/extensions/crmsci/versions/2.0/S21_Measurement#S21_Measurement -->


    <owl:Class rdf:about="http://www.cidoc-crm.org/extensions/crmsci/versions/2.0/S21_Measurement#S21_Measurement">
        <rdfs:subClassOf rdf:resource="http://www.cidoc-crm.org/extensions/crmsci/versions/2.0/S4_Observation#S4_Observation"/>
        <rdfs:comment>URI:	http://www.cidoc-crm.org/extensions/crmsci/S21_Measurement
SubClass Of:
S4 Observation
SuperClass Of:
S3 Measurement by Sampling
E16 Measurement
Scope Note:
This class comprises actions measuring instances of S15 Observable Entity, properties of physical things, or phenomena, states and interactions or events, that can be determined by a systematic procedure. Primary data from measurement devices are regarded to be results of an observation process.

Examples:
the magnitude measurement of the earthquake of Mexico city in 2017. (S21) [It had the magnitude 6.2 Richter] (Mindock, 2017)
the sensor measurement by IGME in 1999 which measured the landslide displacement in the area of Parnitha, Greece. (S21) (Lucchese et al., 2013; Kritikos et al., 2013; InGeoCloudS, 2012; InGeoCloudS, 2013)</rdfs:comment>
    </owl:Class>
    


    <!-- http://www.cidoc-crm.org/extensions/crmsci/versions/2.0/S4_Observation#S4_Observation -->


    <owl:Class rdf:about="http://www.cidoc-crm.org/extensions/crmsci/versions/2.0/S4_Observation#S4_Observation">
        <owl:equivalentClass rdf:resource="http://www.opengis.net/ont/geosparql#Feature"/>
        <rdfs:subClassOf rdf:resource="http://cidoc-crm.org/cidoc-crm/7.1.3/E13_Attribute_Assignment#E13_Attribute_Assignment"/>
        <rdfs:comment>URI:	http://www.cidoc-crm.org/extensions/crmsci/S4_Observation
SubClass Of:
E13 Attribute Assignment
SuperClass Of:
S21 Measurement
S19 Encounter Event
S23 Position Determination
Scope Note:
This class comprises the activity of gaining scientific knowledge about particular states of physical reality through empirical evidence, experiments and measurements.

We define observation in the sense of natural sciences, as a kind of human activity: at some place and within some time-span, certain physical things and their behavior and interactions are observed by human sensory impression, and often enhanced by tools and measurement devices.

Observed situations or dimensions may pertain to properties confined to a single instance of S15 Observable Entity or pertain to constellations of multiple instances and relations between them, in particular distances between them.

The output of the internal processes of measurement devices that do not require additional human interaction are in general regarded as part of the observation and not as additional inference. Primary data from measurement devices are regarded in this model to be results of observation and can be interpreted as propositions believed to be true within the (known) tolerances and degree of reliability of the device.

Measurements and witnessing of events are special cases of observations. Observations result in a belief that certain propositions held at a time within the time-span of the observation. In this model, the degree of confidence in the observed properties is regarded to be &apos;true&apos; by default, but could be described differently by adding a property P3 has note to an instance of S4 Observation

Examples:
the excavation of unit XI by the Archaeological Institute of Crete in 2004 (S4)
the excavation (S4) in the NE section of the central court of the Knossos palace by the Ephorate of Antiquities of Heraklion in 1997 (S4) (Επιστημονική Επιτροπή Κνωσού, 2008)
the observation of the density of the X-Ray image of cupid&apos;s head from the painting ‘Cupid complaining to Venus’ as ‘high density’, on the 19th of March 1963 (S4) (The National Gallery, London, 1963).
the observation of visible light absorption of the painting ‘Cupid complaining to Venus’ as ‘having red pigment’, in 2015 (S4) (Foister, 2015)</rdfs:comment>
    </owl:Class>
    


    <!-- http://www.opengis.net/ont/geosparql#Coverage -->


    <owl:Class rdf:about="http://www.opengis.net/ont/geosparql#Coverage">
        <owl:equivalentClass rdf:resource="https://photogrammetry.altervista.org/items/show/158#F71_Final_Use_of_Digital_Twin"/>
    </owl:Class>
    


    <!-- http://www.opengis.net/ont/geosparql#Feature -->


    <owl:Class rdf:about="http://www.opengis.net/ont/geosparql#Feature"/>
    


    <!-- http://www.opengis.net/ont/geosparql#Geometry -->


    <owl:Class rdf:about="http://www.opengis.net/ont/geosparql#Geometry">
        <owl:equivalentClass rdf:resource="https://photogrammetry.altervista.org/items/show/104#F18_Dominant_Geometry_Type"/>
    </owl:Class>
    


    <!-- http://www.semanticweb.org/vitto/ontologies/2024/9/PODS_1#E12_Production -->


    <owl:Class rdf:about="http://www.semanticweb.org/vitto/ontologies/2024/9/PODS_1#E12_Production">
        <rdfs:subClassOf rdf:resource="http://cidoc-crm.org/cidoc-crm/7.1.3/E11_Modification#E11_Modification"/>
        <rdfs:comment>URI:	http://www.cidoc-crm.org/cidoc-crm/E12_Production
SubClass Of:
E11 Modification
E63 Beginning of Existence
SuperClass Of:
-
Scope Note:
This class comprises activities that are designed to, and succeed in, creating one or more new items.

It specializes the notion of modification into production. The decision as to whether or not an object is regarded as new is context sensitive. Normally, items are considered &apos;new&apos; if there is no obvious overall similarity between them and the consumed items and material used in their production. In other cases, an item is considered &apos;new&apos; because it becomes relevant to documentation by a modification. For example, the scribbling of a name on a potsherd may make it a voting token. The original potsherd may not be worth documenting, in contrast to the inscribed one.

This entity can be collective: the printing of a thousand books, for example, would normally be considered a single event.

An event should also be documented using an instance of E81 Transformation if it results in the destruction of one or more objects and the simultaneous production of others using parts or material from the originals. In this case, the new items have separate identities and matter is preserved, but identity is not.

Examples:
the construction of the SS Great Britain (Gregor, 1971)
the first casting of the Little Mermaid from the harbour of Copenhagen (Dewey, 2003)
Rembrandt’s creating of the seventh state of his etching &apos;Woman sitting half dressed beside a stove&apos;, 1658, identified by Bartsch Number 197 (E12, E65, E81) (Hind, 1923)</rdfs:comment>
    </owl:Class>
    


    <!-- http://www.semanticweb.org/vitto/ontologies/2024/9/PODS_1Protocol_of_Ontological_Digital_Survey/extensions/versions/1_1/F12_Acquisition_Trajectory#F12_Acquisition_Trajectory -->


    <owl:Class rdf:about="http://www.semanticweb.org/vitto/ontologies/2024/9/PODS_1Protocol_of_Ontological_Digital_Survey/extensions/versions/1_1/F12_Acquisition_Trajectory#F12_Acquisition_Trajectory">
        <rdfs:subClassOf rdf:resource="http://cidoc-crm.org/cidoc-crm/7.1.3/E29_Design_or_Procedure#E29_Design_or_Procedure"/>
        <rdfs:label xml:lang="en">AcquisitionPath</rdfs:label>
        <skos:definition xml:lang="en">Definition of the class F12 Acquisition Trajectory as a subclass of E29 Design and Procedure</skos:definition>
        <skos:example xml:lang="en">&quot;A modular scanning setup, where a laser scanner is placed at different strategic positions around an architectural site to capture comprehensive point cloud data.&quot; .</skos:example>
        <skos:example xml:lang="en">&quot;A spiral trajectory executed by a camera as it moves around an archaeological artifact for a photogrammetric survey.&quot; ;</skos:example>
        <skos:scopeNote xml:lang="en">&quot;The Acquisition Trajectory class refers to the physical path or series of positions followed by an acquisition device (such as a camera or laser scanner) during the data acquisition phase of photogrammetric or other survey processes. This trajectory defines the movement or stationary positions of the device relative to the object or area being documented, affecting the quality, coverage, and accuracy of the data captured. The Acquisition Trajectory can include linear paths, spirals, concentric movements, or modular setups in the case of a laser scanner, depending on the methodology adopted. Accurate documentation of the trajectory is essential for ensuring comprehensive and consistent capture of an object’s geometry, which is vital for subsequent processing and modeling phases.&quot; ;</skos:scopeNote>
    </owl:Class>
    


    <!-- http://www.semanticweb.org/vitto/ontologies/2024/9/PODS_1Protocol_of_Ontological_Digital_Survey/extensions/versions/1_1/F47_Densification#F47__Densification -->


    <owl:Class rdf:about="http://www.semanticweb.org/vitto/ontologies/2024/9/PODS_1Protocol_of_Ontological_Digital_Survey/extensions/versions/1_1/F47_Densification#F47__Densification">
        <rdfs:subClassOf rdf:resource="http://cidoc-crm.org/cidoc-crm/7.1.3/E71_Human-Made_Thing#E71_Human-Made_Thing"/>
        <skos:definition xml:lang="en">Definition of the class F47 Densification as a subclass of F3 Processing</skos:definition>
        <skos:example xml:lang="en">&quot;The densification of a LiDAR point cloud to enhance the resolution and clarity of a 3D terrain model.&quot;</skos:example>
        <skos:example xml:lang="en">Example:
&quot;The application of dense matching techniques to generate a more detailed point cloud in architectural surveys.&quot;</skos:example>
        <skos:example xml:lang="en">Example:
&quot;The densification of a photogrammetric point cloud by increasing the number of points using stereo-matching algorithms.&quot;</skos:example>
        <skos:scopeNote xml:lang="en">Scope Note:
The Densification class refers to the process of enriching the initial sparse point cloud obtained from the Matching phase by adding more data points. This step employs algorithms that interpolate or calculate additional points to create a more detailed and dense representation of the object or scene being scanned. Densification is crucial for achieving higher accuracy and detail in 3D reconstruction processes such as meshing.</skos:scopeNote>
    </owl:Class>
    


    <!-- http://www.semanticweb.org/vitto/ontologies/2024/9/PODS_1Protocol_of_Ontological_Digital_Survey/extensions/versions/1_1/F54_Point_Cloud_Vertex_Quality#F54_Point_Cloud_Vertex_Quality -->


    <owl:Class rdf:about="http://www.semanticweb.org/vitto/ontologies/2024/9/PODS_1Protocol_of_Ontological_Digital_Survey/extensions/versions/1_1/F54_Point_Cloud_Vertex_Quality#F54_Point_Cloud_Vertex_Quality">
        <rdfs:subClassOf rdf:resource="http://cidoc-crm.org/cidoc-crm/7.1.3/E13_Attribute_Assignment#E13_Attribute_Assignment"/>
        <rdfs:label xml:lang="en">ProcessingAttributeVertexQuality</rdfs:label>
        <skos:definition xml:lang="en">Definition of the class F54 Point Cloud Vertex Quality as a subclass of E13 Attribute Assignment</skos:definition>
        <skos:scopeNote xml:lang="en">The Point Cloud Vertex Quality class refers to the assignment of quality attributes to individual vertices (points) in a point cloud (F26 Point Cloud). This class records metrics such as positional accuracy, intensity, color information, or other quality-related characteristics that indicate the reliability and precision of the individual vertices in the point cloud dataset.</skos:scopeNote>
    </owl:Class>
    


    <!-- http://www.w3.org/ns/prov#Activity -->


    <owl:Class rdf:about="http://www.w3.org/ns/prov#Activity">
        <rdfs:label xml:lang="en">MAINZED_3D_METADATA_ONTOLOGY: Activity</rdfs:label>
    </owl:Class>
    


    <!-- http://www.w3.org/ns/prov#Entity -->


    <owl:Class rdf:about="http://www.w3.org/ns/prov#Entity">
        <rdfs:label xml:lang="en">MAINZED_3D_METADATA_ONTOLOGY: Entity</rdfs:label>
    </owl:Class>
    


    <!-- http://xmlns.com/foaf/0.1/Person -->


    <owl:Class rdf:about="http://xmlns.com/foaf/0.1/Person"/>
    


    <!-- https://photogrammetry.altervista.org/admin/items/show/87#F1_Survey_Object -->


    <owl:Class rdf:about="https://photogrammetry.altervista.org/admin/items/show/87#F1_Survey_Object">
        <rdfs:subClassOf rdf:resource="http://www.cidoc-crm.org/extensions/crmsci/versions/2.0/S10_Material_Substantial#S10_Material_Substantial"/>
        <rdfs:label xml:lang="en">SurveyObject</rdfs:label>
        <skos:definition xml:lang="en">Defining the class F1 Survey Object as a subclass of S10 Material Substantial</skos:definition>
        <skos:example xml:lang="en">&quot;A castle surveyed with photogrammetric technique (Artopoulos 2015)&quot; ;</skos:example>
        <skos:example xml:lang="en">&quot;A fresco in a medieval chapel (D. Abate 2016)&quot; ;</skos:example>
        <skos:example xml:lang="en">&quot;A wild boar jaw AFMNM005 detected with photogrammetric technique at the laboratory of the archaeological museum of Okayama (Japan) coming from the Minamikata excavation in the context of the BeArchaeo project (Lauro, 2019)&quot; ;</skos:example>
        <skos:scopeNote xml:lang="en">&quot;Survey Object denotes any object subjected to photogrammetric surveying or any kind of digital surveying. It represents the target of data acquisition processes, crucial for generating detailed digital records, analyses, and reconstructions within the FOPPA model for archaeological documentation. It must be a solid and visible object. The expression visible means that it interacts with light.&quot; ;</skos:scopeNote>
    </owl:Class>
    


    <!-- https://photogrammetry.altervista.org/admin/items/show/88#F2_Acquisition -->


    <owl:Class rdf:about="https://photogrammetry.altervista.org/admin/items/show/88#F2_Acquisition">
        <rdfs:subClassOf rdf:resource="http://www.cidoc-crm.org/extensions/crmdig/versions/4.0/D2_Digitization_Process#D2_Digitization_Process"/>
        <rdfs:label xml:lang="en">Acquisition</rdfs:label>
        <skos:definition xml:lang="en">Definition of the class F2 Acquisition as a subclass of D2 Digitization Process</skos:definition>
        <skos:example xml:lang="en">&quot;The photogrammetric survey of a contemporary art sculpture (Ucakar 2022).&quot; ;</skos:example>
        <skos:example xml:lang="en">&quot;The photogrammetric survey of the walls of Cortona (Lauro 2023).&quot; ;</skos:example>
        <skos:example xml:lang="en">&quot;The survey of the facade of Bedzin Castle using laser scanning and photogrammetry (Klapa 2017).&quot; ;</skos:example>
        <skos:scopeNote xml:lang="en">&quot;Acquisition refers to the process of capturing detailed photographic data of an object or structure. This involves systematically taking overlapping photographs from various angles to create a comprehensive and accurate 3D model, crucial for archaeological documentation and analysis.&quot; ;</skos:scopeNote>
    </owl:Class>
    


    <!-- https://photogrammetry.altervista.org/items/show/100#F14_Matching_Method -->


    <owl:Class rdf:about="https://photogrammetry.altervista.org/items/show/100#F14_Matching_Method">
        <rdfs:subClassOf rdf:resource="http://cidoc-crm.org/cidoc-crm/7.1.3/E29_Design_or_Procedure#E29_Design_or_Procedure"/>
        <rdfs:label xml:lang="en">Processing_MatchingMethod</rdfs:label>
        <skos:definition xml:lang="en">Definition of the class F13 Acquisition Method as a subclass of E29 Design and Procedure</skos:definition>
        <skos:example xml:lang="en">&quot;The FOPPA protocol for archaeological photogrammetry, which prescribes specific camera settings and trajectories for artifact documentation.&quot; ;</skos:example>
        <skos:example xml:lang="en">&quot;The McGlone Method, which provides a standardized set of steps for capturing imagery in aerial photogrammetry surveys.&quot; .</skos:example>
        <skos:scopeNote xml:lang="en">&quot;The Acquisition Method class refers to the set of protocols, guidelines, or operational instructions that dictate how the acquisition process is conducted during a photogrammetric or other survey operation. This class captures the methodology adopted for data capture, specifying procedural elements such as device settings, trajectory planning, object coverage, and environmental considerations. The Acquisition Method can range from formalized protocols, such as the Metashape Manual or the McGlone Method, to custom or ad-hoc procedures defined for specific projects or objects. The choice of method impacts the completeness and quality of the raw data produced, influencing all subsequent phases of processing and modeling.&quot; ;
  skos:broader cidoc:E29_Design_and_Procedure .</skos:scopeNote>
    </owl:Class>
    


    <!-- https://photogrammetry.altervista.org/items/show/101#F15_Recontruction_Method -->


    <owl:Class rdf:about="https://photogrammetry.altervista.org/items/show/101#F15_Recontruction_Method">
        <rdfs:subClassOf rdf:resource="http://cidoc-crm.org/cidoc-crm/7.1.3/E29_Design_or_Procedure#E29_Design_or_Procedure"/>
        <rdfs:label xml:lang="en">Modelling_ReconstructionMethod</rdfs:label>
        <skos:definition xml:lang="en">F15 Reconstruction Method 
 &quot;The Reconstruction Method encompasses the techniques and processes that convert point cloud data into a usable 3D mesh, facilitating further analysis and visualization.&quot; .</skos:definition>
        <skos:example xml:lang="en">&quot;Applying the Poisson Surface Reconstruction algorithm in Metashape to create a high-fidelity mesh from a dense point cloud.&quot;</skos:example>
        <skos:scopeNote xml:lang="en">&quot;The Reconstruction Method class refers to the procedures and algorithms used to transform a densified point cloud into a polygonal mesh, thereby creating a structured 3D representation of an object or scene. This process involves generating polygons, typically triangles or quads, that form the mesh surface based on the spatial data from the point cloud. The Reconstruction Method also includes steps like mesh optimization, hole filling, and refinement to improve accuracy and ensure the continuity of the 3D surface. Different software solutions and algorithms such as Poisson Surface Reconstruction, Delaunay Triangulation, or Ball-Pivoting Algorithm are examples of methods employed during this phase.&quot; ;</skos:scopeNote>
    </owl:Class>
    


    <!-- https://photogrammetry.altervista.org/items/show/102#F16_Texturing_Method -->


    <owl:Class rdf:about="https://photogrammetry.altervista.org/items/show/102#F16_Texturing_Method">
        <rdfs:subClassOf rdf:resource="http://cidoc-crm.org/cidoc-crm/7.1.3/E29_Design_or_Procedure#E29_Design_or_Procedure"/>
        <rdfs:label xml:lang="en">Modelling_TexturingMethod</rdfs:label>
        <skos:definition xml:lang="en">Definition of the class F16 Texturing Method as a subclass of E29 Design and Procedure</skos:definition>
        <skos:example xml:lang="en">&quot;Applying the UV Mapping technique in Blender to unwrap a mesh and create texture coordinates for an optimized 3D model.&quot; .</skos:example>
        <skos:example xml:lang="en">&quot;Using Metashape&apos;s Blended Mapping algorithm to generate a unified texture from multiple photographs.&quot;</skos:example>
        <skos:scopeNote xml:lang="en">&quot;The Texturing Method class refers to the procedures and algorithms used to map color information onto a 3D mesh, creating a realistic representation by applying textures that enhance the visual fidelity of the model. This process involves associating 2D images (or texture maps) with the 3D geometry of the mesh, either by projecting photographs directly onto the surface or by generating UV maps that accurately correspond to the model’s topology. The Texturing Method ensures that each polygon in the mesh receives appropriate color information from the photographic data, and may also involve steps like blending multiple images to eliminate seams or inconsistencies. Textures can either be embedded in the model file or stored externally, depending on the file format and desired use of the model.&quot; ;</skos:scopeNote>
    </owl:Class>
    


    <!-- https://photogrammetry.altervista.org/items/show/103#F17_Acquisition_Trajectory_Type -->


    <owl:Class rdf:about="https://photogrammetry.altervista.org/items/show/103#F17_Acquisition_Trajectory_Type">
        <rdfs:subClassOf rdf:resource="http://cidoc-crm.org/cidoc-crm/7.1.3/E55_Type#E55_Type"/>
        <rdfs:label xml:lang="en">AcquisitionPath/TrajectoryTypology</rdfs:label>
        <skos:definition xml:lang="en">Definition of the class F17 Acquisition Trajectory Type as a subclass of E55 Type</skos:definition>
        <skos:example xml:lang="en">&quot;Linear Trajectory: Straightforward movement along a defined line to ensure consistent coverage of the object.&quot; ;</skos:example>
        <skos:example xml:lang="en">&quot;Vertical Scan: Upward or downward movements intended to gather data from different height levels of the subject.&quot; .</skos:example>
        <skos:scopeNote xml:lang="en">&quot;The Acquisition Trajectory Type class encompasses the various classifications of movement patterns executed by the acquisition device during the data collection process. These types are essential for understanding the methodology of data capture and are critical for accurately interpreting the resulting raw data. Different trajectory types can include linear movements, spiral paths, vertical scans, and other systematic approaches tailored to the specific context of the survey. Each trajectory type informs the photogrammetric workflow by dictating how the acquisition device interacts with the subject, which ultimately affects the quality and detail of the captured data.&quot; ;</skos:scopeNote>
    </owl:Class>
    


    <!-- https://photogrammetry.altervista.org/items/show/104#F18_Dominant_Geometry_Type -->


    <owl:Class rdf:about="https://photogrammetry.altervista.org/items/show/104#F18_Dominant_Geometry_Type">
        <rdfs:subClassOf rdf:resource="http://cidoc-crm.org/cidoc-crm/7.1.3/E55_Type#E55_Type"/>
        <rdfs:label xml:lang="en">AcquisitionGeometryTypology</rdfs:label>
        <skos:definition xml:lang="en">Definition of the class F18 Dominant Geometry Type as a subclass of E55 Type
:F18_Dominant_Geometry_Type rdf:type skos:Concept ;</skos:definition>
        <skos:example xml:lang="en">&quot;Cylinder: A bottle, defined by its elongated form.&quot; ;</skos:example>
        <skos:example xml:lang="en">&quot;Parallelepiped: A book, reduced to its rectangular prism shape.&quot;</skos:example>
        <skos:example xml:lang="en">&quot;Sphere: A basketball, characterized by its round shape.&quot; ;</skos:example>
        <skos:scopeNote xml:lang="en">&quot;The Dominant Geometry Type class refers to the primary geometric form of the surveyed object, conceptualized as the essential shape to which the object can be reduced. This classification aligns with specific reference thesauri, such as the FOPPA Geometry Thesaurus, which delineates these forms based on the principle that the dominant geometry is determined by the conjunction of the opposite vertices of the object, considering an approximation that does not exceed a 45-degree inclination of the faces.&quot; ;</skos:scopeNote>
    </owl:Class>
    


    <!-- https://photogrammetry.altervista.org/items/show/105#F19_Scale_Type -->


    <owl:Class rdf:about="https://photogrammetry.altervista.org/items/show/105#F19_Scale_Type">
        <rdfs:subClassOf rdf:resource="http://cidoc-crm.org/cidoc-crm/7.1.3/E55_Type#E55_Type"/>
        <rdfs:label xml:lang="en">AcquisitionScaleObjectType</rdfs:label>
        <skos:definition xml:lang="en">Definition of the class F19 Scale Type as a subclass of E55 Type</skos:definition>
        <skos:example xml:lang="en">&quot;Bend (COSCHKR).&quot; ;</skos:example>
        <skos:example xml:lang="en">&quot;Corner (COSCHKR).&quot; ;</skos:example>
        <skos:example xml:lang="en">&quot;Joint (COSCHKR).&quot; .</skos:example>
        <skos:example xml:lang="en">&quot;Medium Object: Ranging from 1 cm to 30 cm (FOPPA).&quot; ;</skos:example>
        <skos:example xml:lang="en">&quot;Open Architectural Structure: Entire buildings or significant structures (FOPPA).&quot; ;</skos:example>
        <skos:example xml:lang="en">&quot;Small Object: Equal to or smaller than 1 cm (FOPPA).&quot; ;</skos:example>
        <skos:scopeNote xml:lang="en">&quot;The Scale Type class pertains to the classification of the size of an object according to various available thesauri. This classification reflects the volume of the object and, depending on the thesaurus employed, may also relate to its functional characteristics. This class serves as a basis for understanding the object&apos;s scale in relation to its volume and, when applicable, its function according to the selected thesaurus.&quot; ;</skos:scopeNote>
    </owl:Class>
    


    <!-- https://photogrammetry.altervista.org/items/show/106#F20_Acquisition_Device_Type -->


    <owl:Class rdf:about="https://photogrammetry.altervista.org/items/show/106#F20_Acquisition_Device_Type">
        <rdfs:subClassOf rdf:resource="http://cidoc-crm.org/cidoc-crm/7.1.3/E55_Type#E55_Type"/>
        <rdfs:label xml:lang="en">AcquisitionDeviceType</rdfs:label>
        <skos:definition xml:lang="en">Definition of the class F20 Acquisition Device Type as a subclass of E55 Type</skos:definition>
        <skos:example xml:lang="en">&quot;Camera: Standard photographic equipment for capturing images.&quot; ;</skos:example>
        <skos:example xml:lang="en">&quot;Handheld Scanners: Portable devices for capturing detailed surface information.&quot; .</skos:example>
        <skos:example xml:lang="en">&quot;Laser Scanner: Device used for capturing 3D data of surfaces through laser measurements.&quot; ;</skos:example>
        <skos:example xml:lang="en">&quot;LiDAR: Technology that measures distances by illuminating a target with laser light and analyzing the reflected light.&quot;</skos:example>
        <skos:example xml:lang="en">&quot;Total Station: An optical/electronic instrument used for surveying and building construction.&quot; ;</skos:example>
        <skos:scopeNote xml:lang="en">&quot;The Acquisition Device Type class refers to the various types of acquisition instruments used in photogrammetry and surveying, such as cameras, laser scanners, and LiDAR systems. This class is essential for categorizing and managing the different instruments employed for data capture in archaeological documentation.&quot; ;
  skos:broader cidoc:E55_Type</skos:scopeNote>
    </owl:Class>
    


    <!-- https://photogrammetry.altervista.org/items/show/107#F21_Matching_Algorithm_Type -->


    <owl:Class rdf:about="https://photogrammetry.altervista.org/items/show/107#F21_Matching_Algorithm_Type">
        <rdfs:subClassOf rdf:resource="http://cidoc-crm.org/cidoc-crm/7.1.3/E55_Type#E55_Type"/>
        <rdfs:label xml:lang="en">Processing_MatchingAlgorithmType</rdfs:label>
        <skos:definition xml:lang="en">Definition of the class F21 Matching Algorithm Type as a subclass of E55 Type</skos:definition>
        <skos:example xml:lang="en">&quot;Depth Map Algorithms: Methods that generate depth information from laser scanner data.&quot; .</skos:example>
        <skos:example xml:lang="en">&quot;Feature Matching: Algorithms that identify and match distinctive features in overlapping images.&quot; ;</skos:example>
        <skos:example xml:lang="en">&quot;Stereo Matching: Techniques that derive depth information from two or more images taken from different viewpoints.&quot; ;</skos:example>
        <skos:example xml:lang="en">&quot;Structure from Motion (SfM): Algorithms that reconstruct 3D structures from a series of 2D images.&quot;</skos:example>
        <skos:scopeNote xml:lang="en">&quot;The Matching Algorithm Type class encompasses the various types of algorithms utilized for extracting the initial point cloud from images in photogrammetry or from positional information in laser scanning. This class is crucial for categorizing the different methodologies employed in point cloud generation.&quot; ;</skos:scopeNote>
    </owl:Class>
    


    <!-- https://photogrammetry.altervista.org/items/show/108#F22_Densification_Algorithm_Type -->


    <owl:Class rdf:about="https://photogrammetry.altervista.org/items/show/108#F22_Densification_Algorithm_Type">
        <rdfs:subClassOf rdf:resource="http://cidoc-crm.org/cidoc-crm/7.1.3/E55_Type#E55_Type"/>
        <rdfs:label xml:lang="en">Processing_DensificationAlgorithmType</rdfs:label>
        <skos:definition xml:lang="en">Definition of the class F22 Densification Algorithm Type as a subclass of E55 Type</skos:definition>
        <skos:example xml:lang="en">&quot;Depth Map Fusion: Algorithms that combine depth maps from multiple scans to create a denser point cloud.&quot; ;</skos:example>
        <skos:example xml:lang="en">&quot;Multi-View Densification: Methods that utilize multiple images to enhance point cloud density through additional data capture.&quot; ;</skos:example>
        <skos:example xml:lang="en">&quot;Point Cloud Densification: Algorithms that interpolate additional points between existing points to increase density.&quot; ;</skos:example>
        <skos:example xml:lang="en">&quot;Regularization Techniques: Approaches that improve point distribution and reduce noise in the densified point cloud.&quot; .</skos:example>
        <skos:scopeNote xml:lang="en">&quot;The Densification Algorithm Type class refers to the various types of algorithms used to obtain a densified point cloud from an initial point cloud. These algorithms enhance the resolution and detail of the point cloud, making it more suitable for detailed analysis and modeling.&quot; ;</skos:scopeNote>
    </owl:Class>
    


    <!-- https://photogrammetry.altervista.org/items/show/109#F23_Reconstruction_Algorithm_Type -->


    <owl:Class rdf:about="https://photogrammetry.altervista.org/items/show/109#F23_Reconstruction_Algorithm_Type">
        <rdfs:subClassOf rdf:resource="http://cidoc-crm.org/cidoc-crm/7.1.3/E55_Type#E55_Type"/>
        <rdfs:label xml:lang="en">Modelling_ReconstructionAlgorithmType</rdfs:label>
        <skos:definition xml:lang="en">Definition of the class F23 Reconstruction Algorithm Type as a subclass of E55 Type</skos:definition>
        <skos:example xml:lang="en">&quot;Alpha Shapes: Approaches that create a mesh based on the shape and distribution of points, defining boundaries for the reconstructed surface.&quot; ;</skos:example>
        <skos:example xml:lang="en">&quot;Delaunay Triangulation: Algorithms that maximize the minimum angle of triangles in the mesh, ensuring quality and even distribution of mesh elements.&quot; ;</skos:example>
        <skos:example xml:lang="en">&quot;Incremental Surface Reconstruction: Techniques that progressively build the surface by adding points and connecting them as more data becomes available.&quot; .</skos:example>
        <skos:example xml:lang="en">&quot;Poisson Surface Reconstruction: A method that generates a smooth surface by solving a Poisson equation based on point cloud data.&quot; ;</skos:example>
        <skos:example xml:lang="en">&quot;Triangulation Algorithms: Techniques that connect points in the point cloud to form triangular meshes.&quot; ;</skos:example>
        <skos:scopeNote xml:lang="en">&quot;The Reconstruction Algorithm Type class refers to the various types of algorithms used to create a mesh or surface from a point cloud. These algorithms transform the discrete points into a continuous representation, facilitating the modeling and visualization of 3D objects.&quot; ;</skos:scopeNote>
    </owl:Class>
    


    <!-- https://photogrammetry.altervista.org/items/show/110#F24__Texturing_Type -->


    <owl:Class rdf:about="https://photogrammetry.altervista.org/items/show/110#F24__Texturing_Type">
        <rdfs:subClassOf rdf:resource="http://cidoc-crm.org/cidoc-crm/7.1.3/E55_Type#E55_Type"/>
        <rdfs:label xml:lang="en">Modelling_TexturingType</rdfs:label>
        <skos:definition xml:lang="en">Definition of the class F24 Texturing Type as a subclass of E55 Type</skos:definition>
        <skos:example xml:lang="en">Bump Mapping: An algorithm that simulates surface detail by altering the lighting of a model without changing its geometry, giving the illusion of depth.&quot; ;</skos:example>
        <skos:example xml:lang="en">Normal Mapping: Similar to bump mapping, this technique uses a normal map to create detailed surface features by modifying the surface normals of the geometry.&quot; ;</skos:example>
        <skos:example xml:lang="en">Procedural Texturing: Methods that generate textures algorithmically rather than using bitmap images, allowing for dynamic and complex surface appearances.&quot; ;</skos:example>
        <skos:scopeNote xml:lang="en">&quot;The Texturing Type class refers to the various techniques, algorithms, or methods used to create textures for 3D models. These processes enhance the visual detail of models by applying color, patterns, and surface characteristics that mimic real-world appearances.&quot; ;</skos:scopeNote>
    </owl:Class>
    


    <!-- https://photogrammetry.altervista.org/items/show/111#F25_Acquisition_Raw_Data -->


    <owl:Class rdf:about="https://photogrammetry.altervista.org/items/show/111#F25_Acquisition_Raw_Data">
        <rdfs:subClassOf rdf:resource="http://www.cidoc-crm.org/extensions/crmdig/versions/4.0/D9_Data_Object#D9_Data_Object"/>
        <rdfs:label xml:lang="en">AcquiredRawData</rdfs:label>
        <skos:definition xml:lang="en">Definition of the class F25 Acquisition Raw Data as a subclass of D9 Data Object</skos:definition>
        <skos:example xml:lang="en">&quot;LiDAR point cloud data that has not undergone filtering or classification.&quot; ;</skos:example>
        <skos:example xml:lang="en">&quot;Raw laser scan data collected from a laser scanner without any preprocessing.&quot; ;</skos:example>
        <skos:example xml:lang="en">&quot;Unedited images captured by a camera during a photogrammetric survey.&quot; ;</skos:example>
        <skos:scopeNote xml:lang="en">&quot;The Acquisition Raw Data class refers to the unprocessed data resulting from the acquisition phase of photogrammetric surveys or laser scanning. These data serve as the foundational elements for subsequent processing steps and are essential for creating accurate 3D models. The raw data maintain original details and metadata critical for ensuring fidelity in model reconstruction.&quot; ;</skos:scopeNote>
    </owl:Class>
    


    <!-- https://photogrammetry.altervista.org/items/show/112#F26_Point_Cloud -->


    <owl:Class rdf:about="https://photogrammetry.altervista.org/items/show/112#F26_Point_Cloud">
        <rdfs:subClassOf rdf:resource="http://www.cidoc-crm.org/extensions/crmdig/versions/4.0/D9_Data_Object#D9_Data_Object"/>
        <rdfs:subClassOf rdf:resource="http://www.cidoc-crm.org/extensions/crmsci/versions/2.0/S15_Observable_Entity#S15_Observable_Entity"/>
        <rdfs:label xml:lang="en">ProcessedPointCloud</rdfs:label>
        <skos:definition xml:lang="en">Definition of the class F26 Point Cloud as a subclass of D9 Data Object</skos:definition>
        <skos:example xml:lang="en">&quot;A collection of 3D points representing the surface of an archaeological artifact as captured from raw data.&quot; ;</skos:example>
        <skos:example xml:lang="en">&quot;Initial point cloud data generated from a laser scanner before any further processing steps.&quot; ;</skos:example>
        <skos:example xml:lang="en">&quot;Sparse point data that outlines the basic shape and features of an object without refinement.&quot; ;</skos:example>
        <skos:example xml:lang="en">&quot;The set of points collected from an acquisition with a total station placed in relation in a coordinate grid.&quot; .</skos:example>
        <skos:scopeNote xml:lang="en">&quot;The Point Cloud class represents the initial output generated from the processing of raw data in photogrammetry or laser scanning. This class includes unrefined sets of data points that define the three-dimensional spatial distribution of the scanned object. The point cloud is a crucial intermediary stage prior to any densification processes, providing a preliminary representation of the object&apos;s surface geometry.&quot; ;</skos:scopeNote>
    </owl:Class>
    


    <!-- https://photogrammetry.altervista.org/items/show/113#F27_Densified_Point_Cloud -->


    <owl:Class rdf:about="https://photogrammetry.altervista.org/items/show/113#F27_Densified_Point_Cloud">
        <rdfs:subClassOf rdf:resource="http://www.cidoc-crm.org/extensions/crmdig/versions/4.0/D9_Data_Object#D9_Data_Object"/>
        <rdfs:subClassOf rdf:resource="http://www.cidoc-crm.org/extensions/crmsci/versions/2.0/S15_Observable_Entity#S15_Observable_Entity"/>
        <rdfs:label xml:lang="en">ProcessedDensifiedPointCloud</rdfs:label>
        <skos:example xml:lang="en">&quot;A point cloud obtained after applying algorithms that increase the density of points to capture finer details of an archaeological site.&quot; ;</skos:example>
        <skos:example xml:lang="en">&quot;A processed point cloud used for advanced analysis and 3D reconstruction, characterized by a higher density of points compared to the initial output.&quot; ;</skos:example>
        <skos:example xml:lang="en">&quot;Densified point data generated from a laser scanner, where additional points are added to improve spatial resolution.&quot; ;</skos:example>
        <skos:example xml:lang="en">&quot;Enhanced point cloud data created through interpolation techniques to fill gaps in the original point set.&quot; .</skos:example>
        <skos:example xml:lang="en">Definition of the class F27 Densified Point Cloud as a subclass of D9 Data Object</skos:example>
        <skos:scopeNote xml:lang="en">&quot;The Densified Point Cloud class refers to a refined set of three-dimensional data points that have undergone an additional processing stage to enhance point density. This process occurs independently from the initial matching phase and results in a more detailed representation of the object&apos;s surface geometry. Densified point clouds are crucial for improving the accuracy and quality of subsequent modeling and visualization tasks.&quot; ;</skos:scopeNote>
    </owl:Class>
    


    <!-- https://photogrammetry.altervista.org/items/show/114#F28_3D_Mesh -->


    <owl:Class rdf:about="https://photogrammetry.altervista.org/items/show/114#F28_3D_Mesh">
        <rdfs:subClassOf rdf:resource="http://www.cidoc-crm.org/extensions/crmsci/versions/2.0/S15_Observable_Entity#S15_Observable_Entity"/>
        <rdfs:subClassOf rdf:resource="https://photogrammetry.altervista.org/items/show/188#F102:_3D_Digital_Asset"/>
        <rdfs:label xml:lang="en">ProcessedMesh</rdfs:label>
        <skos:definition xml:lang="en">Definition of the class F28 3D Mesh as a subclass of D9 Data Object</skos:definition>
        <skos:example xml:lang="en">&quot;A 3D model of a building produced from point cloud data that highlights the architectural elements without color or texture as the Buddha of Bamiyan (Gruen 2004).&quot; .</skos:example>
        <skos:example xml:lang="en">&quot;A geometric representation of an archaeological artifact created from a densified point cloud, showing its contours and surface features as the AF005MNM (Lauro 2019).&quot; ;</skos:example>
        <skos:scopeNote xml:lang="en">&quot;The 3D Mesh class refers to a three-dimensional model constructed from a densified point cloud. This mesh represents the geometric structure of the object and is generated prior to any texturing processes. It includes the surface topology and spatial relationships derived solely from the point cloud data, making it essential for visualizing the basic form and structure of the scanned object before adding detailed textures.&quot; ;</skos:scopeNote>
    </owl:Class>
    


    <!-- https://photogrammetry.altervista.org/items/show/115#F29_Textured_3D_Mesh -->


    <owl:Class rdf:about="https://photogrammetry.altervista.org/items/show/115#F29_Textured_3D_Mesh">
        <rdfs:subClassOf rdf:resource="https://photogrammetry.altervista.org/items/show/188#F102:_3D_Digital_Asset"/>
        <rdfs:label xml:lang="en">ProcessedTexturedMesh</rdfs:label>
        <skos:definition xml:lang="en">Definition of the class F29 Textured 3D Mesh as a subclass of D9 Data Object</skos:definition>
        <skos:example xml:lang="en">&quot;A detailed representation of a historical artifact, showing surface textures and markings based on high-resolution photographs.&quot; ;</skos:example>
        <skos:example xml:lang="en">&quot;A fully textured 3D model of an archaeological site that reflects the original colors and patterns of the materials used as for the excavation in Gobelklitepe (Polat 2020).&quot; ;</skos:example>
        <skos:example xml:lang="en">&quot;An interactive exhibition display featuring a textured model that enhances the viewer&apos;s understanding of the object&apos;s form and details as the objects displayed in project BeaVIR (Murtas 2023).&quot; .</skos:example>
        <skos:scopeNote xml:lang="en">&quot;The Textured 3D Mesh class refers to a three-dimensional model that has been enhanced with texture mapping, providing detailed surface appearances and color information. This model integrates visual details onto the geometric structure established by the 3D mesh, allowing for realistic representations of artifacts or objects. The texture is applied based on the UV mapping or other texturing techniques, creating a lifelike visual experience suitable for presentation, analysis, and interactive applications.&quot; ;</skos:scopeNote>
    </owl:Class>
    


    <!-- https://photogrammetry.altervista.org/items/show/116#F30_Acquisition_Software -->


    <owl:Class rdf:about="https://photogrammetry.altervista.org/items/show/116#F30_Acquisition_Software">
        <rdfs:subClassOf rdf:resource="http://www.cidoc-crm.org/extensions/crmdig/versions/4.0/D14_Software#D14_Software"/>
        <rdfs:label xml:lang="en">AcquisitionSoftware</rdfs:label>
        <skos:definition xml:lang="en">Definition of the class F30 Acquisition Software as a subclass of D14 Software</skos:definition>
        <skos:example xml:lang="en">&quot;An app that controls a handheld 3D scanner during the acquisition phase of a survey.&quot; ;</skos:example>
        <skos:example xml:lang="en">&quot;Dedicated acquisition software used by a laser scanner to record raw point cloud data without performing any processing steps.&quot; ;</skos:example>
        <skos:example xml:lang="en">&quot;The camera control software used during a photogrammetric survey to capture high-resolution images.&quot; ;</skos:example>
        <skos:example xml:lang="en">&quot;The onboard software of a drone camera used for capturing a series of photographs for 3D modeling purposes.&quot; .</skos:example>
        <skos:scopeNote xml:lang="en">&quot;The Acquisition Software class refers to the specific software used to perform the acquisition of raw data during a photogrammetric or laser scanning survey. In photogrammetry, it typically refers to the software controlling the camera or capturing images, while for laser scanners or other devices with integrated processing tools, it refers to software exclusively dedicated to data acquisition rather than processing. This software manages the interface between the hardware and the raw data being collected, ensuring that images, point clouds, or other data formats are accurately captured for further processing.&quot; ;</skos:scopeNote>
    </owl:Class>
    


    <!-- https://photogrammetry.altervista.org/items/show/117#F31_Processing_Software -->


    <owl:Class rdf:about="https://photogrammetry.altervista.org/items/show/117#F31_Processing_Software">
        <rdfs:subClassOf rdf:resource="http://www.cidoc-crm.org/extensions/crmdig/versions/4.0/D14_Software#D14_Software"/>
        <rdfs:label xml:lang="en">ProcessingSoftware</rdfs:label>
        <skos:definition xml:lang="en">Definition of the class F31 Processing Software as a subclass of D14 Software</skos:definition>
        <skos:example xml:lang="en">&quot;A 3D laser scanner’s companion software that converts raw scan data into a structured point cloud and performs densification.&quot; ;</skos:example>
        <skos:example xml:lang="en">&quot;LiDAR processing software that translates raw light detection and ranging data into a detailed and accurate point cloud.&quot; ;</skos:example>
        <skos:example xml:lang="en">&quot;Software that processes photogrammetric images into an initial sparse point cloud and subsequently applies densification algorithms.&quot; ;</skos:example>
        <skos:scopeNote xml:lang="en">&quot;The Processing Software class refers to software specifically used to process raw data into point clouds and densified point clouds during the 3D modeling workflow. This software transforms the data acquired during the acquisition phase (e.g., images from photogrammetry or raw point clouds from laser scanning) and applies algorithms to generate an initial point cloud, followed by densification processes to refine and enrich the dataset. Processing Software is responsible for tasks such as matching, densification, and initial 3D reconstruction steps, ultimately laying the foundation for later stages of modeling.&quot; ;</skos:scopeNote>
    </owl:Class>
    


    <!-- https://photogrammetry.altervista.org/items/show/118#F32_Modelling_Software -->


    <owl:Class rdf:about="https://photogrammetry.altervista.org/items/show/118#F32_Modelling_Software">
        <rdfs:subClassOf rdf:resource="http://www.cidoc-crm.org/extensions/crmdig/versions/4.0/D14_Software#D14_Software"/>
        <rdfs:label xml:lang="en">ModifyngMeshSoftware</rdfs:label>
        <skos:definition xml:lang="en">Definition of the class F32 Modelling Software as a subclass of D14 Software</skos:definition>
        <skos:example xml:lang="en">&quot;Programs like Blender, 3ds Max, or Maya, where operators refine models through direct interaction, optimizing them for specific use cases (e.g., rendering, simulation, or 3D printing).&quot; ;</skos:example>
        <skos:example xml:lang="en">&quot;Rhino or SketchUp used for detailed architectural model editing and enhancement.&quot; .</skos:example>
        <skos:example xml:lang="en">&quot;Software used to modify 3D meshes, adding or removing details, or reshaping the model.&quot; ;</skos:example>
        <skos:scopeNote xml:lang="en">&quot;The Modelling Software class refers to software specifically used to create, modify, and refine 3D models based on processed data, such as point clouds or meshes. Unlike processing software, which applies algorithms for point cloud generation and densification, Modelling Software allows direct manipulation of the 3D model by an operator according to the project&apos;s needs. These tasks include editing, reshaping, optimizing the geometry, adjusting scale, and ensuring the model aligns with design specifications or project requirements. The operator has a more hands-on role in this phase, making manual adjustments to the 3D model without intermediary algorithmic processes.&quot; ;</skos:scopeNote>
    </owl:Class>
    


    <!-- https://photogrammetry.altervista.org/items/show/119#F33_Acquisition_Phase -->


    <owl:Class rdf:about="https://photogrammetry.altervista.org/items/show/119#F33_Acquisition_Phase">
        <rdfs:subClassOf rdf:resource="http://cidoc-crm.org/cidoc-crm/7.1.3/E29_Design_or_Procedure#E29_Design_or_Procedure"/>
        <rdfs:subClassOf rdf:resource="https://photogrammetry.altervista.org/items/show/187#F101_Survey_Phase"/>
        <rdfs:label xml:lang="en">AcquisitionPhase</rdfs:label>
        <skos:definition xml:lang="en">Definition of the class F33 Acquisition Phase as a subclass of E29 Design and Procedure</skos:definition>
        <skos:example xml:lang="en">&quot;Laser scanner operating manuals detailing the step-by-step process for capturing modular scans of a structure as Faro Manual (FARO).&quot; ;</skos:example>
        <skos:example xml:lang="en">&quot;LiDAR survey guidelines that outline specific trajectories and scanning methods for archaeological site documentation.&quot; ;</skos:example>
        <skos:example xml:lang="en">&quot;Photogrammetry acquisition protocols that specify camera settings, shooting angles, and distances for capturing a complete set of images as FOPPA protocol (FOPPA).&quot; ;</skos:example>
        <skos:example xml:lang="en">&quot;Workflow instructions from photogrammetric or laser scanning handbooks guiding users through the acquisition process as the INCEPTION protocol (Iadanza 2019).&quot; .</skos:example>
        <skos:scopeNote xml:lang="en">&quot;The Acquisition Phase class refers to the specific set of instructions, protocols, and procedures followed during the acquisition process, as outlined in acquisition manuals or specific acquisition protocols. These guidelines ensure that the collection of raw data (such as photographs, laser scans, or LiDAR readings) follows a standardized and repeatable process, allowing for accurate data capture and the successful reconstruction of 3D models. This class captures all aspects of the acquisition stage, including the positioning of devices, environmental considerations, and calibration steps necessary for consistent data quality across different surveys.&quot; ;</skos:scopeNote>
    </owl:Class>
    


    <!-- https://photogrammetry.altervista.org/items/show/120#F34_Processing_Phase -->


    <owl:Class rdf:about="https://photogrammetry.altervista.org/items/show/120#F34_Processing_Phase">
        <rdfs:subClassOf rdf:resource="http://cidoc-crm.org/cidoc-crm/7.1.3/E29_Design_or_Procedure#E29_Design_or_Procedure"/>
        <rdfs:subClassOf rdf:resource="https://photogrammetry.altervista.org/items/show/187#F101_Survey_Phase"/>
        <rdfs:label xml:lang="en">ProcessingPhase</rdfs:label>
        <skos:definition xml:lang="en">Definition of the class F34 Processing Phase as a subclass of E29 Design and Procedure</skos:definition>
        <skos:example xml:lang="en">&quot;Guidelines for densifying a point cloud, using specific software configurations (Douglas 2017).&quot; .</skos:example>
        <skos:example xml:lang="en">&quot;Instructions for generating initial point clouds from photogrammetric images, detailing matching algorithm parameters (FOPPA).&quot; ;</skos:example>
        <skos:example xml:lang="en">&quot;Protocols for processing laser scan data, including steps for point cloud registration and noise filtering (Iadanza 2019).&quot; ;</skos:example>
        <skos:scopeNote xml:lang="en">&quot;The Processing Phase class refers to the set of instructions, protocols, and procedures related to the data processing stage, as described in acquisition manuals or specific acquisition and processing protocols. This phase includes the operations that take place after the acquisition of raw data, such as the generation of point clouds, densification, and the refinement of data through algorithms. These guidelines ensure the transformation of raw data into usable 3D models or datasets, adhering to established methods that guarantee accuracy, consistency, and reproducibility of the processed results.&quot; ;</skos:scopeNote>
    </owl:Class>
    


    <!-- https://photogrammetry.altervista.org/items/show/121#F35_Raw_Data_Carrier -->


    <owl:Class rdf:about="https://photogrammetry.altervista.org/items/show/121#F35_Raw_Data_Carrier">
        <rdfs:subClassOf rdf:resource="http://www.cidoc-crm.org/extensions/crmdig/versions/4.0/D13_Digital_Information_Carrier#D13_Digital_Information_Carrier"/>
        <rdfs:label xml:lang="en">AcquiredRawDataCarrier</rdfs:label>
        <skos:definition xml:lang="en">Definition of the class F35 Raw Data Carrier as a subclass of D13 Digital Information Carrier</skos:definition>
        <skos:example xml:lang="en">&quot;A USB flash drive with raw laser scan data from an architectural survey.&quot; ;</skos:example>
        <skos:example xml:lang="en">&quot;A cloud storage account holding raw data from a multi-sensor acquisition process.&quot; .</skos:example>
        <skos:example xml:lang="en">&quot;An SD card storing raw image data captured during a photogrammetric acquisition.&quot; ;</skos:example>
        <skos:example xml:lang="en">&quot;An external hard drive containing raw LiDAR data from a topographic survey.&quot; ;</skos:example>
        <skos:scopeNote xml:lang="en">&quot;The Raw Data Carrier class refers to the physical object that stores digital raw data resulting from an acquisition process, irrespective of the type of acquisition (e.g., photogrammetric, laser scanning, LiDAR, etc.). This class includes devices such as external hard drives, SD cards, USB drives, and any other digital storage media used to preserve and transport unprocessed raw data. The Raw Data Carrier plays a vital role in ensuring that raw data remains accessible for subsequent processing, analysis, and archiving.&quot; ;</skos:scopeNote>
    </owl:Class>
    


    <!-- https://photogrammetry.altervista.org/items/show/122#F36_Picture_Carrier -->


    <owl:Class rdf:about="https://photogrammetry.altervista.org/items/show/122#F36_Picture_Carrier">
        <rdfs:subClassOf rdf:resource="https://photogrammetry.altervista.org/items/show/121#F35_Raw_Data_Carrier"/>
        <rdfs:label xml:lang="en">AcquiredPictureCarrier</rdfs:label>
        <skos:definition xml:lang="en">Definition of the class F36 Picture Carrier as a subclass of F35 Raw Data Carrier</skos:definition>
        <skos:example xml:lang="en">&quot;An SD card storing raw image data from a photogrammetric survey.&quot; ;</skos:example>
        <skos:example xml:lang="en">&quot;An external hard drive containing processed image sets used for 3D reconstruction.&quot;</skos:example>
        <skos:example xml:lang="en">&quot;The server that hosts a cloud storage account that houses the acquired images for future reference and processing.&quot; .</skos:example>
        <skos:scopeNote xml:lang="en">&quot;The Picture Carrier class refers to the physical object that contains digital data, specifically the images captured during a photogrammetric acquisition. This class includes storage devices such as external drives, SD cards, and other digital media that store unprocessed or processed images necessary for the photogrammetric workflow. The Picture Carrier is crucial for the preservation, transportation, and access to the digital image data, ensuring that the photogrammetric survey&apos;s raw images remain available for processing and analysis.&quot; ;</skos:scopeNote>
    </owl:Class>
    


    <!-- https://photogrammetry.altervista.org/items/show/123#F37_Survey_Operator -->


    <owl:Class rdf:about="https://photogrammetry.altervista.org/items/show/123#F37_Survey_Operator">
        <rdfs:subClassOf rdf:resource="http://cidoc-crm.org/cidoc-crm/7.1.3/E39_Actor#E39_Actor"/>
        <rdfs:label xml:lang="en">AcquisitionOperator</rdfs:label>
        <skos:definition xml:lang="en">Definition of the class F37 Survey Operator as a subclass of E39 Actor</skos:definition>
        <skos:example xml:lang="en">&quot;A photogrammetrist operating a drone-mounted camera for aerial image acquisition of an archaeological site.&quot; ;</skos:example>
        <skos:example xml:lang="en">&quot;A surveyor manually collecting geospatial data using a handheld GPS device.&quot; ;</skos:example>
        <skos:example xml:lang="en">&quot;A technician using a laser scanner to capture a 3D model of a historical building.&quot; ;</skos:example>
        <skos:scopeNote xml:lang="en">&quot;The Survey Operator class refers to the individual responsible for physically performing the survey or acquisition. This person operates the acquisition devices (such as cameras, laser scanners, or LiDAR systems) during the process of data collection. The Survey Operator is in charge of executing the specific survey protocol, ensuring that the equipment functions correctly, and adhering to the instructions or guidelines outlined in the acquisition methodology. This role is crucial for the successful gathering of accurate and high-quality raw data. Where applicable, the operating subject must be indicated with their corresponding ORCID; alternatively, their direct LinkedIn link should be provided. &quot; ;</skos:scopeNote>
    </owl:Class>
    


    <!-- https://photogrammetry.altervista.org/items/show/124#F38_Processing_Operator -->


    <owl:Class rdf:about="https://photogrammetry.altervista.org/items/show/124#F38_Processing_Operator">
        <rdfs:subClassOf rdf:resource="http://cidoc-crm.org/cidoc-crm/7.1.3/E39_Actor#E39_Actor"/>
        <rdfs:label xml:lang="en">ProcessingOperator</rdfs:label>
        <skos:definition xml:lang="en">Definition of the class F38 Processing Operator as a subclass of E39 Actor</skos:definition>
        <skos:example xml:lang="en">&quot;A 3D specialist refining raw data from a LiDAR survey into a structured, usable format.&quot; ;</skos:example>
        <skos:example xml:lang="en">&quot;A technician using photogrammetric software to process raw images and generate a point cloud.&quot; ;</skos:example>
        <skos:example xml:lang="en">&quot;An archaeologist processing drone-acquired images to produce orthophotos and digital terrain models.&quot; .</skos:example>
        <skos:example xml:lang="en">&quot;An engineer running processing software on laser scan data to create a densified point cloud.&quot; ;</skos:example>
        <skos:scopeNote xml:lang="en">&quot;The Processing Operator class refers to the individual responsible for processing the raw data collected during the acquisition phase. This person uses specific software and algorithms to transform raw data, such as point clouds or images, into more refined outputs like densified point clouds or 3D models. The Processing Operator has to be skilled in utilizing various processing tools to ensure the data is cleaned, aligned, and prepared for subsequent modeling and analysis stages. Where applicable, the operating subject must be indicated with their corresponding ORCID; alternatively, their direct LinkedIn link should be provided.&quot; ;</skos:scopeNote>
    </owl:Class>
    


    <!-- https://photogrammetry.altervista.org/items/show/125#F39_Modelling_Operator -->


    <owl:Class rdf:about="https://photogrammetry.altervista.org/items/show/125#F39_Modelling_Operator">
        <rdfs:subClassOf rdf:resource="http://cidoc-crm.org/cidoc-crm/7.1.3/E39_Actor#E39_Actor"/>
        <rdfs:label xml:lang="en">ModellingOperator</rdfs:label>
        <skos:definition xml:lang="en">Definition of the class F39 Modelling Operator as a subclass of E39 Actor</skos:definition>
        <skos:example xml:lang="en">&quot;A 3D artist refining a photogrammetric model by adjusting the mesh and geometry to create an accurate virtual reconstruction.&quot; ;</skos:example>
        <skos:example xml:lang="en">&quot;A heritage specialist applying corrections and detailing to a 3D model of a historical building to prepare it for digital archiving.&quot; .</skos:example>
        <skos:example xml:lang="en">&quot;An archaeologist adjusting the 3D model of an ancient artifact to correct deformations or enhance missing sections.&quot; ;</skos:example>
        <skos:example xml:lang="en">&quot;An engineer modifying a 3D laser scan model to meet the specific dimensions needed for a structural analysis project.&quot; ;</skos:example>
        <skos:scopeNote xml:lang="en">&quot;The Modelling Operator class refers to the individual responsible for the manipulation, modification, and transformation of the 3D model. This person works on refining and adjusting the model based on the specific parameters and requirements of a project, utilizing modeling software to create accurate and detailed 3D representations. The Modelling Operator has to be skilled in various aspects of 3D modeling, such as mesh creation, geometry refinement, and the application of project-specific modifications. Where applicable, the operating subject must be indicated with their corresponding ORCID; alternatively, their direct LinkedIn link should be provided.&quot; ;</skos:scopeNote>
    </owl:Class>
    


    <!-- https://photogrammetry.altervista.org/items/show/126#F40_Eidotype -->


    <owl:Class rdf:about="https://photogrammetry.altervista.org/items/show/126#F40_Eidotype">
        <rdfs:subClassOf rdf:resource="http://cidoc-crm.org/cidoc-crm/7.1.3/E29_Design_or_Procedure#E29_Design_or_Procedure"/>
        <rdfs:label xml:lang="en">AcquisitionEidotype</rdfs:label>
        <skos:definition xml:lang="en">Definition of the class F40 Eydotipe as a subclass of E29 Design and Procedure</skos:definition>
        <skos:example xml:lang="en">&quot;A digital sketch indicating the lighting setup during the survey of a sculptural piece, noting shadows and reflections.&quot; ;</skos:example>
        <skos:example xml:lang="en">&quot;A hand-drawn diagram outlining the positions and angles from which photographs will be taken around an archaeological site.&quot; ;</skos:example>
        <skos:example xml:lang="en">&quot;A visual representation capturing the environmental conditions at the time of acquisition, such as sunlight direction and weather influences.&quot; .</skos:example>
        <skos:example xml:lang="en">&quot;An annotated drawing that describes the planned trajectory of a laser scanner while capturing data from a complex architectural structure.&quot; ;</skos:example>
        <skos:scopeNote xml:lang="en">&quot;The Eydotipe class refers to the sketch or drawing (whether digital or hand-drawn) created by the operator at the time of the survey. This drawing serves to document the general conditions of the surveyed object, including factors such as lighting conditions and the planned trajectory for the acquisition in relation to the object. The Eydotipe is an essential part of the surveying process, providing context and clarity regarding the approach and conditions of the survey.&quot; ;</skos:scopeNote>
    </owl:Class>
    


    <!-- https://photogrammetry.altervista.org/items/show/127#F41_Number_of_Picture -->


    <owl:Class rdf:about="https://photogrammetry.altervista.org/items/show/127#F41_Number_of_Picture">
        <rdfs:subClassOf rdf:resource="http://cidoc-crm.org/cidoc-crm/7.1.3/E60_Number#E60_Number"/>
        <rdfs:label xml:lang="en">AcquiredNumberOfPicture</rdfs:label>
        <owl:versionInfo xml:lang="en">Express according to 
 http://qudt.org/vocab/soqk/SI</owl:versionInfo>
        <skos:definition xml:lang="en">Definition of the class F41 Number of Picture as a subclass of E60 Number</skos:definition>
        <skos:example xml:lang="en">&quot;A photogrammetric acquisition that consists of 150 images captured from various angles around an archaeological site, where F41 would denote the number &apos;150.&apos;&quot; .</skos:example>
        <skos:scopeNote xml:lang="en">&quot;The Number of Picture class refers to the quantitative measurement of the number of individual pictures (F8) that constitute a Picture Set (F7) in a photogrammetric acquisition. This class is used to represent the total count of images captured during a specific acquisition process, which is critical for assessing the completeness and detail of the data collected.&quot; ;</skos:scopeNote>
    </owl:Class>
    


    <!-- https://photogrammetry.altervista.org/items/show/128#F42_Place_Of_Acquisition -->


    <owl:Class rdf:about="https://photogrammetry.altervista.org/items/show/128#F42_Place_Of_Acquisition">
        <rdfs:subClassOf rdf:resource="http://cidoc-crm.org/cidoc-crm/7.1.3/E53_Place#E53_Place"/>
        <rdfs:label xml:lang="en">AcquisitionLocation</rdfs:label>
        <skos:definition xml:lang="en">Definition of the class F42 Place Of Acquisition as a subclass of E53 Place</skos:definition>
        <skos:example xml:lang="en">&quot; A historic building, like a medieval castle, where the acquisition was performed, serving as the Place of Acquisition.&quot; ;</skos:example>
        <skos:example xml:lang="en">&quot;A landscape feature, such as a valley or a mountain, where the acquisition took place, denoting its significance in geographical studies.&quot; ;</skos:example>
        <skos:example xml:lang="en">&quot;An archaeological site, such as the ruins of an ancient temple, identified as the Place of Acquisition for the photogrammetric survey.&quot; ;</skos:example>
        <skos:example xml:lang="en">&quot;An urban area, like a city square, where multiple structures were surveyed, specified as the Place of Acquisition.&quot; .</skos:example>
        <skos:scopeNote xml:lang="en">&quot;The Place of Acquisition class refers to the physical space where the acquisition took place, encompassing the location where the acquisition occurred or where the architectural structure that was surveyed is situated. This class is essential for contextualizing the data collected during the acquisition process and provides information on the geographical and cultural relevance of the acquired data. Any coordinate model may be used; however, the reference model must be specified along with the provided data. &quot; ;</skos:scopeNote>
    </owl:Class>
    


    <!-- https://photogrammetry.altervista.org/items/show/129#F43_Survey_Date -->


    <owl:Class rdf:about="https://photogrammetry.altervista.org/items/show/129#F43_Survey_Date">
        <rdfs:subClassOf rdf:resource="http://cidoc-crm.org/cidoc-crm/7.1.3/E52_Time-Span#E52_Time-Span"/>
        <rdfs:label xml:lang="en">AcquisitionDate</rdfs:label>
        <skos:definition xml:lang="en">Definition of the class F43 Survey Date as a subclass of E52 Time Span</skos:definition>
        <skos:example xml:lang="en">&quot;A series of survey dates used for environmental monitoring, indicating repeated data collection at a particular location.&quot;</skos:example>
        <skos:example xml:lang="en">&quot;A timeframe marking different phases of an archaeological excavation, with specific survey dates documenting progress.&quot;</skos:example>
        <skos:example xml:lang="en">&quot;The exact date when a photogrammetric survey was performed at a historic site, such as June 15, 2022.&quot;</skos:example>
        <skos:example xml:lang="en">Example:
&quot;The date of a structural survey conducted on a bridge to assess its condition, such as March 1, 2023.&quot;</skos:example>
        <skos:scopeNote xml:lang="en">The Survey Date class refers to the specific date or time period when a survey was conducted. This class is crucial for documenting the temporal context of the acquisition process, helping establish a chronological framework for the collected data. The recorded date(s) provide insight into the conditions during the survey and can serve as a reference for subsequent analysis or future comparisons.</skos:scopeNote>
    </owl:Class>
    


    <!-- https://photogrammetry.altervista.org/items/show/130#F44_Acquisition_Description -->


    <owl:Class rdf:about="https://photogrammetry.altervista.org/items/show/130#F44_Acquisition_Description">
        <rdfs:subClassOf rdf:resource="http://cidoc-crm.org/cidoc-crm/7.1.3/E62_String#E62_String"/>
        <rdfs:label xml:lang="en">AcquisitionDescription</rdfs:label>
        <skos:definition xml:lang="en">Definition of the class F44 Acquisition Description as a subclass of E62 String</skos:definition>
        <skos:example xml:lang="en">&quot;A comprehensive account of the photogrammetric survey at an archaeological site, detailing the equipment used, environmental factors, and challenges encountered during the process.&quot;</skos:example>
        <skos:example xml:lang="en">&quot;A narrative summarizing the purpose and methods of the acquisition, such as &apos;The survey was performed to assess the structural integrity of the building using both photogrammetry and laser scanning techniques.&apos;&quot;</skos:example>
        <skos:example xml:lang="en">Example:
&quot;A description of the laser scanning session, outlining the device&apos;s trajectory and highlighting unique features of the scanned object.&quot;</skos:example>
        <skos:scopeNote xml:lang="en">:The Acquisition Description class represents a detailed narrative of the acquisition process. This class provides a structured way to document contextual information about the methodologies, conditions, and observations made during data collection. It enhances the interpretation of the collected data by offering insights into the circumstances and procedures followed during the acquisition.
A description is distinguished from the information already established by other classes as it represents a string where elements not already classified can be annotated and allows a free annotation of information that can help guide the creation of new classes for the ontology.</skos:scopeNote>
    </owl:Class>
    


    <!-- https://photogrammetry.altervista.org/items/show/131#F45__Acquisition_Coordinates -->


    <owl:Class rdf:about="https://photogrammetry.altervista.org/items/show/131#F45__Acquisition_Coordinates">
        <rdfs:subClassOf rdf:resource="http://cidoc-crm.org/cidoc-crm/7.1.3/E94_Space_Primitive#E94_Space_Primitive"/>
        <rdfs:label xml:lang="en">AcquisitionCoordinates</rdfs:label>
        <skos:definition xml:lang="en">Definition of the class F45 Acquisition Coordinates as a subclass of E94 Space Primitive</skos:definition>
        <skos:scopeNote xml:lang="en">&quot;A description of the coordinate reference system used during the acquisition, such as WGS84 or a local coordinate system customized for the survey site.&quot;</skos:scopeNote>
        <skos:scopeNote xml:lang="en">&quot;The Cartesian coordinates specifying the position of a laser scanner as it moved around an object during a 3D survey.&quot;</skos:scopeNote>
        <skos:scopeNote xml:lang="en">&quot;The geographic coordinates (latitude, longitude, and altitude) marking the exact location where a photogrammetric survey was performed.&quot;</skos:scopeNote>
        <skos:scopeNote xml:lang="en">Example:
&quot;A set of coordinates detailing the specific points at which measurements were captured, along with their spatial relationship to the surveyed object.&quot;</skos:scopeNote>
        <skos:scopeNote xml:lang="en">The Acquisition Coordinates class refers to the spatial coordinates that define the position and orientation of the acquisition device during data collection. This class is crucial for accurately representing the spatial context of the acquired data, facilitating precise alignment and integration with other spatial datasets.</skos:scopeNote>
    </owl:Class>
    


    <!-- https://photogrammetry.altervista.org/items/show/132#F46:_Matching -->


    <owl:Class rdf:about="https://photogrammetry.altervista.org/items/show/132#F46:_Matching">
        <rdfs:subClassOf rdf:resource="https://photogrammetry.altervista.org/items/show/89#F3_Processing"/>
        <rdfs:label xml:lang="en">Processing_Matching</rdfs:label>
        <skos:definition xml:lang="en">Definition of the class F46 Matching as a subclass of F3 Processing</skos:definition>
        <skos:example xml:lang="en">&quot;Matching points between historical photographs and contemporary images for comparative analysis in archaeological studies.&quot;</skos:example>
        <skos:example xml:lang="en">&quot;The automatic feature matching between pairs of photographs in a photogrammetric workflow to generate an initial sparse point cloud.&quot;</skos:example>
        <skos:example xml:lang="en">&quot;The manual identification of common points between overlapping images when automatic matching algorithms fail.&quot;</skos:example>
        <skos:example xml:lang="en">&quot;The matching of points from multiple LiDAR scans to unify different scan positions into a coherent 3D point cloud.&quot;</skos:example>
        <skos:scopeNote xml:lang="en">The Matching class refers to the process of identifying and pairing corresponding points or features across multiple images or other raw data forms. This process is vital in photogrammetry and surveying methods, as it establishes spatial relationships between images, enabling the creation of a 3D point cloud. Various algorithms and techniques are employed to ensure accurate matching between different perspectives or data sources.</skos:scopeNote>
    </owl:Class>
    


    <!-- https://photogrammetry.altervista.org/items/show/133#F47:_Densification -->


    <owl:Class rdf:about="https://photogrammetry.altervista.org/items/show/133#F47:_Densification">
        <rdfs:subClassOf rdf:resource="https://photogrammetry.altervista.org/items/show/89#F3_Processing"/>
        <rdfs:label xml:lang="en">Processing_Densification</rdfs:label>
        <skos:definition xml:lang="en">Definition of the class F47 Densification as a subclass of F3 Processing</skos:definition>
        <skos:example xml:lang="en">Applying densification algorithms in UAV (drone) imagery processing to achieve high-definition surface models.</skos:example>
        <skos:example xml:lang="en">The densification of a LiDAR point cloud to increase the resolution and clarity of a 3D terrain model.</skos:example>
        <skos:example xml:lang="en">The densification of a photogrammetric point cloud by increasing the number of points through stereo-matching algorithms.</skos:example>
        <skos:example xml:lang="en">The use of dense matching techniques to generate a more detailed point cloud in architectural surveys.</skos:example>
        <skos:scopeNote xml:lang="en">The Densification class refers to the process of enriching the initial sparse point cloud obtained from the Matching phase by adding more data points. This step involves algorithms that interpolate or directly calculate additional points to generate a more detailed and dense representation of the scanned object or scene. Densification is crucial for achieving higher accuracy and detail in the subsequent stages of 3D reconstruction, such as meshing.</skos:scopeNote>
    </owl:Class>
    


    <!-- https://photogrammetry.altervista.org/items/show/134#F48_Densification_Method -->


    <owl:Class rdf:about="https://photogrammetry.altervista.org/items/show/134#F48_Densification_Method">
        <rdfs:subClassOf rdf:resource="http://cidoc-crm.org/cidoc-crm/7.1.3/E29_Design_or_Procedure#E29_Design_or_Procedure"/>
        <rdfs:label xml:lang="en">Processing_DensificationMethod</rdfs:label>
        <skos:definition xml:lang="en">Definition of the class F48 Densification Method as a subclass of E29 Design or Procedure</skos:definition>
        <skos:example xml:lang="en">&quot;A specialized LiDAR data densification method used to capture finer features of a landscape.&quot;</skos:example>
        <skos:example xml:lang="en">&quot;The Semi-Global Matching (SGM) algorithm applied during densification to create detailed terrain models in UAV mapping.&quot;</skos:example>
        <skos:example xml:lang="en">&quot;The algorithm used for dense matching in software to enhance point density in architectural heritage documentation.&quot;</skos:example>
        <skos:example xml:lang="en">&quot;The multi-view stereo (MVS) algorithm for densifying a sparse photogrammetric point cloud.&quot;</skos:example>
        <skos:scopeNote xml:lang="en">The Densification Method class refers to the specific procedures, instructions, or algorithms used to perform densification in the creation of a 3D model. This process enriches an initial sparse point cloud by adding more points through techniques such as interpolation, dense matching, or other computational approaches. The chosen densification method directly impacts the level of detail and accuracy in the 3D reconstruction, playing a critical role in achieving a precise representation of the captured object or scene.</skos:scopeNote>
    </owl:Class>
    


    <!-- https://photogrammetry.altervista.org/items/show/135#F49__Near_Sampling_Points_Range_SFM_Point_Seeds -->


    <owl:Class rdf:about="https://photogrammetry.altervista.org/items/show/135#F49__Near_Sampling_Points_Range_SFM_Point_Seeds">
        <rdfs:subClassOf rdf:resource="http://cidoc-crm.org/cidoc-crm/7.1.3/E13_Attribute_Assignment#E13_Attribute_Assignment"/>
        <rdfs:label xml:lang="en">DensificationAttribute_NearSamplingPointRange</rdfs:label>
        <skos:definition xml:lang="en">Definition of the class F49 Near Sampling Points Range_SFM Point Seeds as a subclass of E13 Attribute Assignment</skos:definition>
        <skos:example xml:lang="en">&quot;Setting a sampling radius of 10 pixels around SfM point seeds to guide the densification process in photogrammetry software (Regard 3D).&quot;</skos:example>
        <skos:example xml:lang="en">&quot;Specifying the attribute in software that defines the maximum distance within which new points are generated around existing SfM point seeds for terrain modeling (Zephyr 3D).&quot;</skos:example>
        <skos:scopeNote xml:lang="en">The Near Sampling Points Range_SFM Point Seeds class refers to the attribute assignment process that defines the proximity or range of sampling points used during densification, specifically when working with Structure-from-Motion (SfM) point seeds. This class addresses the specification of a radius or tolerance around each seed point in the initial sparse point cloud, controlling where additional points are generated or matched during densification. It is a critical factor in determining the density and quality of the final point cloud by regulating how closely points are sampled near the seed points.</skos:scopeNote>
    </owl:Class>
    


    <!-- https://photogrammetry.altervista.org/items/show/136#F50_Point_Cloud_Measurement -->


    <owl:Class rdf:about="https://photogrammetry.altervista.org/items/show/136#F50_Point_Cloud_Measurement">
        <rdfs:subClassOf rdf:resource="http://www.cidoc-crm.org/extensions/crmsci/versions/2.0/S21_Measurement#S21_Measurement"/>
        <rdfs:label xml:lang="en">ProcessedPointCloudMesaurement</rdfs:label>
        <skos:definition xml:lang="en">Definition of the class F50 Point Cloud Measurement as a subclass of S21 Measurement</skos:definition>
        <skos:example xml:lang="en">&quot;Assessing the density of points within a 1 cm² area of a point cloud representing an archaeological artifact.&quot;</skos:example>
        <skos:example xml:lang="en">&quot;Measuring the completeness of a point cloud in terms of coverage percentage over a given surface.&quot;</skos:example>
        <skos:example xml:lang="en">&quot;Measuring the number of points in a point cloud generated by a terrestrial laser scanner.&quot;</skos:example>
        <skos:example xml:lang="en">&quot;Recording the spatial accuracy of a point cloud based on the standard deviation of point positions.&quot;</skos:example>
        <skos:scopeNote xml:lang="en">The Point Cloud Measurement class refers to the measurement activity that records the quantitative properties of a point cloud, such as the number of points, distribution density, or spatial accuracy. It acts as an intermediary between the F26 Point Cloud and the F51 Point Cloud Number Point, facilitating the process of capturing and evaluating relevant metrics from point clouds produced during 3D acquisition processes. This class is vital for assessing the completeness and precision of the point cloud prior to further processing or analysis.</skos:scopeNote>
    </owl:Class>
    


    <!-- https://photogrammetry.altervista.org/items/show/137#F51_Point_Cloud_Number_of_Point -->


    <owl:Class rdf:about="https://photogrammetry.altervista.org/items/show/137#F51_Point_Cloud_Number_of_Point">
        <rdfs:subClassOf rdf:resource="http://cidoc-crm.org/cidoc-crm/7.1.3/E54_Dimension#E54_Dimension"/>
        <rdfs:label xml:lang="en">ProcessedPointCloudNumberOfPoint</rdfs:label>
        <owl:versionInfo xml:lang="en">Express according to 
 http://qudt.org/vocab/soqk/SI</owl:versionInfo>
        <skos:definition xml:lang="en">Definition of the class F51 Point Cloud Number of Point as a subclass of E54 Dimension</skos:definition>
        <skos:example xml:lang="en">&quot;A laser-scanned point cloud consisting of 1.2 million points.&quot;</skos:example>
        <skos:example xml:lang="en">&quot;A point cloud generated from a photogrammetry survey containing 500,000 points.&quot;</skos:example>
        <skos:example xml:lang="en">&quot;A point cloud obtained from aerial photogrammetry with 750,000 points.&quot;</skos:example>
        <skos:scopeNote xml:lang="en">The Point Cloud Number of Point class refers to the specific dimension that expresses the total number of points composing a non-densified point cloud (F26 Point Cloud). This class quantifies the size of the point cloud in terms of its individual points before the densification process takes place. It is essential for understanding the initial resolution and completeness of the dataset prior to further processing, such as densification or mesh reconstruction.</skos:scopeNote>
    </owl:Class>
    


    <!-- https://photogrammetry.altervista.org/items/show/138#F52_Dense_Point_Cloud_Measurement -->


    <owl:Class rdf:about="https://photogrammetry.altervista.org/items/show/138#F52_Dense_Point_Cloud_Measurement">
        <rdfs:subClassOf rdf:resource="http://www.cidoc-crm.org/extensions/crmsci/versions/2.0/S21_Measurement#S21_Measurement"/>
        <rdfs:label xml:lang="en">ProcessedDensePointCloudMeasurement</rdfs:label>
        <skos:definition xml:lang="en">Definition of the class F52 Dense Point Cloud Measurement as a subclass of S21 Measurement</skos:definition>
        <skos:scopeNote xml:lang="en">Scope Note:
The Dense Point Cloud Measurement class refers to the measurement activity specifically related to the dense point cloud (F27 Densified Point Cloud). This class represents the act of assessing and recording dimensions or values that describe the characteristics of a densified point cloud, such as the total number of points. It serves as an intermediary to convey the results of such measurements and link them to the corresponding dense point cloud.</skos:scopeNote>
    </owl:Class>
    


    <!-- https://photogrammetry.altervista.org/items/show/139#F53_Dense_Point_Cloud_Number_of_Point -->


    <owl:Class rdf:about="https://photogrammetry.altervista.org/items/show/139#F53_Dense_Point_Cloud_Number_of_Point">
        <rdfs:subClassOf rdf:resource="http://cidoc-crm.org/cidoc-crm/7.1.3/E54_Dimension#E54_Dimension"/>
        <rdfs:label xml:lang="en">ProcessedDensePointCloudNumberOfPoint</rdfs:label>
        <owl:versionInfo xml:lang="en">Express according to 
 http://qudt.org/vocab/soqk/SI</owl:versionInfo>
        <skos:definition xml:lang="en">Definition of the class F53 Dense Point Cloud Number of Point as a subclass of E54 Dimension</skos:definition>
        <skos:example xml:lang="en">&quot;A dense point cloud of a scanned monument containing 15 million points.&quot;</skos:example>
        <skos:scopeNote xml:lang="en">The Dense Point Cloud Number of Point class refers to the specific dimension that indicates the number of points in a densified point cloud (F27 Densified Point Cloud). This class records the total count of points generated after the densification process, offering crucial data about the granularity and density of the final point cloud used for 3D modeling and analysis.</skos:scopeNote>
    </owl:Class>
    


    <!-- https://photogrammetry.altervista.org/items/show/141#F55_Depth_Noise_Filtering -->


    <owl:Class rdf:about="https://photogrammetry.altervista.org/items/show/141#F55_Depth_Noise_Filtering">
        <rdfs:subClassOf rdf:resource="http://cidoc-crm.org/cidoc-crm/7.1.3/E13_Attribute_Assignment#E13_Attribute_Assignment"/>
        <rdfs:label xml:lang="en">DensificationAttributeDepthNoiseFiltering</rdfs:label>
        <skos:definition xml:lang="en">Definition of the class F55 Depth Noise Filtering as a subclass of E13 Attribute Assignment</skos:definition>
        <skos:example xml:lang="en">&quot;In the densified point cloud of AFMNM005, the Depth Noise Filtering includes Adaptive Feature Extraction (AFE), Gradient Field Estimation (GFE), and further Accelerated Gradient Ascent (FAGA) techniques (Lauro 2019).&quot;</skos:example>
        <skos:scopeNote xml:lang="en">The Depth Noise Filtering class refers to the assignment of depth noise reduction techniques or parameters applied to densified point clouds (F27 Densified Point Cloud). This class captures the process of identifying and filtering out noise, errors, or inaccuracies in the depth values of a point cloud. These filtering operations are particularly necessary in dense datasets where inaccuracies can affect the quality and reliability of subsequent reconstructions.</skos:scopeNote>
    </owl:Class>
    


    <!-- https://photogrammetry.altervista.org/items/show/142#F56_Mesh_Reconstruction -->


    <owl:Class rdf:about="https://photogrammetry.altervista.org/items/show/142#F56_Mesh_Reconstruction">
        <rdfs:subClassOf rdf:resource="https://photogrammetry.altervista.org/items/show/90#F4_Modelling"/>
        <rdfs:label xml:lang="en">Modelling_MeshReconstruction</rdfs:label>
        <skos:definition xml:lang="en">Definition of the class F56 Mesh Reconstruction as a subclass of F4 Modelling</skos:definition>
        <skos:example xml:lang="en">&quot;Reconstructing the mesh of a building facade from a point cloud acquired through laser scanning in order to create a geometric model for preservation purposes.&quot;</skos:example>
        <skos:example xml:lang="en">Examples:
&quot;Generating a 3D mesh from a densified point cloud of an archaeological artifact.&quot;</skos:example>
        <skos:scopeNote xml:lang="en">The Mesh Reconstruction class refers to the process of generating a 3D mesh from a densified point cloud (F27 Densified Point Cloud). This class captures the modeling operation where a continuous surface (mesh) is reconstructed, typically using algorithms that define the relationships between individual points within the cloud. This surface representation becomes the foundation for the final 3D model before any texturing is applied, and is crucial for the geometrical definition of the object in digital form.</skos:scopeNote>
    </owl:Class>
    


    <!-- https://photogrammetry.altervista.org/items/show/143#F57_Texturing_Mesh -->


    <owl:Class rdf:about="https://photogrammetry.altervista.org/items/show/143#F57_Texturing_Mesh">
        <rdfs:subClassOf rdf:resource="https://photogrammetry.altervista.org/items/show/90#F4_Modelling"/>
        <rdfs:label xml:lang="en">Modelling_TexturingMesh</rdfs:label>
        <skos:definition xml:lang="en">Definition of the class F57 Texturing Mesh as a subclass of F4 Modelling</skos:definition>
        <skos:example xml:lang="en">&quot;Applying high-resolution photographic textures to a 3D mesh of a historic building to accurately reflect its original appearance.&quot;</skos:example>
        <skos:example xml:lang="en">&quot;Mapping surface details onto a 3D model of a statue using images captured from various angles to ensure comprehensive coverage and detail.&quot;</skos:example>
        <skos:example xml:lang="en">&quot;Using UV mapping techniques to accurately position and scale textures on a mesh of an archaeological artifact for virtual exhibition.&quot;</skos:example>
        <skos:scopeNote xml:lang="en">Scope Note:
The Texturing Mesh class refers to the process of applying textures to a 3D mesh in order to enhance its visual appearance. The texture is generally derived from photographs or other 2D image data and is mapped onto the 3D surface to represent the color, material, and finer surface details. This step follows the mesh reconstruction phase and is crucial for adding realism to the 3D model, especially in cultural heritage applications where visual accuracy is important.</skos:scopeNote>
    </owl:Class>
    


    <!-- https://photogrammetry.altervista.org/items/show/144#F58_Modifying_Mesh -->


    <owl:Class rdf:about="https://photogrammetry.altervista.org/items/show/144#F58_Modifying_Mesh">
        <rdfs:subClassOf rdf:resource="https://photogrammetry.altervista.org/items/show/90#F4_Modelling"/>
        <rdfs:label xml:lang="en">Modelling_ModifyingTexturedMesh</rdfs:label>
        <skos:definition xml:lang="en">Definition of the class F58 Modifying Mesh as a subclass of F4 Modelling</skos:definition>
        <skos:example xml:lang="en">&quot;Applying smoothing techniques to a 3D mesh of an archaeological artifact to remove noise and enhance surface quality for digital preservation.&quot;</skos:example>
        <skos:example xml:lang="en">Examples:
&quot;Modifying the mesh of a historical monument to correct errors introduced during the scanning process, ensuring a more accurate representation of its geometry.&quot;</skos:example>
        <skos:example xml:lang="en">Examples:
&quot;Simplifying the geometry of a complex 3D model for use in a real-time virtual reality environment, reducing the polygon count while preserving essential details.&quot;</skos:example>
        <skos:scopeNote xml:lang="en">Scope Note:
The Modifying Mesh class refers to the process of altering or refining a 3D mesh to correct geometrical inaccuracies, simplify the model, or adapt it for specific use cases. This modification can involve smoothing, decimating (reducing the number of polygons), or adjusting the mesh to meet certain criteria, such as improving visual fidelity or optimizing for real-time applications. This step is performed manually or through semi-automated processes and can be part of the workflow in the creation of accurate and efficient 3D models.</skos:scopeNote>
    </owl:Class>
    


    <!-- https://photogrammetry.altervista.org/items/show/145#F100_3D_Digital_Twin -->


    <owl:Class rdf:about="https://photogrammetry.altervista.org/items/show/145#F100_3D_Digital_Twin">
        <rdfs:subClassOf rdf:resource="https://photogrammetry.altervista.org/items/show/188#F102:_3D_Digital_Asset"/>
        <rdfs:label xml:lang="en">TridimensionalDigitalTwin</rdfs:label>
        <skos:definition xml:lang="en">Definition of the class F100 3D Digital Twin as a subclass of D9 Data Object</skos:definition>
        <skos:example xml:lang="en">&quot;The digital twin of the boar jaw preserved at the Okayama archaeological museum and signed as AF005MNM (Lauro 2019).&quot;</skos:example>
        <skos:example xml:lang="en">&quot;The digital twin of the excavation section of the Gobekli Tepe site (Polat 2020).&quot;</skos:example>
        <skos:example xml:lang="en">&quot;The digital twin of the no longer existing Bamiyan Buddhas (Gruen 2004).&quot;</skos:example>
        <skos:scopeNote xml:lang="en">The 3D Digital Twin class refers to the ultimate 3D model resulting from the complete acquisition and processing workflow. This model may be the outcome of either the F5 Exporting process or F4 Modelling, depending on the workflow followed. At this stage, the model is considered complete and will not undergo any further modifications. It is the final product that represents the culmination of all previous acquisition, processing, and modeling efforts, encapsulating all the geometric and textural information. This final model is typically used for documentation, analysis, visualization, or presentation purposes in various fields such as cultural heritage, architecture, and archaeology.</skos:scopeNote>
    </owl:Class>
    


    <!-- https://photogrammetry.altervista.org/items/show/146#F59_Digital_Scale -->


    <owl:Class rdf:about="https://photogrammetry.altervista.org/items/show/146#F59_Digital_Scale">
        <rdfs:subClassOf rdf:resource="http://cidoc-crm.org/cidoc-crm/7.1.3/E54_Dimension#E54_Dimension"/>
        <rdfs:label xml:lang="en">TridimensionalDigitalTwinDigitalScale</rdfs:label>
        <skos:definition xml:lang="en">Definition of the class F59 Digital Scale as a subclass of E54 Dimension</skos:definition>
        <skos:example xml:lang="en">&quot;A digital scale of 1:1 for a final 3D model of a sculpture, indicating that the model is an exact replica of the original size.&quot;</skos:example>
        <skos:example xml:lang="en">&quot;A digital scale of 1:50 for an architectural model, showing that the digital representation is 50 times smaller than the actual building.&quot;</skos:example>
        <skos:scopeNote xml:lang="en">The Digital Scale class refers to the scale of the 3D Digital Twin (F100), specifically in relation to the actual size of the object being represented. It indicates the proportional relationship between the dimensions of the digital model and the real-world measurements of the original object. This scale can be expressed in various formats, such as 1:1, 1:20, or other ratios, depending on how the 3D model has been created or intended to be used. The Digital Scale is crucial for accurate representation, visualization, and analysis, ensuring that the digital twin correctly reflects the physical dimensions of the object it represents.</skos:scopeNote>
    </owl:Class>
    


    <!-- https://photogrammetry.altervista.org/items/show/147#F60_Smoothing_Filter -->


    <owl:Class rdf:about="https://photogrammetry.altervista.org/items/show/147#F60_Smoothing_Filter">
        <rdfs:subClassOf rdf:resource="http://cidoc-crm.org/cidoc-crm/7.1.3/E13_Attribute_Assignment#E13_Attribute_Assignment"/>
        <rdfs:label xml:lang="en">ProcessedMeshSmoothingFilter</rdfs:label>
        <skos:definition xml:lang="en">Definition of the class F60 Smoothing Filter as a subclass of E13 Attribute Assignment</skos:definition>
        <skos:example xml:lang="en">&quot;A Gaussian smoothing filter applied to a 3D mesh to create a more fluid surface by averaging the vertices of the mesh.&quot;</skos:example>
        <skos:example xml:lang="en">&quot;A Laplacian smoothing filter used during the creation of a 3D mesh to reduce sharp edges and create a smoother transition between different surface areas.&quot;</skos:example>
        <skos:scopeNote xml:lang="en">The Smoothing Filter class refers to the smoothing filter applied to the 3D Mesh (F28) during its creation process. This filter is used to enhance the quality of the mesh by reducing noise and irregularities, resulting in a more visually appealing and geometrically accurate representation of the 3D object. The application of a smoothing filter is a crucial step in the modeling workflow, as it contributes to the overall aesthetic and functional quality of the final mesh, facilitating better visualization and analysis.</skos:scopeNote>
    </owl:Class>
    


    <!-- https://photogrammetry.altervista.org/items/show/148#F61_Color_Balance/Multiband_Texture -->


    <owl:Class rdf:about="https://photogrammetry.altervista.org/items/show/148#F61_Color_Balance/Multiband_Texture">
        <rdfs:subClassOf rdf:resource="http://cidoc-crm.org/cidoc-crm/7.1.3/E13_Attribute_Assignment#E13_Attribute_Assignment"/>
        <rdfs:label xml:lang="en">ProcessedTexturedMeshColorBalance</rdfs:label>
        <skos:definition xml:lang="en">Definition of the class F61 Color Balance/Multiband Texture as a subclass of E13 Attribute Assignment</skos:definition>
        <skos:example xml:lang="en">&quot;A color balance adjustment applied to the texture of a 3D architectural model to ensure that the colors accurately reflect the materials used in the real-world structure.&quot;</skos:example>
        <skos:example xml:lang="en">&quot;A multiband texture that combines data from different spectral bands (such as RGB and infrared) to create a detailed and informative texture for a 3D model of a vegetation area.&quot;</skos:example>
        <skos:scopeNote xml:lang="en">The Color Balance/Multiband Texture class refers to the type of texture utilized in the creation of the Textured 3D Mesh (F29). This class encompasses techniques that adjust the color balance and integrate multiple spectral bands to enhance the visual quality of the texture applied to the 3D model. By managing color saturation, brightness, and contrast, this attribute ensures that the texture accurately represents the surface properties of the object, leading to a more realistic and visually appealing 3D representation.</skos:scopeNote>
    </owl:Class>
    


    <!-- https://photogrammetry.altervista.org/items/show/149#F62_Texture_Set_of_3D_Mesh -->


    <owl:Class rdf:about="https://photogrammetry.altervista.org/items/show/149#F62_Texture_Set_of_3D_Mesh">
        <rdfs:subClassOf rdf:resource="http://www.cidoc-crm.org/extensions/crmdig/versions/4.0/D9_Data_Object#D9_Data_Object"/>
        <rdfs:label xml:lang="en">ProcessedTexturedMeshTextureSet</rdfs:label>
        <skos:definition xml:lang="en">Definition of the class F62 Texture Set of 3D Mesh as a subclass of D9 Data Object</skos:definition>
        <skos:example xml:lang="en">&quot;A collection of multiple textures applied to different parts of a 3D character model, including skin texture, clothing texture, and accessory texture, to achieve a rich and detailed visual representation.&quot;</skos:example>
        <skos:example xml:lang="en">&quot;A texture set consisting of a diffuse map, a normal map, and a specular map used to create a realistic surface appearance for a 3D model of a stone wall.&quot;</skos:example>
        <skos:scopeNote xml:lang="en">The Texture Set of 3D Mesh class refers to the collection of textures, which can be either singular or multiple, that are associated with a Textured 3D Mesh (F29). This class encompasses all the visual information applied to the 3D model&apos;s surface, which may include different texture maps such as diffuse, specular, normal, and bump maps. The texture set is crucial for enhancing the realism of the 3D model, providing detailed surface characteristics and visual cues that represent the physical properties of the object being modeled.</skos:scopeNote>
    </owl:Class>
    


    <!-- https://photogrammetry.altervista.org/items/show/150#F63_Number_of_Texture -->


    <owl:Class rdf:about="https://photogrammetry.altervista.org/items/show/150#F63_Number_of_Texture">
        <rdfs:subClassOf rdf:resource="http://cidoc-crm.org/cidoc-crm/7.1.3/E60_Number#E60_Number"/>
        <rdfs:label xml:lang="en">ProcessedTexturedMeshNumberOfTexture</rdfs:label>
        <owl:versionInfo xml:lang="en">Express according to 
 http://qudt.org/vocab/soqk/SI</owl:versionInfo>
        <skos:definition xml:lang="en">Definition of the class F63 Number of Texture as a subclass of E60 Number</skos:definition>
        <skos:example xml:lang="en">&quot;A Texture Set of 3D Mesh consisting of 3 textures, including a diffuse texture for the base color, a normal texture for surface detail, and a specular texture for shininess.&quot;</skos:example>
        <skos:example xml:lang="en">&quot;A Texture Set of 3D Mesh that incorporates 5 different textures, each applied to various components of a complex architectural model, such as walls, roofs, windows, and doors.&quot;</skos:example>
        <skos:scopeNote xml:lang="en">The Number of Texture class refers to the quantity of textures present in a Texture Set of 3D Mesh (F62). This class provides a quantitative measure of the textures utilized in the texturing process of a 3D model, allowing for an understanding of the complexity and detail involved in the visual representation of the model. The number of textures can vary widely depending on the design requirements, intended realism, and specific characteristics of the object being represented.</skos:scopeNote>
    </owl:Class>
    


    <!-- https://photogrammetry.altervista.org/items/show/151#F64_Modelling_Description -->


    <owl:Class rdf:about="https://photogrammetry.altervista.org/items/show/151#F64_Modelling_Description">
        <rdfs:subClassOf rdf:resource="http://cidoc-crm.org/cidoc-crm/7.1.3/E62_String#E62_String"/>
        <rdfs:label xml:lang="en">Modelling_ModifyingDescription</rdfs:label>
        <skos:definition xml:lang="en">Definition of the class F64 Modelling Description as a subclass of E62 String</skos:definition>
        <skos:example xml:lang="en">&quot;A description detailing how the texture was adjusted to enhance realism by applying a specific smoothing filter and how additional vertices were added to refine the model&apos;s geometry.&quot;</skos:example>
        <skos:example xml:lang="en">&quot;The string &apos;elimination of the elements of the table and the set and focus on the find&apos; in the context of modeling the 3D model of AF005MNM (Lauro 2019).&quot;</skos:example>
        <skos:scopeNote xml:lang="en">The Modelling Description class refers to a prose description of the modelling operations performed on a Textured Mesh (F29) within the context of Modelling (F4). This description provides a narrative account of the changes and modifications made to the 3D model, detailing the techniques, tools, and processes employed during the modelling phase. Such descriptions are essential for documentation purposes, allowing users to understand the adjustments made and the rationale behind them.
A description is distinguished from the information already established by other classes as it represents a string where elements not already classified can be annotated and allows a free annotation of information that can help guide the creation of new classes for the ontology.</skos:scopeNote>
    </owl:Class>
    


    <!-- https://photogrammetry.altervista.org/items/show/152#F65_Modelling_Date -->


    <owl:Class rdf:about="https://photogrammetry.altervista.org/items/show/152#F65_Modelling_Date">
        <rdfs:subClassOf rdf:resource="http://cidoc-crm.org/cidoc-crm/7.1.3/E52_Time-Span#E52_Time-Span"/>
        <rdfs:label xml:lang="en">Modelling_ModifyngTexturedMeshDate</rdfs:label>
        <skos:definition xml:lang="en">Definition of the class F65 Modelling Date as a subclass of E52 Time Span</skos:definition>
        <skos:example xml:lang="en">&quot;The F58 Modifyng Mesh of AFMNM005 occurred on 16/03/2019 (Lauro 2019).&quot;</skos:example>
        <skos:scopeNote xml:lang="en">The Modelling Date class refers to the specific date when the F58 Modifying Mesh took place. This date is crucial for documenting the timeline of the modelling process, allowing for tracking of changes, revisions, and the overall progression of the 3D model development. Recording the modelling date can aid in understanding the evolution of the model and its context within the broader project timeline.</skos:scopeNote>
    </owl:Class>
    


    <!-- https://photogrammetry.altervista.org/items/show/153#F66_Modelling_Determination -->


    <owl:Class rdf:about="https://photogrammetry.altervista.org/items/show/153#F66_Modelling_Determination">
        <rdfs:subClassOf rdf:resource="https://photogrammetry.altervista.org/items/show/90#F4_Modelling"/>
        <rdfs:label xml:lang="en">Modelling_ModifyingTexturedMeshDetermination</rdfs:label>
        <skos:definition xml:lang="en">Definition of the class F66 Modelling Determination as a subclass of D7 Digital Machine Event</skos:definition>
        <skos:example xml:lang="en">&quot;Assessing which elements of a complex architectural model can be simplified or removed to improve rendering performance, such as reducing the number of polygons in non-visible areas.&quot;</skos:example>
        <skos:example xml:lang="en">&quot;Deciding which details in a character model are necessary for animation and which can be omitted to optimize the mesh, focusing on maintaining key features while enhancing computational efficiency.&quot;</skos:example>
        <skos:example xml:lang="en">&quot;Determining the essential structural elements of a historical building model to be preserved while omitting modern additions that detract from its historical integrity.</skos:example>
        <skos:scopeNote xml:lang="en">The Modelling Determination class refers to the activity of determining which parts of a 3D model should be preserved and which should be eliminated based on project requirements, spatial constraints, and other considerations. This process involves critical decision-making regarding the functionality and aesthetics of the model, ensuring that the final output meets the intended objectives of the project.</skos:scopeNote>
    </owl:Class>
    


    <!-- https://photogrammetry.altervista.org/items/show/154#F67_Modelling_Elimination -->


    <owl:Class rdf:about="https://photogrammetry.altervista.org/items/show/154#F67_Modelling_Elimination">
        <rdfs:subClassOf rdf:resource="https://photogrammetry.altervista.org/items/show/90#F4_Modelling"/>
        <rdfs:label xml:lang="en">Modelling_ModifyingTexturedMeshElimination</rdfs:label>
        <skos:definition xml:lang="en">Definition of the class F67 Modelling Elimination as a subclass of D7 Digital Machine Event</skos:definition>
        <skos:example xml:lang="en">&quot;Executing the deletion of unnecessary polygons from a high-resolution model to reduce file size and processing time, ensuring that the model remains manageable for rendering and analysis.&quot;</skos:example>
        <skos:example xml:lang="en">&quot;Implementing changes to a 3D asset by removing elements deemed redundant or not relevant to the final output, such as extraneous details that do not contribute to the overall visual narrative.&quot;</skos:example>
        <skos:scopeNote xml:lang="en">The Modelling Elimination class refers to the actual activity of removing the identified parts from the 3D model as part of the modelling process. This action is taken after the determination phase and is critical for refining the model to meet project specifications and performance requirements.</skos:scopeNote>
    </owl:Class>
    


    <!-- https://photogrammetry.altervista.org/items/show/155#F68_Digital_Twin_Physical_Carrier -->


    <owl:Class rdf:about="https://photogrammetry.altervista.org/items/show/155#F68_Digital_Twin_Physical_Carrier">
        <rdfs:subClassOf rdf:resource="http://www.cidoc-crm.org/extensions/crmdig/versions/4.0/D13_Digital_Information_Carrier#D13_Digital_Information_Carrier"/>
        <rdfs:label xml:lang="en">TridimensionalDigitalTwinCarrier</rdfs:label>
        <skos:definition xml:lang="en">Definition of the class F68 Digital Twin Physical Carrier as a subclass of D13 Digital Information Carrier</skos:definition>
        <skos:example xml:lang="en">&quot;An external hard drive containing the files of a Digital Twin for an architectural project, ensuring that all relevant data is securely stored and easily retrievable for future reference.&quot;</skos:example>
        <skos:example xml:lang="en">&quot;The server that hosts the cloud storage service that stores backups of a Digital Twin for an industrial application, providing redundancy and access from multiple locations.&quot;</skos:example>
        <skos:scopeNote xml:lang="en">The Digital Twin Physical Carrier class refers to the physical storage medium where the Digital Twin (F58) is preserved. This can include various types of physical storage devices, such as external hard drives, SSDs, or any other digital information carriers that ensure the safe storage and accessibility of the Digital Twin for future use.</skos:scopeNote>
    </owl:Class>
    


    <!-- https://photogrammetry.altervista.org/items/show/156#F69_Exporting_Description -->


    <owl:Class rdf:about="https://photogrammetry.altervista.org/items/show/156#F69_Exporting_Description">
        <rdfs:subClassOf rdf:resource="http://cidoc-crm.org/cidoc-crm/7.1.3/E62_String#E62_String"/>
        <rdfs:label xml:lang="en">ExportingOfTridimensionalDigitalTwinDescription</rdfs:label>
        <skos:definition xml:lang="en">Definition of the class F69 Exporting Description as a subclass of E62 String</skos:definition>
        <skos:example xml:lang="en">&quot;A description detailing the export settings used to generate a 3D model in OBJ format from the Digital Twin, specifying resolution and texture mapping options.&quot;</skos:example>
        <skos:example xml:lang="en">&quot;Notes explaining the conversion process of a Digital Twin from a proprietary format to a standard interchange format for wider accessibility, including adjustments made to preserve data integrity.&quot;</skos:example>
        <skos:scopeNote xml:lang="en">The Exporting Description class refers to a textual string that contains information and details regarding the operations carried out during the export of the Digital Twin. This description is essential for documenting the export process and can include specifications about formats, settings, and any modifications made during the export.
A description is distinguished from the information already established by other classes as it represents a string where elements not already classified can be annotated and allows a free annotation of information that can help guide the creation of new classes for the ontology.</skos:scopeNote>
    </owl:Class>
    


    <!-- https://photogrammetry.altervista.org/items/show/157#F70_Number_of_Final_Destination -->


    <owl:Class rdf:about="https://photogrammetry.altervista.org/items/show/157#F70_Number_of_Final_Destination">
        <rdfs:subClassOf rdf:resource="http://cidoc-crm.org/cidoc-crm/7.1.3/E60_Number#E60_Number"/>
        <rdfs:label xml:lang="en">ExportingNumberOfFinalDestination</rdfs:label>
        <owl:versionInfo xml:lang="en">Express according to 
 http://qudt.org/vocab/soqk/SI</owl:versionInfo>
        <skos:definition xml:lang="en">Definition of the class F70 Number of Final Destination as a subclass of E60 Number</skos:definition>
        <skos:example xml:lang="en">&quot;Count of different cloud storage platforms where copies of a Digital Twin are kept for disaster recovery, including local servers and remote backups.&quot;</skos:example>
        <skos:example xml:lang="en">&quot;The number of backup locations designated for an industrial Digital Twin model, ensuring data redundancy and recovery options in case of system failures.&quot;</skos:example>
        <skos:scopeNote xml:lang="en">The Number of Final Destination class refers to the quantity of final storage locations for the Digital Twin and all its copies. This metric is important for understanding the distribution and redundancy of the Digital Twin across various storage media, ensuring that the model is preserved in multiple locations for safety and accessibility.</skos:scopeNote>
    </owl:Class>
    


    <!-- https://photogrammetry.altervista.org/items/show/158#F71_Final_Use_of_Digital_Twin -->


    <owl:Class rdf:about="https://photogrammetry.altervista.org/items/show/158#F71_Final_Use_of_Digital_Twin">
        <rdfs:subClassOf rdf:resource="http://www.cidoc-crm.org/extensions/crmdig/versions/4.0/D7_Digital_Machine_Event#D7_Digital_Machine_Event"/>
        <rdfs:label xml:lang="en">Exporting_FinalTridimensionalDigitalTwin</rdfs:label>
        <skos:definition xml:lang="en">Definition of the class F71 Final Use of Digital Twin as a subclass of D7 Digital Machine Event</skos:definition>
        <skos:example xml:lang="en">&quot;Creating various renditions of a Digital Twin to support different stages of an architectural review process, including detailed models for technical analysis and simplified versions for stakeholder presentations.&quot;</skos:example>
        <skos:example xml:lang="en">&quot;Modifying a Digital Twin for use in a virtual reality simulation for a client presentation, ensuring an immersive experience that highlights key design features.&quot;</skos:example>
        <skos:scopeNote xml:lang="en">The Final Use of Digital Twin class refers to the final preparations and operations performed on the Digital Twin in accordance with the project&apos;s requirements. This class encompasses the generation of all necessary variants of the Digital Twin tailored for specific purposes, ensuring that the final outputs meet the intended application, whether for visualization, simulation, or analysis.</skos:scopeNote>
    </owl:Class>
    


    <!-- https://photogrammetry.altervista.org/items/show/159#F72_3D_Model_Video_Rendering -->


    <owl:Class rdf:about="https://photogrammetry.altervista.org/items/show/159#F72_3D_Model_Video_Rendering">
        <rdfs:subClassOf rdf:resource="http://www.cidoc-crm.org/extensions/crmdig/versions/4.0/D9_Data_Object#D9_Data_Object"/>
        <rdfs:label xml:lang="en">Exported3DModelVideoRendering</rdfs:label>
        <skos:definition xml:lang="en">Definition of the class F72 3D Model Video Rendering as a subclass of D9 Data Object</skos:definition>
        <skos:example xml:lang="en">&quot;A video showcasing the architectural model of a building, rendered to highlight its design elements for a client presentation, including animated walk-throughs and exterior views.&quot;</skos:example>
        <skos:example xml:lang="en">&quot;An educational video demonstrating the features of a historical artifact through 3D rendering, illustrating its significance and context in an engaging manner.&quot;</skos:example>
        <skos:scopeNote xml:lang="en">The 3D Model Video Rendering class refers to the output generated by rendering a 3D model into a video format. This video can be utilized for various purposes, such as presentations, educational demonstrations, or promotional content. The rendering process involves creating a visual representation of the 3D model in motion, showcasing its features, textures, and overall design.</skos:scopeNote>
    </owl:Class>
    


    <!-- https://photogrammetry.altervista.org/items/show/160#F73_Editing_Video -->


    <owl:Class rdf:about="https://photogrammetry.altervista.org/items/show/160#F73_Editing_Video">
        <rdfs:subClassOf rdf:resource="http://www.cidoc-crm.org/extensions/crmdig/versions/4.0/D7_Digital_Machine_Event#D7_Digital_Machine_Event"/>
        <rdfs:label xml:lang="en">Exporting_EditingRenderingVideo</rdfs:label>
        <skos:definition xml:lang="en">Definition of the class F73 Editing Video as a subclass of D7 Digital Machine Event</skos:definition>
        <skos:example xml:lang="en">&quot;Adding background music and transitions to the video of a 3D model for promotional purposes, enhancing viewer engagement and aesthetic appeal.&quot;</skos:example>
        <skos:example xml:lang="en">&quot;Cutting segments of the 3D rendering video to create a more concise presentation for a seminar, ensuring the key points are highlighted effectively.&quot;</skos:example>
        <skos:scopeNote xml:lang="en">The Editing Video class refers to the actions performed on the rendered video of the 3D model to modify, enhance, or refine its content. This includes tasks such as cutting, splicing, adding effects, and incorporating audio, all aimed at improving the final presentation quality of the video.</skos:scopeNote>
    </owl:Class>
    


    <!-- https://photogrammetry.altervista.org/items/show/161#F74_Video_Editing_Software -->


    <owl:Class rdf:about="https://photogrammetry.altervista.org/items/show/161#F74_Video_Editing_Software">
        <rdfs:subClassOf rdf:resource="http://www.cidoc-crm.org/extensions/crmdig/versions/4.0/D14_Software#D14_Software"/>
        <rdfs:label xml:lang="en">Exporting_EditingRenderingVideoSoftware</rdfs:label>
        <skos:definition xml:lang="en">Definition of the class F74 Video Editing Software as a subclass of D14 Software</skos:definition>
        <skos:example xml:lang="en">&quot;Adobe Premiere Pro, used for editing and refining videos of rendered 3D models, offering advanced features like multi-track editing and color correction.&quot;</skos:example>
        <skos:example xml:lang="en">&quot;Final Cut Pro, a software application employed in the editing of architectural visualization videos, known for its intuitive interface and powerful editing tools.&quot;</skos:example>
        <skos:scopeNote xml:lang="en">The Video Editing Software class refers to the specific applications or programs used to perform the editing operations on the video produced from the 3D model rendering. This software provides tools and features necessary for video manipulation and enhancement, enabling users to create professional-quality videos.</skos:scopeNote>
    </owl:Class>
    


    <!-- https://photogrammetry.altervista.org/items/show/162#F75_Project_Video -->


    <owl:Class rdf:about="https://photogrammetry.altervista.org/items/show/162#F75_Project_Video">
        <rdfs:subClassOf rdf:resource="http://www.cidoc-crm.org/extensions/crmdig/versions/4.0/D9_Data_Object#D9_Data_Object"/>
        <rdfs:label xml:lang="en">ExportedVideo3DRendering</rdfs:label>
        <skos:definition xml:lang="en">Definition of the class F75 Project Video as a subclass of D9 Data Object</skos:definition>
        <skos:example xml:lang="en">&quot;A promotional video that highlights the features of a virtual tour created from a 3D model, incorporating narration and background music for an engaging experience.&quot;</skos:example>
        <skos:example xml:lang="en">&quot;The final video output showcasing a 3D architectural design, ready for client delivery, featuring dynamic angles and detailed animations.&quot;</skos:example>
        <skos:scopeNote xml:lang="en">The Project Video class refers to the final video product that contains the rendered 3D model, after undergoing editing processes. This video represents the completed work, showcasing the 3D model in a polished format, and is typically used for presentations, marketing, or documentation purposes.</skos:scopeNote>
    </owl:Class>
    


    <!-- https://photogrammetry.altervista.org/items/show/163#F76_3D_Model_for_3D_Print -->


    <owl:Class rdf:about="https://photogrammetry.altervista.org/items/show/163#F76_3D_Model_for_3D_Print">
        <rdfs:subClassOf rdf:resource="https://photogrammetry.altervista.org/items/show/188#F102:_3D_Digital_Asset"/>
        <rdfs:label xml:lang="en">Exported3DModelForPrinting</rdfs:label>
        <skos:definition xml:lang="en">Definition of the class F76 3D Model for 3D Print as a subclass of D9 Data Object</skos:definition>
        <skos:example xml:lang="en">&quot;A 3D architectural model adjusted for printing, with specific wall thickness and support structures included to ensure stability during the printing process.&quot;</skos:example>
        <skos:example xml:lang="en">&quot;A prototype design modified for 3D printing, ensuring all parts are printable without failure, featuring reinforced joints and proper scaling for accurate representation.&quot;</skos:example>
        <skos:scopeNote xml:lang="en">The 3D Model for 3D Print class refers to a 3D model that has been specifically modified and prepared for 3D printing. This model undergoes adjustments to ensure it meets the necessary specifications and requirements for successful printing, including geometry optimization, scaling, and format compatibility.</skos:scopeNote>
    </owl:Class>
    


    <!-- https://photogrammetry.altervista.org/items/show/164#F77_Printing_Digital_Twin -->


    <owl:Class rdf:about="https://photogrammetry.altervista.org/items/show/164#F77_Printing_Digital_Twin">
        <rdfs:subClassOf rdf:resource="http://www.semanticweb.org/vitto/ontologies/2024/9/PODS_1#E12_Production"/>
        <rdfs:label xml:lang="en">Exporting_Printing3DModel</rdfs:label>
        <skos:definition xml:lang="en">Definition of the class F77 Printing Digital Twin as a subclass of E12 Production</skos:definition>
        <skos:example xml:lang="en">&quot;The act of 3D printing a prototype based on a digitally designed engineering component, facilitating functional testing and design validation.&quot;</skos:example>
        <skos:example xml:lang="en">&quot;The operation of a 3D printer producing a scaled model of a historical artifact from a digital file, allowing for preservation and study of the original object&apos;s features.&quot;</skos:example>
        <skos:scopeNote xml:lang="en">The Printing Digital Twin class refers to the physical action of producing a 3D print of a digital model. This process involves using a 3D printer to convert the digital file of the 3D model into a tangible object, resulting in a physical representation of the digital twin.</skos:scopeNote>
    </owl:Class>
    


    <!-- https://photogrammetry.altervista.org/items/show/165#F78_Material_for_3D_Printing -->


    <owl:Class rdf:about="https://photogrammetry.altervista.org/items/show/165#F78_Material_for_3D_Printing">
        <rdfs:subClassOf rdf:resource="http://cidoc-crm.org/cidoc-crm/7.1.3/E57_Material#E57_Material"/>
        <rdfs:label xml:lang="en">Printed3DModelMaterial</rdfs:label>
        <skos:definition xml:lang="en">Definition of the class F78 Material for 3D Printing as a subclass of E57 Material</skos:definition>
        <skos:example xml:lang="en">&quot;ABS (Acrylonitrile Butadiene Styrene) chosen for its durability in engineering applications, making it suitable for creating functional parts that require impact resistance.&quot;</skos:example>
        <skos:example xml:lang="en">&quot;PLA (Polylactic Acid) used for printing biodegradable models, offering an eco-friendly alternative for producing prototypes and consumer products.&quot;</skos:example>
        <skos:scopeNote xml:lang="en">The Material for 3D Printing class refers to the specific type of material selected for use in the 3D printing process. This material is essential for defining the properties and characteristics of the printed object, including its strength, flexibility, and appearance.</skos:scopeNote>
    </owl:Class>
    


    <!-- https://photogrammetry.altervista.org/items/show/166#F79_Printing_Device -->


    <owl:Class rdf:about="https://photogrammetry.altervista.org/items/show/166#F79_Printing_Device">
        <rdfs:subClassOf rdf:resource="http://cidoc-crm.org/cidoc-crm/7.1.3/E70_Thing#E70_Thing"/>
        <rdfs:label xml:lang="en">3DPrintingDevice</rdfs:label>
        <skos:definition xml:lang="en">Definition of the class F79 Printing Device as a subclass of E70 Thing</skos:definition>
        <skos:example xml:lang="en">&quot;A SLA (Stereolithography) printer employed for high-resolution prints of intricate designs, which utilizes a laser to cure liquid resin layer by layer.&quot;</skos:example>
        <skos:example xml:lang="en">&quot;An FDM (Fused Deposition Modeling) 3D printer used for creating plastic prototypes, which utilizes a continuous filament of thermoplastic material to construct objects.&quot;</skos:example>
        <skos:scopeNote xml:lang="en">The Printing Device class refers to the specific model or type of 3D printer utilized for producing the 3D model. This device is responsible for the additive manufacturing process, which builds up the object layer by layer from the material.</skos:scopeNote>
    </owl:Class>
    


    <!-- https://photogrammetry.altervista.org/items/show/167#F80_Printed_Digital_Twin -->


    <owl:Class rdf:about="https://photogrammetry.altervista.org/items/show/167#F80_Printed_Digital_Twin">
        <rdfs:subClassOf rdf:resource="http://cidoc-crm.org/cidoc-crm/7.1.3/E18_Physical_Thing#E18_Physical_Thing"/>
        <rdfs:label xml:lang="en">PrintedTridimensionalDigitalTwin</rdfs:label>
        <skos:definition xml:lang="en">Definition of the class F80 Printed Digital Twin as a subclass of E18 Physical Thing</skos:definition>
        <skos:example xml:lang="en">&quot;A 3D printed model of a historical structure used for educational purposes in a museum, allowing visitors to explore architectural details in a hands-on manner.&quot;</skos:example>
        <skos:example xml:lang="en">&quot;A prototype of a product that has been physically produced from its digital twin for testing and evaluation, enabling designers to assess form, fit, and function before mass production.&quot;</skos:example>
        <skos:scopeNote xml:lang="en">The Printed Digital Twin class refers to the tangible object that results from the 3D printing of a digital twin model. This physical representation retains the features and characteristics of the original digital design and serves various purposes, including prototyping, display, and educational use.</skos:scopeNote>
    </owl:Class>
    


    <!-- https://photogrammetry.altervista.org/items/show/168#F81_3D_Model_for_G.I.S. -->


    <owl:Class rdf:about="https://photogrammetry.altervista.org/items/show/168#F81_3D_Model_for_G.I.S.">
        <rdfs:subClassOf rdf:resource="https://photogrammetry.altervista.org/items/show/188#F102:_3D_Digital_Asset"/>
        <rdfs:label xml:lang="en">ExportedGIS3DModel</rdfs:label>
        <skos:definition xml:lang="en">Definition of the class F81 3D Model for G.I.S. as a subclass of D9 Data Object</skos:definition>
        <skos:example xml:lang="en">&quot;A 3D representation of urban infrastructure, adjusted for integration with city planning GIS applications, enabling planners to visualize and analyze spatial relationships and resource allocation.&quot;</skos:example>
        <skos:example xml:lang="en">&quot;A topographical model of a geographical area prepared for environmental analysis within a GIS framework, facilitating assessments of land use, resource management, and ecological impacts.&quot;</skos:example>
        <skos:scopeNote xml:lang="en">The 3D Model for G.I.S. class refers to a 3D model that has been specifically modified and prepared for implementation within a Geographic Information System (GIS). This model is designed to meet the requirements of GIS applications, including spatial accuracy, scalability, and compatibility with various GIS data formats.</skos:scopeNote>
    </owl:Class>
    


    <!-- https://photogrammetry.altervista.org/items/show/169#F82_Reference_GIS_System -->


    <owl:Class rdf:about="https://photogrammetry.altervista.org/items/show/169#F82_Reference_GIS_System">
        <rdfs:subClassOf rdf:resource="http://www.cidoc-crm.org/extensions/crmdig/versions/4.0/D9_Data_Object#D9_Data_Object"/>
        <rdfs:label xml:lang="en">GISSystem</rdfs:label>
        <skos:definition xml:lang="en">Definition of the class F82 Reference GIS System as a subclass of D9 Data Object</skos:definition>
        <skos:example xml:lang="en">&quot;A conservation GIS employed in environmental management, integrating 3D models of natural landscapes to analyze habitat changes, biodiversity, and land use impacts.&quot;</skos:example>
        <skos:example xml:lang="en">&quot;A municipal GIS used for urban planning and zoning, where the 3D model represents building structures, allowing city planners to visualize spatial relationships and assess the impact of new developments.&quot;</skos:example>
        <skos:scopeNote xml:lang="en">The Reference GIS System class refers to the specific Geographic Information System in which the 3D model will be inserted. This system serves as the platform for managing, analyzing, and visualizing spatial data, including the 3D model.</skos:scopeNote>
    </owl:Class>
    


    <!-- https://photogrammetry.altervista.org/items/show/170#F83_GIS_Software -->


    <owl:Class rdf:about="https://photogrammetry.altervista.org/items/show/170#F83_GIS_Software">
        <rdfs:subClassOf rdf:resource="http://www.cidoc-crm.org/extensions/crmdig/versions/4.0/D14_Software#D14_Software"/>
        <rdfs:label xml:lang="en">GISSoftware</rdfs:label>
        <skos:definition xml:lang="en">Definition of the class F83 GIS Software as a subclass of D14 Software</skos:definition>
        <skos:example xml:lang="en">&quot;ArcGIS, a popular GIS software for mapping and spatial analysis, supporting the integration of 3D models to enhance geographical insights and decision-making processes.&quot;</skos:example>
        <skos:example xml:lang="en">&quot;QGIS, an open-source GIS application that allows users to work with 3D representations of spatial data, facilitating collaborative analysis and data sharing.&quot;</skos:example>
        <skos:scopeNote xml:lang="en">The GIS Software class refers to the specific software application used for managing and analyzing geographical information. This software supports the functionality necessary to incorporate 3D models into the GIS, enabling spatial analysis, visualization, and data manipulation.</skos:scopeNote>
    </owl:Class>
    


    <!-- https://photogrammetry.altervista.org/items/show/171#F84_3D_Model_for_Prospectus -->


    <owl:Class rdf:about="https://photogrammetry.altervista.org/items/show/171#F84_3D_Model_for_Prospectus">
        <rdfs:subClassOf rdf:resource="https://photogrammetry.altervista.org/items/show/188#F102:_3D_Digital_Asset"/>
        <rdfs:label xml:lang="en">Exported3DModelForProspectus</rdfs:label>
        <skos:definition xml:lang="en">Definition of the class F84 3D Model for Prospectus as a subclass of D9 Data Object</skos:definition>
        <skos:example xml:lang="en">&quot;A modified 3D model of a building used to create architectural plans and sections, facilitating detailed design reviews and construction documentation.&quot;</skos:example>
        <skos:example xml:lang="en">&quot;A terrain model used to generate topographic maps and orthophotos for environmental studies, supporting land use planning and conservation efforts.&quot;</skos:example>
        <skos:scopeNote xml:lang="en">The 3D Model for Prospectus class refers to a 3D model that has been specifically modified and prepared to derive plans, elevations, orthophotos, and other information regarding sections, topographical features, and architectural elements. This model serves as a foundational tool for generating accurate representations and documentation related to the spatial attributes of a structure or area.</skos:scopeNote>
    </owl:Class>
    


    <!-- https://photogrammetry.altervista.org/items/show/172#F85_CAD_Analysis -->


    <owl:Class rdf:about="https://photogrammetry.altervista.org/items/show/172#F85_CAD_Analysis">
        <rdfs:subClassOf rdf:resource="http://www.cidoc-crm.org/extensions/crmdig/versions/4.0/D7_Digital_Machine_Event#D7_Digital_Machine_Event"/>
        <rdfs:label xml:lang="en">Exporting_CADAnalysis</rdfs:label>
        <skos:definition xml:lang="en">Definition of the class F85 CAD Analysis as a subclass of D7 Digital Machine Event</skos:definition>
        <skos:example xml:lang="en">&quot;Analyzing a 3D terrain model to produce accurate orthophotos for cartographic purposes, enhancing geographical representation and analysis.&quot;</skos:example>
        <skos:example xml:lang="en">&quot;Using CAD software to create detailed floor plans and architectural drawings from a 3D model, facilitating design communication and project documentation.&quot;</skos:example>
        <skos:scopeNote xml:lang="en">The CAD Analysis class refers to the actions performed to extract plans, elevations, orthophotos, and other information regarding sections, topographical features, and architectural data from the 3D model. This process involves various analytical and computational techniques to ensure the accuracy and utility of the generated outputs.</skos:scopeNote>
    </owl:Class>
    


    <!-- https://photogrammetry.altervista.org/items/show/173#F86_Software_CAD -->


    <owl:Class rdf:about="https://photogrammetry.altervista.org/items/show/173#F86_Software_CAD">
        <rdfs:subClassOf rdf:resource="http://www.cidoc-crm.org/extensions/crmdig/versions/4.0/D14_Software#D14_Software"/>
        <rdfs:label xml:lang="en">CADSoftware</rdfs:label>
        <skos:definition xml:lang="en">Definition of the class F86 Software CAD as a subclass of D14 Software</skos:definition>
        <skos:example xml:lang="en">&quot;AutoCAD, a widely-used CAD software that allows architects and engineers to create precise 2D and 3D drawings and designs, streamlining the design process.&quot;</skos:example>
        <skos:example xml:lang="en">&quot;Revit, a BIM (Building Information Modeling) software that enables users to design buildings and infrastructure with integrated 3D modeling capabilities, enhancing collaboration among project stakeholders.&quot;</skos:example>
        <skos:scopeNote xml:lang="en">The Software CAD class refers to specific software applications used for Computer-Aided Design (CAD). This software supports the creation, modification, and analysis of 3D models to derive architectural and topographical information, facilitating detailed design and engineering processes.</skos:scopeNote>
    </owl:Class>
    


    <!-- https://photogrammetry.altervista.org/items/show/174#F87_3D_Model_Prospectus -->


    <owl:Class rdf:about="https://photogrammetry.altervista.org/items/show/174#F87_3D_Model_Prospectus">
        <rdfs:subClassOf rdf:resource="http://www.cidoc-crm.org/extensions/crmdig/versions/4.0/D9_Data_Object#D9_Data_Object"/>
        <rdfs:label xml:lang="en">ExportedCAD3DModelProspectus</rdfs:label>
        <skos:definition xml:lang="en">Definition of the class F87 3D Model Prospectus as a subclass of D9 Data Object</skos:definition>
        <skos:example xml:lang="en">&quot;A set of architectural elevations and floor plans derived from a 3D building model, providing essential information for construction and design validation.&quot;</skos:example>
        <skos:example xml:lang="en">&quot;An orthophoto map created from a topographical model after CAD analysis, serving as a precise representation of land features for environmental studies.&quot;</skos:example>
        <skos:scopeNote xml:lang="en">The 3D Model Prospectus class refers to the output products such as plans, orthophotos, and any type of information generated from the CAD analysis performed on the 3D model. This class encompasses the documentation and visual representations that emerge from the analytical processes.</skos:scopeNote>
    </owl:Class>
    


    <!-- https://photogrammetry.altervista.org/items/show/175#F88_Archaeometric_3D_Model -->


    <owl:Class rdf:about="https://photogrammetry.altervista.org/items/show/175#F88_Archaeometric_3D_Model">
        <rdfs:subClassOf rdf:resource="https://photogrammetry.altervista.org/items/show/188#F102:_3D_Digital_Asset"/>
        <rdfs:label xml:lang="en">ExportedArchaeometricTridimensionalDigitalTwin</rdfs:label>
        <skos:definition xml:lang="en">Definition of the class F88 Archaeometric 3D Model as a subclass of D9 Data Object</skos:definition>
        <skos:example xml:lang="en">&quot;A 3D scan of an ancient artifact prepared for materials analysis, enabling researchers to study composition, structural integrity, and historical context.&quot;</skos:example>
        <skos:example xml:lang="en">&quot;A detailed model of a historic building surface analyzed for degradation patterns, assisting in conservation efforts and restoration planning.&quot;</skos:example>
        <skos:scopeNote xml:lang="en">The Archaeometric 3D Model class refers to a 3D model that has been specifically prepared for archaeometric analysis, as well as for general analysis of the object&apos;s surface characteristics. This type of model is intended for detailed examination, allowing researchers to assess material properties, deterioration, and other relevant factors.</skos:scopeNote>
    </owl:Class>
    


    <!-- https://photogrammetry.altervista.org/items/show/176#F89_Project_Analysis -->


    <owl:Class rdf:about="https://photogrammetry.altervista.org/items/show/176#F89_Project_Analysis">
        <rdfs:subClassOf rdf:resource="http://www.cidoc-crm.org/extensions/crmdig/versions/4.0/D7_Digital_Machine_Event#D7_Digital_Machine_Event"/>
        <rdfs:label xml:lang="en">Exporting_ArchaeometricAnalysis</rdfs:label>
        <skos:definition xml:lang="en">Definition of the class F89 Project Analysis as a subclass of D7 Digital Machine Event</skos:definition>
        <skos:example xml:lang="en">&quot;Conducting a surface analysis of a 3D archaeological model to identify wear patterns, providing valuable data for understanding historical usage.&quot;</skos:example>
        <skos:example xml:lang="en">&quot;Performing a digital evaluation of a historical artifact to assess its preservation status, helping conservators determine necessary interventions.&quot;</skos:example>
        <skos:scopeNote xml:lang="en">The Project Analysis class refers to the digital operations performed to analyze the 3D model and study its surface in detail. This analysis may involve various techniques and methodologies aimed at revealing insights about the object&apos;s structure, condition, and materials.</skos:scopeNote>
    </owl:Class>
    


    <!-- https://photogrammetry.altervista.org/items/show/177#F90_Data_Log_Analysis -->


    <owl:Class rdf:about="https://photogrammetry.altervista.org/items/show/177#F90_Data_Log_Analysis">
        <rdfs:subClassOf rdf:resource="http://www.cidoc-crm.org/extensions/crmdig/versions/4.0/D9_Data_Object#D9_Data_Object"/>
        <rdfs:label xml:lang="en">ExportedArchaeometricDataLogAnalysis</rdfs:label>
        <skos:definition xml:lang="en">Definition of the class F90 Data Log Analysis as a subclass of D9 Data Object</skos:definition>
        <skos:example xml:lang="en">&quot;A CSV file detailing measurements and observations from a 3D surface analysis, capturing data points such as depth, texture, and anomalies.&quot;</skos:example>
        <skos:example xml:lang="en">&quot;A log of the parameters used in digital analysis processes, including any findings related to the object being studied, providing context for subsequent evaluations.&quot;</skos:example>
        <skos:scopeNote xml:lang="en">The Data Log Analysis class refers to a text file that contains information derived from the analysis or produced directly from the digital analysis processes. This file serves as a record of findings and observations, enabling further investigation and documentation.</skos:scopeNote>
    </owl:Class>
    


    <!-- https://photogrammetry.altervista.org/items/show/178#F91_Model_for_Interactive -->


    <owl:Class rdf:about="https://photogrammetry.altervista.org/items/show/178#F91_Model_for_Interactive">
        <rdfs:subClassOf rdf:resource="https://photogrammetry.altervista.org/items/show/188#F102:_3D_Digital_Asset"/>
        <rdfs:label xml:lang="en">ExportedTridimensionalDigitalTwinForInteractive</rdfs:label>
        <skos:definition xml:lang="en">Definition of the class F91 Model for Interactive as a subclass of D9 Data Object</skos:definition>
        <skos:example xml:lang="en">&quot;A 3D reconstruction of an archaeological site created for interactive educational software, allowing users to navigate through the site and access additional information about its history.&quot;
en</skos:example>
        <skos:example xml:lang="en">&quot;A digitally enhanced model of a historical building intended for virtual tours, enabling users to explore the interior and exterior while interacting with contextual information about architectural elements.&quot;</skos:example>
        <skos:scopeNote xml:lang="en">The Model for Interactive class refers to a 3D model that has been prepared and modified for display in an interactive digital presentation. This model is designed to enhance user engagement and provide an immersive experience in exploring the model&apos;s features and characteristics.</skos:scopeNote>
    </owl:Class>
    


    <!-- https://photogrammetry.altervista.org/items/show/179#F92_Interactive_Project_Implementation -->


    <owl:Class rdf:about="https://photogrammetry.altervista.org/items/show/179#F92_Interactive_Project_Implementation">
        <rdfs:subClassOf rdf:resource="http://www.cidoc-crm.org/extensions/crmdig/versions/4.0/D7_Digital_Machine_Event#D7_Digital_Machine_Event"/>
        <rdfs:label xml:lang="en">Exporting_InteractiveProjectImplementation</rdfs:label>
        <skos:definition xml:lang="en">Definition of the class F92 Interactive Project Implementation as a subclass of D7 Digital Machine Event</skos:definition>
        <skos:example xml:lang="en">&quot;Incorporating a 3D model into a virtual reality application for educational purposes, allowing students to explore historical sites in an immersive way.&quot;</skos:example>
        <skos:scopeNote xml:lang="en">The Interactive Project Implementation class refers to the process of integrating the Model for Interactive (F91) into a specific interactive visualization project. This activity encompasses the technical steps required to ensure that the model functions effectively within the interactive environment.</skos:scopeNote>
    </owl:Class>
    


    <!-- https://photogrammetry.altervista.org/items/show/180#F93_Interactive_Software -->


    <owl:Class rdf:about="https://photogrammetry.altervista.org/items/show/180#F93_Interactive_Software">
        <rdfs:subClassOf rdf:resource="http://www.cidoc-crm.org/extensions/crmdig/versions/4.0/D14_Software#D14_Software"/>
        <rdfs:label xml:lang="en">InteractiveProjectSoftware</rdfs:label>
        <skos:definition xml:lang="en">Definition of the class F93 Interactive Software as a subclass of D14 Software</skos:definition>
        <skos:example xml:lang="en">Unity: A powerful game engine commonly used for creating interactive applications, allowing developers to incorporate 3D models and develop immersive experiences across various platforms.</skos:example>
        <skos:example xml:lang="en">Unreal Engine: A comprehensive suite for game development and interactive content creation, providing high-fidelity graphics and tools for integrating complex 3D models into interactive environments.</skos:example>
        <skos:scopeNote xml:lang="en">The Interactive Software class refers to the software utilized to create the interactive project, such as Unity or other platforms designed for developing interactive visual experiences. This software supports the creation and integration of 3D models into engaging formats.</skos:scopeNote>
    </owl:Class>
    


    <!-- https://photogrammetry.altervista.org/items/show/181#F94_3D_Model_for_Database -->


    <owl:Class rdf:about="https://photogrammetry.altervista.org/items/show/181#F94_3D_Model_for_Database">
        <rdfs:subClassOf rdf:resource="https://photogrammetry.altervista.org/items/show/188#F102:_3D_Digital_Asset"/>
        <rdfs:label xml:lang="en">Exported3DModelForDatabase</rdfs:label>
        <skos:definition xml:lang="en">Definition of the class F94 3D Model for Database as a subclass of D9 Data Object</skos:definition>
        <skos:example xml:lang="en">A 3D representation of an archaeological artifact prepared for storage in a digital archive: This model includes specific metadata and formatting to ensure compatibility with the database schema, allowing for easy access and analysis by researchers.</skos:example>
        <skos:example xml:lang="en">A model of a historical site optimized for inclusion in a geographic database: This 3D model is designed with spatial data attributes and optimized for geographic information systems (GIS), enabling users to integrate it with other geospatial data for comprehensive analysis.</skos:example>
        <skos:scopeNote xml:lang="en">The 3D Model for Database class refers to a 3D model that has been modified and prepared for upload to a project database. This model is structured to meet the requirements of database management systems and is intended for efficient storage, retrieval, and management within a digital environment.</skos:scopeNote>
    </owl:Class>
    


    <!-- https://photogrammetry.altervista.org/items/show/182#F95_Database_Project_Implementation -->


    <owl:Class rdf:about="https://photogrammetry.altervista.org/items/show/182#F95_Database_Project_Implementation">
        <rdfs:subClassOf rdf:resource="http://www.cidoc-crm.org/extensions/crmdig/versions/4.0/D7_Digital_Machine_Event#D7_Digital_Machine_Event"/>
        <rdfs:label xml:lang="en">Exporting_DatabaseImplementation</rdfs:label>
        <skos:definition xml:lang="en">Definition of the class F95 Database Project Implementation as a subclass of D7 Digital Machine Event</skos:definition>
        <skos:example xml:lang="en">The process of importing a 3D model into a cultural heritage database: This activity includes validating the model&apos;s format, ensuring compliance with database schema, and performing quality checks to facilitate accurate representation and retrieval.</skos:example>
        <skos:example xml:lang="en">Uploading a digital representation of a building to a municipal database for urban planning: This implementation involves configuring the model to align with urban planning standards, tagging it with relevant metadata, and ensuring it integrates seamlessly with existing data layers within the database.</skos:example>
        <skos:scopeNote xml:lang="en">The Database Project Implementation class refers to the activity of uploading the 3D model (F94) to a specific database. This process involves the technical steps necessary to ensure the model is correctly integrated and accessible within the database framework.</skos:scopeNote>
    </owl:Class>
    


    <!-- https://photogrammetry.altervista.org/items/show/183#F96_Database_Architecture -->


    <owl:Class rdf:about="https://photogrammetry.altervista.org/items/show/183#F96_Database_Architecture">
        <rdfs:subClassOf rdf:resource="http://www.cidoc-crm.org/extensions/crmdig/versions/4.0/D14_Software#D14_Software"/>
        <rdfs:label xml:lang="en">DatabaseArchitectureSoftware</rdfs:label>
        <skos:definition xml:lang="en">Definition of the class F96 Database Architecture as a subclass of D14 Software</skos:definition>
        <skos:example xml:lang="en">SQL-based databases used for managing 3D models in cultural heritage projects, such as Omeka-s: This architecture supports a structured approach to data management, allowing for the storage of complex data types, including multimedia files, alongside associated metadata.</skos:example>
        <skos:example xml:lang="en">Wikibase: This platform offers a flexible architecture for storing and retrieving 3D models with rich semantic data, enabling collaborative editing and querying capabilities that enhance accessibility and integration with other datasets.</skos:example>
        <skos:scopeNote xml:lang="en">The Database Architecture class refers to the software and/or specific architecture utilized in the database where the 3D model (F94) has been uploaded. This may include details about the database management system, data structure, and design principles that facilitate effective data storage and access.</skos:scopeNote>
    </owl:Class>
    


    <!-- https://photogrammetry.altervista.org/items/show/184#F97_AR_3D_Model -->


    <owl:Class rdf:about="https://photogrammetry.altervista.org/items/show/184#F97_AR_3D_Model">
        <rdfs:subClassOf rdf:resource="https://photogrammetry.altervista.org/items/show/188#F102:_3D_Digital_Asset"/>
        <rdfs:label xml:lang="en">ExportedAR3DModel</rdfs:label>
        <skos:definition xml:lang="en">Definition of the class F97 AR 3D Model as a subclass of D9 Data Object</skos:definition>
        <skos:example xml:lang="en">A 3D reconstruction of a historical site intended for an AR application: This model allows users to visualize and interact with the historical site in real time, integrating virtual elements with the physical environment to provide contextual information.</skos:example>
        <skos:example xml:lang="en">A virtual artifact designed to be viewed in a mixed reality setting: This model enhances educational experiences by enabling users to examine and manipulate digital representations of artifacts while simultaneously engaging with their physical surroundings.</skos:example>
        <skos:scopeNote xml:lang="en">The AR 3D Model class refers to a 3D model that has been modified and prepared for implementation in an Augmented Reality (AR) or Mixed Reality (MR) project. This model is designed to interact with real-world environments and enhance user experiences through digital overlays.</skos:scopeNote>
    </owl:Class>
    


    <!-- https://photogrammetry.altervista.org/items/show/185#F98_AR/MR_Project_Implementation -->


    <owl:Class rdf:about="https://photogrammetry.altervista.org/items/show/185#F98_AR/MR_Project_Implementation">
        <rdfs:subClassOf rdf:resource="http://www.cidoc-crm.org/extensions/crmdig/versions/4.0/D7_Digital_Machine_Event#D7_Digital_Machine_Event"/>
        <rdfs:label xml:lang="en">Exporting_AR-MRProjectImplementation</rdfs:label>
        <skos:definition xml:lang="en">Definition of the class F98 AR/MR Project Implementation as a subclass of D7 Digital Machine Event</skos:definition>
        <skos:example xml:lang="en">Integrating a virtual object into a mixed reality experience for educational purposes: This step includes aligning the virtual object with real-world surroundings, allowing users to interact with both digital and physical elements seamlessly during an educational activity.</skos:example>
        <skos:example xml:lang="en">Loading a 3D model into an AR application for mobile devices: This process involves preparing the model for compatibility with mobile AR software, ensuring it can be rendered accurately and interactively in a real-world context.</skos:example>
        <skos:scopeNote xml:lang="en">The AR/MR Project Implementation class refers to the process of integrating the AR 3D model (F97) into a specific Augmented Reality or Mixed Reality project. This includes the technical steps required to ensure the model functions properly within the AR/MR environment.</skos:scopeNote>
    </owl:Class>
    


    <!-- https://photogrammetry.altervista.org/items/show/186#F99_AR_Software_Modelling -->


    <owl:Class rdf:about="https://photogrammetry.altervista.org/items/show/186#F99_AR_Software_Modelling">
        <rdfs:subClassOf rdf:resource="http://www.cidoc-crm.org/extensions/crmdig/versions/4.0/D14_Software#D14_Software"/>
        <rdfs:label xml:lang="en">AR-MRImplementationSoftware</rdfs:label>
        <skos:definition xml:lang="en">Definition of the class F99 AR Software Modelling as a subclass of D14 Software</skos:definition>
        <skos:example xml:lang="en">Unity: A versatile game engine widely used for developing AR applications, providing tools for 3D modeling, animation, and interaction within augmented environments.</skos:example>
        <skos:example xml:lang="en">Vuforia: An AR development platform that enables developers to create robust augmented reality experiences by recognizing images and objects in real-time, seamlessly integrating virtual content with the physical world.</skos:example>
        <skos:scopeNote xml:lang="en">The AR Software Modelling class refers to the software used in the Augmented Reality or Mixed Reality project where the AR 3D model (F97) has been loaded. This software facilitates the creation and deployment of interactive AR experiences.</skos:scopeNote>
    </owl:Class>
    


    <!-- https://photogrammetry.altervista.org/items/show/187#F101_Survey_Phase -->


    <owl:Class rdf:about="https://photogrammetry.altervista.org/items/show/187#F101_Survey_Phase">
        <rdfs:subClassOf rdf:resource="http://cidoc-crm.org/cidoc-crm/7.1.3/E29_Design_or_Procedure#E29_Design_or_Procedure"/>
        <rdfs:label xml:lang="en">SurveyPhase</rdfs:label>
        <skos:definition xml:lang="en">Definition of the class F101 Survey Phase as a subclass of E29 Design and Procedure</skos:definition>
        <skos:example xml:lang="en">The Survey Phase involved an initial site walk-through and preparation, followed by the actual data acquisition using a terrestrial laser scanner.</skos:example>
        <skos:scopeNote xml:lang="en">The Survey Phase refers to a stage within the acquisition process, which can be divided into various moments such as acquisition, processing, and analysis. Each phase within the survey process addresses a specific task or set of tasks that contribute to the overall objective of collecting spatial, visual, or other relevant data about an object or environment. A Survey Phase may encompass the preparation of equipment, calibration, field operations, and initial data checks, ensuring that the collected data adheres to predefined technical standards. The phases may vary depending on the project’s design and procedural requirements, contributing to the systematic and reproducible execution of the survey.</skos:scopeNote>
    </owl:Class>
    


    <!-- https://photogrammetry.altervista.org/items/show/188#F102:_3D_Digital_Asset -->


    <owl:Class rdf:about="https://photogrammetry.altervista.org/items/show/188#F102:_3D_Digital_Asset">
        <rdfs:subClassOf rdf:resource="http://www.cidoc-crm.org/extensions/crmdig/versions/4.0/D9_Data_Object#D9_Data_Object"/>
        <rdfs:label xml:lang="en">TridimensionalDigitalAsset</rdfs:label>
        <skos:definition xml:lang="en">Definition of the class F102 3D Digital Asset as a subclass of D9 Data Object</skos:definition>
        <skos:example xml:lang="en">A 3D Digital Asset was created as a Textured 3D Mesh (F29) of a historical monument, used for digital documentation and preservation.</skos:example>
        <skos:example xml:lang="en">A 3D Model for GIS (F81) was developed to integrate geographical and cultural heritage data into a spatial analysis platform.</skos:example>
        <skos:example xml:lang="en">The 3D Digital Twin (F100) of an industrial component was generated for predictive maintenance and simulations.</skos:example>
        <skos:scopeNote xml:lang="en">The 3D Digital Asset class refers to a broad category of digital objects that represent three-dimensional entities. This class includes various specific types of 3D models, such as F100 3D Digital Twin, F28 3D Mesh, F29 Textured 3D Mesh, F76 3D Model for 3D Print, F81 3D Model for GIS, F84 3D Model for Prospectuses, F88 Archaeometric 3D Model, F91 3D Model for Interactive, F94 3D Model for Database, and F97 AR 3D Model.
A 3D Digital Asset is defined by its ability to represent surfaces, volumes, and textures of objects in a coherent and structured manner, typically through vertices, edges, faces, or other geometric components (such as meshes) that form the basis of digital three-dimensional models. These assets are often the result of post-processing stages that follow raw data collection, such as point clouds, and include enhanced visual and structural information like textures, color mapping, or other metadata related to the object&apos;s properties or context.
It is important to note that Point Clouds (as represented by F26 Point Cloud and F27 Dense Point Cloud) are excluded from this class. Point clouds are raw collections of data points in a three-dimensional space that define the surface of an object or scene without structured geometric relationships (e.g., faces, volumes). While point clouds represent a step in the acquisition process, they lack the interconnected geometry and texturing that are characteristic of 3D Digital Assets. A 3D Digital Asset, on the other hand, contains processed, refined, and sometimes enriched information, making it suitable for various applications, including simulations, renderings, interactive platforms, and analysis tools.</skos:scopeNote>
    </owl:Class>
    


    <!-- https://photogrammetry.altervista.org/items/show/189#F103:_Calibration_(Camera_Calibration) -->


    <owl:Class rdf:about="https://photogrammetry.altervista.org/items/show/189#F103:_Calibration_(Camera_Calibration)">
        <rdfs:subClassOf rdf:resource="https://photogrammetry.altervista.org/items/show/132#F46:_Matching"/>
        <rdfs:label xml:lang="en">Processing_Matching_Calibration</rdfs:label>
        <skos:definition xml:lang="en">F103: Calibration (Camera Calibration)

Subclass of:
F46 Matching</skos:definition>
        <skos:example xml:lang="en">A camera calibration (F103) was performed prior to a photogrammetric survey to correct for optical lens distortion and improve the accuracy of the generated 3D model.</skos:example>
        <skos:example xml:lang="en">During image acquisition for an archaeological project, camera calibration (F103) enabled the collection of optimized data for subsequent 3D model creation.</skos:example>
        <skos:example xml:lang="en">The calibration (F103) was applied to correctly align multiple images in photogrammetry software, ensuring an accurate reconstruction of the 3D scene.</skos:example>
        <skos:scopeNote xml:lang="en">The F103 Calibration class represents the camera calibration process used during photogrammetric data acquisition. Camera calibration is a crucial step in the photogrammetric workflow to ensure that the captured images are accurately mapped to a three-dimensional coordinate system and to correct any intrinsic and extrinsic optical distortions in the camera. The class describes the calibration parameters related to the camera, including focal length, principal point, radial and tangential distortion coefficients, and other optical properties.
Calibration aims to enhance the quality and accuracy of the 3D models generated through photogrammetry by minimizing systematic errors that may affect the final result. This process can be carried out before or during the image acquisition phase and typically involves a known set of reference points or calibration grids to determine the camera’s geometric properties.
F103 is part of the broader process of matching and optimizing data in the context of digital surveying, represented by F46 Matching, of which F103 is a subclass. Calibration ensures accurate correspondence between image data and the physical world, facilitating the subsequent processing and 3D modeling phases.</skos:scopeNote>
    </owl:Class>
    


    <!-- https://photogrammetry.altervista.org/items/show/190#F104:_Registration_(Fusion_of_Multiple_Point_Clouds_or_3D_Models) -->


    <owl:Class rdf:about="https://photogrammetry.altervista.org/items/show/190#F104:_Registration_(Fusion_of_Multiple_Point_Clouds_or_3D_Models)">
        <rdfs:subClassOf rdf:resource="https://photogrammetry.altervista.org/items/show/113#F27_Densified_Point_Cloud"/>
        <rdfs:label xml:lang="en">ProcessedDensifiedPointCloudRegistration</rdfs:label>
        <skos:definition xml:lang="en">F104: Registration (Fusion of Multiple Point Clouds or 3D Models)

Subclass of:

F27 Densified Cloud Point</skos:definition>
        <skos:example xml:lang="en">Automated registration (F104) was applied to fuse point clouds captured from aerial and ground-based photogrammetry, creating a comprehensive 3D model for analysis.</skos:example>
        <skos:example xml:lang="en">During the photogrammetric survey of a large site, registration (F104) was used to merge multiple 3D models captured from different sections, resulting in a unified representation of the site.</skos:example>
        <skos:example xml:lang="en">The registration (F104) of two overlapping point clouds from different vantage points was performed to generate a complete 3D model of an ancient temple.</skos:example>
        <skos:scopeNote xml:lang="en">The F104 Registration class refers to the process of aligning and merging multiple point clouds or 3D models into a single, coherent model. This class captures the concept of registration, a key step in photogrammetry and 3D reconstruction workflows where data collected from different viewpoints or sources is combined to create a comprehensive representation of an object or scene.
In this process, registration involves the precise alignment of overlapping regions of point clouds or 3D models, ensuring that they share a common coordinate system and that the surfaces match accurately. This can be done manually or, more commonly, through automated algorithms that minimize alignment errors by detecting corresponding points or features across the datasets.
Registration is an essential step, especially when working with large datasets or complex scenes that require the integration of multiple scans. This class describes the methodology and actions taken to perform the registration, including the matching of common features, alignment algorithms used, and optimization techniques to reduce errors.
F104 is a subclass of F27 Densified Cloud Point, as registration often begins with individual densified point clouds—highly detailed datasets representing surfaces—which are then combined into a unified model for further processing or analysis.</skos:scopeNote>
    </owl:Class>
    


    <!-- https://photogrammetry.altervista.org/items/show/191#F105:_Interrogation_Tools -->


    <owl:Class rdf:about="https://photogrammetry.altervista.org/items/show/191#F105:_Interrogation_Tools">
        <rdfs:subClassOf rdf:resource="http://www.cidoc-crm.org/extensions/crmdig/versions/4.0/D14_Software#D14_Software"/>
        <rdfs:label xml:lang="en">InterrogationToolsSoftware</rdfs:label>
        <skos:definition xml:lang="en">F105: Interrogation Tools (Digital Instruments for Measuring Cloud Points or 3D Models)
Subclass of:
D14 Software</skos:definition>
        <skos:example xml:lang="en">A curvature analysis tool (F105) was used to evaluate the surface smoothness of a digital 3D model of an ancient sculpture.</skos:example>
        <skos:example xml:lang="en">A point cloud comparison tool (F105) was employed to assess differences between two scans of a building facade taken months apart to monitor structural changes.</skos:example>
        <skos:example xml:lang="en">Software-based tools (F105) were applied to a dense point cloud to measure the volume of an archaeological excavation site.</skos:example>
        <skos:example xml:lang="en">Texture mapping interrogation software (F105) was utilized to assess how accurately textures were applied to a 3D model for virtual exhibition purposes.</skos:example>
        <skos:scopeNote xml:lang="en">The F105 Interrogation Tools class refers to software-based tools and algorithms used for measuring, analyzing, and manipulating Cloud Points or 3D Models in a digital environment. This class includes a variety of specialized software solutions, plugins, or standalone programs that allow users to perform precise measurements on 3D digital representations, such as calculating distances, volumes, surface areas, and other geometrical or spatial properties.
These interrogation tools are integral to post-processing and analysis in photogrammetry and 3D modeling workflows. They enable deeper examination and understanding of 3D data by applying advanced algorithms or providing user-friendly interfaces to visualize and interact with the data. Examples of functions provided by F105 Interrogation Tools include surface analysis, point cloud comparison, texture mapping, and deformation tracking.
By being a subclass of D14 Software, F105 reflects that the tools in this class are entirely software-based digital devices rather than hardware, and are designed to process and interact with digital models or datasets within a virtual environment.</skos:scopeNote>
    </owl:Class>
    


    <!-- https://photogrammetry.altervista.org/items/show/286#F106_Acquisition_Location_Type -->


    <owl:Class rdf:about="https://photogrammetry.altervista.org/items/show/286#F106_Acquisition_Location_Type">
        <rdfs:subClassOf rdf:resource="http://cidoc-crm.org/cidoc-crm/7.1.3/E55_Type#E55_Type"/>
        <rdfs:label xml:lang="en">acquisition_location_type</rdfs:label>
        <skos:definition xml:lang="en">F106 Acquisition Location Type

Subclass of: E55 Type</skos:definition>
        <skos:example xml:lang="en">An indoor environment with low light, such as a museum display room.</skos:example>
        <skos:example xml:lang="en">An outdoor archaeological site without additional lighting.</skos:example>
        <skos:scopeNote xml:lang="en">The Acquisition Location Type class categorizes the setting in which data acquisition took place. It specifies whether the location was outdoors, indoors with natural lighting, indoors with controlled lighting, in a dark space (such as a cave), outdoors with no natural lighting, outdoors with supplementary artificial lighting, or entirely illuminated by artificial sources.</skos:scopeNote>
    </owl:Class>
    


    <!-- https://photogrammetry.altervista.org/items/show/287#F108_Calibration_of_the_Instrument -->


    <owl:Class rdf:about="https://photogrammetry.altervista.org/items/show/287#F108_Calibration_of_the_Instrument">
        <rdfs:subClassOf rdf:resource="https://photogrammetry.altervista.org/admin/items/show/88#F2_Acquisition"/>
        <rdfs:label xml:lang="en">Acquisition_InstrumentCalibration</rdfs:label>
        <skos:definition xml:lang="en">F108 Calibration of the Instrument
 
Subclass of: F2 Acquisition</skos:definition>
        <skos:example xml:lang="en">Calibration of a fixed photogrammetry camera system for high-resolution artifact capture.</skos:example>
        <skos:example xml:lang="en">Pre-acquisition calibration of a laser scanner.</skos:example>
        <skos:scopeNote xml:lang="en">The Calibration of the Instrument class records the calibration process of the acquisition device, such as a camera, laser scanner, fixed-camera photogrammetry system (e.g., ATOS III), or LiDAR. This includes any calibration procedures conducted before acquisition or throughout the data capture process to ensure accuracy and reliability in measurement.</skos:scopeNote>
    </owl:Class>
    


    <!-- https://photogrammetry.altervista.org/items/show/288#F109_Marker_and_Calibration_Tools -->


    <owl:Class rdf:about="https://photogrammetry.altervista.org/items/show/288#F109_Marker_and_Calibration_Tools">
        <rdfs:subClassOf rdf:resource="https://photogrammetry.altervista.org/items/show/95#F9_Acquisition_Device"/>
        <rdfs:label xml:lang="en">AcquisitionDeviceMarker&amp;Calibration</rdfs:label>
        <skos:definition xml:lang="en">F109 Marker and Calibration Tools

Subclass of: F9 Acquisition Device</skos:definition>
        <skos:example xml:lang="en">Markers used in photogrammetry software for real-time calibration.</skos:example>
        <skos:example xml:lang="en">Prisms applied in total station systems for external coordinate accuracy.</skos:example>
        <skos:scopeNote xml:lang="en">The Marker and Calibration Tools class encompasses all tools used for instrument calibration, including markers placed prior to acquisition (e.g., those required by fixed-camera systems like ATOS III) and those used during data capture (such as markers for software like Agisoft). This class also includes total station prisms and any external coordinate assignment tools.</skos:scopeNote>
    </owl:Class>
    


    <!-- https://photogrammetry.altervista.org/items/show/89#F3_Processing -->


    <owl:Class rdf:about="https://photogrammetry.altervista.org/items/show/89#F3_Processing">
        <rdfs:subClassOf rdf:resource="http://www.cidoc-crm.org/extensions/crmdig/versions/4.0/D7_Digital_Machine_Event#D7_Digital_Machine_Event"/>
        <rdfs:label xml:lang="en">Processing</rdfs:label>
        <skos:definition xml:lang="en"># Definition of the class F3 Processing as a subclass of D7 Digital Machine Event
:F3_Processing rdf:type skos:Concept ;</skos:definition>
        <skos:example xml:lang="en">&quot;The processing of Bayman&apos;s photographs of the Buddha (A. Gruen 2004).&quot; ;</skos:example>
        <skos:example xml:lang="en">&quot;The processing of photographs of the photogrammetric survey of a wild boar jaw from the Minamikata site (Lauro 2019).&quot; ;</skos:example>
        <skos:scopeNote xml:lang="en">&quot;Processing in photogrammetry involves transforming raw data files into usable outputs. This includes validating image quality, stitching photographs, generating 3D models, and correcting errors like texture and polygon mismatches. It ensures data consistency, enhances detail accuracy, and prepares the images for further modeling and analysis in archaeological contexts. This specific action is in a state of dependence on the RawDataFile and on the Acquisition action and although intentional and therefore Activity depends on the choices made in the previous classes.&quot; ;</skos:scopeNote>
    </owl:Class>
    


    <!-- https://photogrammetry.altervista.org/items/show/90#F4_Modelling -->


    <owl:Class rdf:about="https://photogrammetry.altervista.org/items/show/90#F4_Modelling">
        <rdfs:subClassOf rdf:resource="http://www.cidoc-crm.org/extensions/crmdig/versions/4.0/D7_Digital_Machine_Event#D7_Digital_Machine_Event"/>
        <rdfs:label xml:lang="en">Modelling</rdfs:label>
        <skos:definition xml:lang="en">Definition of the class F4 Modelling as a subclass of D7 Digital Machine Event</skos:definition>
        <skos:example xml:lang="en">&quot;Mesh processing of an excavation sector of the Oglala National Grassland (Douglas 2015).&quot; ;</skos:example>
        <skos:example xml:lang="en">&quot;The reconstructive modeling of the Temple of Saturn at the Forum in Rome based on the photogrammetric survey of the structure (Koller 2009).&quot; ;</skos:example>
        <skos:scopeNote xml:lang="en">&quot;Modeling a 3D model involves creating and refining a digital representation of an object using specialized software. This process includes shaping the geometry and adding details to achieve an accurate and detailed virtual model, ready for analysis, visualization, or further processing. This is an activity confined to modeling, not to be confused with the Modeling instructions which already include the construction of the mesh, and which however are continuous with it. The modeling is driven by design and research considerations and has no aesthetic character, distinguishing itself from 3D design modeling, which is not the subject of this analysis.&quot; ;</skos:scopeNote>
    </owl:Class>
    


    <!-- https://photogrammetry.altervista.org/items/show/91#F5_Exporting -->


    <owl:Class rdf:about="https://photogrammetry.altervista.org/items/show/91#F5_Exporting">
        <rdfs:subClassOf rdf:resource="http://www.cidoc-crm.org/extensions/crmdig/versions/4.0/D7_Digital_Machine_Event#D7_Digital_Machine_Event"/>
        <rdfs:label xml:lang="en">Exporting</rdfs:label>
        <skos:definition xml:lang="en">Definition of the class F5 Exporting as a subclass of D7 Digital Machine Event</skos:definition>
        <skos:scopeNote xml:lang="en">&quot;Exporting involves the final stages of digital asset management. This phase encompasses exporting the processed data and archiving it for long-term preservation, ensuring the integrity and accessibility of digital records.&quot; ;</skos:scopeNote>
    </owl:Class>
    


    <!-- https://photogrammetry.altervista.org/items/show/92#F6_Acquisition_Raw_Data -->


    <owl:Class rdf:about="https://photogrammetry.altervista.org/items/show/92#F6_Acquisition_Raw_Data">
        <rdfs:subClassOf rdf:resource="http://www.cidoc-crm.org/extensions/crmdig/versions/4.0/D1_Digital_Object#D1_Digital_Object"/>
        <rdfs:label xml:lang="en">AcquisitionRawData</rdfs:label>
        <skos:definition xml:lang="en">Definition of the class F6 Acquisition Raw Data as a subclass of D1 Digital Object</skos:definition>
        <skos:scopeNote xml:lang="en">&quot;A Raw Data File contains unprocessed image data captured during photogrammetric surveys or digital information acquired by a laser scanner in the acquisition phase and not yet processed, or even the raw data of a LiDar survey. This class generally refers to any form of raw data resulting from the processing of a visible object as described in the F1 Survey Object class. These files preserve original color, detail, and metadata, crucial for accurate 3D model reconstruction. In archaeological contexts, they ensure comprehensive documentation of artifacts and structures, facilitating detailed analysis and interpretation. Raw Data files are distinguished as &apos;incomplete&apos; Conceptual Objects, in the sense that they are complete in their existence but their function is aimed at the processing which constitutes their reason for being. In photogrammetry it is the photographs that make up the survey.&quot; ;</skos:scopeNote>
    </owl:Class>
    


    <!-- https://photogrammetry.altervista.org/items/show/93#F7_Picture_Set -->


    <owl:Class rdf:about="https://photogrammetry.altervista.org/items/show/93#F7_Picture_Set">
        <rdfs:subClassOf rdf:resource="https://photogrammetry.altervista.org/items/show/92#F6_Acquisition_Raw_Data"/>
        <rdfs:label xml:lang="en">AcquisitionPictureSet</rdfs:label>
        <skos:definition xml:lang="en">Definition of the class F7 Picture Set as a subclass of F6 Acquisition Raw Data</skos:definition>
        <skos:example xml:lang="en">&quot;Photographs captured for a photogrammetric survey of an archaeological artifact or a historical building.&quot; ;</skos:example>
        <skos:example xml:lang="en">&quot;The 181 photographs that form the photogrammetric survey of the AFMNM005 jaw from the Minamikata excavation (Lauro 2019).&quot; ;</skos:example>
        <skos:scopeNote xml:lang="en">&quot;The Picture Set class refers to a collection of unprocessed digital images captured during the acquisition phase of a photogrammetric survey. These images, taken systematically from multiple viewpoints, are critical for reconstructing 3D models of surveyed objects or environments. Each picture within the set is treated as part of a coherent whole, as the completeness and quality of the survey depend on the collective set rather than individual photographs. Picture Sets preserve high-resolution details, color information, and metadata essential for subsequent processing stages, ensuring accurate spatial and geometric reconstructions.&quot; ;</skos:scopeNote>
    </owl:Class>
    


    <!-- https://photogrammetry.altervista.org/items/show/94#F8_Picture -->


    <owl:Class rdf:about="https://photogrammetry.altervista.org/items/show/94#F8_Picture">
        <rdfs:subClassOf rdf:resource="https://photogrammetry.altervista.org/items/show/93#F7_Picture_Set"/>
        <rdfs:label xml:lang="en">AcquisitionSinglePicture</rdfs:label>
        <skos:definition xml:lang="en">Definition of the class F8 Picture as a subclass of F7 Picture Set</skos:definition>
        <skos:example>&quot;A single high-resolution image of an archaeological artifact taken from a specific angle as part of a complete photogrammetric survey.&quot; ;</skos:example>
        <skos:scopeNote xml:lang="en">&quot;The Picture class represents a single digital photograph taken during the acquisition phase of a photogrammetric survey. Each Picture is an unprocessed image that contributes to the overall Picture Set and is crucial for reconstructing precise 3D models. These photographs capture detailed visual data, including color, texture, and spatial relationships, and serve as foundational raw data for photogrammetric processing. Although each Picture is valuable individually, its full significance is realized when integrated into the entire Picture Set.&quot; ;</skos:scopeNote>
    </owl:Class>
    


    <!-- https://photogrammetry.altervista.org/items/show/95#F9_Acquisition_Device -->


    <owl:Class rdf:about="https://photogrammetry.altervista.org/items/show/95#F9_Acquisition_Device">
        <rdfs:subClassOf rdf:resource="http://www.cidoc-crm.org/extensions/crmdig/versions/4.0/D8_Digital_Device#D8_Digital_Device"/>
        <rdfs:label xml:lang="en">AcquisitionDevice</rdfs:label>
        <skos:definition xml:lang="en">Definition of the class F9 Acquisition Device as a subclass of D8 Digital Device</skos:definition>
        <skos:scopeNote xml:lang="en">&quot;The Acquisition Device class represents any digital tool or instrument used during the acquisition phase of a photogrammetric survey or other data collection processes. These devices capture raw data such as photographs, point clouds, or laser scans, which serve as the foundation for subsequent processing and modeling. Examples of Acquisition Devices include digital cameras, 360° cameras, laser scanners, or LiDAR devices. Each device has specific technical capabilities that influence the quality and precision of the data collected, playing a critical role in the accuracy of the final 3D reconstruction.&quot; ;</skos:scopeNote>
    </owl:Class>
    


    <!-- https://photogrammetry.altervista.org/items/show/96#F10_Processing_Device -->


    <owl:Class rdf:about="https://photogrammetry.altervista.org/items/show/96#F10_Processing_Device">
        <rdfs:subClassOf rdf:resource="http://www.cidoc-crm.org/extensions/crmdig/versions/4.0/D8_Digital_Device#D8_Digital_Device"/>
        <rdfs:label xml:lang="en">ProcessingDevice</rdfs:label>
        <skos:definition xml:lang="en">Definition of the class F10 Processing Device as a subclass of D8 Digital Device</skos:definition>
        <skos:example xml:lang="en">A high-performance computer equipped with photogrammetry software (e.g., Agisoft Metashape or Zephyr) used to process survey images into 3D models.</skos:example>
        <skos:example xml:lang="en">A laser scanner that both collects and processes point cloud data directly within its onboard system.</skos:example>
        <skos:scopeNote xml:lang="en">&quot;The Processing Device class refers to any digital apparatus responsible for executing the computational tasks involved in the processing phase of data collected during a photogrammetric survey or other types of acquisition. This device typically includes computers running specialized software used to transform raw data (such as images or point clouds) into processed outputs like 3D models or Densified Point Clouds. In certain cases, such as laser scanners or other integrated systems, the same device used for acquisition may also perform data processing. The technical specifications and capabilities of the Processing Device directly influence the efficiency, speed, and quality of the final results.&quot; ;</skos:scopeNote>
    </owl:Class>
    


    <!-- https://photogrammetry.altervista.org/items/show/97#F11_Modelling_Device -->


    <owl:Class rdf:about="https://photogrammetry.altervista.org/items/show/97#F11_Modelling_Device">
        <rdfs:subClassOf rdf:resource="http://www.cidoc-crm.org/extensions/crmdig/versions/4.0/D8_Digital_Device#D8_Digital_Device"/>
        <rdfs:label xml:lang="en">ModellingDevice</rdfs:label>
        <skos:definition xml:lang="en">Definition of the class F11 Modelling Device as a subclass of D8 Digital Device</skos:definition>
        <skos:example xml:lang="en">&quot;A high-spec PC equipped with advanced GPUs to handle complex textures and lighting setups for archaeological 3D models.&quot; .</skos:example>
        <skos:example xml:lang="en">&quot;A workstation running 3D modeling software like Blender, Rhino, or Autodesk Maya used for finalizing and optimizing a 3D mesh created from photogrammetry.&quot; ;</skos:example>
        <skos:scopeNote xml:lang="en">&quot;The Modelling Device class refers to any digital apparatus specifically used to perform the modeling and transformation of 3D models derived from processed data during photogrammetric surveys or other similar workflows. This device is most commonly a high-performance computer equipped with specialized software for 3D modeling, texturing, and refinement of point clouds or meshes. The Modelling Device plays a crucial role in converting raw or processed data into final, high-quality 3D models ready for visualization, analysis, or export. Its processing power and graphic capabilities directly impact the accuracy, level of detail, and speed of the 3D model&apos;s refinement.&quot; ;</skos:scopeNote>
    </owl:Class>
    


    <!-- https://photogrammetry.altervista.org/items/show/99#F13_Acquisition_Method -->


    <owl:Class rdf:about="https://photogrammetry.altervista.org/items/show/99#F13_Acquisition_Method">
        <rdfs:subClassOf rdf:resource="http://cidoc-crm.org/cidoc-crm/7.1.3/E29_Design_or_Procedure#E29_Design_or_Procedure"/>
        <rdfs:label xml:lang="en">AcquisitionMethod</rdfs:label>
        <skos:definition xml:lang="en">Definition of the class F13 Acquisition Method as a subclass of E29 Design and Procedure</skos:definition>
        <skos:example xml:lang="en">&quot;The McGlone Method, which provides a standardized set of steps for capturing imagery in aerial photogrammetry surveys.&quot; .</skos:example>
        <skos:example xml:lang="en">:F13_Acquisition_Method skos:example &quot;The FOPPA protocol for archaeological photogrammetry, which prescribes specific camera settings and trajectories for artifact documentation.&quot; ;</skos:example>
        <skos:scopeNote xml:lang="en">&quot;The Acquisition Method class refers to the set of protocols, guidelines, or operational instructions that dictate how the acquisition process is conducted during a photogrammetric or other survey operation. This class captures the methodology adopted for data capture, specifying procedural elements such as device settings, trajectory planning, object coverage, and environmental considerations. The Acquisition Method can range from formalized protocols, such as the Metashape Manual or the McGlone Method, to custom or ad-hoc procedures defined for specific projects or objects. The choice of method impacts the completeness and quality of the raw data produced, influencing all subsequent phases of processing and modeling.&quot; ;
  skos:broader cidoc:E29_Design_and_Procedure .</skos:scopeNote>
    </owl:Class>
    


    <!-- 
    ///////////////////////////////////////////////////////////////////////////////////////
    //
    // Individuals
    //
    ///////////////////////////////////////////////////////////////////////////////////////
     -->


    


    <!-- http://www.semanticweb.org/vitto/ontologies/2024/9/PODS_1#ACQUISITION_of_AF_MNM_005__ALFAfsB001 -->


    <owl:NamedIndividual rdf:about="http://www.semanticweb.org/vitto/ontologies/2024/9/PODS_1#ACQUISITION_of_AF_MNM_005__ALFAfsB001">
        <rdf:type rdf:resource="https://photogrammetry.altervista.org/admin/items/show/88#F2_Acquisition"/>
        <skos:altLabel xml:lang="en">ALFAfsB001_Acquisition</skos:altLabel>
        <skos:definition xml:lang="en">Photogrammetric acquisition of the archaeological artifact AFMNM005, workflow chain ALFAfsB001. This pertains to a jawbone of a wild boar that has undergone anthropogenic manipulations.</skos:definition>
    </owl:NamedIndividual>
    


    <!-- http://www.semanticweb.org/vitto/ontologies/2024/9/PODS_1#AF_MNM_005_PROCESSING_ALFAfsB001 -->


    <owl:NamedIndividual rdf:about="http://www.semanticweb.org/vitto/ontologies/2024/9/PODS_1#AF_MNM_005_PROCESSING_ALFAfsB001">
        <rdf:type rdf:resource="https://photogrammetry.altervista.org/items/show/89#F3_Processing"/>
        <skos:altLabel xml:lang="en">ALFAfsB001_Processing</skos:altLabel>
        <skos:definition xml:lang="en">Processing of the photographs from the photogrammetric acquisition of the archaeological artifact AFMNM005, workflow chain ALFAfsB001. This pertains to a jawbone of a wild boar that has undergone anthropogenic manipulations.</skos:definition>
    </owl:NamedIndividual>
    


    <!-- http://www.semanticweb.org/vitto/ontologies/2024/9/PODS_1#AcquisitionDeviceType_for_ALFAfsB001 -->


    <owl:NamedIndividual rdf:about="http://www.semanticweb.org/vitto/ontologies/2024/9/PODS_1#AcquisitionDeviceType_for_ALFAfsB001">
        <rdf:type rdf:resource="https://photogrammetry.altervista.org/items/show/106#F20_Acquisition_Device_Type"/>
        <skos:definition xml:lang="en">Compact camera with built-in extendable lens</skos:definition>
    </owl:NamedIndividual>
    


    <!-- http://www.semanticweb.org/vitto/ontologies/2024/9/PODS_1#AcquisitionDeviceType_for_BETAfsF001 -->


    <owl:NamedIndividual rdf:about="http://www.semanticweb.org/vitto/ontologies/2024/9/PODS_1#AcquisitionDeviceType_for_BETAfsF001">
        <rdf:type rdf:resource="https://photogrammetry.altervista.org/items/show/106#F20_Acquisition_Device_Type"/>
        <skos:definition xml:lang="en">Reflex camera with standard lens</skos:definition>
    </owl:NamedIndividual>
    


    <!-- http://www.semanticweb.org/vitto/ontologies/2024/9/PODS_1#AcquisitionDeviceType_for_DELTArmA001 -->


    <owl:NamedIndividual rdf:about="http://www.semanticweb.org/vitto/ontologies/2024/9/PODS_1#AcquisitionDeviceType_for_DELTArmA001">
        <rdf:type rdf:resource="https://photogrammetry.altervista.org/items/show/106#F20_Acquisition_Device_Type"/>
        <skos:definition xml:lang="en">Reflex camera with standard lens</skos:definition>
    </owl:NamedIndividual>
    


    <!-- http://www.semanticweb.org/vitto/ontologies/2024/9/PODS_1#AcquisitionDevice_for_ALFAfsB001 -->


    <owl:NamedIndividual rdf:about="http://www.semanticweb.org/vitto/ontologies/2024/9/PODS_1#AcquisitionDevice_for_ALFAfsB001">
        <rdf:type rdf:resource="https://photogrammetry.altervista.org/items/show/95#F9_Acquisition_Device"/>
        <skos:definition xml:lang="en">Lumix DMC-TZ70 of Vittorio Lauro</skos:definition>
    </owl:NamedIndividual>
    


    <!-- http://www.semanticweb.org/vitto/ontologies/2024/9/PODS_1#AcquisitionDevice_for_BETAfsF001 -->


    <owl:NamedIndividual rdf:about="http://www.semanticweb.org/vitto/ontologies/2024/9/PODS_1#AcquisitionDevice_for_BETAfsF001">
        <rdf:type rdf:resource="https://photogrammetry.altervista.org/items/show/95#F9_Acquisition_Device"/>
        <skos:definition xml:lang="en">Canon EOS 1100D  from Okayama University, Deprtament of Antiquity</skos:definition>
    </owl:NamedIndividual>
    


    <!-- http://www.semanticweb.org/vitto/ontologies/2024/9/PODS_1#AcquisitionDevice_for_DELTArmA001 -->


    <owl:NamedIndividual rdf:about="http://www.semanticweb.org/vitto/ontologies/2024/9/PODS_1#AcquisitionDevice_for_DELTArmA001">
        <rdf:type rdf:resource="https://photogrammetry.altervista.org/items/show/95#F9_Acquisition_Device"/>
        <skos:definition xml:lang="en">EOS 2000D from Computer Science Department, University of Turin</skos:definition>
    </owl:NamedIndividual>
    


    <!-- http://www.semanticweb.org/vitto/ontologies/2024/9/PODS_1#Acquisition_Coordinates_of_ALFAfsB001 -->


    <owl:NamedIndividual rdf:about="http://www.semanticweb.org/vitto/ontologies/2024/9/PODS_1#Acquisition_Coordinates_of_ALFAfsB001">
        <rdf:type rdf:resource="https://photogrammetry.altervista.org/items/show/131#F45__Acquisition_Coordinates"/>
        <skos:definition>34°38&apos;45.15&quot;N 133°56&apos;17.43&quot;E (WGS84)</skos:definition>
    </owl:NamedIndividual>
    


    <!-- http://www.semanticweb.org/vitto/ontologies/2024/9/PODS_1#Acquisition_DESCRIPTION_ALFAfsB001 -->


    <owl:NamedIndividual rdf:about="http://www.semanticweb.org/vitto/ontologies/2024/9/PODS_1#Acquisition_DESCRIPTION_ALFAfsB001">
        <rdf:type rdf:resource="https://photogrammetry.altervista.org/items/show/130#F44_Acquisition_Description"/>
        <rdfs:comment>&apos;This is the acquisition record of the AF MNM 005 carried out with photogrammetry
Freehand spiral acquisition with three degrees of progressive inclination (75°, 45°, 15°)</rdfs:comment>
    </owl:NamedIndividual>
    


    <!-- http://www.semanticweb.org/vitto/ontologies/2024/9/PODS_1#Acquisition_Location_ALFAfsB001 -->


    <owl:NamedIndividual rdf:about="http://www.semanticweb.org/vitto/ontologies/2024/9/PODS_1#Acquisition_Location_ALFAfsB001">
        <rdf:type rdf:resource="https://photogrammetry.altervista.org/items/show/128#F42_Place_Of_Acquisition"/>
        <skos:definition xml:lang="en">The location where the photogrammetric survey of the artifact AFMNM005 was conducted (work chain ALFAfsB001).</skos:definition>
    </owl:NamedIndividual>
    


    <!-- http://www.semanticweb.org/vitto/ontologies/2024/9/PODS_1#Acquisition_Method_of_ALFAfsB001 -->


    <owl:NamedIndividual rdf:about="http://www.semanticweb.org/vitto/ontologies/2024/9/PODS_1#Acquisition_Method_of_ALFAfsB001">
        <rdf:type rdf:resource="https://photogrammetry.altervista.org/items/show/99#F13_Acquisition_Method"/>
        <skos:definition xml:lang="en">Acquisition Method  used for  the photogrammetric acquisition of the archaeological artifact AFMNM005, workflow chain ALFAfsB001. This pertains to a jawbone of a wild boar that has undergone anthropogenic manipulations. The acquisition method used complies with the FOPPA Manual</skos:definition>
    </owl:NamedIndividual>
    


    <!-- http://www.semanticweb.org/vitto/ontologies/2024/9/PODS_1#Acquisition_Method_of_DELTArmA001 -->


    <owl:NamedIndividual rdf:about="http://www.semanticweb.org/vitto/ontologies/2024/9/PODS_1#Acquisition_Method_of_DELTArmA001">
        <rdf:type rdf:resource="https://photogrammetry.altervista.org/items/show/99#F13_Acquisition_Method"/>
        <skos:definition xml:lang="en">Acquisition Method  used for  the photogrammetric acquisition of the archaeological artifact NO01, workflow chain DELTArmA001. This concerns a coloured glass bead. The acquisition method used complies with the FOPPA Manual</skos:definition>
    </owl:NamedIndividual>
    


    <!-- http://www.semanticweb.org/vitto/ontologies/2024/9/PODS_1#Acquisition_Method_of__BETAfsF001 -->


    <owl:NamedIndividual rdf:about="http://www.semanticweb.org/vitto/ontologies/2024/9/PODS_1#Acquisition_Method_of__BETAfsF001">
        <rdf:type rdf:resource="https://photogrammetry.altervista.org/items/show/99#F13_Acquisition_Method"/>
        <skos:definition xml:lang="en">Acquisition Method used for the photogrammetric acquisition of the funerary archaeological site Tobiotsuka Kofuna (TBZ_K), workflow chain BETAfs001. This consists of a stone burial chamber situated within a tumulus known as Kofun. The acquisition method used complies with the Agisoft Metashape Acquisition Manual</skos:definition>
    </owl:NamedIndividual>
    


    <!-- http://www.semanticweb.org/vitto/ontologies/2024/9/PODS_1#Acquisition_Phase_of_ALFAfsB001 -->


    <owl:NamedIndividual rdf:about="http://www.semanticweb.org/vitto/ontologies/2024/9/PODS_1#Acquisition_Phase_of_ALFAfsB001">
        <rdf:type rdf:resource="https://photogrammetry.altervista.org/items/show/119#F33_Acquisition_Phase"/>
        <skos:definition xml:lang="en">Acquisition Phase  of the photogrammetric acquisition of the archaeological artifact AFMNM005, workflow chain ALFAfsB001. This pertains to a jawbone of a wild boar that has undergone anthropogenic manipulations. The acquisition phase respected the scans and indications as established by the BeA-PG protocol</skos:definition>
    </owl:NamedIndividual>
    


    <!-- http://www.semanticweb.org/vitto/ontologies/2024/9/PODS_1#Acquisition_Phase_of_DELTArmA001 -->


    <owl:NamedIndividual rdf:about="http://www.semanticweb.org/vitto/ontologies/2024/9/PODS_1#Acquisition_Phase_of_DELTArmA001">
        <rdf:type rdf:resource="https://photogrammetry.altervista.org/items/show/119#F33_Acquisition_Phase"/>
        <skos:definition xml:lang="en">Acquisition Phase  of  the photogrammetric acquisition of the archaeological artifact NO01, workflow chain DELTArmA001. This concerns a coloured glass bead.

The acquisition phase respected the scans and indications as established by the FOPPA Manual</skos:definition>
    </owl:NamedIndividual>
    


    <!-- http://www.semanticweb.org/vitto/ontologies/2024/9/PODS_1#Acquisition_Raw_Data_of_ALFAfsB001 -->


    <owl:NamedIndividual rdf:about="http://www.semanticweb.org/vitto/ontologies/2024/9/PODS_1#Acquisition_Raw_Data_of_ALFAfsB001">
        <rdf:type rdf:resource="https://photogrammetry.altervista.org/items/show/92#F6_Acquisition_Raw_Data"/>
        <skos:definition xml:lang="en">Acquisition Raw Data from the photogrammetric acquisition of the archaeological artifact AFMNM005, workflow chain ALFAfsB001. This pertains to a jawbone of a wild boar that has undergone anthropogenic manipulations.  These Raw Data are the result of photogrammetric acquisition and are made up of a set of photographs</skos:definition>
    </owl:NamedIndividual>
    


    <!-- http://www.semanticweb.org/vitto/ontologies/2024/9/PODS_1#Acquisition_Raw_Data_of_DELTArmA001 -->


    <owl:NamedIndividual rdf:about="http://www.semanticweb.org/vitto/ontologies/2024/9/PODS_1#Acquisition_Raw_Data_of_DELTArmA001">
        <rdf:type rdf:resource="https://photogrammetry.altervista.org/items/show/92#F6_Acquisition_Raw_Data"/>
        <skos:definition xml:lang="en">Acquisition Raw Data from the photogrammetric acquisition of the archaeological artifact NO01, workflow chain DELTArmA001.  These Raw Data are the result of photogrammetric acquisition and are made up of a set of photographs</skos:definition>
    </owl:NamedIndividual>
    


    <!-- http://www.semanticweb.org/vitto/ontologies/2024/9/PODS_1#Acquisition_Raw_Data_of__BETAfsF001 -->


    <owl:NamedIndividual rdf:about="http://www.semanticweb.org/vitto/ontologies/2024/9/PODS_1#Acquisition_Raw_Data_of__BETAfsF001">
        <rdf:type rdf:resource="https://photogrammetry.altervista.org/items/show/92#F6_Acquisition_Raw_Data"/>
        <skos:definition xml:lang="en">Acquisition Raw Data from  the photogrammetric acquisition of the funerary archaeological site Tobiotsuka Kofuna (TBZ_K), workflow chain BETAfs001. This consists of a stone burial chamber situated within a tumulus known as Kofun.These Raw Data are the result of photogrammetric acquisition and are made up of a set of photographs</skos:definition>
    </owl:NamedIndividual>
    


    <!-- http://www.semanticweb.org/vitto/ontologies/2024/9/PODS_1#Acquisition_Software_for_BETAfsF001 -->


    <owl:NamedIndividual rdf:about="http://www.semanticweb.org/vitto/ontologies/2024/9/PODS_1#Acquisition_Software_for_BETAfsF001">
        <rdf:type rdf:resource="https://photogrammetry.altervista.org/items/show/116#F30_Acquisition_Software"/>
        <skos:definition xml:lang="en">Camera Software EOS 1.0.6</skos:definition>
    </owl:NamedIndividual>
    


    <!-- http://www.semanticweb.org/vitto/ontologies/2024/9/PODS_1#Acquisition_Software_for_DELTArmA001 -->


    <owl:NamedIndividual rdf:about="http://www.semanticweb.org/vitto/ontologies/2024/9/PODS_1#Acquisition_Software_for_DELTArmA001">
        <rdf:type rdf:resource="https://photogrammetry.altervista.org/items/show/116#F30_Acquisition_Software"/>
        <skos:definition xml:lang="en">Camera Software EOS 3.8.0 Utility</skos:definition>
    </owl:NamedIndividual>
    


    <!-- http://www.semanticweb.org/vitto/ontologies/2024/9/PODS_1#Acquisition_Trajectory_of_ALFAfsB001 -->


    <owl:NamedIndividual rdf:about="http://www.semanticweb.org/vitto/ontologies/2024/9/PODS_1#Acquisition_Trajectory_of_ALFAfsB001">
        <rdf:type rdf:resource="http://www.semanticweb.org/vitto/ontologies/2024/9/PODS_1Protocol_of_Ontological_Digital_Survey/extensions/versions/1_1/F12_Acquisition_Trajectory#F12_Acquisition_Trajectory"/>
        <skos:definition xml:lang="en">Acquisition Trajectory of ALFAfsB001     Acquisition Trajectory used for  the photogrammetric acquisition of the archaeological artifact AFMNM005, workflow chain ALFAfsB001. This pertains to a jawbone of a wild boar that has undergone anthropogenic manipulations. The selected trajectory is a Freehand Spiral as defined by the FOPPA Manual</skos:definition>
    </owl:NamedIndividual>
    


    <!-- http://www.semanticweb.org/vitto/ontologies/2024/9/PODS_1#Acquisition_Trajectory_of_DELTArmA001 -->


    <owl:NamedIndividual rdf:about="http://www.semanticweb.org/vitto/ontologies/2024/9/PODS_1#Acquisition_Trajectory_of_DELTArmA001">
        <rdf:type rdf:resource="http://www.semanticweb.org/vitto/ontologies/2024/9/PODS_1Protocol_of_Ontological_Digital_Survey/extensions/versions/1_1/F12_Acquisition_Trajectory#F12_Acquisition_Trajectory"/>
        <skos:definition xml:lang="en">Acquisition Trajectory used for  the photogrammetric acquisition of the archaeological artifact NO01, workflow chain DELTArmA001. This concerns a coloured glass bead. The selected trajectory is a Close Survey on a Rotating Base as defined by the FOPPA Manual</skos:definition>
    </owl:NamedIndividual>
    


    <!-- http://www.semanticweb.org/vitto/ontologies/2024/9/PODS_1#Acquisition_Trajectory_of__BETAfsF001 -->


    <owl:NamedIndividual rdf:about="http://www.semanticweb.org/vitto/ontologies/2024/9/PODS_1#Acquisition_Trajectory_of__BETAfsF001">
        <rdf:type rdf:resource="http://www.semanticweb.org/vitto/ontologies/2024/9/PODS_1Protocol_of_Ontological_Digital_Survey/extensions/versions/1_1/F12_Acquisition_Trajectory#F12_Acquisition_Trajectory"/>
        <skos:definition xml:lang="en">Acquisition Trajectory used for the photogrammetric acquisition of the funerary archaeological site Tobiotsuka Kofuna (TBZ_K), workflow chain BETAfs001. This consists of a stone burial chamber situated within a tumulus known as Kofun.The selected trajectory is an Interior Acquisition as defined by the Agisoft Metashape Manual</skos:definition>
    </owl:NamedIndividual>
    


    <!-- http://www.semanticweb.org/vitto/ontologies/2024/9/PODS_1#Acquisition_of_NO01_DELTArmA001 -->


    <owl:NamedIndividual rdf:about="http://www.semanticweb.org/vitto/ontologies/2024/9/PODS_1#Acquisition_of_NO01_DELTArmA001">
        <rdf:type rdf:resource="https://photogrammetry.altervista.org/admin/items/show/88#F2_Acquisition"/>
        <skos:altLabel xml:lang="en">DELTArmA001_Acquisition</skos:altLabel>
        <skos:definition xml:lang="en">Photogrammetric acquisition of the archaeological artifact NO01, workflow chain DELTArmA001. This concerns a colored glass bead.</skos:definition>
    </owl:NamedIndividual>
    


    <!-- http://www.semanticweb.org/vitto/ontologies/2024/9/PODS_1#Acquisition_of_TBZ._K._BETAfsF001 -->


    <owl:NamedIndividual rdf:about="http://www.semanticweb.org/vitto/ontologies/2024/9/PODS_1#Acquisition_of_TBZ._K._BETAfsF001">
        <rdf:type rdf:resource="https://photogrammetry.altervista.org/admin/items/show/88#F2_Acquisition"/>
        <skos:altLabel xml:lang="en">BETAfsF001_Acquisition</skos:altLabel>
        <skos:definition xml:lang="en">Photogrammetric acquisition of the funerary archaeological site Tobiotsuka Kofuna (TBZ_K), workflow chain BETAfs001. This consists of a stone burial chamber situated within a tumulus known as Kofun.</skos:definition>
    </owl:NamedIndividual>
    


    <!-- http://www.semanticweb.org/vitto/ontologies/2024/9/PODS_1#Color_Balance_Texture_of_ALFAfsB001 -->


    <owl:NamedIndividual rdf:about="http://www.semanticweb.org/vitto/ontologies/2024/9/PODS_1#Color_Balance_Texture_of_ALFAfsB001">
        <rdf:type rdf:resource="https://photogrammetry.altervista.org/items/show/148#F61_Color_Balance/Multiband_Texture"/>
        <skos:definition xml:lang="en">In the context of color balance for the texture of the 3D model obtained from the photogrammetric acquisition of the archaeological artifact AFMNM005, workflow chain ALFAfsB001 (which is a boar&apos;s jaw subjected to anthropic modifications), a color balancing technique combined with gradient ramps has been utilized.</skos:definition>
    </owl:NamedIndividual>
    


    <!-- http://www.semanticweb.org/vitto/ontologies/2024/9/PODS_1#Dense_Point_Cloud_Mesaurement_of_ALFAfsB001 -->


    <owl:NamedIndividual rdf:about="http://www.semanticweb.org/vitto/ontologies/2024/9/PODS_1#Dense_Point_Cloud_Mesaurement_of_ALFAfsB001">
        <rdf:type rdf:resource="https://photogrammetry.altervista.org/items/show/138#F52_Dense_Point_Cloud_Measurement"/>
        <skos:definition xml:lang="en">Measurement of the number of points comprising the densified point cloud obtained from the survey of the archaeological artifact AFMNM005, workflow chain ALFAfsB001 (which is a boar&apos;s jaw subjected to anthropic modifications).</skos:definition>
    </owl:NamedIndividual>
    


    <!-- http://www.semanticweb.org/vitto/ontologies/2024/9/PODS_1#Dense_Point_Cloud_of_DELTArmA001 -->


    <owl:NamedIndividual rdf:about="http://www.semanticweb.org/vitto/ontologies/2024/9/PODS_1#Dense_Point_Cloud_of_DELTArmA001">
        <rdf:type rdf:resource="https://photogrammetry.altervista.org/items/show/113#F27_Densified_Point_Cloud"/>
        <skos:definition xml:lang="en">Dense Point Cloud from the photogrammetric acquisition of the archaeological artifact NO01, workflow chain DELTArmA001. This concerns a coloured glass bead.</skos:definition>
    </owl:NamedIndividual>
    


    <!-- http://www.semanticweb.org/vitto/ontologies/2024/9/PODS_1#Dense_Point_Cloud_of__ALFAfsB001 -->


    <owl:NamedIndividual rdf:about="http://www.semanticweb.org/vitto/ontologies/2024/9/PODS_1#Dense_Point_Cloud_of__ALFAfsB001">
        <rdf:type rdf:resource="https://photogrammetry.altervista.org/items/show/113#F27_Densified_Point_Cloud"/>
        <skos:definition xml:lang="en">Dense Point Cloud from the photogrammetric acquisition of the archaeological artifact AFMNM005, workflow chain ALFAfsB001. This pertains to a jawbone of a wild boar that has undergone anthropogenic manipulations.</skos:definition>
    </owl:NamedIndividual>
    


    <!-- http://www.semanticweb.org/vitto/ontologies/2024/9/PODS_1#Densification_Alghoritm_for_ALFAfsB001 -->


    <owl:NamedIndividual rdf:about="http://www.semanticweb.org/vitto/ontologies/2024/9/PODS_1#Densification_Alghoritm_for_ALFAfsB001">
        <rdf:type rdf:resource="https://photogrammetry.altervista.org/items/show/108#F22_Densification_Algorithm_Type"/>
        <skos:definition xml:lang="en">mathematical detail unknown, certain use of decimation algorithms to manage point cloud density with application of density reduction techniques to optimize computational resources and optimization of point cloud management to reduce computational load.</skos:definition>
    </owl:NamedIndividual>
    


    <!-- http://www.semanticweb.org/vitto/ontologies/2024/9/PODS_1#Densification_Method_of_DELTArmA001 -->


    <owl:NamedIndividual rdf:about="http://www.semanticweb.org/vitto/ontologies/2024/9/PODS_1#Densification_Method_of_DELTArmA001">
        <rdf:type rdf:resource="https://photogrammetry.altervista.org/items/show/134#F48_Densification_Method"/>
        <skos:definition xml:lang="en">Densification Method of the Cloud Point in the context of the processing from  the photogrammetric acquisition of the archaeological artifact NO01, workflow chain DELTArmA001. This concerns a coloured glass bead.

Multi View Stereo Method</skos:definition>
    </owl:NamedIndividual>
    


    <!-- http://www.semanticweb.org/vitto/ontologies/2024/9/PODS_1#Densification_of_ALFAfsB001 -->


    <owl:NamedIndividual rdf:about="http://www.semanticweb.org/vitto/ontologies/2024/9/PODS_1#Densification_of_ALFAfsB001">
        <rdf:type rdf:resource="https://photogrammetry.altervista.org/items/show/133#F47:_Densification"/>
        <skos:definition xml:lang="en">Regarding the densification of the point cloud of the 3D Model of AFMNM005 (workflow chain ALFAfsB001) mathematical detail unknown, certain use of decimation algorithms to manage point cloud density with application of density reduction techniques to optimize computational resources and optimization of point cloud management to reduce computational load.</skos:definition>
    </owl:NamedIndividual>
    


    <!-- http://www.semanticweb.org/vitto/ontologies/2024/9/PODS_1#Densification_of_DELTArmA001. -->


    <owl:NamedIndividual rdf:about="http://www.semanticweb.org/vitto/ontologies/2024/9/PODS_1#Densification_of_DELTArmA001.">
        <rdf:type rdf:resource="http://www.semanticweb.org/vitto/ontologies/2024/9/PODS_1Protocol_of_Ontological_Digital_Survey/extensions/versions/1_1/F47_Densification#F47__Densification"/>
        <skos:definition xml:lang="en">Densification of the Cloud Point in the context of the processing from  the photogrammetric acquisition of the archaeological artifact NO01, workflow chain DELTArmA001. This concerns a coloured glass bead</skos:definition>
    </owl:NamedIndividual>
    


    <!-- http://www.semanticweb.org/vitto/ontologies/2024/9/PODS_1#DigitalScale_of_ALFAfsB001 -->


    <owl:NamedIndividual rdf:about="http://www.semanticweb.org/vitto/ontologies/2024/9/PODS_1#DigitalScale_of_ALFAfsB001">
        <rdf:type rdf:resource="https://photogrammetry.altervista.org/items/show/146#F59_Digital_Scale"/>
        <skos:definition>1:1</skos:definition>
    </owl:NamedIndividual>
    


    <!-- http://www.semanticweb.org/vitto/ontologies/2024/9/PODS_1#Eidotype_of_ALFAfsB001 -->


    <owl:NamedIndividual rdf:about="http://www.semanticweb.org/vitto/ontologies/2024/9/PODS_1#Eidotype_of_ALFAfsB001">
        <rdf:type rdf:resource="https://photogrammetry.altervista.org/items/show/126#F40_Eidotype"/>
        <skos:definition xml:lang="en">Eidotype  of the photogrammetric acquisition of the archaeological artifact AFMNM005, workflow chain ALFAfsB001. This pertains to a jawbone of a wild boar that has undergone anthropogenic manipulations. The Eidotype represents a sketch of the survey context, the acquisition set, the positioning of the lights and the possible trajectories that can be followed also taking into account the obstacles along the path. The Eidotype of ALFAfsB001 is originally in pen on paper and saved as JPG</skos:definition>
    </owl:NamedIndividual>
    


    <!-- http://www.semanticweb.org/vitto/ontologies/2024/9/PODS_1#Final_Use_of_ALFAfsB001 -->


    <owl:NamedIndividual rdf:about="http://www.semanticweb.org/vitto/ontologies/2024/9/PODS_1#Final_Use_of_ALFAfsB001">
        <rdf:type rdf:resource="https://photogrammetry.altervista.org/items/show/158#F71_Final_Use_of_Digital_Twin"/>
        <skos:altLabel xml:lang="en">ALFAfsB001_FinalUse</skos:altLabel>
        <skos:definition xml:lang="en">Final use of the 3D model resulting from the photogrammetric acquisition of the archaeological artifact AFMNM005, workflow chain ALFAfsB001. This artifact is a boar&apos;s jaw subjected to anthropic modifications. Final use refers to the application of the 3D model within the context of the project according to the established parameters.</skos:definition>
    </owl:NamedIndividual>
    


    <!-- http://www.semanticweb.org/vitto/ontologies/2024/9/PODS_1#GeometryType_for_ALFAfsB001 -->


    <owl:NamedIndividual rdf:about="http://www.semanticweb.org/vitto/ontologies/2024/9/PODS_1#GeometryType_for_ALFAfsB001">
        <rdf:type rdf:resource="https://photogrammetry.altervista.org/items/show/104#F18_Dominant_Geometry_Type"/>
        <skos:definition xml:lang="en">Parallelepiped by FOPPA Thesaurus</skos:definition>
    </owl:NamedIndividual>
    


    <!-- http://www.semanticweb.org/vitto/ontologies/2024/9/PODS_1#GeometryType_for_DELTArmA001 -->


    <owl:NamedIndividual rdf:about="http://www.semanticweb.org/vitto/ontologies/2024/9/PODS_1#GeometryType_for_DELTArmA001">
        <rdf:type rdf:resource="https://photogrammetry.altervista.org/items/show/104#F18_Dominant_Geometry_Type"/>
        <skos:definition xml:lang="en">Sphere by FOPPA Thesaurus</skos:definition>
    </owl:NamedIndividual>
    


    <!-- http://www.semanticweb.org/vitto/ontologies/2024/9/PODS_1#Implementation_in_Pject_BeaVIR_of_ALFAfsB001 -->


    <owl:NamedIndividual rdf:about="http://www.semanticweb.org/vitto/ontologies/2024/9/PODS_1#Implementation_in_Pject_BeaVIR_of_ALFAfsB001">
        <rdf:type rdf:resource="https://photogrammetry.altervista.org/items/show/179#F92_Interactive_Project_Implementation"/>
        <skos:altLabel xml:lang="en">ALFAfsB001_InteractiveImplementation</skos:altLabel>
        <skos:definition xml:lang="en">Implementation of the 3D model resulting from the photogrammetric acquisition of the archaeological artifact AFMNM005, workflow chain ALFAfsB001 (which is a boar&apos;s jaw subjected to anthropic modifications), in the interactive project BeA-VIR for the visualization of 3D models within the BeArchaeo project.</skos:definition>
    </owl:NamedIndividual>
    


    <!-- http://www.semanticweb.org/vitto/ontologies/2024/9/PODS_1#Interactive_Software_for_ALFAfsB001 -->


    <owl:NamedIndividual rdf:about="http://www.semanticweb.org/vitto/ontologies/2024/9/PODS_1#Interactive_Software_for_ALFAfsB001">
        <rdf:type rdf:resource="https://photogrammetry.altervista.org/items/show/180#F93_Interactive_Software"/>
        <skos:definition xml:lang="en">Unity 2021.3.33f1</skos:definition>
    </owl:NamedIndividual>
    


    <!-- http://www.semanticweb.org/vitto/ontologies/2024/9/PODS_1#Matching_Algorithm_for_ALFAfsB001 -->


    <owl:NamedIndividual rdf:about="http://www.semanticweb.org/vitto/ontologies/2024/9/PODS_1#Matching_Algorithm_for_ALFAfsB001">
        <rdf:type rdf:resource="https://photogrammetry.altervista.org/items/show/107#F21_Matching_Algorithm_Type"/>
        <skos:definition xml:lang="en">feature-based approach, probably integrating AI techniques</skos:definition>
    </owl:NamedIndividual>
    


    <!-- http://www.semanticweb.org/vitto/ontologies/2024/9/PODS_1#Matching_Method_of__DELTArmA001 -->


    <owl:NamedIndividual rdf:about="http://www.semanticweb.org/vitto/ontologies/2024/9/PODS_1#Matching_Method_of__DELTArmA001">
        <rdf:type rdf:resource="https://photogrammetry.altervista.org/items/show/100#F14_Matching_Method"/>
        <skos:definition xml:lang="en">Matching Method  used for the processing in the context of the photogrammetric acquisition of the archaeological artifact NO01, workflow chain DELTArmA001. This concerns a coloured glass bead.
Feature-based matching algorithm</skos:definition>
    </owl:NamedIndividual>
    


    <!-- http://www.semanticweb.org/vitto/ontologies/2024/9/PODS_1#Matching_of_ALFAfsB001 -->


    <owl:NamedIndividual rdf:about="http://www.semanticweb.org/vitto/ontologies/2024/9/PODS_1#Matching_of_ALFAfsB001">
        <rdf:type rdf:resource="https://photogrammetry.altervista.org/items/show/132#F46:_Matching"/>
        <skos:altLabel xml:lang="en">ALFArmA001_Matching</skos:altLabel>
        <skos:definition xml:lang="en">Matching, that is, in the context of processing, extraction of points from the photographs collected for the photogrammetric acquisition of the archaeological artifact AFMNM005, workflow chain ALFAfsB001. This pertains to a jawbone of a wild boar that has undergone anthropogenic manipulations.</skos:definition>
    </owl:NamedIndividual>
    


    <!-- http://www.semanticweb.org/vitto/ontologies/2024/9/PODS_1#Matching_of_BETAfs001 -->


    <owl:NamedIndividual rdf:about="http://www.semanticweb.org/vitto/ontologies/2024/9/PODS_1#Matching_of_BETAfs001">
        <rdf:type rdf:resource="https://photogrammetry.altervista.org/items/show/132#F46:_Matching"/>
        <skos:altLabel xml:lang="en">BETAfs001_Matching</skos:altLabel>
        <skos:definition xml:lang="en">Matching, that is, in the context of processing, extraction of points from the photographs collected for the photogrammetric acquisition of the funerary archaeological site Tobiotsuka Kofuna (TBZ_K), workflow chain BETAfs001. This consists of a stone burial chamber situated within a tumulus known as Kofun.</skos:definition>
    </owl:NamedIndividual>
    


    <!-- http://www.semanticweb.org/vitto/ontologies/2024/9/PODS_1#Matching_of_NO01__DELTArmA001 -->


    <owl:NamedIndividual rdf:about="http://www.semanticweb.org/vitto/ontologies/2024/9/PODS_1#Matching_of_NO01__DELTArmA001">
        <rdf:type rdf:resource="https://photogrammetry.altervista.org/items/show/132#F46:_Matching"/>
        <skos:altLabel xml:lang="en">DELTArmA001_Matching</skos:altLabel>
        <skos:definition xml:lang="en">Matching, that is, in the context of processing, extraction of points from the photographs collected for the photogrammetric acquisition of the archaeological artifact NO01, workflow chain DELTArmA001. This concerns a colored glass bead.</skos:definition>
    </owl:NamedIndividual>
    


    <!-- http://www.semanticweb.org/vitto/ontologies/2024/9/PODS_1#Mesh_Reconstruction_of_AFMNM005 -->


    <owl:NamedIndividual rdf:about="http://www.semanticweb.org/vitto/ontologies/2024/9/PODS_1#Mesh_Reconstruction_of_AFMNM005">
        <rdf:type rdf:resource="https://photogrammetry.altervista.org/items/show/142#F56_Mesh_Reconstruction"/>
        <skos:altLabel xml:lang="en">ALFAfsB001_MeshReconstruction</skos:altLabel>
        <skos:definition xml:lang="en">For Mesh Reconstruction based on Dense Point Cloud, probably use of Neural Marching Cube and Neural Dual Contouring</skos:definition>
    </owl:NamedIndividual>
    


    <!-- http://www.semanticweb.org/vitto/ontologies/2024/9/PODS_1#Mesh_Reconstruction_of_NO01_DELTArmA001 -->


    <owl:NamedIndividual rdf:about="http://www.semanticweb.org/vitto/ontologies/2024/9/PODS_1#Mesh_Reconstruction_of_NO01_DELTArmA001">
        <rdf:type rdf:resource="https://photogrammetry.altervista.org/items/show/142#F56_Mesh_Reconstruction"/>
        <skos:altLabel xml:lang="en">DELTArmA001_Reconstruction</skos:altLabel>
        <skos:definition xml:lang="en">Reconstruction of the mesh from the photogrammetric survey of the archaeological artifact NO01, workflow chain DELTArmA001. This pertains to a colored glass bead.</skos:definition>
    </owl:NamedIndividual>
    


    <!-- http://www.semanticweb.org/vitto/ontologies/2024/9/PODS_1#ModellingDetemination_of_ALFAfsB001 -->


    <owl:NamedIndividual rdf:about="http://www.semanticweb.org/vitto/ontologies/2024/9/PODS_1#ModellingDetemination_of_ALFAfsB001">
        <rdf:type rdf:resource="https://photogrammetry.altervista.org/items/show/153#F66_Modelling_Determination"/>
        <skos:definition xml:lang="en">In the context of determining the elements of the textured 3D model of ALFAfsB001, the focus was established on the object and all visible parts of the surface.</skos:definition>
    </owl:NamedIndividual>
    


    <!-- http://www.semanticweb.org/vitto/ontologies/2024/9/PODS_1#ModellingElimination_of_ALFAfsB001 -->


    <owl:NamedIndividual rdf:about="http://www.semanticweb.org/vitto/ontologies/2024/9/PODS_1#ModellingElimination_of_ALFAfsB001">
        <rdf:type rdf:resource="https://photogrammetry.altervista.org/items/show/154#F67_Modelling_Elimination"/>
        <skos:definition xml:lang="en">In the context of the elimination of parts from the textured 3D model of ALFAfsB001, the removal of any elements related to the acquisition set was established.</skos:definition>
    </owl:NamedIndividual>
    


    <!-- http://www.semanticweb.org/vitto/ontologies/2024/9/PODS_1#Modelling_3D_Mesh_of_NO01_DELTArmA001 -->


    <owl:NamedIndividual rdf:about="http://www.semanticweb.org/vitto/ontologies/2024/9/PODS_1#Modelling_3D_Mesh_of_NO01_DELTArmA001">
        <rdf:type rdf:resource="https://photogrammetry.altervista.org/items/show/144#F58_Modifying_Mesh"/>
        <skos:altLabel xml:lang="en">DELTArmA001_Modelling</skos:altLabel>
        <skos:definition xml:lang="en">Modification of the 3D model resulting from the photogrammetric survey of the archaeological artifact NO01, workflow chain DELTArmA001. This artifact is a colored glass bead. Modeling refers to the transformation of the format and any alterations made to the 3D model.</skos:definition>
    </owl:NamedIndividual>
    


    <!-- http://www.semanticweb.org/vitto/ontologies/2024/9/PODS_1#Modelling_Date_ALFAfsB001 -->


    <owl:NamedIndividual rdf:about="http://www.semanticweb.org/vitto/ontologies/2024/9/PODS_1#Modelling_Date_ALFAfsB001">
        <rdf:type rdf:resource="https://photogrammetry.altervista.org/items/show/152#F65_Modelling_Date"/>
        <skos:definition>19/03/2019</skos:definition>
    </owl:NamedIndividual>
    


    <!-- http://www.semanticweb.org/vitto/ontologies/2024/9/PODS_1#Modelling_Description_ALFAfsB001 -->


    <owl:NamedIndividual rdf:about="http://www.semanticweb.org/vitto/ontologies/2024/9/PODS_1#Modelling_Description_ALFAfsB001">
        <rdf:type rdf:resource="https://photogrammetry.altervista.org/items/show/151#F64_Modelling_Description"/>
        <skos:definition xml:lang="en">elimination of the elements of the table and the set and focus on the find</skos:definition>
    </owl:NamedIndividual>
    


    <!-- http://www.semanticweb.org/vitto/ontologies/2024/9/PODS_1#Modelling_Device_of_DELTArmA001 -->


    <owl:NamedIndividual rdf:about="http://www.semanticweb.org/vitto/ontologies/2024/9/PODS_1#Modelling_Device_of_DELTArmA001">
        <rdf:type rdf:resource="https://photogrammetry.altervista.org/items/show/97#F11_Modelling_Device"/>
        <skos:definition xml:lang="en">Alienware 1, Intel(R) Core(TM) i7-10870H CPU Processor @ 2.20GHz, 2208 Mhz, 8 cores, 16 logical processors, of Department of Computer Science, University of Turin</skos:definition>
    </owl:NamedIndividual>
    


    <!-- http://www.semanticweb.org/vitto/ontologies/2024/9/PODS_1#Modelling_Operator_ALFAfsB001 -->


    <owl:NamedIndividual rdf:about="http://www.semanticweb.org/vitto/ontologies/2024/9/PODS_1#Modelling_Operator_ALFAfsB001">
        <rdf:type rdf:resource="https://photogrammetry.altervista.org/items/show/125#F39_Modelling_Operator"/>
        <skos:definition xml:lang="en">Vittorio Lauro
https://orcid.org/0000-0003-3446-6127</skos:definition>
    </owl:NamedIndividual>
    


    <!-- http://www.semanticweb.org/vitto/ontologies/2024/9/PODS_1#Modelling_Software_for_ALFAfsB001 -->


    <owl:NamedIndividual rdf:about="http://www.semanticweb.org/vitto/ontologies/2024/9/PODS_1#Modelling_Software_for_ALFAfsB001">
        <rdf:type rdf:resource="https://photogrammetry.altervista.org/items/show/118#F32_Modelling_Software"/>
        <skos:definition xml:lang="en">Blender 7.74</skos:definition>
    </owl:NamedIndividual>
    


    <!-- http://www.semanticweb.org/vitto/ontologies/2024/9/PODS_1#Modelling_of_AFMNM005_ALFAfsB001 -->


    <owl:NamedIndividual rdf:about="http://www.semanticweb.org/vitto/ontologies/2024/9/PODS_1#Modelling_of_AFMNM005_ALFAfsB001">
        <rdf:type rdf:resource="https://photogrammetry.altervista.org/items/show/90#F4_Modelling"/>
        <skos:altLabel xml:lang="en">ALFAfsB001_Modelling</skos:altLabel>
        <skos:definition xml:lang="en">Modeling, that is, the set of activities involving the reconstruction, coloration, and manipulation of the mesh of the 3D model resulting from the photogrammetric acquisition of the archaeological artifact AFMNM005, workflow chain ALFAfsB001. This pertains to a jawbone of a wild boar that has undergone anthropogenic manipulations.</skos:definition>
    </owl:NamedIndividual>
    


    <!-- http://www.semanticweb.org/vitto/ontologies/2024/9/PODS_1#Modelling_of_NO01_DELTArmA001 -->


    <owl:NamedIndividual rdf:about="http://www.semanticweb.org/vitto/ontologies/2024/9/PODS_1#Modelling_of_NO01_DELTArmA001">
        <rdf:type rdf:resource="https://photogrammetry.altervista.org/items/show/90#F4_Modelling"/>
        <skos:altLabel xml:lang="en">DELTArmA001_Modelling</skos:altLabel>
        <skos:definition xml:lang="en">Modeling, that is, the set of activities involving the reconstruction, coloration, and manipulation of the mesh of the 3D model resulting from the photogrammetric acquisition of the archaeological artifact NO01, workflow chain DELTArmA001. This concerns a colored glass bead.</skos:definition>
    </owl:NamedIndividual>
    


    <!-- http://www.semanticweb.org/vitto/ontologies/2024/9/PODS_1#Number_of_Picture_ALFAfsB001 -->


    <owl:NamedIndividual rdf:about="http://www.semanticweb.org/vitto/ontologies/2024/9/PODS_1#Number_of_Picture_ALFAfsB001">
        <rdf:type rdf:resource="https://photogrammetry.altervista.org/items/show/127#F41_Number_of_Picture"/>
        <rdfs:isDefinedBy>http://qudt.org/vocab/soqk/SI</rdfs:isDefinedBy>
        <skos:definition rdf:datatype="http://www.w3.org/2001/XMLSchema#integer">180</skos:definition>
    </owl:NamedIndividual>
    


    <!-- http://www.semanticweb.org/vitto/ontologies/2024/9/PODS_1#Number_of_Point_Dense_Point_Cloud_ALFAfsB001 -->


    <owl:NamedIndividual rdf:about="http://www.semanticweb.org/vitto/ontologies/2024/9/PODS_1#Number_of_Point_Dense_Point_Cloud_ALFAfsB001">
        <rdf:type rdf:resource="https://photogrammetry.altervista.org/items/show/139#F53_Dense_Point_Cloud_Number_of_Point"/>
        <rdfs:comment rdf:datatype="http://www.w3.org/2001/XMLSchema#integer">75399</rdfs:comment>
    </owl:NamedIndividual>
    


    <!-- http://www.semanticweb.org/vitto/ontologies/2024/9/PODS_1#Number_of_TExture_ALFAfsB001 -->


    <owl:NamedIndividual rdf:about="http://www.semanticweb.org/vitto/ontologies/2024/9/PODS_1#Number_of_TExture_ALFAfsB001">
        <rdf:type rdf:resource="https://photogrammetry.altervista.org/items/show/150#F63_Number_of_Texture"/>
        <rdfs:comment rdf:datatype="http://www.w3.org/2001/XMLSchema#integer">1</rdfs:comment>
    </owl:NamedIndividual>
    


    <!-- http://www.semanticweb.org/vitto/ontologies/2024/9/PODS_1#Picture_Set__of_ALFAfsB001 -->


    <owl:NamedIndividual rdf:about="http://www.semanticweb.org/vitto/ontologies/2024/9/PODS_1#Picture_Set__of_ALFAfsB001">
        <rdf:type rdf:resource="https://photogrammetry.altervista.org/items/show/93#F7_Picture_Set"/>
        <skos:definition xml:lang="en">Picture Set  from the photogrammetric acquisition of the archaeological artifact AFMNM005, workflow chain ALFAfsB001. This pertains to a jawbone of a wild boar that has undergone anthropogenic manipulations.  Picture Set are the result of photogrammetric acquisition and are made up of multiple photographs of the object under examination observed from different points of view</skos:definition>
    </owl:NamedIndividual>
    


    <!-- http://www.semanticweb.org/vitto/ontologies/2024/9/PODS_1#Picture_Set__of_DELTArmA001 -->


    <owl:NamedIndividual rdf:about="http://www.semanticweb.org/vitto/ontologies/2024/9/PODS_1#Picture_Set__of_DELTArmA001">
        <rdf:type rdf:resource="https://photogrammetry.altervista.org/items/show/93#F7_Picture_Set"/>
        <skos:definition xml:lang="en">Picture Set  from the photogrammetric acquisition of the archaeological artifact NO01, workflow chain DELTArmA001.  Picture Set  are the result of photogrammetric acquisition and are made up of multiple photographs of the object under examination observed from different points of view</skos:definition>
    </owl:NamedIndividual>
    


    <!-- http://www.semanticweb.org/vitto/ontologies/2024/9/PODS_1#Pocessing_Software_for_ALFAfsB001 -->


    <owl:NamedIndividual rdf:about="http://www.semanticweb.org/vitto/ontologies/2024/9/PODS_1#Pocessing_Software_for_ALFAfsB001">
        <rdf:type rdf:resource="https://photogrammetry.altervista.org/items/show/117#F31_Processing_Software"/>
        <skos:definition xml:lang="en">Recap Autodesk Research Licence of International Research Institute for Archaeology and Ethnology</skos:definition>
    </owl:NamedIndividual>
    


    <!-- http://www.semanticweb.org/vitto/ontologies/2024/9/PODS_1#Pocessing_Software_for_BETAfsF001 -->


    <owl:NamedIndividual rdf:about="http://www.semanticweb.org/vitto/ontologies/2024/9/PODS_1#Pocessing_Software_for_BETAfsF001">
        <rdf:type rdf:resource="https://photogrammetry.altervista.org/items/show/117#F31_Processing_Software"/>
        <skos:definition xml:lang="en">Agistoft Metashape Licence Unkonwn</skos:definition>
    </owl:NamedIndividual>
    


    <!-- http://www.semanticweb.org/vitto/ontologies/2024/9/PODS_1#Pocessing_Software_for_DELTArmA001 -->


    <owl:NamedIndividual rdf:about="http://www.semanticweb.org/vitto/ontologies/2024/9/PODS_1#Pocessing_Software_for_DELTArmA001">
        <rdf:type rdf:resource="https://photogrammetry.altervista.org/items/show/117#F31_Processing_Software"/>
        <skos:definition xml:lang="en">Zephyr 3D Professional Licence  of Computer Science Department University of Turin</skos:definition>
    </owl:NamedIndividual>
    


    <!-- http://www.semanticweb.org/vitto/ontologies/2024/9/PODS_1#Point_Cloud_of_DELTArmA001 -->


    <owl:NamedIndividual rdf:about="http://www.semanticweb.org/vitto/ontologies/2024/9/PODS_1#Point_Cloud_of_DELTArmA001">
        <rdf:type rdf:resource="https://photogrammetry.altervista.org/items/show/112#F26_Point_Cloud"/>
        <skos:definition xml:lang="en">Point Cloud from the photogrammetric acquisition of the archaeological artifact NO01, workflow chain DELTArmA001. This concerns a colored glass bead.</skos:definition>
    </owl:NamedIndividual>
    


    <!-- http://www.semanticweb.org/vitto/ontologies/2024/9/PODS_1#Point_Cloud_of__ALFAfsB001 -->


    <owl:NamedIndividual rdf:about="http://www.semanticweb.org/vitto/ontologies/2024/9/PODS_1#Point_Cloud_of__ALFAfsB001">
        <rdf:type rdf:resource="https://photogrammetry.altervista.org/items/show/112#F26_Point_Cloud"/>
        <skos:definition xml:lang="en">Point Cloud from the photogrammetric acquisition of the archaeological artifact AFMNM005, workflow chain ALFAfsB001. This pertains to a jawbone of a wild boar that has undergone anthropogenic manipulations.</skos:definition>
    </owl:NamedIndividual>
    


    <!-- http://www.semanticweb.org/vitto/ontologies/2024/9/PODS_1#Processing_Device_of_ALFAfsB001 -->


    <owl:NamedIndividual rdf:about="http://www.semanticweb.org/vitto/ontologies/2024/9/PODS_1#Processing_Device_of_ALFAfsB001">
        <rdf:type rdf:resource="https://photogrammetry.altervista.org/items/show/96#F10_Processing_Device"/>
        <skos:definition xml:lang="en">DELL Vostro 3525 AMD Ryzen™ 7 5700U Computer of International Research Intstitute of Archaeology and Ethnography</skos:definition>
    </owl:NamedIndividual>
    


    <!-- http://www.semanticweb.org/vitto/ontologies/2024/9/PODS_1#Processing_Device_of_DELTArmA001 -->


    <owl:NamedIndividual rdf:about="http://www.semanticweb.org/vitto/ontologies/2024/9/PODS_1#Processing_Device_of_DELTArmA001">
        <rdf:type rdf:resource="https://photogrammetry.altervista.org/items/show/96#F10_Processing_Device"/>
        <skos:definition xml:lang="en">MSI Cyborg 15 A13VE-602IT Intel® Core™ i7 i7-13620H of the Computer Science Department University of Turin</skos:definition>
    </owl:NamedIndividual>
    


    <!-- http://www.semanticweb.org/vitto/ontologies/2024/9/PODS_1#Processing_Phase_of_ALFAfsB001 -->


    <owl:NamedIndividual rdf:about="http://www.semanticweb.org/vitto/ontologies/2024/9/PODS_1#Processing_Phase_of_ALFAfsB001">
        <rdf:type rdf:resource="https://photogrammetry.altervista.org/items/show/120#F34_Processing_Phase"/>
        <skos:definition xml:lang="en">Processing Phase  of the photogrammetric acquisition of the archaeological artifact AFMNM005, workflow chain ALFAfsB001. This pertains to a jawbone of a wild boar that has undergone anthropogenic manipulations. The acquisition phase respected the scans and indications as established by the BeA-PG protocol</skos:definition>
    </owl:NamedIndividual>
    


    <!-- http://www.semanticweb.org/vitto/ontologies/2024/9/PODS_1#Processing_Phase_of_DELTArmA001 -->


    <owl:NamedIndividual rdf:about="http://www.semanticweb.org/vitto/ontologies/2024/9/PODS_1#Processing_Phase_of_DELTArmA001">
        <rdf:type rdf:resource="https://photogrammetry.altervista.org/items/show/120#F34_Processing_Phase"/>
        <skos:definition xml:lang="en">Processing Phase  of  the photogrammetric acquisition of the archaeological artifact NO01, workflow chain DELTArmA001. This concerns a coloured glass bead.

The acquisition phase respected the scans and indications as established by the FOPPA Manual</skos:definition>
    </owl:NamedIndividual>
    


    <!-- http://www.semanticweb.org/vitto/ontologies/2024/9/PODS_1#Processing_of_NO01_DELTArmA001 -->


    <owl:NamedIndividual rdf:about="http://www.semanticweb.org/vitto/ontologies/2024/9/PODS_1#Processing_of_NO01_DELTArmA001">
        <rdf:type rdf:resource="https://photogrammetry.altervista.org/items/show/89#F3_Processing"/>
        <skos:altLabel xml:lang="en">DELTArmA001_Processing</skos:altLabel>
        <skos:definition xml:lang="en">Processing of the photographs from the photogrammetric acquisition of the archaeological artifact NO01, workflow chain DELTArmA001. This concerns a colored glass bead.</skos:definition>
    </owl:NamedIndividual>
    


    <!-- http://www.semanticweb.org/vitto/ontologies/2024/9/PODS_1#Processing_of_TBZ._K._BETAfsF001 -->


    <owl:NamedIndividual rdf:about="http://www.semanticweb.org/vitto/ontologies/2024/9/PODS_1#Processing_of_TBZ._K._BETAfsF001">
        <rdf:type rdf:resource="https://photogrammetry.altervista.org/items/show/89#F3_Processing"/>
        <skos:altLabel xml:lang="en">BETAfsF001_Processing</skos:altLabel>
        <skos:definition xml:lang="en">Processing of the photographs from the photogrammetric acquisition of the funerary archaeological site Tobiotsuka Kofuna (TBZ_K), workflow chain BETAfs001. This consists of a stone burial chamber situated within a tumulus known as Kofun.</skos:definition>
    </owl:NamedIndividual>
    


    <!-- http://www.semanticweb.org/vitto/ontologies/2024/9/PODS_1#Reconstruction_Algorithm_for_ALFAfsB001 -->


    <owl:NamedIndividual rdf:about="http://www.semanticweb.org/vitto/ontologies/2024/9/PODS_1#Reconstruction_Algorithm_for_ALFAfsB001">
        <rdf:type rdf:resource="https://photogrammetry.altervista.org/items/show/109#F23_Reconstruction_Algorithm_Type"/>
        <skos:definition xml:lang="en">Neural Marching Cube and Neural Dual Contouring</skos:definition>
    </owl:NamedIndividual>
    


    <!-- http://www.semanticweb.org/vitto/ontologies/2024/9/PODS_1#Reconstruction_Algorithm_for_DELTArmA001 -->


    <owl:NamedIndividual rdf:about="http://www.semanticweb.org/vitto/ontologies/2024/9/PODS_1#Reconstruction_Algorithm_for_DELTArmA001">
        <rdf:type rdf:resource="https://photogrammetry.altervista.org/items/show/109#F23_Reconstruction_Algorithm_Type"/>
        <skos:definition xml:lang="en">Poisson</skos:definition>
    </owl:NamedIndividual>
    


    <!-- http://www.semanticweb.org/vitto/ontologies/2024/9/PODS_1#Reconstruction_Method_of__DELTArmA001 -->


    <owl:NamedIndividual rdf:about="http://www.semanticweb.org/vitto/ontologies/2024/9/PODS_1#Reconstruction_Method_of__DELTArmA001">
        <rdf:type rdf:resource="https://photogrammetry.altervista.org/items/show/101#F15_Recontruction_Method"/>
        <skos:definition xml:lang="en">Reconstruction  used for the modelling in the context of the photogrammetric acquisition of the archaeological artifact NO01, workflow chain DELTArmA001. This concerns a coloured glass bead.
SASHA Method integrated in Zephyr 3D.</skos:definition>
    </owl:NamedIndividual>
    


    <!-- http://www.semanticweb.org/vitto/ontologies/2024/9/PODS_1#Scale_for_ALFAfsB001 -->


    <owl:NamedIndividual rdf:about="http://www.semanticweb.org/vitto/ontologies/2024/9/PODS_1#Scale_for_ALFAfsB001">
        <rdf:type rdf:resource="https://photogrammetry.altervista.org/items/show/105#F19_Scale_Type"/>
        <skos:definition xml:lang="en">Medium Object (1 cm to 30 cm) by FOPPA Thesaurus</skos:definition>
    </owl:NamedIndividual>
    


    <!-- http://www.semanticweb.org/vitto/ontologies/2024/9/PODS_1#Scale_for_BETAfs001 -->


    <owl:NamedIndividual rdf:about="http://www.semanticweb.org/vitto/ontologies/2024/9/PODS_1#Scale_for_BETAfs001">
        <rdf:type rdf:resource="https://photogrammetry.altervista.org/items/show/105#F19_Scale_Type"/>
        <skos:definition xml:lang="en">Cave or underground structure by FOPPA Thesaurus</skos:definition>
    </owl:NamedIndividual>
    


    <!-- http://www.semanticweb.org/vitto/ontologies/2024/9/PODS_1#Scale_for_DELTArmA001 -->


    <owl:NamedIndividual rdf:about="http://www.semanticweb.org/vitto/ontologies/2024/9/PODS_1#Scale_for_DELTArmA001">
        <rdf:type rdf:resource="https://photogrammetry.altervista.org/items/show/105#F19_Scale_Type"/>
        <skos:definition xml:lang="en">Small object (equal to or smaller than 1 cm) by FOPPA thesaurus</skos:definition>
    </owl:NamedIndividual>
    


    <!-- http://www.semanticweb.org/vitto/ontologies/2024/9/PODS_1#Smoothing_Filter_of_ALFAfsB001 -->


    <owl:NamedIndividual rdf:about="http://www.semanticweb.org/vitto/ontologies/2024/9/PODS_1#Smoothing_Filter_of_ALFAfsB001">
        <rdf:type rdf:resource="https://photogrammetry.altervista.org/items/show/147#F60_Smoothing_Filter"/>
        <skos:definition xml:lang="en">Concerning the smoothing filter in the context of mesh reconstruction based on the dense point cloud obtained from the photogrammetric acquisition of the archaeological artifact AFMNM005, workflow chain ALFAfsB001 (which is a boar&apos;s jaw subjected to anthropic modifications), a Laplacian smoothing technique has been employed.</skos:definition>
    </owl:NamedIndividual>
    


    <!-- http://www.semanticweb.org/vitto/ontologies/2024/9/PODS_1#Survey_Date_of_AFMNM005_ALFAfsB001 -->


    <owl:NamedIndividual rdf:about="http://www.semanticweb.org/vitto/ontologies/2024/9/PODS_1#Survey_Date_of_AFMNM005_ALFAfsB001">
        <rdf:type rdf:resource="https://photogrammetry.altervista.org/items/show/129#F43_Survey_Date"/>
        <rdfs:comment>09/03/2019</rdfs:comment>
    </owl:NamedIndividual>
    


    <!-- http://www.semanticweb.org/vitto/ontologies/2024/9/PODS_1#Survey_OPERATOR_of_AFMNM005_ALFAfsB001 -->


    <owl:NamedIndividual rdf:about="http://www.semanticweb.org/vitto/ontologies/2024/9/PODS_1#Survey_OPERATOR_of_AFMNM005_ALFAfsB001">
        <rdf:type rdf:resource="https://photogrammetry.altervista.org/items/show/123#F37_Survey_Operator"/>
        <skos:definition xml:lang="en">Vittorio Lauro
https://orcid.org/0000-0003-3446-6127</skos:definition>
    </owl:NamedIndividual>
    


    <!-- http://www.semanticweb.org/vitto/ontologies/2024/9/PODS_1#Survey_Object_for__ALFAfsB001 -->


    <owl:NamedIndividual rdf:about="http://www.semanticweb.org/vitto/ontologies/2024/9/PODS_1#Survey_Object_for__ALFAfsB001">
        <rdf:type rdf:resource="https://photogrammetry.altervista.org/admin/items/show/87#F1_Survey_Object"/>
        <skos:definition xml:lang="en">Object of the photogrammetric survey. 
Jaw of a wild boar belonging to the late Yayoi culture and found at the Minamikata excavation during the construction excavations of the Okayama hospital concluded in 2016. The jaw shows signs of processing on the sides and two artificial holes produced in the attachment of the jaw. It is assumed that the object was hung thanks to the use of a rope passing through the holes. Its purpose is unknown. 
The object is marked in the BeArchaeo project database as AF MNM 005
In the work chain the identifier  ALFAfsB001  was assigned according to the FOPPA method</skos:definition>
    </owl:NamedIndividual>
    


    <!-- http://www.semanticweb.org/vitto/ontologies/2024/9/PODS_1#Survey_Object_for__BETAfsF001 -->


    <owl:NamedIndividual rdf:about="http://www.semanticweb.org/vitto/ontologies/2024/9/PODS_1#Survey_Object_for__BETAfsF001">
        <rdf:type rdf:resource="https://photogrammetry.altervista.org/admin/items/show/87#F1_Survey_Object"/>
        <skos:definition xml:lang="en">Object of the photogrammetric survey. 
Burial chamber made of stone blocks set in a mound according to the typology of Japanese monumental tombs known as Kofun. In particular, the object of the Survey is the so-called Tobiotsuka Kofun located in Okayama Prefecture and dating back to the late Kofun period and subject to investigation and excavation from 2019 to 2023 in the context of the BeArchaeo project. 
The object is marked in the BeArchaeo project database as TBZ-K
In the work chain the identifier BETAfsF001 was assigned according to the FOPPA method</skos:definition>
    </owl:NamedIndividual>
    


    <!-- http://www.semanticweb.org/vitto/ontologies/2024/9/PODS_1#Survey_Object_for__DELTArmA001 -->


    <owl:NamedIndividual rdf:about="http://www.semanticweb.org/vitto/ontologies/2024/9/PODS_1#Survey_Object_for__DELTArmA001">
        <rdf:type rdf:resource="https://photogrammetry.altervista.org/admin/items/show/87#F1_Survey_Object"/>
        <skos:definition xml:lang="en">Object of the Survey. Colored glass bead in blue and black paste from the Nima Otsuka site and dating back to the late Kofun period and detected in the context of investigations promoted by the University of Turin and the University of Okayama which took place in 2024. The object has a temporary identifier of Nima Otsuka 01 or alternatively NM01
In the work chain the identifier DELTArmA001 was assigned according to the FOPPA method</skos:definition>
    </owl:NamedIndividual>
    


    <!-- http://www.semanticweb.org/vitto/ontologies/2024/9/PODS_1#Textured_3D_Mesh_of_DELTArmA001 -->


    <owl:NamedIndividual rdf:about="http://www.semanticweb.org/vitto/ontologies/2024/9/PODS_1#Textured_3D_Mesh_of_DELTArmA001">
        <rdf:type rdf:resource="https://photogrammetry.altervista.org/items/show/115#F29_Textured_3D_Mesh"/>
        <skos:definition xml:lang="en">3d Mesh from the photogrammetric acquisition of the archaeological artifact NO01, workflow chain DELTArmA001. This concerns a coloured glass bead.   This Mesh is enriched with the texture and represents the morphological surface of the object and the colours displacement</skos:definition>
    </owl:NamedIndividual>
    


    <!-- http://www.semanticweb.org/vitto/ontologies/2024/9/PODS_1#Textured_3D_Mesh_of__ALFAfsB001 -->


    <owl:NamedIndividual rdf:about="http://www.semanticweb.org/vitto/ontologies/2024/9/PODS_1#Textured_3D_Mesh_of__ALFAfsB001">
        <rdf:type rdf:resource="https://photogrammetry.altervista.org/items/show/115#F29_Textured_3D_Mesh"/>
        <skos:definition xml:lang="en">3d Mesh from the photogrammetric acquisition of the archaeological artifact AFMNM005, workflow chain ALFAfsB001. This pertains to a jawbone of a wild boar that has undergone anthropogenic manipulations.  This Mesh is enriched with the texture and represents the morphological surface of the object and the colours displacement</skos:definition>
    </owl:NamedIndividual>
    


    <!-- http://www.semanticweb.org/vitto/ontologies/2024/9/PODS_1#Texturing_Mesh_of_NO01__DELTArmA001 -->


    <owl:NamedIndividual rdf:about="http://www.semanticweb.org/vitto/ontologies/2024/9/PODS_1#Texturing_Mesh_of_NO01__DELTArmA001">
        <rdf:type rdf:resource="https://photogrammetry.altervista.org/items/show/143#F57_Texturing_Mesh"/>
        <skos:altLabel xml:lang="en">DELTArmA001_Reconstruction</skos:altLabel>
        <skos:definition xml:lang="en">Texturing of the mesh obtained from the photogrammetric survey of the archaeological artifact NO01, workflow chain DELTArmA001. This artifact is a colored glass bead, and the texturing is based on the extraction of color information from the photographs collected during the acquisition phase.</skos:definition>
    </owl:NamedIndividual>
    


    <!-- http://www.semanticweb.org/vitto/ontologies/2024/9/PODS_1#Texturing_Method_of__DELTArmA001 -->


    <owl:NamedIndividual rdf:about="http://www.semanticweb.org/vitto/ontologies/2024/9/PODS_1#Texturing_Method_of__DELTArmA001">
        <rdf:type rdf:resource="https://photogrammetry.altervista.org/items/show/102#F16_Texturing_Method"/>
        <skos:definition xml:lang="en">Texturing Method used for the modelling in the context of the photogrammetric acquisition of the archaeological artifact NO01, workflow chain DELTArmA001. This concerns a coloured glass bead.

Parameterization + Texturing from registered rasters</skos:definition>
    </owl:NamedIndividual>
    


    <!-- http://www.semanticweb.org/vitto/ontologies/2024/9/PODS_1#Texturing_Type_ALFAfsB001 -->


    <owl:NamedIndividual rdf:about="http://www.semanticweb.org/vitto/ontologies/2024/9/PODS_1#Texturing_Type_ALFAfsB001">
        <rdf:type rdf:resource="https://photogrammetry.altervista.org/items/show/110#F24__Texturing_Type"/>
        <skos:definition xml:lang="en">Single Texture jpg</skos:definition>
    </owl:NamedIndividual>
    


    <!-- http://www.semanticweb.org/vitto/ontologies/2024/9/PODS_1#Texturing_Type_DELTArmA001 -->


    <owl:NamedIndividual rdf:about="http://www.semanticweb.org/vitto/ontologies/2024/9/PODS_1#Texturing_Type_DELTArmA001">
        <rdf:type rdf:resource="https://photogrammetry.altervista.org/items/show/110#F24__Texturing_Type"/>
        <skos:definition xml:lang="en">Multi Texturing</skos:definition>
    </owl:NamedIndividual>
    


    <!-- http://www.semanticweb.org/vitto/ontologies/2024/9/PODS_1#TrajectoryType_for_ALFAfsB001 -->


    <owl:NamedIndividual rdf:about="http://www.semanticweb.org/vitto/ontologies/2024/9/PODS_1#TrajectoryType_for_ALFAfsB001">
        <rdf:type rdf:resource="https://photogrammetry.altervista.org/items/show/103#F17_Acquisition_Trajectory_Type"/>
        <skos:definition xml:lang="en">Free hand spiral acquisition by FOPPA Manual</skos:definition>
    </owl:NamedIndividual>
    


    <!-- http://www.semanticweb.org/vitto/ontologies/2024/9/PODS_1#TrajectoryType_for_BETAfsF001 -->


    <owl:NamedIndividual rdf:about="http://www.semanticweb.org/vitto/ontologies/2024/9/PODS_1#TrajectoryType_for_BETAfsF001">
        <rdf:type rdf:resource="https://photogrammetry.altervista.org/items/show/103#F17_Acquisition_Trajectory_Type"/>
        <skos:definition xml:lang="en">Interior by MetaShape Agisoft Manual</skos:definition>
    </owl:NamedIndividual>
    


    <!-- http://www.semanticweb.org/vitto/ontologies/2024/9/PODS_1#TrajectoryType_for_DELTArmA001 -->


    <owl:NamedIndividual rdf:about="http://www.semanticweb.org/vitto/ontologies/2024/9/PODS_1#TrajectoryType_for_DELTArmA001">
        <rdf:type rdf:resource="https://photogrammetry.altervista.org/items/show/103#F17_Acquisition_Trajectory_Type"/>
        <skos:definition xml:lang="en">Rotating base microscope by FOPPA Manual</skos:definition>
    </owl:NamedIndividual>
    


    <!-- http://www.semanticweb.org/vitto/ontologies/2024/9/PODS_1#interactive_software_for_BETAfsF001 -->


    <owl:NamedIndividual rdf:about="http://www.semanticweb.org/vitto/ontologies/2024/9/PODS_1#interactive_software_for_BETAfsF001">
        <rdf:type rdf:resource="https://photogrammetry.altervista.org/items/show/180#F93_Interactive_Software"/>
        <skos:definition xml:lang="en">Unity 2021.3.3f1</skos:definition>
    </owl:NamedIndividual>
    


    <!-- http://www.semanticweb.org/vitto/ontologies/2024/9/PODS_1#processing_operator_ALFAfsB001 -->


    <owl:NamedIndividual rdf:about="http://www.semanticweb.org/vitto/ontologies/2024/9/PODS_1#processing_operator_ALFAfsB001">
        <rdf:type rdf:resource="https://photogrammetry.altervista.org/items/show/124#F38_Processing_Operator"/>
        <skos:definition xml:lang="en">Vittorio Lauro
https://orcid.org/0000-0003-3446-6127</skos:definition>
    </owl:NamedIndividual>
    


    <!-- http://www.semanticweb.org/vitto/ontologies/2024/9/PODS_1#3D_Digital_Twin___ALFAfsB001 -->


    <owl:NamedIndividual rdf:about="http://www.semanticweb.org/vitto/ontologies/2024/9/PODS_1#3D_Digital_Twin___ALFAfsB001">
        <rdf:type rdf:resource="https://photogrammetry.altervista.org/items/show/145#F100_3D_Digital_Twin"/>
        <skos:definition xml:lang="en">Obj 3D Model, 180 MB 
3D Model from the photogrammetric acquisition of the archaeological artifact AFMNM005, workflow chain ALFAfsB001. This pertains to a jawbone of a wild boar that has undergone anthropogenic manipulations.</skos:definition>
    </owl:NamedIndividual>
    


    <!-- http://www.semanticweb.org/vitto/ontologies/2024/9/PODS_1#3D_Digital_Twin___BETAfsF001 -->


    <owl:NamedIndividual rdf:about="http://www.semanticweb.org/vitto/ontologies/2024/9/PODS_1#3D_Digital_Twin___BETAfsF001">
        <rdf:type rdf:resource="https://photogrammetry.altervista.org/items/show/145#F100_3D_Digital_Twin"/>
        <skos:definition xml:lang="en">FBX 3D Model, 290 MB
3D Model from  the photogrammetric acquisition of the funerary archaeological site Tobiotsuka Kofuna (TBZ_K), workflow chain BETAfs001. This consists of a stone burial chamber situated within a tumulus known as Kofun.</skos:definition>
    </owl:NamedIndividual>
    


    <!-- http://www.semanticweb.org/vitto/ontologies/2024/9/PODS_1#3D_Digital_Twin____DELTArmA001 -->


    <owl:NamedIndividual rdf:about="http://www.semanticweb.org/vitto/ontologies/2024/9/PODS_1#3D_Digital_Twin____DELTArmA001">
        <rdf:type rdf:resource="https://photogrammetry.altervista.org/items/show/145#F100_3D_Digital_Twin"/>
        <skos:definition xml:lang="en">Obj 3D Model, 480 MB 
3d Model  from the photogrammetric acquisition of the archaeological artifact NO01, workflow chain DELTArmA001. This concerns a colored glass bead.</skos:definition>
    </owl:NamedIndividual>
    


    <!-- http://www.semanticweb.org/vitto/ontologies/2024/9/PODS_1#3D_Mesh_of__ALFAfsB001 -->


    <owl:NamedIndividual rdf:about="http://www.semanticweb.org/vitto/ontologies/2024/9/PODS_1#3D_Mesh_of__ALFAfsB001">
        <rdf:type rdf:resource="https://photogrammetry.altervista.org/items/show/114#F28_3D_Mesh"/>
        <skos:definition xml:lang="en">3d Mesh from the photogrammetric acquisition of the archaeological artifact AFMNM005, workflow chain ALFAfsB001. This pertains to a jawbone of a wild boar that has undergone anthropogenic manipulations. This Mesh is without texture and represents just the morphological surface of the object</skos:definition>
    </owl:NamedIndividual>
    


    <!-- http://www.semanticweb.org/vitto/ontologies/2024/9/PODS_1#3D_Mesh_of___of_DELTArmA001 -->


    <owl:NamedIndividual rdf:about="http://www.semanticweb.org/vitto/ontologies/2024/9/PODS_1#3D_Mesh_of___of_DELTArmA001">
        <rdf:type rdf:resource="https://photogrammetry.altervista.org/items/show/114#F28_3D_Mesh"/>
        <skos:definition xml:lang="en">3d Mesh from the photogrammetric acquisition of the archaeological artifact NO01, workflow chain DELTArmA001. This concerns a coloured glass bead.   This Mesh is without texture and represents just the morphological surface of the object</skos:definition>
    </owl:NamedIndividual>
    


    <!-- http://www.semanticweb.org/vitto/ontologies/2024/9/PODS_1#Dense_Point_Cloud:_Depth_Noise_Filtering_ALFAfsB001 -->


    <owl:NamedIndividual rdf:about="http://www.semanticweb.org/vitto/ontologies/2024/9/PODS_1#Dense_Point_Cloud:_Depth_Noise_Filtering_ALFAfsB001">
        <rdf:type rdf:resource="https://photogrammetry.altervista.org/items/show/141#F55_Depth_Noise_Filtering"/>
        <skos:altLabel xml:lang="en">ALFAfsB001_depth noise filtering</skos:altLabel>
        <skos:definition xml:lang="en">Concerning the dense point cloud resulting from the photogrammetric acquisition of the archaeological artifact AFMNM005, workflow chain ALFAfsB001 (which is a boar&apos;s jaw subjected to anthropic modifications), the depth noise filtering is based on adaptive feature extraction (AFE), gradient field estimation (GFE), and further accelerated gradient ascent (FAGA).</skos:definition>
    </owl:NamedIndividual>
    


    <!-- 
    ///////////////////////////////////////////////////////////////////////////////////////
    //
    // Annotations
    //
    ///////////////////////////////////////////////////////////////////////////////////////
     -->


    <rdf:Description rdf:about="http://objects.mainzed.org/metadata/ont#Environment">
        <rdfs:label xml:lang="en">MAINZED_3D_METADATA_ONTOLOGY: Enviroment</rdfs:label>
    </rdf:Description>
    <rdf:Description rdf:about="http://www.w3.org/ns/prov#Agent">
        <rdfs:label xml:lang="en">MAINZED_3D_METADATA_ONTOLOGY: Agent</rdfs:label>
    </rdf:Description>
</rdf:RDF>



<!-- Generated by the OWL API (version 5.1.18) https://github.com/owlcs/owlapi/ -->


